@prefix cc: <http://creativecommons.org/ns#> .
@prefix dc11: <http://purl.org/dc/elements/1.1/> .
@prefix skos: <http://www.w3.org/2004/02/skos/core#> .
@prefix xsd: <http://www.w3.org/2001/XMLSchema#> .
@prefix dc: <http://purl.org/dc/terms/> .
@prefix owl: <http://www.w3.org/2002/07/owl#> .

<http://creativecommons.org/licenses/by/4.0/>
  a cc:License ;
  cc:requires cc:Notice, cc:Attribution ;
  dc11:title "Attribution 4.0 International"@en ;
  cc:permits cc:Reproduction, cc:Distribution, cc:DerivativeWorks .

<http://data.loterre.fr/ark:/67375/TSO>
  a skos:ConceptScheme ;
  cc:attributionName "Institut de l’information scientifique et technique (Inist) - CNRS/UAR76"@fr, "Institute for scientific and technical information (Inist) - CNRS/UAR76"@en, "Institute for scientific and technical information (Inist) - CNRS/UAR76"@es ;
  cc:attributionURL "http://www.inist.fr"^^xsd:string ;
  cc:license <http://creativecommons.org/licenses/by/4.0/> ;
  dc11:creator "Institut de l’information scientifique et technique (Inist) - CNRS/UAR76"^^xsd:string ;
  dc11:description "Ce thésaurus multilingue rassemble et structure, avec une polyhiérarchie, les concepts principaux de la science ouverte. Il a été initié en s'appuyant sur les glossaires existants et sur la taxonomie proposée dans le cadre du projet FOSTER. Il est enrichi grâce à une fouille des documents de référence du domaine."@fr, "Este tesauro multilingüe recoge y estructura, con una polijerarquía, los principales conceptos de la ciencia abierta. Se ha iniciado a partir de los glosarios existentes y de la taxonomía propuesta en el marco del proyecto FOSTER. Se enriquece gracias a la búsqueda de documentos de referencia en el ámbito."@es, "This multilingual thesaurus structures, with a polyhierarchy, the main concepts of open science. It was initiated by building on existing glossaries and on the taxonomy proposed in the framework of the FOSTER project. It is enriched through a text-mining task of reference documents in the field."@en ;
  dc11:identifier "https://dx.doi.org/10.13143/lotr.9297" ;
  dc11:title "Open science thesaurus"@en, "Thésaurus de la science ouverte"@fr, "Tesauro de la ciencia abierta"@es ;
  dc:created "2021-03-18"^^xsd:date ;
  dc:modified "2021-07-05"^^xsd:date ;
  dc:language <http://lexvo.org/id/iso639-3/eng>, <http://lexvo.org/id/iso639-3/fra>, <http://lexvo.org/id/iso639-3/spa> ;
  owl:versionInfo "1.1"^^xsd:string ;
  skos:hasTopConcept <http://data.loterre.fr/ark:/67375/TSO-T84RPJRB-K>, <http://data.loterre.fr/ark:/67375/TSO-ZQ0Q8HMP-Q>, <http://data.loterre.fr/ark:/67375/TSO-XWVJBKN6-S>, <http://data.loterre.fr/ark:/67375/TSO-JFJGKFN2-H>, <http://data.loterre.fr/ark:/67375/TSO-SMGMJFLJ-Q>, <http://data.loterre.fr/ark:/67375/TSO-V0HZ66HD-4>, <http://data.loterre.fr/ark:/67375/TSO-V0KSG0NC-P>, <http://data.loterre.fr/ark:/67375/TSO-J64S3QDL-1>, <http://data.loterre.fr/ark:/67375/TSO-H93WKMMJ-B>, <http://data.loterre.fr/ark:/67375/TSO-V6F4ZS65-G>, <http://data.loterre.fr/ark:/67375/TSO-H0BSK47H-Z>, <http://data.loterre.fr/ark:/67375/TSO-PSFFQLXV-2>, <http://data.loterre.fr/ark:/67375/TSO-MJRKBMDW-Q>, <http://data.loterre.fr/ark:/67375/TSO-F2VJ1STQ-Z> .

<http://data.loterre.fr/ark:/67375/TSO-BRLNRV51-S>
  a skos:Concept ;
  dc:modified "2021-07-05"^^xsd:date ;
  skos:altLabel "datos vinculados"@es ;
  skos:definition "A set of best practices for publishing and interlinking structured data on the Web. These best practices were introduced by Tim Berners-Lee in his Web architecture note Linked Data and have become known as the Linked Data principles. (Source : http://linkeddatabook.com/editions/1.0/)"@en, "Conjunto de buenas prácticas para publicar y conectar datos estructurados en la web. (https://datos.gob.es/es/noticia/linked-data-como-modelo-de-datos)"@es, "Ensemble de principes de conception pour le partage de données lisibles par machine sur le Web pour une utilisation par les administrations publiques, les entreprises et les citoyens. (Source : https://data.europa.eu)"@fr ;
  skos:prefLabel "datos enlazados"@es, "données liées"@fr, "linked data"@en ;
  skos:inScheme <http://data.loterre.fr/ark:/67375/TSO> ;
  skos:broader <http://data.loterre.fr/ark:/67375/TSO-MJRKBMDW-Q> ;
  skos:related <http://data.loterre.fr/ark:/67375/TSO-C676TDJV-H>, <http://data.loterre.fr/ark:/67375/TSO-WBDZJK00-P>, <http://data.loterre.fr/ark:/67375/TSO-X1K9R85M-K> .

<http://data.loterre.fr/ark:/67375/TSO-MWXTBMQ8-9>
  a skos:Concept ;
  skos:prefLabel "financement du libre accès"@fr, "financiación del acceso abierto"@es, "open access funding"@en ;
  skos:inScheme <http://data.loterre.fr/ark:/67375/TSO> ;
  skos:broader <http://data.loterre.fr/ark:/67375/TSO-T84RPJRB-K> ;
  skos:related <http://data.loterre.fr/ark:/67375/TSO-STWL5MWS-W> ;
  skos:narrower <http://data.loterre.fr/ark:/67375/TSO-D83BMN3W-M>, <http://data.loterre.fr/ark:/67375/TSO-WFHTSVS6-0>, <http://data.loterre.fr/ark:/67375/TSO-SJ6X9JL0-3>, <http://data.loterre.fr/ark:/67375/TSO-RKX32RM6-2>, <http://data.loterre.fr/ark:/67375/TSO-XTZMJ2W8-J>, <http://data.loterre.fr/ark:/67375/TSO-NJS8254Q-B>, <http://data.loterre.fr/ark:/67375/TSO-QL8P69BW-V> .

<http://data.loterre.fr/ark:/67375/TSO-T84RPJRB-K>
  a skos:Concept ;
  dc:modified "2021-06-28"^^xsd:date ;
  skos:definition "Modèle définissant qui assume les coûts de financement de l'accès aux revues en libre accès."@fr ;
  skos:prefLabel "economic model of open access"@en, "modelo económico del acceso abierto"@es, "modèle économique du libre accès"@fr ;
  skos:inScheme <http://data.loterre.fr/ark:/67375/TSO> ;
  skos:narrower <http://data.loterre.fr/ark:/67375/TSO-MWXTBMQ8-9>, <http://data.loterre.fr/ark:/67375/TSO-KHL25V0F-4> ;
  skos:topConceptOf <http://data.loterre.fr/ark:/67375/TSO> .

<http://data.loterre.fr/ark:/67375/TSO-SVH6TCP0-3>
  a skos:Concept ;
  dc:modified "2021-06-29"^^xsd:date ;
  skos:altLabel "identificador de cita abierta"@es, "open citation identifier"@en ;
  skos:definition "A globally unique persistent identifier for the identification of open bibliographic citations stored in a specific database or in other kinds of storages. (Source : https://doi.org/10.6084/m9.figshare.7127816.v2)"@en, "Identifiant pérenne universel pour les citations bibliographiques."@fr ;
  skos:prefLabel "OCI"@en, "OCI"@es, "OCI"@fr ;
  skos:inScheme <http://data.loterre.fr/ark:/67375/TSO> ;
  skos:broader <http://data.loterre.fr/ark:/67375/TSO-H5ZG6DX6-4> ;
  skos:related <http://data.loterre.fr/ark:/67375/TSO-MZ8BL730-S> .

<http://data.loterre.fr/ark:/67375/TSO-MZ8BL730-S>
  a skos:Concept ;
  dc:modified "2021-06-24"^^xsd:date ;
  skos:altLabel "I4OC"@en ;
  skos:definition "Collaboration between scholarly publishers, researchers, and other interested parties to promote the unrestricted availability of scholarly citation data. (Source : https://i4oc.org/)"@en, "Collaboration entre les éditeurs, les chercheurs et tous les acteurs intéressés pour promouvoir la disponibilité sans restriction des données sur les citations des publications scientifiques. (Source : https://www.ouvrirlascience.fr/initiative-for-open-citations/)"@fr ;
  skos:prefLabel "Initiative for Open Citations"@en, "Initiative for Open Citations"@es, "Initiative for Open Citations"@fr ;
  skos:inScheme <http://data.loterre.fr/ark:/67375/TSO> ;
  skos:broader <http://data.loterre.fr/ark:/67375/TSO-J64S3QDL-1> ;
  skos:related <http://data.loterre.fr/ark:/67375/TSO-R1CSCWWG-D>, <http://data.loterre.fr/ark:/67375/TSO-SVH6TCP0-3> .

<http://data.loterre.fr/ark:/67375/TSO-F864TC3S-K>
  a skos:Concept ;
  dc:modified "2021-06-29"^^xsd:date ;
  skos:altLabel "almacén institucional"@es, "archive institutionnelle"@fr, "dépôt institutionnel"@fr, "institutional depository"@en ;
  skos:definition "Dépôt qui relève d’une institution (université, grande école, organisme de recherche, association professionnelle) et a pour objectif de contenir, valoriser et conserver l’ensemble de la production scientifique de celle-ci. (Source : https://openaccess.inist.fr/glossaire/)"@fr ;
  skos:prefLabel "entrepôt institutionnel"@fr, "institutional repository"@en, "repositorio institucional"@es ;
  skos:inScheme <http://data.loterre.fr/ark:/67375/TSO> ;
  skos:broader <http://data.loterre.fr/ark:/67375/TSO-W9KRS5Q3-6> ;
  skos:related <http://data.loterre.fr/ark:/67375/TSO-PGSFQSNR-1>, <http://data.loterre.fr/ark:/67375/TSO-XF2L7W5Z-V> .

<http://data.loterre.fr/ark:/67375/TSO-ZQ0Q8HMP-Q>
  a skos:Concept ;
  dc:modified "2021-06-25"^^xsd:date ;
  skos:definition "Issues dealing with the problems of whether certain behaviour is or is not compliant with the law. (Source : Foster)"@en ;
  skos:exactMatch <https://vocabularyserver.com/openscience/index.php?tema=52> ;
  skos:prefLabel "aspect légal de la science ouverte"@fr, "aspecto legal de la ciencia abierta"@es, "open science legal aspect"@en ;
  skos:inScheme <http://data.loterre.fr/ark:/67375/TSO> ;
  skos:related <http://data.loterre.fr/ark:/67375/TSO-JFJGKFN2-H> ;
  skos:narrower <http://data.loterre.fr/ark:/67375/TSO-MGZJDL80-2>, <http://data.loterre.fr/ark:/67375/TSO-RGKFQW9J-K>, <http://data.loterre.fr/ark:/67375/TSO-LJWH8NFT-D> ;
  skos:topConceptOf <http://data.loterre.fr/ark:/67375/TSO> .

<http://data.loterre.fr/ark:/67375/TSO-H0Q13JB3-N>
  a skos:Concept ;
  dc:created "2021-06-25"^^xsd:date ;
  dc:modified "2021-07-05"^^xsd:date ;
  skos:definition "A platform that provides information on all aspects of scholarly sharing. The site includes practical information and tools to ensure articles can be shared with colleagues quickly and easily. It also includes information on how you can share, where you can share and recommendations for sharing sites where you can engage and collaborate with the research community. (Source: https://www.howcanishareit.com/about-us)"@en, "Plataforma que ofrece información sobre todos los aspectos del intercambio de artículos científicos."@es, "Plateforme qui fournit des informations sur tous les aspects du partage d'articles scientifiques."@fr ;
  skos:prefLabel "How Can I Share It"@en, "How Can I Share It"@es, "How Can I Share It"@fr ;
  skos:inScheme <http://data.loterre.fr/ark:/67375/TSO> ;
  skos:broader <http://data.loterre.fr/ark:/67375/TSO-DXZZDQSM-3> .

<http://data.loterre.fr/ark:/67375/TSO-VQD3856X-4>
  a skos:Concept ;
  dc:modified "2021-06-29"^^xsd:date ;
  skos:altLabel "psychology in open access"@en ;
  skos:definition "Organisation qui œuvre pour la transition des revues de psychologie vers des modèles de publication respectant les principes du « libre accès juste »."@fr, "Organization that facilitates conversion to fair open access of journals in psychology (source: https://www.fairopenaccess.org/)"@en ;
  skos:prefLabel "psyOA"@en, "psyOA"@es, "psyOA"@fr ;
  skos:inScheme <http://data.loterre.fr/ark:/67375/TSO> ;
  skos:broader <http://data.loterre.fr/ark:/67375/TSO-J64S3QDL-1> ;
  skos:related <http://data.loterre.fr/ark:/67375/TSO-GCTBW7HJ-P> .

<http://data.loterre.fr/ark:/67375/TSO-RGFVRS3V-Q>
  a skos:Concept ;
  dc:modified "2021-06-03"^^xsd:date ;
  skos:definition "La science qui tente d’analyser l’étendue de la Toile. (Source : Foster)"@fr, "The science at which there is an attempt to compute the extent of the World Wide Web. (Source : Foster)"@en ;
  skos:exactMatch <https://vocabularyserver.com/openscience/index.php?tema=33> ;
  skos:prefLabel "webometrics"@en, "webometría"@es, "webométrie"@fr ;
  skos:inScheme <http://data.loterre.fr/ark:/67375/TSO> ;
  skos:broader <http://data.loterre.fr/ark:/67375/TSO-T9Q25G6Q-S> .

<http://data.loterre.fr/ark:/67375/TSO-W30LBC9X-X>
  a skos:Concept ;
  skos:definition "Analyse de citations utilisée en science ouverte. (Source : Foster)"@fr, "Citation and content analysis used in Open Science. (Source : Foster)"@en ;
  skos:exactMatch <https://vocabularyserver.com/openscience/index.php?tema=32> ;
  skos:prefLabel "bibliometrics"@en, "bibliometría"@es, "bibliométrie"@fr ;
  skos:inScheme <http://data.loterre.fr/ark:/67375/TSO> ;
  skos:broader <http://data.loterre.fr/ark:/67375/TSO-T9Q25G6Q-S> ;
  skos:related <http://data.loterre.fr/ark:/67375/TSO-JFR1FLWQ-R> .

<http://data.loterre.fr/ark:/67375/TSO-FTK2F4DH-T>
  a skos:Concept ;
  dc:modified "2021-06-03"^^xsd:date ;
  skos:altLabel "politique d'un établissement"@fr ;
  skos:definition "Courses of actions adopted by an academic establishment or foundation. (Source : Foster)"@en, "Lignes de conduite adoptées par un établissement universitaire ou une fondation. (Source : Foster)"@fr ;
  skos:exactMatch <https://vocabularyserver.com/openscience/index.php?tema=40> ;
  skos:prefLabel "institutional policy"@en, "politique institutionnelle"@fr, "política institucional"@es ;
  skos:inScheme <http://data.loterre.fr/ark:/67375/TSO> ;
  skos:broader <http://data.loterre.fr/ark:/67375/TSO-QL0JTPZ5-J> .

<http://data.loterre.fr/ark:/67375/TSO-F124WT34-H>
  a skos:Concept ;
  dc:modified "2021-06-18"^^xsd:date ;
  skos:altLabel "Fostering Fair Data Practices in Europe"@en ;
  skos:definition "Project funded under the H2020 programme H2020-INFRAEOSC-2018-2020 of the European Commission, that will address, over a 36 month time plan, the development and concrete realisation of an overall knowledge infrastructure on academic quality data management, procedures, standards and metrics, based on the FAIR (Findable, Accessible, Interoperable, Reusable) principles. (Source : https://www.fairsfair.eu/)"@en, "Projet coordonné par DANS (Data Archiving and Networked Services) qui a pour but d’aider les instances de gouvernance de l’EOSC (European Open Science Cloud) à mettre en place des règles de participation à l’EOSC alignées sur celles de FAIR. (Source : https://www.ouvrirlascience.fr/fairsfair-project/)"@fr ;
  skos:prefLabel "FAIRsFAIR"@en, "FAIRsFAIR"@es, "FAIRsFAIR"@fr ;
  skos:inScheme <http://data.loterre.fr/ark:/67375/TSO> ;
  skos:broader <http://data.loterre.fr/ark:/67375/TSO-H93WKMMJ-B> .

<http://data.loterre.fr/ark:/67375/TSO-H96QTTW7-Z>
  a skos:Concept ;
  dc:modified "2021-06-18"^^xsd:date ;
  skos:altLabel "Digital Republic Bill"@en, "Digital Republic Law"@en, "French Digital Republic Act"@en, "loi numérique"@fr, "loi n° 2016-1321 du 7 octobre 2016 pour une République numérique"@fr, "loi pour une République numérique"@en ;
  skos:definition "French law first voted on 10/07/2016. This law enables the government to fulfill a two-fold purpose : \"to give France a head start in the digital field by promoting an open data and knowledge policy\" and to \"adopt a progressive digital approach, based on individuals, to strengthen their power to act and their rights in the digital world\". To do so, the law is organized around three lines: the circulation of data and knowledge, the protection of individuals in the digital society and access to digital for all. (Source : Wikipedia)"@en, "Loi française promulguée le 7 octobre 2016. Par cette loi, l'objectif du gouvernement est double : « donner une longueur d'avance à la France dans le domaine du numérique en favorisant une politique d'ouverture des données et des connaissances » et « adopter une approche progressiste du numérique, qui s'appuie sur les individus, pour renforcer leur pouvoir d'agir et leurs droits dans le monde numérique ». Pour ce faire, la loi s'organise autour de trois axes : la circulation des données et du savoir, la protection des individus dans la société du numérique et l'accès au numérique pour tous. (Source : Wikipedia)"@fr ;
  skos:prefLabel "Digital Republic Act"@en, "Ley de República Digital"@es, "loi pour une République numérique"@fr ;
  skos:inScheme <http://data.loterre.fr/ark:/67375/TSO> ;
  skos:broader <http://data.loterre.fr/ark:/67375/TSO-MGZJDL80-2> .

<http://data.loterre.fr/ark:/67375/TSO-GDCXNW8F-5>
  a skos:Concept ;
  dc:modified "2021-06-17"^^xsd:date ;
  skos:definition "Research Data management comprises the disciplines related to managing research data as a valuable resource. These can include, but are not limited to, research data governance, security and quality. (Source : Foster)"@en ;
  skos:exactMatch <https://vocabularyserver.com/openscience/index.php?tema=46> ;
  skos:prefLabel "gestion des données de recherche"@fr, "gestión de datos de investigación"@es, "research data management"@en ;
  skos:inScheme <http://data.loterre.fr/ark:/67375/TSO> ;
  skos:broader <http://data.loterre.fr/ark:/67375/TSO-NJ1CVNL6-F> ;
  skos:related <http://data.loterre.fr/ark:/67375/TSO-DP8MN2RF-P>, <http://data.loterre.fr/ark:/67375/TSO-MJZBK64J-5>, <http://data.loterre.fr/ark:/67375/TSO-Q3D3R4D9-C>, <http://data.loterre.fr/ark:/67375/TSO-T4KV78Z3-L> .

<http://data.loterre.fr/ark:/67375/TSO-NJ1CVNL6-F>
  a skos:Concept ;
  dc:created "2021-06-17"^^xsd:date ;
  dc:modified "2021-06-25"^^xsd:date ;
  skos:prefLabel "data management"@en, "gestion des données"@fr, "gestión de datos"@es ;
  skos:inScheme <http://data.loterre.fr/ark:/67375/TSO> ;
  skos:broader <http://data.loterre.fr/ark:/67375/TSO-SMGMJFLJ-Q> ;
  skos:narrower <http://data.loterre.fr/ark:/67375/TSO-GDCXNW8F-5>, <http://data.loterre.fr/ark:/67375/TSO-WJBVSL22-1>, <http://data.loterre.fr/ark:/67375/TSO-K62D86BQ-H>, <http://data.loterre.fr/ark:/67375/TSO-TM6BH53Q-3>, <http://data.loterre.fr/ark:/67375/TSO-MJLHMDNM-S>, <http://data.loterre.fr/ark:/67375/TSO-B25PW4X4-N>, <http://data.loterre.fr/ark:/67375/TSO-GQVTBXJ4-X>, <http://data.loterre.fr/ark:/67375/TSO-FJ7V5LJC-R> .

<http://data.loterre.fr/ark:/67375/TSO-D91MV7TW-D>
  a skos:Concept ;
  dc:modified "2021-06-25"^^xsd:date ;
  skos:altLabel "Transparency and Openness Promotion guidelines"@en ;
  skos:definition "Directives publiées en 2015 par le Center for Open Science, déclinées en huit niveaux, et visant à promouvoir la transparence et l'ouverture des données chez les éditeurs de revues scientifiques."@fr, "Published in Science in 2015 (OA), the Transparency and Openness Promotion Guidelines (PDF and HTML) include eight modular standards, each with three levels of increasing stringency. Journals select which of the eight transparency standards they wish to implement and select a level of implementation for each. These features provide flexibility for adoption depending on disciplinary variation, but simultaneously establish community standards. (Source : Center for Open Science, https://www.cos.io/initiatives/top-guidelines)"@en ;
  skos:prefLabel "TOP guidelines"@en, "directives TOP"@fr, "directrices TOP"@es ;
  skos:inScheme <http://data.loterre.fr/ark:/67375/TSO> ;
  skos:broader <http://data.loterre.fr/ark:/67375/TSO-CV5H9HZH-V> ;
  skos:related <http://data.loterre.fr/ark:/67375/TSO-BTFX00Q2-P>, <http://data.loterre.fr/ark:/67375/TSO-STWL5MWS-W> .

<http://data.loterre.fr/ark:/67375/TSO-B8PFXG89-F>
  a skos:Concept ;
  dc:modified "2021-06-30"^^xsd:date ;
  skos:altLabel "communicación científica abierta"@es ;
  skos:definition "Accès ouvert au contenu scientifique par sa mise à disposition en ligne gratuite et sans restriction."@fr, "Open access to scholarly content by making scholarly information available online, free and unrestricted."@en ;
  skos:prefLabel "communicación académica abierta"@es, "communication savante ouverte"@fr, "open scholarly communication"@en ;
  skos:inScheme <http://data.loterre.fr/ark:/67375/TSO> ;
  skos:broader <http://data.loterre.fr/ark:/67375/TSO-SMGMJFLJ-Q> ;
  skos:related <http://data.loterre.fr/ark:/67375/TSO-DJ828LKC-C> .

<http://data.loterre.fr/ark:/67375/TSO-BQ1Q40TK-V>
  a skos:Concept ;
  dc:modified "2021-06-04"^^xsd:date ;
  skos:definition "Données gouvernementales accessibles gratuitement en ligne en vertu de conditions qui en permettent la réutilisation et la redistribution. (Source : Foster)"@fr, "Online government data, offered free of cost supported with terms that allow reuse and redistribution. (Source : Foster)"@en ;
  skos:exactMatch <https://vocabularyserver.com/openscience/index.php?tema=22> ;
  skos:prefLabel "datos gubernamentales abiertos"@es, "données gouvernementales ouvertes"@fr, "open government data"@en ;
  skos:inScheme <http://data.loterre.fr/ark:/67375/TSO> ;
  skos:broader <http://data.loterre.fr/ark:/67375/TSO-V08MCZVP-H> .

<http://data.loterre.fr/ark:/67375/TSO-K4MZGJ48-6>
  a skos:Concept ;
  dc:modified "2021-06-09"^^xsd:date ;
  skos:definition "Principaux énoncés qui ont établi le mouvement pour le libre accès aux publications scientifiques"@fr, "The leading statements having established Open Access as a movement."@en, "Three leading statements established Open Access as a movement; Budapest Open Access Initiative (2002), Bethesda Statement on Open Access Publishing (2003) and the Berlin Declaration on Open Access to Knowledge in the Sciences and Humanities (2003). (Source : Foster)"@en, "Trois principaux énoncés ont établi le mouvement pour le libre accès: l’Initiative de Budapest pour l’Accès Ouvert (2002), le Bethesda Statement on Open Access Publishing (2003) et la Déclaration de Berlin sur le libre accès à la connaissance en sciences exactes, sciences de la vie, sciences humaines et sociales (2003). (Source : Foster)"@fr ;
  skos:exactMatch <https://vocabularyserver.com/openscience/index.php?tema=12> ;
  skos:prefLabel "open access reference text"@en, "texte de référence du libre accès"@fr, "texto de referencia sobre el libre acceso"@es ;
  skos:inScheme <http://data.loterre.fr/ark:/67375/TSO> ;
  skos:broader <http://data.loterre.fr/ark:/67375/TSO-V6F4ZS65-G> ;
  skos:narrower <http://data.loterre.fr/ark:/67375/TSO-CXNG80P6-X>, <http://data.loterre.fr/ark:/67375/TSO-NK8GHW7D-6>, <http://data.loterre.fr/ark:/67375/TSO-D7TJZP51-Z> .

<http://data.loterre.fr/ark:/67375/TSO-FBNDZZDV-2>
  a skos:Concept ;
  dc:modified "2021-06-29"^^xsd:date ;
  skos:definition "Appel lancé en 2017 et qui s’adresse aux communautés scientifiques et aux établissements de recherche, en vue de promouvoir un accès ouvert aux publications scientifiques qui encourage la bibliodiversité et l’innovation et n’implique pas le transfert exclusif des abonnements vers les frais de publication (APC). (Source : https://www.ouvrirlascience.fr/appel-de-jussieu-pour-la-science-ouverte-et-la-bibliodiversite/)"@fr ;
  skos:prefLabel "Jussieu call for open science and bibliodiversity"@en, "appel de Jussieu pour la science ouverte et la bibliodiversité"@fr, "llamada de Jussieu para la ciencia abierta y la bibliodiversidad"@es ;
  skos:inScheme <http://data.loterre.fr/ark:/67375/TSO> ;
  skos:broader <http://data.loterre.fr/ark:/67375/TSO-V6F4ZS65-G> .

<http://data.loterre.fr/ark:/67375/TSO-V08MCZVP-H>
  a skos:Concept ;
  dc:modified "2021-07-05"^^xsd:date ;
  skos:definition "Datos disponibles gratuitamente en línea que pueden ser utilizados, reutilizados y distribuidos siempre que se identifique la fuente de los datos. (Fuente: Foster)"@es, "Données accessibles gratuitement en ligne qui peuvent être utilisées, réutilisées et distribuées à condition que la source des données soit identifiée. (Source : Foster)"@fr, "Online, free of cost, accessible data that can be used, reused and distributed provided that the data source is attributed. (Source : Foster)"@en ;
  skos:exactMatch <https://vocabularyserver.com/openscience/index.php?tema=3> ;
  skos:prefLabel "datos abiertos"@es, "données ouvertes"@fr, "open data"@en ;
  skos:inScheme <http://data.loterre.fr/ark:/67375/TSO> ;
  skos:broader <http://data.loterre.fr/ark:/67375/TSO-JFJGKFN2-H>, <http://data.loterre.fr/ark:/67375/TSO-MJRKBMDW-Q> ;
  skos:related <http://data.loterre.fr/ark:/67375/TSO-G591ZH6Q-X>, <http://data.loterre.fr/ark:/67375/TSO-PPDJJQ22-H> ;
  skos:narrower <http://data.loterre.fr/ark:/67375/TSO-BQ1Q40TK-V>, <http://data.loterre.fr/ark:/67375/TSO-MRSCXRR9-2>, <http://data.loterre.fr/ark:/67375/TSO-X1K9R85M-K>, <http://data.loterre.fr/ark:/67375/TSO-PCHZG84P-8>, <http://data.loterre.fr/ark:/67375/TSO-R1CSCWWG-D> .

<http://data.loterre.fr/ark:/67375/TSO-BSS8DN99-W>
  a skos:Concept ;
  dc:modified "2021-06-17"^^xsd:date ;
  skos:definition "L’acte de pratiquer la science ouverte en offrant aux utilisateurs et utilisatrices l’accès gratuit aux éléments de l’expérimentation nécessaires pour reproduire la recherche. (Source : Foster)"@fr, "The act of practicing Open Science and the provision of offering to users free access to experimental elements for research reproduction. (Source : Foster)"@en ;
  skos:exactMatch <https://vocabularyserver.com/openscience/index.php?tema=7> ;
  skos:prefLabel "investigación reproducible abierta"@es, "open reproducible research"@en, "recherche reproductible ouverte"@fr ;
  skos:inScheme <http://data.loterre.fr/ark:/67375/TSO> ;
  skos:broader <http://data.loterre.fr/ark:/67375/TSO-XK0JJTS6-2> ;
  skos:related <http://data.loterre.fr/ark:/67375/TSO-BV57RDXC-6>, <http://data.loterre.fr/ark:/67375/TSO-CXZVW41C-2>, <http://data.loterre.fr/ark:/67375/TSO-JWXHV1CM-9>, <http://data.loterre.fr/ark:/67375/TSO-W6MVTRLK-5> .

<http://data.loterre.fr/ark:/67375/TSO-GWKKFWMR-C>
  a skos:Concept ;
  dc:created "2021-06-17"^^xsd:date ;
  dc:modified "2021-06-24"^^xsd:date ;
  skos:definition "Ensemble des activités et opérations nécessaires à une gestion active des données de recherche numériques, tout au long de leur cycle de vie. L’objectif est de les rendre accessibles, partageables et réutilisables de façon pérenne. (Source : https://openaccess.inist.fr/glossaire/)"@fr ;
  skos:prefLabel "curación de datos"@es, "curation de données"@fr, "data curation"@en ;
  skos:inScheme <http://data.loterre.fr/ark:/67375/TSO> ;
  skos:broader <http://data.loterre.fr/ark:/67375/TSO-MJLHMDNM-S> .

<http://data.loterre.fr/ark:/67375/TSO-TM0MS2GV-7>
  a skos:Concept ;
  dc:modified "2021-07-05"^^xsd:date ;
  skos:altLabel "journal en libre accès"@fr ;
  skos:definition "A journal that exclusively comprises open access articles. (Source: http://www.righttoresearch.org/resources/OpenResearchGlossary)"@en, "Revista que publica únicamente artículos de acceso abierto."@es, "Revue qui ne publie que des articles en libre accès."@fr ;
  skos:prefLabel "open access journal"@en, "revista en libre acceso"@es, "revue en libre accès"@fr ;
  skos:inScheme <http://data.loterre.fr/ark:/67375/TSO> ;
  skos:broader <http://data.loterre.fr/ark:/67375/TSO-JFJGKFN2-H> ;
  skos:related <http://data.loterre.fr/ark:/67375/TSO-STWL5MWS-W> ;
  skos:narrower <http://data.loterre.fr/ark:/67375/TSO-G591ZH6Q-X>, <http://data.loterre.fr/ark:/67375/TSO-NX4NVXX2-L>, <http://data.loterre.fr/ark:/67375/TSO-RN1XP625-F>, <http://data.loterre.fr/ark:/67375/TSO-RVCX7V2W-C>, <http://data.loterre.fr/ark:/67375/TSO-QT5MLV48-P>, <http://data.loterre.fr/ark:/67375/TSO-JL9MGMVK-W> .

<http://data.loterre.fr/ark:/67375/TSO-J6QSX265-4>
  a skos:Concept ;
  dc:modified "2021-06-10"^^xsd:date ;
  skos:altLabel "VoR"@en ;
  skos:definition "The final version of a journal article as it appears from the journal’s website or bibliographic databases. Copyright to the formatting of this version lies with the publisher and it is usually not possible to upload this version to an open archive,"@en, "Version finale publiée d'un article, avec mise en page par l'éditeur et mention de copyright qui interdit parfois le dépôt dans une archive ouverte,"@fr ;
  skos:prefLabel "version of record"@en, "version éditeur"@fr, "versión final de la editorial"@es ;
  skos:inScheme <http://data.loterre.fr/ark:/67375/TSO> ;
  skos:broader <http://data.loterre.fr/ark:/67375/TSO-FP5VCTTB-4> ;
  skos:related <http://data.loterre.fr/ark:/67375/TSO-PSFFQLXV-2> .

<http://data.loterre.fr/ark:/67375/TSO-D83BMN3W-M>
  a skos:Concept ;
  skos:definition "Modèle dans lequel le financement de la publication (revue et/ou plate-forme) est pris en charge par une institution, une société savante, un organisme de recherche, une association ou une fondation. (Source : Science ouverte France)"@fr ;
  skos:prefLabel "subsidy"@en, "subvención"@es, "subvention"@fr ;
  skos:inScheme <http://data.loterre.fr/ark:/67375/TSO> ;
  skos:broader <http://data.loterre.fr/ark:/67375/TSO-MWXTBMQ8-9> .

<http://data.loterre.fr/ark:/67375/TSO-PPDJJQ22-H>
  a skos:Concept ;
  dc:modified "2021-06-10"^^xsd:date ;
  skos:definition "Norme qui devrait s’appliquer à la configuration des outils, aux formats et aux protocoles liés aux données ouvertes. (Source : Foster)"@fr, "Standard that should be applied to tool configuration, formats and protocols relating to open data. (Source : Foster)"@en ;
  skos:exactMatch <https://vocabularyserver.com/openscience/index.php?tema=19> ;
  skos:prefLabel "norma de datos abiertos"@es, "norme de données ouvertes"@fr, "open data standard"@en ;
  skos:inScheme <http://data.loterre.fr/ark:/67375/TSO> ;
  skos:broader <http://data.loterre.fr/ark:/67375/TSO-XWVJBKN6-S> ;
  skos:related <http://data.loterre.fr/ark:/67375/TSO-V08MCZVP-H> ;
  skos:narrower <http://data.loterre.fr/ark:/67375/TSO-RJP3KXDF-1> .

<http://data.loterre.fr/ark:/67375/TSO-XWVJBKN6-S>
  a skos:Concept ;
  dc:created "2021-06-10"^^xsd:date ;
  dc:modified "2021-06-10"^^xsd:date ;
  skos:prefLabel "estándar de ciencia abierta"@es, "open science standard"@en, "standard de science ouverte"@fr ;
  skos:inScheme <http://data.loterre.fr/ark:/67375/TSO> ;
  skos:narrower <http://data.loterre.fr/ark:/67375/TSO-PPDJJQ22-H>, <http://data.loterre.fr/ark:/67375/TSO-P0WRKFZJ-X>, <http://data.loterre.fr/ark:/67375/TSO-J3R15XFV-K>, <http://data.loterre.fr/ark:/67375/TSO-D2DS95K6-0>, <http://data.loterre.fr/ark:/67375/TSO-T161C80T-Q> ;
  skos:topConceptOf <http://data.loterre.fr/ark:/67375/TSO> .

<http://data.loterre.fr/ark:/67375/TSO-P0PB3HHR-8>
  a skos:Concept ;
  dc:modified "2021-07-05"^^xsd:date ;
  skos:altLabel "green OA"@en, "green open access"@en, "green road"@en, "libre accès vert"@fr ;
  skos:definition "Consiste en depositar un documento en un repositorio -antes o después ser publicado o no en una revista- sin que ello sea sufragado por nadie. (Fuente: https://universoabierto.org/2017/06/09/que-es-la-ruta-diamante-de-acceso-abierto/)"@es, "La voie verte vers le libre accès est atteinte en auto-archivant (déposant) un résultat de recherche dans un dépôt ouvert. (Source : Foster)"@fr, "The Green route to open access is delivered via self-archiving (depositing) an output into a repository. (Source : Foster)"@en ;
  skos:exactMatch <https://vocabularyserver.com/openscience/index.php?tema=15> ;
  skos:prefLabel "green route"@en, "ruta verde"@es, "voie verte"@fr ;
  skos:inScheme <http://data.loterre.fr/ark:/67375/TSO> ;
  skos:broader <http://data.loterre.fr/ark:/67375/TSO-KHL25V0F-4> ;
  skos:related <http://data.loterre.fr/ark:/67375/TSO-TM6BH53Q-3> .

<http://data.loterre.fr/ark:/67375/TSO-XZ5703Z4-Q>
  a skos:Concept ;
  dc:modified "2021-06-29"^^xsd:date ;
  skos:altLabel "archive disciplinaire"@fr, "dépôt disciplinaire"@fr, "subject depository"@en ;
  skos:definition "Dépôt qui réunit l’ensemble de la production de plusieurs institutions dans un domaine scientifique donné. (Source : https://openaccess.inist.fr/glossaire/)"@fr ;
  skos:prefLabel "almacén disciplinario"@es, "entrepôt disciplinaire"@fr, "subject repository"@en ;
  skos:inScheme <http://data.loterre.fr/ark:/67375/TSO> ;
  skos:broader <http://data.loterre.fr/ark:/67375/TSO-W9KRS5Q3-6> ;
  skos:related <http://data.loterre.fr/ark:/67375/TSO-C4027K67-Q>, <http://data.loterre.fr/ark:/67375/TSO-CX6BNH0X-Z>, <http://data.loterre.fr/ark:/67375/TSO-KBZ7QKR9-W>, <http://data.loterre.fr/ark:/67375/TSO-L1X7N7S8-V>, <http://data.loterre.fr/ark:/67375/TSO-PZNHPP7J-7>, <http://data.loterre.fr/ark:/67375/TSO-R19NG9JL-2>, <http://data.loterre.fr/ark:/67375/TSO-S30N1B85-1>, <http://data.loterre.fr/ark:/67375/TSO-S784H10S-P>, <http://data.loterre.fr/ark:/67375/TSO-WD1R50MM-6>, <http://data.loterre.fr/ark:/67375/TSO-XHFB8590-0> .

<http://data.loterre.fr/ark:/67375/TSO-TRTL77DD-T>
  a skos:Concept ;
  dc:modified "2021-07-05"^^xsd:date ;
  skos:altLabel "OSS"@en, "logiciel open source"@fr ;
  skos:definition "Logiciel dont le code source est disponible gratuitement en vertu de conditions qui en permettent la diffusion et la modification. (Source : Foster)"@fr, "Software cuyo código fuente está disponible gratuitamente en condiciones que permiten su distribución y modificación. (Fuente: Foster)"@es, "Software where the source code is available free of cost with terms that allow dissemination and adaptation. (Source : Foster)"@en ;
  skos:exactMatch <https://vocabularyserver.com/openscience/index.php?tema=29> ;
  skos:prefLabel "logiciel ouvert"@fr, "open source software"@en, "software de código abierto"@es ;
  skos:inScheme <http://data.loterre.fr/ark:/67375/TSO> ;
  skos:broader <http://data.loterre.fr/ark:/67375/TSO-JFJGKFN2-H> ;
  skos:related <http://data.loterre.fr/ark:/67375/TSO-B4WKXG50-6> .

<http://data.loterre.fr/ark:/67375/TSO-KHGQZ6NK-4>
  a skos:Concept ;
  dc:modified "2021-06-17"^^xsd:date ;
  skos:altLabel "evaluación abierta de la investigación"@es, "open evaluation of research"@en, "open science evaluation"@en, "évaluation ouverte de la recherche"@fr ;
  skos:exactMatch <https://vocabularyserver.com/openscience/index.php?tema=8> ;
  skos:prefLabel "evaluación abierta"@es, "open evaluation"@en, "évaluation ouverte"@fr ;
  skos:inScheme <http://data.loterre.fr/ark:/67375/TSO> ;
  skos:broader <http://data.loterre.fr/ark:/67375/TSO-JFJGKFN2-H>, <http://data.loterre.fr/ark:/67375/TSO-SMGMJFLJ-Q> ;
  skos:narrower <http://data.loterre.fr/ark:/67375/TSO-RZQ2K0K6-K>, <http://data.loterre.fr/ark:/67375/TSO-W81HHLG2-F>, <http://data.loterre.fr/ark:/67375/TSO-HK29ZRSC-0> .

<http://data.loterre.fr/ark:/67375/TSO-CXZVW41C-2>
  a skos:Concept ;
  dc:modified "2021-06-29"^^xsd:date ;
  skos:definition "A sequence of processes scientists make to administer and disseminate convoluted scientific examinations offered online and free of cost allowing the reuse of the material. (Source : Foster)"@en, "Séquence de processus mise en œuvre par les scientifiques pour gérer et diffuser leurs travaux de recherche, gratuitement, en ligne et en permettant la réutilisation du matériel."@fr ;
  skos:exactMatch <https://vocabularyserver.com/openscience/index.php?tema=28> ;
  skos:prefLabel "flujo de trabajo de ciencia abierta"@es, "flux de travail de science ouverte"@fr, "open science workflow"@en ;
  skos:inScheme <http://data.loterre.fr/ark:/67375/TSO> ;
  skos:broader <http://data.loterre.fr/ark:/67375/TSO-SMGMJFLJ-Q> ;
  skos:related <http://data.loterre.fr/ark:/67375/TSO-BSS8DN99-W> .

<http://data.loterre.fr/ark:/67375/TSO-STWL5MWS-W>
  a skos:Concept ;
  dc:modified "2021-07-05"^^xsd:date ;
  skos:altLabel "free open access"@en, "gratis open access"@en, "libre acceso"@es, "libre accès"@fr ;
  skos:definition "Le libre accès réfère à l’accès en ligne gratuit à du contenu scientifique évalué par les pairs, et ce, avec un nombre limité de restrictions découlant du droit d’auteur et des licences. (Source : Foster)"@fr, "Open Access refers to online, free of cost access to peer reviewed scientific content with limited copyright and licensing restrictions. (Source : Foster)"@en, "acceso gratis a investigaciones científicas evaluadas por los pares, con pocas restricciones en relación con los derechos de autor y licencias."@es ;
  skos:exactMatch <https://vocabularyserver.com/openscience/index.php?tema=2> ;
  skos:prefLabel "acceso abierto"@es, "accès ouvert"@fr, "open access"@en ;
  skos:scopeNote "Les notions recouvertes par le concept \"open access\" sont sujettes à interprétations, selon les auteurs ou les revues, qui intègrent ou non dans ce concept la notion de réutilisation."@fr ;
  skos:inScheme <http://data.loterre.fr/ark:/67375/TSO> ;
  skos:broader <http://data.loterre.fr/ark:/67375/TSO-JFJGKFN2-H> ;
  skos:related <http://data.loterre.fr/ark:/67375/TSO-B7FV4N90-B>, <http://data.loterre.fr/ark:/67375/TSO-D91MV7TW-D>, <http://data.loterre.fr/ark:/67375/TSO-FP5VCTTB-4>, <http://data.loterre.fr/ark:/67375/TSO-KHL25V0F-4>, <http://data.loterre.fr/ark:/67375/TSO-MWXTBMQ8-9>, <http://data.loterre.fr/ark:/67375/TSO-TM0MS2GV-7> ;
  skos:narrower <http://data.loterre.fr/ark:/67375/TSO-BTR6P741-6>, <http://data.loterre.fr/ark:/67375/TSO-ZMQ5Z0BN-L>, <http://data.loterre.fr/ark:/67375/TSO-WLFCMS28-F>, <http://data.loterre.fr/ark:/67375/TSO-ZWDW27C7-Q> .

<http://data.loterre.fr/ark:/67375/TSO-JFJGKFN2-H>
  a skos:Concept ;
  dc:modified "2021-06-24"^^xsd:date ;
  skos:altLabel "open access scholarship"@en, "open research"@en, "open scholarship"@en ;
  skos:definition "Mouvement qui vise à rendre la recherche et les données scientifiques, de même que leur diffusion, accessibles à tous et toutes au sein d’une société animée par un esprit de recherche."@fr, "Práctica de la ciencia, en una manera que permite la colaboración y contribución de otros individuos (investigadores o no) a partir de datos de investigación, notas de laboratorio y otros procesos de investigación que se han dispuesto como de libre acceso, en condiciones que permitan la reutilización, redistribución y reproducción de la investigación, sus datos y métodos subyacentes (Fuente: Foster)"@es, "The practice of science in such a way that others can collaborate and contribute, where research data, lab notes and other research processes are freely available, under terms that enable reuse, redistribution and reproduction of the research and its underlying data and methods. (Source : Foster)"@en ;
  skos:exactMatch <https://vocabularyserver.com/openscience/index.php?tema=1> ;
  skos:prefLabel "ciencia abierta"@es, "open science"@en, "science ouverte"@fr ;
  skos:inScheme <http://data.loterre.fr/ark:/67375/TSO> ;
  skos:related <http://data.loterre.fr/ark:/67375/TSO-H93WKMMJ-B>, <http://data.loterre.fr/ark:/67375/TSO-J64S3QDL-1>, <http://data.loterre.fr/ark:/67375/TSO-SMGMJFLJ-Q>, <http://data.loterre.fr/ark:/67375/TSO-V0KSG0NC-P>, <http://data.loterre.fr/ark:/67375/TSO-V6F4ZS65-G>, <http://data.loterre.fr/ark:/67375/TSO-ZQ0Q8HMP-Q> ;
  skos:narrower <http://data.loterre.fr/ark:/67375/TSO-V08MCZVP-H>, <http://data.loterre.fr/ark:/67375/TSO-TM0MS2GV-7>, <http://data.loterre.fr/ark:/67375/TSO-TRTL77DD-T>, <http://data.loterre.fr/ark:/67375/TSO-KHGQZ6NK-4>, <http://data.loterre.fr/ark:/67375/TSO-STWL5MWS-W>, <http://data.loterre.fr/ark:/67375/TSO-W6MVTRLK-5>, <http://data.loterre.fr/ark:/67375/TSO-FP5VCTTB-4>, <http://data.loterre.fr/ark:/67375/TSO-G9J1WQ69-H>, <http://data.loterre.fr/ark:/67375/TSO-L9LLDHZ0-5>, <http://data.loterre.fr/ark:/67375/TSO-GW6WNBGQ-X>, <http://data.loterre.fr/ark:/67375/TSO-KBRVB4PD-K> ;
  skos:topConceptOf <http://data.loterre.fr/ark:/67375/TSO> .

<http://data.loterre.fr/ark:/67375/TSO-BV57RDXC-6>
  a skos:Concept ;
  dc:modified "2021-06-02"^^xsd:date ;
  skos:altLabel "normes de réplicabilité"@fr ;
  skos:definition "Ground rules to assist with the recreation of research experiments and studies. (Source : Foster)"@en, "Règles de base pour aider à recréer les expériences et les études scientifiques. (Source : Foster)"@fr ;
  skos:exactMatch <https://vocabularyserver.com/openscience/index.php?tema=27> ;
  skos:prefLabel "normas de reproductibilidad"@es, "normes de reproductibilité"@fr, "reproducibility guidelines"@en ;
  skos:inScheme <http://data.loterre.fr/ark:/67375/TSO> ;
  skos:broader <http://data.loterre.fr/ark:/67375/TSO-CV5H9HZH-V> ;
  skos:related <http://data.loterre.fr/ark:/67375/TSO-BSS8DN99-W> .

<http://data.loterre.fr/ark:/67375/TSO-SMGMJFLJ-Q>
  a skos:Concept ;
  skos:prefLabel "open science practice"@en, "pratique de la science ouverte"@fr, "práctica de la ciencia abierta"@es ;
  skos:inScheme <http://data.loterre.fr/ark:/67375/TSO> ;
  skos:related <http://data.loterre.fr/ark:/67375/TSO-JFJGKFN2-H> ;
  skos:narrower <http://data.loterre.fr/ark:/67375/TSO-NJ1CVNL6-F>, <http://data.loterre.fr/ark:/67375/TSO-B8PFXG89-F>, <http://data.loterre.fr/ark:/67375/TSO-KHGQZ6NK-4>, <http://data.loterre.fr/ark:/67375/TSO-CXZVW41C-2>, <http://data.loterre.fr/ark:/67375/TSO-T9Q25G6Q-S>, <http://data.loterre.fr/ark:/67375/TSO-VDVFXBCR-C>, <http://data.loterre.fr/ark:/67375/TSO-GZ4Q18P7-8>, <http://data.loterre.fr/ark:/67375/TSO-XK0JJTS6-2>, <http://data.loterre.fr/ark:/67375/TSO-QWKTFN2F-N>, <http://data.loterre.fr/ark:/67375/TSO-MV5H4HGJ-2>, <http://data.loterre.fr/ark:/67375/TSO-NCN8QNX0-N>, <http://data.loterre.fr/ark:/67375/TSO-TC1HRLFR-8> ;
  skos:topConceptOf <http://data.loterre.fr/ark:/67375/TSO> .

<http://data.loterre.fr/ark:/67375/TSO-WBDZJK00-P>
  a skos:Concept ;
  dc:modified "2021-06-17"^^xsd:date ;
  skos:prefLabel "data integration"@en, "integración de los datos"@es, "intégration des données"@fr ;
  skos:inScheme <http://data.loterre.fr/ark:/67375/TSO> ;
  skos:broader <http://data.loterre.fr/ark:/67375/TSO-XK0JJTS6-2> ;
  skos:related <http://data.loterre.fr/ark:/67375/TSO-BRLNRV51-S>, <http://data.loterre.fr/ark:/67375/TSO-C676TDJV-H> .

<http://data.loterre.fr/ark:/67375/TSO-WJBVSL22-1>
  a skos:Concept ;
  dc:modified "2021-06-17"^^xsd:date ;
  skos:altLabel "découvert de données"@fr ;
  skos:prefLabel "data discovery"@en, "descubrimiento de datos"@es, "découverte de donnée"@fr ;
  skos:inScheme <http://data.loterre.fr/ark:/67375/TSO> ;
  skos:broader <http://data.loterre.fr/ark:/67375/TSO-NJ1CVNL6-F> .

<http://data.loterre.fr/ark:/67375/TSO-K62D86BQ-H>
  a skos:Concept ;
  dc:modified "2021-06-17"^^xsd:date ;
  skos:altLabel "archivage numérique pérenne"@fr ;
  skos:definition "Mode de conservation d'un document numérique ayant pour objectifs principaux de conserver le document, de le rendre accessible, d'en préserver l’intelligibilité, et ceci sur le très long terme c’est-à-dire plus de 30 ans."@fr ;
  skos:prefLabel "almacenamiento permanente"@es, "archivage pérenne"@fr, "perennial archiving"@en ;
  skos:inScheme <http://data.loterre.fr/ark:/67375/TSO> ;
  skos:broader <http://data.loterre.fr/ark:/67375/TSO-NJ1CVNL6-F> .

<http://data.loterre.fr/ark:/67375/TSO-TM6BH53Q-3>
  a skos:Concept ;
  dc:modified "2021-06-17"^^xsd:date ;
  skos:definition "Acte par lequel les chercheurs déposent eux-mêmes leurs articles dans des archives ouvertes. (Source : https://openaccess.inist.fr/glossaire/)"@fr ;
  skos:prefLabel "auto-archivage"@fr, "autoarchivo"@es, "self-archiving"@en ;
  skos:inScheme <http://data.loterre.fr/ark:/67375/TSO> ;
  skos:broader <http://data.loterre.fr/ark:/67375/TSO-NJ1CVNL6-F> ;
  skos:related <http://data.loterre.fr/ark:/67375/TSO-P0PB3HHR-8> .

<http://data.loterre.fr/ark:/67375/TSO-F2SDG44T-9>
  a skos:Concept ;
  dc:modified "2021-06-17"^^xsd:date ;
  skos:altLabel "data pseudonymization"@en ;
  skos:definition "Traitement de données à caractère personnel de telle façon que celles-ci ne puissent plus être attribuées à une personne concernée précise sans avoir recours à des informations supplémentaires. (Source : RGPD)"@fr ;
  skos:prefLabel "data pseudonymisation"@en, "pseudonymisation des données"@fr, "seudonimización de datos"@es ;
  skos:inScheme <http://data.loterre.fr/ark:/67375/TSO> ;
  skos:broader <http://data.loterre.fr/ark:/67375/TSO-MJLHMDNM-S> ;
  skos:related <http://data.loterre.fr/ark:/67375/TSO-RH261KDT-S> .

<http://data.loterre.fr/ark:/67375/TSO-MJLHMDNM-S>
  a skos:Concept ;
  dc:created "2021-06-17"^^xsd:date ;
  dc:modified "2021-06-24"^^xsd:date ;
  skos:prefLabel "data processing"@en, "procesamiento de datos"@es, "traitement des données"@fr ;
  skos:inScheme <http://data.loterre.fr/ark:/67375/TSO> ;
  skos:broader <http://data.loterre.fr/ark:/67375/TSO-NJ1CVNL6-F> ;
  skos:narrower <http://data.loterre.fr/ark:/67375/TSO-GWKKFWMR-C>, <http://data.loterre.fr/ark:/67375/TSO-F2SDG44T-9>, <http://data.loterre.fr/ark:/67375/TSO-VNNFL8WB-H> .

<http://data.loterre.fr/ark:/67375/TSO-DLBP9S2L-Z>
  a skos:Concept ;
  dc:modified "2021-06-15"^^xsd:date ;
  skos:altLabel "author-payer level"@en, "author-pays"@en, "author-side fee model"@en ;
  skos:definition "l’auteur ou son institution d’appartenance ou le bailleur de fonds donne une contribution à l’éditeur pour rendre l’article librement et gratuitement accessible à tout lecteur. (source : https://openaccess.inist.fr/glossaire/ )"@fr ;
  skos:prefLabel "author-payer model"@en, "modelo de autor-pago"@es, "modèle auteur-payeur"@fr ;
  skos:inScheme <http://data.loterre.fr/ark:/67375/TSO> ;
  skos:broader <http://data.loterre.fr/ark:/67375/TSO-P2PM5GCP-8> ;
  skos:related <http://data.loterre.fr/ark:/67375/TSO-SJ6X9JL0-3> .

<http://data.loterre.fr/ark:/67375/TSO-B25PW4X4-N>
  a skos:Concept ;
  dc:modified "2021-06-29"^^xsd:date ;
  skos:definition "Pratique qui consiste à gérer et à superviser les données d’une organisation, de façon à fournir aux utilisateurs professionnels des données de haute qualité facilement et uniformément accessibles. (Source : https://www.lemagit.fr/definition/Data-stewardship)"@fr, "The management and oversight of an organization's data assets to help provide users with high-quality data that is easily accessible in a consistent manner. (Source : https://searchdatamanagement.techtarget.com)"@en ;
  skos:prefLabel "administración de datos"@es, "data stewardship"@en, "intendance des données"@fr ;
  skos:inScheme <http://data.loterre.fr/ark:/67375/TSO> ;
  skos:broader <http://data.loterre.fr/ark:/67375/TSO-NJ1CVNL6-F> .

<http://data.loterre.fr/ark:/67375/TSO-W6MVTRLK-5>
  a skos:Concept ;
  skos:altLabel "cahier de laboratoire ouvert"@fr, "carnet de laboratoire ouvert"@fr, "open lab notebook"@en ;
  skos:definition "Dossiers, carnets, classeurs, etc. de recherche en laboratoire accessibles gratuitement en ligne en vertu de conditions qui permettent la réutilisation et la redistribution de l’information consignée. (Source : Foster)"@fr, "Laboratory research records, diaries, journals, workbooks etc. offered online free of cost with terms that allow reuse and redistribution of the recorded material. (Source : Foster)"@en ;
  skos:exactMatch <https://vocabularyserver.com/openscience/index.php?tema=24> ;
  skos:prefLabel "carnet de recherche ouvert"@fr, "cuaderno de laboratorio abierto"@es, "open laboratory notebook"@en ;
  skos:inScheme <http://data.loterre.fr/ark:/67375/TSO> ;
  skos:broader <http://data.loterre.fr/ark:/67375/TSO-JFJGKFN2-H> ;
  skos:related <http://data.loterre.fr/ark:/67375/TSO-BSS8DN99-W> .

<http://data.loterre.fr/ark:/67375/TSO-NZB6R6Z5-J>
  a skos:Concept ;
  skos:altLabel "ARK"@en, "ARK"@es, "ARK"@fr, "archival resource key"@en ;
  skos:definition "Format d’identifiant créé en 2001 par la California Digital Library (CDL) qui a vocation à identifier des ressources de tous types – physiques (échantillons destinés à une expérience scientifique, produits éditoriaux, etc.), numériques (livres numérisés, notices de catalogue, etc.) ou même immatériels (concepts). (Source : BnF)"@fr ;
  skos:prefLabel "ARK identifier"@en, "identifiant ARK"@fr, "identificador ARK"@es ;
  skos:inScheme <http://data.loterre.fr/ark:/67375/TSO> ;
  skos:broader <http://data.loterre.fr/ark:/67375/TSO-H5ZG6DX6-4> .

<http://data.loterre.fr/ark:/67375/TSO-JWXHV1CM-9>
  a skos:Concept ;
  dc:modified "2021-06-17"^^xsd:date ;
  skos:altLabel "irreproducibility study"@en ;
  skos:definition "L’acte par lequel les résultats d’une étude ou d’une expérience peuvent être reproduits. (Source : Foster)"@fr, "The act during which the results of a study or an experiment can be replicated and reproduced. (Source : Foster)"@en ;
  skos:exactMatch <https://vocabularyserver.com/openscience/index.php?tema=26> ;
  skos:prefLabel "estudio de reproducibilidad"@es, "reproducibility study"@en, "étude de reproductibilité"@fr ;
  skos:inScheme <http://data.loterre.fr/ark:/67375/TSO> ;
  skos:broader <http://data.loterre.fr/ark:/67375/TSO-XK0JJTS6-2> ;
  skos:related <http://data.loterre.fr/ark:/67375/TSO-BSS8DN99-W> ;
  skos:narrower <http://data.loterre.fr/ark:/67375/TSO-XDCZ7K0M-B> .

<http://data.loterre.fr/ark:/67375/TSO-T80NJLNF-F>
  a skos:Concept ;
  dc:modified "2021-06-25"^^xsd:date ;
  skos:altLabel "APC"@en, "APC"@es, "APC"@fr, "cargo por procesamiento de artículos"@es, "frais de traitement des articles"@fr ;
  skos:definition "A fee charged to the author, creator, or institution to cover the cost of an article, rather than charging the potential reader of the article. (Source : http://openaccess.ox.ac.uk/glossary/)"@en, "Frais payés par un auteur ou par son institution pour financer la publication d'un document dont la consultation est ensuite libre pour le lecteur."@fr ;
  skos:prefLabel "article processing charge"@en, "article processing charge"@es, "article processing charge"@fr ;
  skos:inScheme <http://data.loterre.fr/ark:/67375/TSO> ;
  skos:broader <http://data.loterre.fr/ark:/67375/TSO-V0KSG0NC-P> ;
  skos:related <http://data.loterre.fr/ark:/67375/TSO-BXDFN89K-P>, <http://data.loterre.fr/ark:/67375/TSO-SJ6X9JL0-3> .

<http://data.loterre.fr/ark:/67375/TSO-NM84XT0B-L>
  a skos:Concept ;
  dc:modified "2021-06-10"^^xsd:date ;
  skos:definition "Ability of the data to provide information that allow potential (re)users to judge the accuracy, reliability and quality of the data, and to determine whether these data meet their needs"@en ;
  skos:prefLabel "data assessability"@en, "evaluación de los datos"@es, "évaluabilité des données"@fr ;
  skos:inScheme <http://data.loterre.fr/ark:/67375/TSO> ;
  skos:broader <http://data.loterre.fr/ark:/67375/TSO-T9Q25G6Q-S> .

<http://data.loterre.fr/ark:/67375/TSO-FP5VCTTB-4>
  a skos:Concept ;
  dc:modified "2021-06-17"^^xsd:date ;
  skos:altLabel "open digital edition"@en, "publicación digital abierta"@es, "publication en accès ouvert"@fr, "édition numérique ouverte"@fr ;
  skos:prefLabel "open publication"@en, "publicación abierta"@es, "publication ouverte"@fr ;
  skos:inScheme <http://data.loterre.fr/ark:/67375/TSO> ;
  skos:broader <http://data.loterre.fr/ark:/67375/TSO-JFJGKFN2-H> ;
  skos:related <http://data.loterre.fr/ark:/67375/TSO-STWL5MWS-W> ;
  skos:narrower <http://data.loterre.fr/ark:/67375/TSO-J6QSX265-4>, <http://data.loterre.fr/ark:/67375/TSO-N8C284KM-Q>, <http://data.loterre.fr/ark:/67375/TSO-GLZ7M59Q-M> .

<http://data.loterre.fr/ark:/67375/TSO-W9KRS5Q3-6>
  a skos:Concept ;
  dc:modified "2021-06-29"^^xsd:date ;
  skos:altLabel "dépôt ouvert"@fr, "open depository"@en ;
  skos:definition "Archives ouvertes qui hébergent de la littérature scientifique et rendent leur contenu accessible gratuitement à tous et toutes à travers le monde. (Source : Foster)"@fr, "Open archives that host scientific literature and make their content freely accessible to everyone in the world. (Source : Foster)"@en ;
  skos:exactMatch <https://vocabularyserver.com/openscience/index.php?tema=45> ;
  skos:prefLabel "entrepôt ouvert"@fr, "open repository"@en, "repositorio abierto"@es ;
  skos:inScheme <http://data.loterre.fr/ark:/67375/TSO> ;
  skos:broader <http://data.loterre.fr/ark:/67375/TSO-V0KSG0NC-P> ;
  skos:related <http://data.loterre.fr/ark:/67375/TSO-CTWNT4VX-W>, <http://data.loterre.fr/ark:/67375/TSO-GGMFZZJF-V>, <http://data.loterre.fr/ark:/67375/TSO-GLZ7M59Q-M>, <http://data.loterre.fr/ark:/67375/TSO-SXD143PV-3>, <http://data.loterre.fr/ark:/67375/TSO-TZDDF74F-J>, <http://data.loterre.fr/ark:/67375/TSO-Z0X2RFQK-4> ;
  skos:narrower <http://data.loterre.fr/ark:/67375/TSO-F864TC3S-K>, <http://data.loterre.fr/ark:/67375/TSO-XZ5703Z4-Q>, <http://data.loterre.fr/ark:/67375/TSO-ZNX5Z1VV-S>, <http://data.loterre.fr/ark:/67375/TSO-XBFF1KGS-V>, <http://data.loterre.fr/ark:/67375/TSO-B8RHV59S-0>, <http://data.loterre.fr/ark:/67375/TSO-LJ49Q4WZ-R>, <http://data.loterre.fr/ark:/67375/TSO-K8V0VJW2-2> .

<http://data.loterre.fr/ark:/67375/TSO-M6RFTL22-T>
  a skos:Concept ;
  skos:definition "Identifiant personnel unique géré dans HAL. Il permet à un utilisateur authentifié, connu comme auteur dans HAL, de regrouper toutes ses publications, quelles que soient les différentes formes sous lesquelles son nom a pu être saisi et d’en choisir une par défaut. (source: https://doc.archives-ouvertes.fr/identifiant-auteur-idhal-cv/)"@fr ;
  skos:prefLabel "IdHAL"@en, "IdHAL"@es, "IdHAL"@fr ;
  skos:inScheme <http://data.loterre.fr/ark:/67375/TSO> ;
  skos:broader <http://data.loterre.fr/ark:/67375/TSO-H5ZG6DX6-4> .

<http://data.loterre.fr/ark:/67375/TSO-FC8JNWR9-L>
  a skos:Concept ;
  skos:definition "Identifiant pérenne attribué à des objets numériques et à d'autres ressources Internet pour fournir l’information nécessaire à la localisation, à l'accès et à l’usage, développé avec le soutien initial de la Defense Advanced Research Projects Agency (DARPA) et géré par la Corporation for National Research Initiatives (CNRI). (Source : Wikipédia)"@fr ;
  skos:prefLabel "handle"@en, "handle"@es, "handle"@fr ;
  skos:inScheme <http://data.loterre.fr/ark:/67375/TSO> ;
  skos:broader <http://data.loterre.fr/ark:/67375/TSO-H5ZG6DX6-4> .

<http://data.loterre.fr/ark:/67375/TSO-V0HZ66HD-4>
  a skos:Concept ;
  dc:modified "2021-07-05"^^xsd:date ;
  skos:definition "Refers to the scholarly communication resources and services, including software, that we depend upon to enable the scientific and scholarly community to collect, store, organise, access, share, and assess research. (Sources : SCOSS)"@en, "Ressources et services de communication scientifique, y compris les logiciels, dont nous dépendons pour permettre à la communauté scientifique et universitaire de collecter, stocker, organiser, accéder, partager et évaluer la recherche."@fr, "Se refiere a los recursos y servicios de comunicación académica, incluido el software, de los que dependemos para permitir a la comunidad científica y académica recopilar, almacenar, organizar, acceder, compartir y evaluar la investigación."@es ;
  skos:prefLabel "infraestructura de la ciencia abierta"@es, "infrastructure de la science ouverte"@fr, "open science infrastructure"@en ;
  skos:inScheme <http://data.loterre.fr/ark:/67375/TSO> ;
  skos:narrower <http://data.loterre.fr/ark:/67375/TSO-CVMGJVKW-W>, <http://data.loterre.fr/ark:/67375/TSO-DXZZDQSM-3>, <http://data.loterre.fr/ark:/67375/TSO-LS0Q2K68-D>, <http://data.loterre.fr/ark:/67375/TSO-G4MG47JW-H>, <http://data.loterre.fr/ark:/67375/TSO-GHZRN0P9-2>, <http://data.loterre.fr/ark:/67375/TSO-B66RVJ4T-J>, <http://data.loterre.fr/ark:/67375/TSO-LSLV4BQG-0>, <http://data.loterre.fr/ark:/67375/TSO-QC8N3MRN-X>, <http://data.loterre.fr/ark:/67375/TSO-QK42D772-3>, <http://data.loterre.fr/ark:/67375/TSO-PM46WP7W-P>, <http://data.loterre.fr/ark:/67375/TSO-TWKDXTXK-N>, <http://data.loterre.fr/ark:/67375/TSO-JXVPRHLQ-P>, <http://data.loterre.fr/ark:/67375/TSO-M32F3P1Q-K>, <http://data.loterre.fr/ark:/67375/TSO-HZ175K8D-R>, <http://data.loterre.fr/ark:/67375/TSO-WZ6DJ64Q-P> ;
  skos:topConceptOf <http://data.loterre.fr/ark:/67375/TSO> .

<http://data.loterre.fr/ark:/67375/TSO-RPCFB5QW-0>
  a skos:Concept ;
  dc:modified "2021-06-24"^^xsd:date ;
  skos:altLabel "HAL archive ouverte"@fr, "hyper articles en ligne"@fr, "open archive HAL"@en ;
  skos:definition "open archive where authors can deposit scholarly documents from all academic fields. (source: https://en.wikipedia.org/wiki/HAL_(open_archive))"@en, "plateforme en ligne destinée au dépôt et à la diffusion d'articles de chercheurs publiés ou non, et de thèses, émanant des établissements d'enseignement et de recherche français ou étrangers, des laboratoires publics ou privés. (source: https://fr.wikipedia.org/wiki/HAL_(archive_ouverte))"@fr ;
  skos:prefLabel "HAL"@en, "HAL"@es, "HAL"@fr ;
  skos:inScheme <http://data.loterre.fr/ark:/67375/TSO> ;
  skos:broader <http://data.loterre.fr/ark:/67375/TSO-HZ175K8D-R> ;
  skos:related <http://data.loterre.fr/ark:/67375/TSO-GLZ7M59Q-M> .

<http://data.loterre.fr/ark:/67375/TSO-LQV42R36-F>
  a skos:Concept ;
  dc:modified "2021-06-24"^^xsd:date ;
  skos:definition "archive ouverte de prépublications électroniques d'articles scientifiques dans les domaines de la physique, des mathématiques, de l'informatique, de la biologie quantitative, de la finance quantitative, de la statistique, de l'ingénierie électrique et des systèmes, et de l'économie, et qui est accessible gratuitement par Internet (source: https://fr.wikipedia.org/wiki/ArXiv)"@fr, "free distribution service and an open-access archive (source: https://arxiv.org/)"@en ;
  skos:prefLabel "arXiv"@en, "arXiv"@es, "arXiv"@fr ;
  skos:inScheme <http://data.loterre.fr/ark:/67375/TSO> ;
  skos:broader <http://data.loterre.fr/ark:/67375/TSO-HZ175K8D-R> ;
  skos:related <http://data.loterre.fr/ark:/67375/TSO-GLZ7M59Q-M> .

<http://data.loterre.fr/ark:/67375/TSO-Z3M8CHXM-K>
  a skos:Concept ;
  dc:modified "2021-06-29"^^xsd:date ;
  skos:altLabel "Open Access Publishing in European Networks"@en, "Open Access Publishing in European Networks"@fr ;
  skos:definition "Bibliothèque en ligne et plateforme de publication qui promeut et soutient la transition vers l'accès libre pour les ouvrages universitaires en fournissant des services d'infrastructure ouverte."@fr, "Online library and publication platform that promotes and supports the transition to open access for academic books by providing open infrastructure services to stakeholders in scholarly communication. (source: https://www.oapen.org/home)"@en ;
  skos:prefLabel "OAPEN"@en, "OAPEN"@es, "OAPEN"@fr ;
  skos:inScheme <http://data.loterre.fr/ark:/67375/TSO> ;
  skos:broader <http://data.loterre.fr/ark:/67375/TSO-WZ6DJ64Q-P> .

<http://data.loterre.fr/ark:/67375/TSO-G0NHM0CJ-G>
  a skos:Concept ;
  dc:modified "2021-07-05"^^xsd:date ;
  skos:definition "Independent infrastructure organization for open scholarship dedicated to the publication of open bibliographic and citation data by the use of Semantic Web (Linked Data) technologies. (Source : http://opencitations.net/)"@en, "Organisation indépendante dédiée à la publication de données bibliographiques et de citations ouvertes, par l'utilisation des technologies du Web sémantique."@fr, "Organización independiente dedicada a la publicación de datos bibliográficos y citas abiertas, utilizando tecnologías de la web semántica."@es ;
  skos:prefLabel "OpenCitations"@en, "OpenCitations"@es, "OpenCitations"@fr ;
  skos:inScheme <http://data.loterre.fr/ark:/67375/TSO> ;
  skos:broader <http://data.loterre.fr/ark:/67375/TSO-LS0Q2K68-D> .

<http://data.loterre.fr/ark:/67375/TSO-CVMGJVKW-W>
  a skos:Concept ;
  dc:created "2021-06-10"^^xsd:date ;
  dc:modified "2021-07-05"^^xsd:date ;
  skos:definition "Colección de documentos digitales (es decir, digitalizados o nacidos digitalmente) (textos, imágenes, sonidos) accesibles a distancia (en particular a través de Internet), que ofrecen al público diferentes formas de acceder a la información."@es, "Collection de documents (textes, images, sons) numériques (c'est-à-dire numérisés ou nés numériques) accessibles à distance (en particulier via Internet), proposant différentes modalités d'accès à l'information aux publics. (Source : https://fr.wikipedia.org/wiki/Biblioth%C3%A8que_num%C3%A9rique)"@fr, "Collection of digital (i.e. digitised or born digital) documents (texts, images, sounds) accessible at a distance (in particular via the Internet), offering different ways of access to information to the public."@en ;
  skos:prefLabel "biblioteca digital"@es, "bibliothèque numérique"@fr, "digital library"@en ;
  skos:inScheme <http://data.loterre.fr/ark:/67375/TSO> ;
  skos:broader <http://data.loterre.fr/ark:/67375/TSO-V0HZ66HD-4> ;
  skos:narrower <http://data.loterre.fr/ark:/67375/TSO-MZGVP0JH-N>, <http://data.loterre.fr/ark:/67375/TSO-XPQ718XW-Z>, <http://data.loterre.fr/ark:/67375/TSO-XJJ971XL-H>, <http://data.loterre.fr/ark:/67375/TSO-SZC96ZN0-H>, <http://data.loterre.fr/ark:/67375/TSO-C4J2BDKS-X>, <http://data.loterre.fr/ark:/67375/TSO-KD25R88J-S> .

<http://data.loterre.fr/ark:/67375/TSO-PN5FRJJD-7>
  a skos:Concept ;
  dc:modified "2021-06-29"^^xsd:date ;
  skos:altLabel "Directory of Open Access Journals"@en, "Directory of Open Access Journals"@fr ;
  skos:definition "Community-curated online directory that indexes and provides access to high quality, open access, peer-reviewed journals. (source: https://doaj.org/)"@en, "Répertoire de revues scientifiques dont les articles sont évalués par les pairs et en libre accès. (Source : https://www.ouvrirlascience.fr/directory-of-open-access-journals-doaj/)"@fr ;
  skos:prefLabel "DOAJ"@en, "DOAJ"@es, "DOAJ"@fr ;
  skos:inScheme <http://data.loterre.fr/ark:/67375/TSO> ;
  skos:broader <http://data.loterre.fr/ark:/67375/TSO-JN2ZSNST-6> .

<http://data.loterre.fr/ark:/67375/TSO-F3J3B0FG-2>
  a skos:Concept ;
  dc:modified "2021-06-25"^^xsd:date ;
  skos:altLabel "Directory of Open Access Books"@en, "Directory of Open Access Books"@fr ;
  skos:definition "Community-driven discovery service that indexes and provides access to scholarly, peer-reviewed open access books and helps users to find trusted open access book publishers. All DOAB services are free of charge and all data is freely available. (source: https://doabooks.org/)"@en, "Répertoire de livres en libre accès."@fr ;
  skos:prefLabel "DOAB"@en, "DOAB"@es, "DOAB"@fr ;
  skos:inScheme <http://data.loterre.fr/ark:/67375/TSO> ;
  skos:broader <http://data.loterre.fr/ark:/67375/TSO-JN2ZSNST-6> .

<http://data.loterre.fr/ark:/67375/TSO-X239JT56-0>
  a skos:Concept ;
  dc:modified "2021-07-05"^^xsd:date ;
  skos:definition "An online resource that aggregates and analyses publisher open access policies from around the world and provides summaries of publisher copyright and open access archiving policies on a journal-by-journal basis. (Source : https://v2.sherpa.ac.uk/romeo/about.html)"@en, "Base de datos elaborada por SHERPA, con sede en la Universidad de Nottingham, que registra las políticas de copyright y autoarchivo de las revistas científicas."@es, "Base de données produite par SHERPA, basé à l'université de Nottingham, qui recense les politiques des revues scientifiques en matière de droit d'auteur et d'auto-archivage. (Source : https://fr.wikipedia.org/wiki/SHERPA/RoMEO)"@fr ;
  skos:prefLabel "Sherpa Romeo"@en, "Sherpa Romeo"@es, "Sherpa Romeo"@fr ;
  skos:inScheme <http://data.loterre.fr/ark:/67375/TSO> ;
  skos:broader <http://data.loterre.fr/ark:/67375/TSO-QK42D772-3> .

<http://data.loterre.fr/ark:/67375/TSO-JKWW3PW1-7>
  a skos:Concept ;
  dc:modified "2021-06-25"^^xsd:date ;
  skos:altLabel "FJN"@en ;
  skos:definition "A nonprofit corporation that promotes scholarly journals run according to the Fair Open Access model. (Source : https://freejournals.org/)"@en, "Société à but non lucratif qui promeut les revues scientifiques gérées selon le modèle du Fair Open Access."@fr, "índice de revistas académicas de acceso abierto, específicamente para aquellos que no cobran cargos por procesamiento de artículos. (fuente: Wikipedia)"@es ;
  skos:prefLabel "Free Journal Network"@en, "Free Journal Network"@es, "Free Journal Network"@fr ;
  skos:inScheme <http://data.loterre.fr/ark:/67375/TSO> ;
  skos:broader <http://data.loterre.fr/ark:/67375/TSO-JN2ZSNST-6> ;
  skos:related <http://data.loterre.fr/ark:/67375/TSO-GKLZDCG9-4> .

<http://data.loterre.fr/ark:/67375/TSO-CTWNT4VX-W>
  a skos:Concept ;
  dc:modified "2021-06-29"^^xsd:date ;
  skos:altLabel "ORE"@en ;
  skos:definition "Open access publishing platform for the publication of research stemming from Horizon 2020 funding across all subject areas. (Source : https://open-research-europe.ec.europa.eu/)"@en, "Plateforme de publication de la Commission européenne, destinée à publier les articles scientifiques issus des travaux de recherche financés par Horizon Europe, le programme de recherche et d’innovation de l’UE pour la période 2021-2027, et par son prédécesseur, Horizon 2020."@fr ;
  skos:prefLabel "Open Research Europe"@en, "Open Research Europe"@es, "Open Research Europe"@fr ;
  skos:inScheme <http://data.loterre.fr/ark:/67375/TSO> ;
  skos:broader <http://data.loterre.fr/ark:/67375/TSO-WZ6DJ64Q-P> ;
  skos:related <http://data.loterre.fr/ark:/67375/TSO-W9KRS5Q3-6> .

<http://data.loterre.fr/ark:/67375/TSO-DXZZDQSM-3>
  a skos:Concept ;
  dc:created "2021-06-10"^^xsd:date ;
  dc:modified "2021-06-24"^^xsd:date ;
  skos:prefLabel "dissemination infrastructure"@en, "infraestructura de difusión"@es, "infrastructure de diffusion"@fr ;
  skos:inScheme <http://data.loterre.fr/ark:/67375/TSO> ;
  skos:broader <http://data.loterre.fr/ark:/67375/TSO-V0HZ66HD-4> ;
  skos:related <http://data.loterre.fr/ark:/67375/TSO-X3TNSQ40-M> ;
  skos:narrower <http://data.loterre.fr/ark:/67375/TSO-H0Q13JB3-N>, <http://data.loterre.fr/ark:/67375/TSO-BXDFN89K-P>, <http://data.loterre.fr/ark:/67375/TSO-BRNV0DF5-3>, <http://data.loterre.fr/ark:/67375/TSO-J0H32WL6-Z>, <http://data.loterre.fr/ark:/67375/TSO-VGLQ1M4D-M>, <http://data.loterre.fr/ark:/67375/TSO-XW567W8B-4> .

<http://data.loterre.fr/ark:/67375/TSO-WQ9RZCBH-P>
  a skos:Concept ;
  dc:created "2021-06-10"^^xsd:date ;
  dc:modified "2021-06-10"^^xsd:date ;
  skos:prefLabel "repertorio de almacenes"@es, "repository registry"@en, "répertoire d'entrepôts"@fr ;
  skos:inScheme <http://data.loterre.fr/ark:/67375/TSO> ;
  skos:broader <http://data.loterre.fr/ark:/67375/TSO-B66RVJ4T-J> ;
  skos:narrower <http://data.loterre.fr/ark:/67375/TSO-Z0X2RFQK-4>, <http://data.loterre.fr/ark:/67375/TSO-VJVHPV6M-P>, <http://data.loterre.fr/ark:/67375/TSO-SJ4WNCS6-L> .

<http://data.loterre.fr/ark:/67375/TSO-NT6B4GTK-3>
  a skos:Concept ;
  dc:modified "2021-06-10"^^xsd:date ;
  skos:definition "Plate-forme d’hébergement d'épi-revues en libre accès, développée et administrée par le CCSD (Centre pour la Communication Scientifique Directe)."@fr ;
  skos:prefLabel "Episciences"@en, "Episciences"@es, "Episciences"@fr ;
  skos:inScheme <http://data.loterre.fr/ark:/67375/TSO> ;
  skos:broader <http://data.loterre.fr/ark:/67375/TSO-WZ6DJ64Q-P> ;
  skos:related <http://data.loterre.fr/ark:/67375/TSO-NX4NVXX2-L> .

<http://data.loterre.fr/ark:/67375/TSO-MDD3CCP5-9>
  a skos:Concept ;
  dc:modified "2021-07-05"^^xsd:date ;
  skos:altLabel "PCI"@en ;
  skos:definition "Non-profit scientific organization that aims to create specific communities of researchers reviewing and recommending, for free, unpublished preprints in their field."@en, "Plataforma gratuita de acceso abierto que permite a los autores que han enviado su manuscrito a un servidor de preimpresos que éste sea evaluado y recomendado por un riguroso proceso de revisión por pares y que se convierta en una referencia por derecho propio."@es, "Plateforme gratuite en accès libre qui permet aux auteurs ayant déposé le manuscrit de leur article sur un serveur de preprints d’en obtenir l’évaluation et la recommandation par une procédure rigoureuse de peer reviewing et d'en faire une référence à part entière."@fr ;
  skos:prefLabel "Peer Community In"@fr, "Peer Community in"@en, "Peer Community in"@es ;
  skos:inScheme <http://data.loterre.fr/ark:/67375/TSO> ;
  skos:broader <http://data.loterre.fr/ark:/67375/TSO-QK42D772-3> ;
  skos:related <http://data.loterre.fr/ark:/67375/TSO-GLZ7M59Q-M>, <http://data.loterre.fr/ark:/67375/TSO-HK29ZRSC-0> .

<http://data.loterre.fr/ark:/67375/TSO-WD1R50MM-6>
  a skos:Concept ;
  dc:modified "2021-06-24"^^xsd:date ;
  skos:definition "Archive gratuite de dépôt et de diffusion de preprints en sciences biologiques hébergée par le Cold Spring Harbor Laboratory (CHSL), institution américaine privée à but non lucratif. (Source : CIRAD)"@fr, "The preprint server for biology. (Source: https://www.biorxiv.org/)"@en ;
  skos:prefLabel "bioRxiv"@en, "bioRxiv"@es, "bioRxiv"@fr ;
  skos:inScheme <http://data.loterre.fr/ark:/67375/TSO> ;
  skos:broader <http://data.loterre.fr/ark:/67375/TSO-HZ175K8D-R> ;
  skos:related <http://data.loterre.fr/ark:/67375/TSO-GLZ7M59Q-M>, <http://data.loterre.fr/ark:/67375/TSO-XZ5703Z4-Q> .

<http://data.loterre.fr/ark:/67375/TSO-PZNHPP7J-7>
  a skos:Concept ;
  dc:modified "2021-06-29"^^xsd:date ;
  skos:definition "Serveur de prépublications en sciences médicales."@fr, "The preprint server for health sciences. (Source : https://www.medrxiv.org/)"@en ;
  skos:prefLabel "medRxiv"@en, "medRxiv"@es, "medRxiv"@fr ;
  skos:inScheme <http://data.loterre.fr/ark:/67375/TSO> ;
  skos:broader <http://data.loterre.fr/ark:/67375/TSO-HZ175K8D-R> ;
  skos:related <http://data.loterre.fr/ark:/67375/TSO-GLZ7M59Q-M>, <http://data.loterre.fr/ark:/67375/TSO-XZ5703Z4-Q> .

<http://data.loterre.fr/ark:/67375/TSO-GGMFZZJF-V>
  a skos:Concept ;
  dc:modified "2021-07-05"^^xsd:date ;
  skos:definition "An open source, community driven project that takes a unique approach to data publication and digital preservation. Dryad focuses on search, presentation, and discovery and delegates the responsibility for the data preservation function to the underlying repository with which it is integrated. (Source: https://datadryad.org/)"@en, "Archivo internacional de datos contenidos en los artículos revisados por pares en el ámbito de las bio-ciencias básicas y aplicadas. Este repositorio permite a los científicos validar las conclusiones publicadas, explorar nuevas metodologías de análisis y reutilizar los datos para una nueva investigación. Dryad está regido por un consorcio de revistas que promueven el archivo colaborativo de datos y garantizan la sostenibilidad del repositorio. (Fuente: https://usalbiomedica.wordpress.com/2012/03/07/dryad-repositorio-de-datos-cientificos/)"@es, "Entrepôt international de données de recherche en libre accès (principalement en biologie évolutive, génétique et écologie) qui permet de découvrir, de réutiliser librement et de citer des données."@fr ;
  skos:prefLabel "Dryad"@en, "Dryad"@es, "Dryad"@fr ;
  skos:inScheme <http://data.loterre.fr/ark:/67375/TSO> ;
  skos:broader <http://data.loterre.fr/ark:/67375/TSO-LS0Q2K68-D> ;
  skos:related <http://data.loterre.fr/ark:/67375/TSO-W9KRS5Q3-6> .

<http://data.loterre.fr/ark:/67375/TSO-QV209F26-T>
  a skos:Concept ;
  dc:modified "2021-06-29"^^xsd:date ;
  skos:definition "A curated, informative and educational resource on data and metadata standards, inter-related to databases and data policies (Source: https://fairsharing.org/)"@en, "Portail web donnant accès à un catalogue de trois registres interconnectés, contenant des descriptions de normes, de bases de données et de politiques en matière de données."@fr ;
  skos:prefLabel "FAIRsharing"@en, "FAIRsharing"@es, "FAIRsharing"@fr ;
  skos:inScheme <http://data.loterre.fr/ark:/67375/TSO> ;
  skos:broader <http://data.loterre.fr/ark:/67375/TSO-B66RVJ4T-J> .

<http://data.loterre.fr/ark:/67375/TSO-SXD143PV-3>
  a skos:Concept ;
  dc:modified "2021-07-05"^^xsd:date ;
  skos:definition "Digital repository where users can make all of their research outputs available in a citable, shareable and discoverable manner. (Source: https://figshare.com/about)"@en, "Entrepôt de données dans lequel les chercheurs peuvent mettre à disposition tous les résultats de leurs recherches, afin qu'ils puissent être cités, partagés et découverts."@fr, "Repositorio donde los investigadores pueden poner a disposición todos los resultados de sus investigaciones para citarlos, compartirlos y descubrirlos."@es ;
  skos:prefLabel "Figshare"@en, "Figshare"@es, "Figshare"@fr ;
  skos:inScheme <http://data.loterre.fr/ark:/67375/TSO> ;
  skos:broader <http://data.loterre.fr/ark:/67375/TSO-LS0Q2K68-D> ;
  skos:related <http://data.loterre.fr/ark:/67375/TSO-W9KRS5Q3-6> .

<http://data.loterre.fr/ark:/67375/TSO-JN2ZSNST-6>
  a skos:Concept ;
  dc:created "2021-06-10"^^xsd:date ;
  dc:modified "2021-06-10"^^xsd:date ;
  skos:prefLabel "journal registry"@en, "repertorio de revistas"@es, "répertoire de revues"@fr ;
  skos:inScheme <http://data.loterre.fr/ark:/67375/TSO> ;
  skos:broader <http://data.loterre.fr/ark:/67375/TSO-B66RVJ4T-J> ;
  skos:narrower <http://data.loterre.fr/ark:/67375/TSO-PN5FRJJD-7>, <http://data.loterre.fr/ark:/67375/TSO-F3J3B0FG-2>, <http://data.loterre.fr/ark:/67375/TSO-JKWW3PW1-7>, <http://data.loterre.fr/ark:/67375/TSO-JBQFB4MB-P>, <http://data.loterre.fr/ark:/67375/TSO-WFN6D4TN-J>, <http://data.loterre.fr/ark:/67375/TSO-GP1DN83S-L> .

<http://data.loterre.fr/ark:/67375/TSO-MSSFPBQ3-S>
  a skos:Concept ;
  dc:modified "2021-06-25"^^xsd:date ;
  skos:definition "Portail de ressources électroniques en sciences humaines et sociales créé par le Centre pour l'édition électronique ouverte, centre spécialisé dans le domaine de l'édition électronique associant le CNRS, l'EHESS, l'Université d'Aix-Marseille et l'Université d'Avignon. C'est une initiative publique travaillant en faveur de l'accès ouvert aux résultats de la recherche scientifique. (Source : https://fr.wikipedia.org/wiki/OpenEdition)"@fr ;
  skos:prefLabel "OpenEdition"@en, "OpenEdition"@es, "OpenEdition"@fr ;
  skos:inScheme <http://data.loterre.fr/ark:/67375/TSO> ;
  skos:broader <http://data.loterre.fr/ark:/67375/TSO-WZ6DJ64Q-P> .

<http://data.loterre.fr/ark:/67375/TSO-W2TL7C50-G>
  a skos:Concept ;
  dc:modified "2021-07-05"^^xsd:date ;
  skos:altLabel "Nuage de données Open Science"@fr, "Open Science Data Cloud"@en, "Open Science Data Cloud"@es, "Open Science Data Cloud"@fr ;
  skos:definition "A data science ecosystem in which researchers can house and share their own scientific data, access complementary public datasets, build and share customized virtual machines with whatever tools necessary to analyze their data, and perform the analysis to answer their research questions. (Source : OSDC)"@en, "Ecosistema de ciencia de datos en el que los investigadores pueden albergar y compartir sus propios datos científicos, acceder a conjuntos de datos públicos complementarios, construir y compartir máquinas virtuales personalizadas con las herramientas necesarias para analizar sus datos y realizar el análisis para responder a sus preguntas de investigación."@es, "Fournit à la communauté scientifique des ressources pour stocker, partager et analyser des ensembles de données scientifiques à l'échelle du téraoctet et du pétaoctet. (Source : https://access2perspectives.org/)"@fr ;
  skos:prefLabel "OSDC"@en, "OSDC"@es, "OSDC"@fr ;
  skos:inScheme <http://data.loterre.fr/ark:/67375/TSO> ;
  skos:broader <http://data.loterre.fr/ark:/67375/TSO-LS0Q2K68-D> .

<http://data.loterre.fr/ark:/67375/TSO-TZDDF74F-J>
  a skos:Concept ;
  dc:modified "2021-06-24"^^xsd:date ;
  skos:definition "A general-purpose open-access repository developed under the European OpenAIRE program and operated by CERN. It allows researchers to deposit research papers, data sets, research software, reports, and any other research related digital artifacts. (Source : Wikipedia)"@en, "Repositorio de acceso abierto de propósito general desarrollado bajo el programa europeo OpenAIRE y operado por CERN. Permite a los investigadores depositar artículos de investigación, conjuntos de datos, software de investigación, informes y cualquier otro artefacto digital relacionado con la investigación. (Fuente: Wikipedia)"@es, "Service d'entrepôt de données du CERN (European Organization for Nuclear Research) issu d’une collaboration avec OpenAire (Open Access Infrastructure for Research in Europe) et financé par la Commission Européenne. L’entrepôt Zenodo a pour objectif le partage des résultats de la recherche (publications et données de recherche) pour lesquels on ne dispose pas de dépôts institutionnels, disciplinaires ou thématiques. (Source : https://cat.opidor.fr/index.php/Zenodo)"@fr ;
  skos:prefLabel "Zenodo"@en, "Zenodo"@es, "Zenodo"@fr ;
  skos:inScheme <http://data.loterre.fr/ark:/67375/TSO> ;
  skos:broader <http://data.loterre.fr/ark:/67375/TSO-LS0Q2K68-D> ;
  skos:related <http://data.loterre.fr/ark:/67375/TSO-W9KRS5Q3-6> .

<http://data.loterre.fr/ark:/67375/TSO-L1X7N7S8-V>
  a skos:Concept ;
  dc:modified "2021-06-29"^^xsd:date ;
  skos:definition "A free preprint service for the psychological sciences maintained by The Society for the Improvement of Psychological Science. (Source : https://psyarxiv.com/)"@en, "Service de dépôt de prépublications en sciences psychologiques, géré par la Society for the Improvement of Psychological Science."@fr ;
  skos:prefLabel "PsyArXiv"@en, "PsyArXiv"@es, "PsyArXiv"@fr ;
  skos:inScheme <http://data.loterre.fr/ark:/67375/TSO> ;
  skos:broader <http://data.loterre.fr/ark:/67375/TSO-HZ175K8D-R> ;
  skos:related <http://data.loterre.fr/ark:/67375/TSO-GLZ7M59Q-M>, <http://data.loterre.fr/ark:/67375/TSO-XZ5703Z4-Q> .

<http://data.loterre.fr/ark:/67375/TSO-RCJ760D7-P>
  a skos:Concept ;
  dc:modified "2021-06-10"^^xsd:date ;
  skos:definition "A French public infrastructure which develops a comprehensive publishing infrastructure based on a modular service catalog towards scientific communities publishing in LaTeX. It also includes a dissemination platform for open access scientific publications. (Source : https://www.centre-mersenne.org)"@en, "Centro editorial para ayudar a las revistas matemáticas de acceso abierto. (fuente: Wikipedia)"@es, "Infrastructure publique française d'édition au service de la communauté scientifique. Elle vise à promouvoir l’édition scientifique et la diffusion de publications (revues, livres, séminaires et colloques) de toutes disciplines scientifiques (mathématiques, physique, statistiques, informatique…), nationales et internationales, engagées dans le libre accès. (Source : https://www.centre-mersenne.org)"@fr ;
  skos:prefLabel "Centre Mersenne"@en, "centre Mersenne"@fr, "centro Mersenne"@es ;
  skos:inScheme <http://data.loterre.fr/ark:/67375/TSO> ;
  skos:broader <http://data.loterre.fr/ark:/67375/TSO-WZ6DJ64Q-P> .

<http://data.loterre.fr/ark:/67375/TSO-XF2L7W5Z-V>
  a skos:Concept ;
  dc:modified "2021-06-29"^^xsd:date ;
  skos:altLabel "Caltech Collection of Open Digital Archives"@en ;
  skos:definition "A collection of the institution's research publications and other content, created by CalTech Library"@en, "Dépôt institutionnel lancé en 1999 par le “California Institute of Technology” de Pasadena."@fr ;
  skos:prefLabel "CODA"@en, "CODA"@es, "CODA"@fr ;
  skos:inScheme <http://data.loterre.fr/ark:/67375/TSO> ;
  skos:broader <http://data.loterre.fr/ark:/67375/TSO-HZ175K8D-R> ;
  skos:related <http://data.loterre.fr/ark:/67375/TSO-F864TC3S-K> .

<http://data.loterre.fr/ark:/67375/TSO-MZGVP0JH-N>
  a skos:Concept ;
  dc:modified "2021-07-05"^^xsd:date ;
  skos:altLabel "Connecting Repositories"@en, "Connecting Repositories"@fr ;
  skos:definition "A platform which mission is to aggregate all open access research worldwide and deliver unrestricted access for all. (Source : https://core.ac.uk/)"@en, "Agregador de documentos de investigación de libre acceso proporcionado por el Knowledge Media Institute, con sede en la Open University, Reino Unido."@es, "Agrégateur de documents de recherche en libre accès fourni par le Knowledge Media Institute, basé à l'Open University, au Royaume-Uni."@fr ;
  skos:prefLabel "CORE"@en, "CORE"@es, "CORE"@fr ;
  skos:inScheme <http://data.loterre.fr/ark:/67375/TSO> ;
  skos:broader <http://data.loterre.fr/ark:/67375/TSO-CVMGJVKW-W> .

<http://data.loterre.fr/ark:/67375/TSO-BXDFN89K-P>
  a skos:Concept ;
  dc:modified "2021-07-05"^^xsd:date ;
  skos:definition "Iniciativa para recopilar y difundir en GitHub, bajo una licencia de base de datos abierta, conjuntos de datos relacionados con los derechos pagados por la publicación de acceso abierto."@es, "Initiative de collecte et de diffusion sur GitHub, sous une licence de base de données ouverte, de jeux de données relatifs aux droits payés pour la publication en libre accès."@fr, "The OpenAPC initiative collects and disseminates datasets on fees paid for open access publishing on GitHub under an open database license. (Source : https://openapc.net/)"@en ;
  skos:prefLabel "openAPC"@en, "openAPC"@es, "openAPC"@fr ;
  skos:inScheme <http://data.loterre.fr/ark:/67375/TSO> ;
  skos:broader <http://data.loterre.fr/ark:/67375/TSO-DXZZDQSM-3> ;
  skos:related <http://data.loterre.fr/ark:/67375/TSO-T80NJLNF-F> .

<http://data.loterre.fr/ark:/67375/TSO-W1F4MWNS-F>
  a skos:Concept ;
  dc:modified "2021-07-05"^^xsd:date ;
  skos:altLabel "Open Access Spectrum"@en, "Open Access Spectrum"@es, "Open Access Spectrum"@fr ;
  skos:definition "Herramienta de evaluación puesta a disposición gratuitamente por la SPARC, que permite evaluar el grado de apertura al Acceso Abierto de una revista."@es, "Outil d’évaluation mis à disposition gratuitement par SPARC, qui permet d’évaluer le degré d’ouverture à l’Open Access d’une revue."@fr ;
  skos:prefLabel "OAS"@en, "OAS"@es, "OAS"@fr ;
  skos:inScheme <http://data.loterre.fr/ark:/67375/TSO> ;
  skos:broader <http://data.loterre.fr/ark:/67375/TSO-QK42D772-3> ;
  skos:related <http://data.loterre.fr/ark:/67375/TSO-G587Q9G3-2> .

<http://data.loterre.fr/ark:/67375/TSO-XPQ718XW-Z>
  a skos:Concept ;
  dc:modified "2021-07-05"^^xsd:date ;
  skos:altLabel "PMC"@en ;
  skos:definition "A free full-text archive of biomedical and life sciences journal literature at the U.S. National Institutes of Health's National Library of Medicine (NIH/NLM). (Source : https://www.ncbi.nlm.nih.gov/pmc/)"@en, "Base de datos bibliográfica de acceso abierto de la literatura científica en ingeniería biomédica y ciencias de la vida."@es, "Base de données bibliographique à accès libre d'ouvrages scientifiques en génie biomédical et dans les sciences de la vie. (Source : https://fr.wikipedia.org/wiki/PubMed_Central)"@fr ;
  skos:prefLabel "PubMed Central"@en, "PubMed Central"@es, "PubMed Central"@fr ;
  skos:inScheme <http://data.loterre.fr/ark:/67375/TSO> ;
  skos:broader <http://data.loterre.fr/ark:/67375/TSO-CVMGJVKW-W> .

<http://data.loterre.fr/ark:/67375/TSO-QXH951LF-0>
  a skos:Concept ;
  dc:modified "2021-06-29"^^xsd:date ;
  skos:altLabel "Registry of Open Access Repository Mandates and Policies"@en, "Registry of Open Access Repository Mandates and Policies"@es, "Registry of Open Access Repository Mandates and Policies"@fr ;
  skos:definition "A searchable international registry charting the growth of open access mandates and policies adopted by universities, research institutions and research funders that require or request their researchers to provide open access to their peer-reviewed research article output by depositing it in an open access repository. (Source : http://roarmap.eprints.org/)"@en, "Base de donnée qui recense les mandats et les politiques de libre accès adoptés par les universités, les institutions de recherche et les bailleurs de fonds de la recherche qui exigent ou demandent à leurs chercheurs de fournir un libre accès à leurs articles de recherche évalués par les pairs en les déposant dans un dépôt en libre accès."@fr ;
  skos:prefLabel "ROARMAP"@en, "ROARMAP"@es, "ROARMAP"@fr ;
  skos:inScheme <http://data.loterre.fr/ark:/67375/TSO> ;
  skos:broader <http://data.loterre.fr/ark:/67375/TSO-B66RVJ4T-J> ;
  skos:related <http://data.loterre.fr/ark:/67375/TSO-H0BSK47H-Z> .

<http://data.loterre.fr/ark:/67375/TSO-PGSFQSNR-1>
  a skos:Concept ;
  dc:modified "2021-06-24"^^xsd:date ;
  skos:definition "Dépôt institutionnel de la production scientifique de Sciences Po. S'inscrivant dans le mouvement de la science ouverte, SPIRE référence, archive et diffuse l'ensemble des publications des chercheurs et doctorants de Sciences Po. (Source : https://spire.sciencespo.fr/)"@fr, "Sciences Po's institutional repository. It aims to be the comprehensive database for the research produced by Sciences Po academic community, its researchers and its Ph.D students. It displays research articles, working papers, books, book chapters, reports, discussion papers, research blogs and more. (Source : https://spire.sciencespo.fr/)"@en ;
  skos:prefLabel "Spire"@en, "Spire"@es, "Spire"@fr ;
  skos:inScheme <http://data.loterre.fr/ark:/67375/TSO> ;
  skos:broader <http://data.loterre.fr/ark:/67375/TSO-HZ175K8D-R> ;
  skos:related <http://data.loterre.fr/ark:/67375/TSO-F864TC3S-K> .

<http://data.loterre.fr/ark:/67375/TSO-C4027K67-Q>
  a skos:Concept ;
  dc:modified "2021-06-24"^^xsd:date ;
  skos:altLabel "Social Science Research Network"@en, "Social Science Research Network"@es, "Social Science Research Network"@fr ;
  skos:definition "A repository for preprints devoted to the rapid dissemination of scholarly research in the social sciences and humanities and more. Elsevier bought SSRN from Social Science Electronic Publishing Inc. in May 2016. (Source : Wikipedia)"@en, "Site Web de dépôt de prépublications d'articles scientifiques créé en 1994 par Michael Jensen et Wayne Marr. Le site a été racheté en 2016 par Elsevier. (Source : https://fr.wikipedia.org/wiki/Social_Science_Research_Network )"@fr ;
  skos:prefLabel "SSRN"@en, "SSRN"@es, "SSRN"@fr ;
  skos:inScheme <http://data.loterre.fr/ark:/67375/TSO> ;
  skos:broader <http://data.loterre.fr/ark:/67375/TSO-HZ175K8D-R> ;
  skos:related <http://data.loterre.fr/ark:/67375/TSO-GLZ7M59Q-M>, <http://data.loterre.fr/ark:/67375/TSO-XZ5703Z4-Q> .

<http://data.loterre.fr/ark:/67375/TSO-T9Q25G6Q-S>
  a skos:Concept ;
  dc:modified "2021-06-11"^^xsd:date ;
  skos:definition "An alternative to traditional impact metrics systems, open metrics have developed new way of evaluating the impact of the scholarly outputs. (Source : Foster)"@en, "Comme solution de rechange aux systèmes de mesures d’impact traditionnels, de nouvelles mesures ont développé une nouvelle façon d’évaluer l’impact de la production savante. (Source : Foster)"@fr ;
  skos:exactMatch <https://vocabularyserver.com/openscience/index.php?tema=30> ;
  skos:prefLabel "métrica abierta y medición del impacto"@es, "métrique et mesure d’impact ouvertes"@fr, "open metrics and impact"@en ;
  skos:semanticRelation <http://data.loterre.fr/ark:/67375/TSO-KHGQZ6NK-4> ;
  skos:inScheme <http://data.loterre.fr/ark:/67375/TSO> ;
  skos:broader <http://data.loterre.fr/ark:/67375/TSO-SMGMJFLJ-Q> ;
  skos:related <http://data.loterre.fr/ark:/67375/TSO-KGHBM8Z5-6>, <http://data.loterre.fr/ark:/67375/TSO-KSZ3VF36-P> ;
  skos:narrower <http://data.loterre.fr/ark:/67375/TSO-RGFVRS3V-Q>, <http://data.loterre.fr/ark:/67375/TSO-W30LBC9X-X>, <http://data.loterre.fr/ark:/67375/TSO-NM84XT0B-L>, <http://data.loterre.fr/ark:/67375/TSO-VTC90GGC-T>, <http://data.loterre.fr/ark:/67375/TSO-BXMNJ1ZN-Q>, <http://data.loterre.fr/ark:/67375/TSO-MSM5HV40-F>, <http://data.loterre.fr/ark:/67375/TSO-NTQ23ZP5-B>, <http://data.loterre.fr/ark:/67375/TSO-N9ZH1LS9-X> .

<http://data.loterre.fr/ark:/67375/TSO-B4WKXG50-6>
  a skos:Concept ;
  dc:modified "2021-07-05"^^xsd:date ;
  skos:definition "Infraestrucutra que tiene la ambición de recopilar, preservar y compartir todo el software que esté públicamente disponible en formato de código fuente. (Fuente: https://www.softwareheritage.org/mision/?lang=es)"@es, "Infrastructure qui a pour mission de collecter, préserver et partager tous les logiciels disponibles publiquement sous forme de code source. (Source : https://www.softwareheritage.org)"@fr, "Infrastructure which has the mission to collect, preserve, and share all software that is publicly available in source code form. (Source : https://www.softwareheritage.org)"@en ;
  skos:prefLabel "Software Heritage"@en, "Software Heritage"@es, "Software Heritage"@fr ;
  skos:inScheme <http://data.loterre.fr/ark:/67375/TSO> ;
  skos:broader <http://data.loterre.fr/ark:/67375/TSO-LS0Q2K68-D> ;
  skos:related <http://data.loterre.fr/ark:/67375/TSO-TRTL77DD-T> .

<http://data.loterre.fr/ark:/67375/TSO-T487PDFX-7>
  a skos:Concept ;
  dc:modified "2021-06-29"^^xsd:date ;
  skos:altLabel "digital object identifier"@en, "identifiant numérique d'objet"@fr, "identificador de objeto digital"@es ;
  skos:definition "A persistent identifier used to identify objects uniquely, standardized by the International Organization for Standardization (ISO). The developer and administrator of the DOI system is the International DOI Foundation (IDF), which introduced it in 2000. (Source : WIkipedia)"@en, "Chaîne de caractères univoque et pérenne qui permet d’identifier, référencer, citer et fournir un lien durable à des ressources numériques de tous types en leur associant des métadonnées. Depuis 2012, le système a été normalisé sous la forme de la norme ISO 263242."@fr ;
  skos:prefLabel "DOI"@en, "DOI"@es, "DOI"@fr ;
  skos:inScheme <http://data.loterre.fr/ark:/67375/TSO> ;
  skos:broader <http://data.loterre.fr/ark:/67375/TSO-H5ZG6DX6-4> ;
  skos:related <http://data.loterre.fr/ark:/67375/TSO-GXCQ58W9-H>, <http://data.loterre.fr/ark:/67375/TSO-RPJVDHMM-Q>, <http://data.loterre.fr/ark:/67375/TSO-XQQ71S90-L> .

<http://data.loterre.fr/ark:/67375/TSO-XDCZ7K0M-B>
  a skos:Concept ;
  dc:modified "2021-06-29"^^xsd:date ;
  skos:altLabel "vérification de la réplicabilité"@fr ;
  skos:definition "Processus qui valide le fait que les résultats de recherche rapportés peuvent être obtenus dans une expérience indépendante. (Source : Foster)"@fr, "The process of validating that the reported research results can be obtained in an independent experiment. (Source : Foster)"@en ;
  skos:exactMatch <https://vocabularyserver.com/openscience/index.php?tema=25> ;
  skos:prefLabel "reproducibility testing"@en, "verificación de la reproducibilidad"@es, "vérification de la reproductibilité"@fr ;
  skos:inScheme <http://data.loterre.fr/ark:/67375/TSO> ;
  skos:broader <http://data.loterre.fr/ark:/67375/TSO-JWXHV1CM-9> .

<http://data.loterre.fr/ark:/67375/TSO-G591ZH6Q-X>
  a skos:Concept ;
  dc:modified "2021-06-24"^^xsd:date ;
  skos:definition "Journal that publishes peer reviewed articles describing openly accessible datasets for future reuse. (Source : Foster)"@en, "Revue qui publie des articles évalués par les pairs qui décrivent des jeux de données en libre accès, pour réutilisation ultérieure. (Source : Foster)"@fr ;
  skos:exactMatch <https://vocabularyserver.com/openscience/index.php?tema=21> ;
  skos:prefLabel "open data journal"@en, "revista de datos abiertos"@es, "revue de données ouvertes"@fr ;
  skos:inScheme <http://data.loterre.fr/ark:/67375/TSO> ;
  skos:broader <http://data.loterre.fr/ark:/67375/TSO-TM0MS2GV-7> ;
  skos:related <http://data.loterre.fr/ark:/67375/TSO-V08MCZVP-H>, <http://data.loterre.fr/ark:/67375/TSO-P0JM96T2-W> .

<http://data.loterre.fr/ark:/67375/TSO-KHL25V0F-4>
  a skos:Concept ;
  dc:modified "2021-06-30"^^xsd:date ;
  skos:altLabel "OA road"@en, "open access road"@en ;
  skos:definition "A model that defines the process leading to open access, characterised by the way in which the costs of publication are covered."@en, "Modèle qui définit le processus aboutissant au libre accès et caractérisé par la manière dont les coûts de publication sont couverts."@fr ;
  skos:exactMatch <https://vocabularyserver.com/openscience/index.php?tema=13> ;
  skos:prefLabel "open access route"@en, "ruta del acceso abierto"@es, "voie du libre accès"@fr ;
  skos:inScheme <http://data.loterre.fr/ark:/67375/TSO> ;
  skos:broader <http://data.loterre.fr/ark:/67375/TSO-T84RPJRB-K> ;
  skos:related <http://data.loterre.fr/ark:/67375/TSO-STWL5MWS-W> ;
  skos:narrower <http://data.loterre.fr/ark:/67375/TSO-P0PB3HHR-8>, <http://data.loterre.fr/ark:/67375/TSO-HS79BV00-V>, <http://data.loterre.fr/ark:/67375/TSO-P2PM5GCP-8>, <http://data.loterre.fr/ark:/67375/TSO-KG87BTKZ-L>, <http://data.loterre.fr/ark:/67375/TSO-T0GXV6XC-Z> .

<http://data.loterre.fr/ark:/67375/TSO-VTC90GGC-T>
  a skos:Concept ;
  dc:modified "2021-06-03"^^xsd:date ;
  skos:definition "Metric for assessing the level of compliance of a repository or process with the FAIR principles"@en, "Métrique adaptée à l'évaluation du niveau de conformation d'un entrepôt ou d'un processus aux principes FAIR"@fr ;
  skos:prefLabel "FAIR metrics"@en, "métrica FAIR"@es, "métrique FAIR"@fr ;
  skos:inScheme <http://data.loterre.fr/ark:/67375/TSO> ;
  skos:broader <http://data.loterre.fr/ark:/67375/TSO-T9Q25G6Q-S> ;
  skos:related <http://data.loterre.fr/ark:/67375/TSO-N9ZH1LS9-X> .

<http://data.loterre.fr/ark:/67375/TSO-BXMNJ1ZN-Q>
  a skos:Concept ;
  dc:modified "2021-06-03"^^xsd:date ;
  skos:definition "As opposed to existing Bibliometrics, Webometrics, Altmetrics, etc., Semantometrics are not based on measuring the number of interactions in the scholarly communication network, but exploit primarily the fulltext of manuscripts to assess the value of a publication. (Source : Foster)"@en, "Par opposition aux paradigmes existants en bibliométrie, en webométrie et dans les mesures d’impact alternatives, les indicateurs sémantométriques ne s’appuient pas sur le calcul du nombre d’interactions dans le réseau de communication savante, mais exploitent d’abord et avant tout le texte intégral des manuscrits pour évaluer ce que vaut une publication. (Source : Foster)"@fr ;
  skos:exactMatch <https://vocabularyserver.com/openscience/index.php?tema=35> ;
  skos:prefLabel "semantometrics"@en, "semantometría"@es, "sémantométrie"@fr ;
  skos:inScheme <http://data.loterre.fr/ark:/67375/TSO> ;
  skos:broader <http://data.loterre.fr/ark:/67375/TSO-T9Q25G6Q-S> .

<http://data.loterre.fr/ark:/67375/TSO-G4CFRKD0-L>
  a skos:Concept ;
  dc:modified "2021-06-11"^^xsd:date ;
  skos:definition "Courses of actions on a specific branch of knowledge. (Source : Foster)"@en, "Lignes de conduite concernant un champ de connaissance particulier. (Source : Foster)"@fr ;
  skos:exactMatch <https://vocabularyserver.com/openscience/index.php?tema=37> ;
  skos:prefLabel "politique disciplinaire"@fr, "política disciplinaria"@es, "subject policy"@en ;
  skos:inScheme <http://data.loterre.fr/ark:/67375/TSO> ;
  skos:broader <http://data.loterre.fr/ark:/67375/TSO-H0BSK47H-Z> .

<http://data.loterre.fr/ark:/67375/TSO-GVVZFV2S-W>
  a skos:Concept ;
  dc:modified "2021-06-29"^^xsd:date ;
  skos:altLabel "decentralized identifier"@en, "identidad descentralizada"@es, "identificador descentralizado"@es, "identité décentralisée"@fr ;
  skos:definition "A type of identifier that enables verifiable, decentralized digital identity. A DID identifies any subject (e.g., a person, organization, thing, data model, abstract entity, etc.) that the controller of the DID decides that it identifies. In contrast to typical, federated identifiers, DIDs have been designed so that they may be decoupled from centralized registries, identity providers, and certificate authorities. (Source : W3C, https://www.w3.org/blog/news/archives/8966)"@en, "Ensemble de caractéristiques qui définit de façon unique un objet."@fr ;
  skos:prefLabel "DID"@en, "DID"@es, "identifiant décentralisé"@fr ;
  skos:inScheme <http://data.loterre.fr/ark:/67375/TSO> ;
  skos:broader <http://data.loterre.fr/ark:/67375/TSO-H5ZG6DX6-4> .

<http://data.loterre.fr/ark:/67375/TSO-T6RG1XJN-7>
  a skos:Concept ;
  dc:modified "2021-06-11"^^xsd:date ;
  skos:definition "Courses of actions adopted from governments. (Source : Foster)"@en, "Lignes de conduite adoptées par les gouvernements. (Source : Foster)"@fr ;
  skos:exactMatch <https://vocabularyserver.com/openscience/index.php?tema=39> ;
  skos:prefLabel "governmental policy"@en, "politique gouvernementale"@fr, "política del gobierno"@es ;
  skos:inScheme <http://data.loterre.fr/ark:/67375/TSO> ;
  skos:broader <http://data.loterre.fr/ark:/67375/TSO-QL0JTPZ5-J> ;
  skos:narrower <http://data.loterre.fr/ark:/67375/TSO-ZLCW75XN-W> .

<http://data.loterre.fr/ark:/67375/TSO-NCZNV1ZN-L>
  a skos:Concept ;
  dc:modified "2021-06-24"^^xsd:date ;
  skos:altLabel "CC0 license"@en, "licence CC0"@fr ;
  skos:definition "Licence de renonciation au droit d'auteur ; aucun droit réservé. Place le contenu aussi ouvertement que possible dans le domaine public."@fr, "Waiver of copyright; no rights reserved. Places content as openly as possible in the public domain. (Source : http://www.righttoresearch.org/resources/OpenResearchGlossary)"@en ;
  skos:prefLabel "CC-ZERO license"@en, "licence CC-ZERO"@fr, "licencia CC-ZERO"@es ;
  skos:inScheme <http://data.loterre.fr/ark:/67375/TSO> ;
  skos:broader <http://data.loterre.fr/ark:/67375/TSO-WH5JC3TT-G>, <http://data.loterre.fr/ark:/67375/TSO-WZ0J1023-D> .

<http://data.loterre.fr/ark:/67375/TSO-WFHTSVS6-0>
  a skos:Concept ;
  dc:modified "2021-06-28"^^xsd:date ;
  skos:altLabel "S2O"@en, "subscribe to open"@en ;
  skos:definition "Modèle selon lequel la diffusion en accès libre des ouvrages et revues s’opère lorsque le seuil financier visé est atteint grâce aux contributions financières des établissements souscripteurs. (Source : Science ouverte France)"@fr ;
  skos:prefLabel "souscription"@fr, "subscription"@en, "suscripción"@es ;
  skos:inScheme <http://data.loterre.fr/ark:/67375/TSO> ;
  skos:broader <http://data.loterre.fr/ark:/67375/TSO-MWXTBMQ8-9> .

<http://data.loterre.fr/ark:/67375/TSO-SJ6X9JL0-3>
  a skos:Concept ;
  skos:altLabel "article processing charges funding"@en, "pago de cargo por procesamiento de artículos"@es, "paiement de frais de traitement des articles"@fr ;
  skos:definition "Modèle selon lequel les frais finançant l'accès ouvert à la publication sont payés par l’auteur ou son institution"@fr ;
  skos:prefLabel "APC funding"@en, "pago de APC"@es, "paiement d'APC"@fr ;
  skos:inScheme <http://data.loterre.fr/ark:/67375/TSO> ;
  skos:broader <http://data.loterre.fr/ark:/67375/TSO-MWXTBMQ8-9> ;
  skos:related <http://data.loterre.fr/ark:/67375/TSO-DCPLM2CT-F>, <http://data.loterre.fr/ark:/67375/TSO-DLBP9S2L-Z>, <http://data.loterre.fr/ark:/67375/TSO-T80NJLNF-F> .

<http://data.loterre.fr/ark:/67375/TSO-HS79BV00-V>
  a skos:Concept ;
  dc:modified "2021-07-05"^^xsd:date ;
  skos:altLabel "diamond OA"@en, "diamond road"@en, "libre accès diamant"@fr ;
  skos:definition "Intenta cubrir la brecha existente entre los modelos verde y dorado, ya que este modelo tiene en cuenta los dos aspectos más débiles de ambos modelos: costes (Gold) y calidad (Green). Siendo el único modelo que garantiza la sostenibilidad de la publicación de acceso abierto. (Fuente: https://universoabierto.org/2017/06/09/que-es-la-ruta-diamante-de-acceso-abierto/)"@es, "Model where publications are available in open access without paying any APCs."@en, "Modèle selon lequel la publication et la diffusion sont totalement gratuites pour le lecteur et pour l’auteur."@fr ;
  skos:prefLabel "diamond route"@en, "ruta diamante"@es, "voie diamant"@fr ;
  skos:inScheme <http://data.loterre.fr/ark:/67375/TSO> ;
  skos:broader <http://data.loterre.fr/ark:/67375/TSO-KHL25V0F-4> ;
  skos:related <http://data.loterre.fr/ark:/67375/TSO-NX4NVXX2-L>, <http://data.loterre.fr/ark:/67375/TSO-QT5MLV48-P> .

<http://data.loterre.fr/ark:/67375/TSO-G425PLR1-B>
  a skos:Concept ;
  dc:modified "2021-06-03"^^xsd:date ;
  skos:definition "Modèle économique qui combine deux modes d’accès à des textes : un accès libre et gratuit pour un service « basique » et un accès payant pour une offre plus évoluée ou des services complémentaires. (Source : https://openaccess.inist.fr/glossaire/)"@fr ;
  skos:prefLabel "freemium model"@en, "modelo freemium"@es, "modèle freemium"@fr ;
  skos:inScheme <http://data.loterre.fr/ark:/67375/TSO> ;
  skos:broader <http://data.loterre.fr/ark:/67375/TSO-P2PM5GCP-8> .

<http://data.loterre.fr/ark:/67375/TSO-DCPLM2CT-F>
  a skos:Concept ;
  dc:modified "2021-06-04"^^xsd:date ;
  skos:definition "Modèle économique qui fait coexister deux types d’articles dans une même revue : ceux qui sont librement accessibles, contre une redevance versée à l’éditeur par l’auteur ou son financeur, et ceux qui sont accessibles par un abonnement. (Source : https://openaccess.inist.fr/glossaire/)"@fr ;
  skos:prefLabel "hybrid model"@en, "modelo híbrido"@es, "modèle hybride"@fr ;
  skos:inScheme <http://data.loterre.fr/ark:/67375/TSO> ;
  skos:broader <http://data.loterre.fr/ark:/67375/TSO-P2PM5GCP-8> ;
  skos:related <http://data.loterre.fr/ark:/67375/TSO-PSFFQLXV-2>, <http://data.loterre.fr/ark:/67375/TSO-RN1XP625-F>, <http://data.loterre.fr/ark:/67375/TSO-SJ6X9JL0-3> .

<http://data.loterre.fr/ark:/67375/TSO-XHQRK84J-T>
  a skos:Concept ;
  dc:modified "2021-06-02"^^xsd:date ;
  skos:definition "alphanumeric code to uniquely identify authors and contributors of scholarly communication (source: https://en.wikipedia.org/wiki/ORCID)"@en, "code alphanumérique non propriétaire, qui permet d'identifier les chercheurs et auteurs de contributions académiques et scientifiques, imposé par les grands éditeurs (source: https://fr.wikipedia.org/wiki/ORCID)"@fr ;
  skos:prefLabel "ORCID"@en, "ORCID"@es, "ORCID"@fr ;
  skos:inScheme <http://data.loterre.fr/ark:/67375/TSO> ;
  skos:broader <http://data.loterre.fr/ark:/67375/TSO-H5ZG6DX6-4> ;
  skos:related <http://data.loterre.fr/ark:/67375/TSO-QL71JGQM-F> .

<http://data.loterre.fr/ark:/67375/TSO-BTR6P741-6>
  a skos:Concept ;
  dc:modified "2021-07-05"^^xsd:date ;
  skos:definition "Modalidad de acceso en la que la consulta de los artículos de una revista está reservada a los suscriptores durante un determinado periodo de tiempo, y luego está abierta a todos. (Fuente: traducción de https://salons.erudit.org/2017/10/18/libre-acces-immediat-et-libre-acces-differe/ )"@es, "Mode d'accès dans lequel la consultation des articles d'une revue est réservée aux abonnés pendant une certaine période, puis est ensuite ouverte à tous. (source: https://salons.erudit.org/2017/10/18/libre-acces-immediat-et-libre-acces-differe/)"@fr, "scholarly articles in subscription journals made available openly on the web directly through the publisher at the expiry of a set embargo period. (source: https://onlinelibrary.wiley.com/doi/abs/10.1002/asi.22856)"@en ;
  skos:prefLabel "delayed open access"@en, "libre acceso diferido"@es, "libre accès différé"@fr ;
  skos:inScheme <http://data.loterre.fr/ark:/67375/TSO> ;
  skos:broader <http://data.loterre.fr/ark:/67375/TSO-STWL5MWS-W> ;
  skos:related <http://data.loterre.fr/ark:/67375/TSO-D2CGSDHD-L> .

<http://data.loterre.fr/ark:/67375/TSO-XHQSGQST-B>
  a skos:Concept ;
  dc:modified "2021-06-10"^^xsd:date ;
  skos:definition "Programme lancé par le fournisseur de services pour la collecte de métadonnées auprès d’un ou plusieurs entrepôts OAI. (Source : https://openaccess.inist.fr/glossaire/)"@fr ;
  skos:prefLabel "OAI harvester"@en, "cosechadora OAI"@es, "moissonneur OAI"@fr ;
  skos:inScheme <http://data.loterre.fr/ark:/67375/TSO> ;
  skos:broader <http://data.loterre.fr/ark:/67375/TSO-XS8KGCJ0-V> ;
  skos:related <http://data.loterre.fr/ark:/67375/TSO-P0WRKFZJ-X>, <http://data.loterre.fr/ark:/67375/TSO-XBFF1KGS-V> .

<http://data.loterre.fr/ark:/67375/TSO-XS8KGCJ0-V>
  a skos:Concept ;
  dc:created "2021-06-10"^^xsd:date ;
  dc:modified "2021-06-10"^^xsd:date ;
  skos:prefLabel "herramienta facilitando el acceso a los datos"@es, "outil facilitant l'accès aux données"@fr, "tool facilitating data access"@en ;
  skos:inScheme <http://data.loterre.fr/ark:/67375/TSO> ;
  skos:broader <http://data.loterre.fr/ark:/67375/TSO-V0KSG0NC-P> ;
  skos:narrower <http://data.loterre.fr/ark:/67375/TSO-XHQSGQST-B>, <http://data.loterre.fr/ark:/67375/TSO-N85W7DT1-Z>, <http://data.loterre.fr/ark:/67375/TSO-KXB7P34Z-4>, <http://data.loterre.fr/ark:/67375/TSO-WQMF6CT2-K>, <http://data.loterre.fr/ark:/67375/TSO-JCX2HR5K-4>, <http://data.loterre.fr/ark:/67375/TSO-P0JM96T2-W> .

<http://data.loterre.fr/ark:/67375/TSO-VDVFXBCR-C>
  a skos:Concept ;
  dc:modified "2021-06-09"^^xsd:date ;
  skos:prefLabel "data retrieval"@en, "repérage des données"@fr, "seguimiento de datos"@es ;
  skos:inScheme <http://data.loterre.fr/ark:/67375/TSO> ;
  skos:broader <http://data.loterre.fr/ark:/67375/TSO-SMGMJFLJ-Q> ;
  skos:related <http://data.loterre.fr/ark:/67375/TSO-JDVCT02T-P> .

<http://data.loterre.fr/ark:/67375/TSO-V0KSG0NC-P>
  a skos:Concept ;
  dc:modified "2021-06-10"^^xsd:date ;
  skos:altLabel "open workflow tool"@en, "outil d’intégration de pratiques ouvertes"@fr ;
  skos:definition "Refers to the tools that can assist in the process of delivering and building on Open Science. (Source : Foster)"@en, "Réfère aux outils qui peuvent aider au quotidien à mettre en œuvre et à étendre les principes de la science ouverte. (Source : Foster)"@fr ;
  skos:exactMatch <https://vocabularyserver.com/openscience/index.php?tema=9> ;
  skos:prefLabel "herramienta de ciencia abierta"@es, "open science tool"@en, "outil de science ouverte"@fr ;
  skos:inScheme <http://data.loterre.fr/ark:/67375/TSO> ;
  skos:related <http://data.loterre.fr/ark:/67375/TSO-JFJGKFN2-H> ;
  skos:narrower <http://data.loterre.fr/ark:/67375/TSO-T80NJLNF-F>, <http://data.loterre.fr/ark:/67375/TSO-W9KRS5Q3-6>, <http://data.loterre.fr/ark:/67375/TSO-XS8KGCJ0-V>, <http://data.loterre.fr/ark:/67375/TSO-CV5H9HZH-V>, <http://data.loterre.fr/ark:/67375/TSO-T4KV78Z3-L>, <http://data.loterre.fr/ark:/67375/TSO-H5ZG6DX6-4>, <http://data.loterre.fr/ark:/67375/TSO-G33B1S7H-W>, <http://data.loterre.fr/ark:/67375/TSO-KSZ3VF36-P>, <http://data.loterre.fr/ark:/67375/TSO-KGHBM8Z5-6>, <http://data.loterre.fr/ark:/67375/TSO-GRJ351P7-S>, <http://data.loterre.fr/ark:/67375/TSO-X3TNSQ40-M> ;
  skos:topConceptOf <http://data.loterre.fr/ark:/67375/TSO> .

<http://data.loterre.fr/ark:/67375/TSO-DDH5932P-J>
  a skos:Concept ;
  dc:modified "2021-06-10"^^xsd:date ;
  skos:altLabel "OER"@en, "REA"@es, "REL"@fr ;
  skos:definition "Freely accessible, openly licensed text, media, and other digital assets that are useful for teaching, learning, and assessing as well as for research purposes. (source: https://en.wikipedia.org/wiki/Open_educational_resources)"@en, "Matériaux d’enseignement, d'apprentissage ou de recherche appartenant au domaine public ou publiés avec une licence de propriété intellectuelle permettant leur utilisation, adaptation et distribution à titre gratuit (source: https://fr.wikipedia.org/wiki/Ressources_éducatives_libres)"@fr ;
  skos:prefLabel "open educational resource"@en, "recursos educativos abiertos"@es, "ressource éducative libre"@fr ;
  skos:inScheme <http://data.loterre.fr/ark:/67375/TSO> ;
  skos:broader <http://data.loterre.fr/ark:/67375/TSO-X3TNSQ40-M> .

<http://data.loterre.fr/ark:/67375/TSO-P0WRKFZJ-X>
  a skos:Concept ;
  dc:modified "2021-06-10"^^xsd:date ;
  skos:altLabel "Open Archives Initiative Protocol for Metadata Harvesting"@en, "Open Archives Initiative Protocol for Metadata Harvesting"@es, "Open Archives Initiative Protocol for Metadata Harvesting"@fr, "protocolo de la iniciativa de archivos abiertos para la colección de metadatos"@es ;
  skos:definition "Estándar técnico desarrollado por la OAI para metadatos de repositorios de Acceso Abierto y de revistas de Acceso Abierto. El cumplimiento de este estándar garantiza la interoperabilidad. (Fuente: http://accesoabierto.uanl.mx/glosario-de-terminos/)"@es, "Protocol developed for harvesting metadata descriptions of records in an archive so that services can be built using metadata from many archives (source: https://en.wikipedia.org/wiki/Open_Archives_Initiative_Protocol_for_Metadata_Harvesting)"@en, "Protocole informatique développé par l'Open Archives Initiative afin d'échanger des métadonnées. Il permet de constituer et de mettre à jour automatiquement des entrepôts centralisés où les métadonnées de sources diverses peuvent être interrogées simultanément. (source: https://fr.wikipedia.org/wiki/Open_Archives_Initiative_Protocol_for_Metadata_Harvesting)"@fr ;
  skos:prefLabel "OAI-PMH"@en, "OAI-PMH"@es, "OAI-PMH"@fr ;
  skos:inScheme <http://data.loterre.fr/ark:/67375/TSO> ;
  skos:broader <http://data.loterre.fr/ark:/67375/TSO-XWVJBKN6-S> ;
  skos:related <http://data.loterre.fr/ark:/67375/TSO-CW11LHBH-Q>, <http://data.loterre.fr/ark:/67375/TSO-JBQFB4MB-P>, <http://data.loterre.fr/ark:/67375/TSO-XHQSGQST-B> .

<http://data.loterre.fr/ark:/67375/TSO-RW8FM312-M>
  a skos:Concept ;
  dc:modified "2021-06-29"^^xsd:date ;
  skos:definition "Manuel produit en 2018 par le TIB de Hanovre. Il vise à soutenir les institutions de recherche qui veulent mettre en œuvre les principes de la science ouverte. Il donne une vue d’ensemble des ressources, méthodes, techniques et outils orientés vers l'enseignement pratique. (Source : https://www.ouvrirlascience.fr/the-open-science-training-handbook/)"@fr, "Open, living handbook on open science training created in February 2018 at the TIB (German National Library of Science and Technology) in Hannover. (Source : https://open-science-training-handbook.gitbook.io/book/)"@en ;
  skos:prefLabel "Open Science Training Handbook"@en, "Open Science Training Handbook"@es, "Open Science Training Handbook"@fr ;
  skos:inScheme <http://data.loterre.fr/ark:/67375/TSO> ;
  skos:broader <http://data.loterre.fr/ark:/67375/TSO-X3TNSQ40-M> .

<http://data.loterre.fr/ark:/67375/TSO-N85W7DT1-Z>
  a skos:Concept ;
  dc:modified "2021-06-25"^^xsd:date ;
  skos:altLabel "application programming interface"@en, "interface de programmation d'application"@fr, "interfaz de programación de aplicaciones"@es ;
  skos:definition "Ensemble normalisé de classes, de méthodes, de fonctions et de constantes qui sert de façade par laquelle un logiciel offre des services à d'autres logiciels. Elle est offerte par une bibliothèque logicielle ou un service web, le plus souvent accompagnée d'une description qui spécifie comment des programmes consommateurs peuvent se servir des fonctionnalités du programme fournisseur. (Source : https://fr.wikipedia.org/wiki/Interface_de_programmation)"@fr ;
  skos:prefLabel "API"@en, "API"@es, "API"@fr ;
  skos:inScheme <http://data.loterre.fr/ark:/67375/TSO> ;
  skos:broader <http://data.loterre.fr/ark:/67375/TSO-XS8KGCJ0-V> .

<http://data.loterre.fr/ark:/67375/TSO-D9HJPTL6-X>
  a skos:Concept ;
  skos:altLabel "FAIR data principles"@en ;
  skos:definition "Ensemble de principes directeurs pour gérer les données de la recherche, visant à les rendre faciles à trouver, accessibles, interopérables et réutilisables par l’homme et la machine. (Source : Ouvrir la science)"@fr, "Principles for scientific data management and stewardship intended to provide guidelines to improve the findability, accessibility, interoperability, and reuse of digital assets. (Source : Ouvrir la science)"@en ;
  skos:prefLabel "FAIR principles"@en, "principes FAIR"@fr, "principios FAIR"@es ;
  skos:inScheme <http://data.loterre.fr/ark:/67375/TSO> ;
  skos:broader <http://data.loterre.fr/ark:/67375/TSO-CV5H9HZH-V> ;
  skos:related <http://data.loterre.fr/ark:/67375/TSO-DP8MN2RF-P>, <http://data.loterre.fr/ark:/67375/TSO-QWKTFN2F-N>, <http://data.loterre.fr/ark:/67375/TSO-XW567W8B-4> ;
  skos:narrower <http://data.loterre.fr/ark:/67375/TSO-KHFX8870-5>, <http://data.loterre.fr/ark:/67375/TSO-JDVCT02T-P>, <http://data.loterre.fr/ark:/67375/TSO-C676TDJV-H>, <http://data.loterre.fr/ark:/67375/TSO-X4ZW5XQD-G> .

<http://data.loterre.fr/ark:/67375/TSO-JK3TZ82D-D>
  a skos:Concept ;
  dc:modified "2021-06-10"^^xsd:date ;
  skos:altLabel "Internationalized Resource Identifier"@en, "identifiant de ressource internationalisé"@fr ;
  skos:definition "Chaîne de caractères Unicode identifiant une ressource de manière permanente sur un réseau (par exemple une ressource Web), même si la ressource est déplacée ou supprimée."@fr ;
  skos:prefLabel "IRI"@en, "IRI"@es, "IRI"@fr ;
  skos:inScheme <http://data.loterre.fr/ark:/67375/TSO> ;
  skos:broader <http://data.loterre.fr/ark:/67375/TSO-H5ZG6DX6-4> .

<http://data.loterre.fr/ark:/67375/TSO-VF5K6BGT-F>
  a skos:Concept ;
  dc:modified "2021-07-05"^^xsd:date ;
  skos:definition "Data that provides information about other data. (Source: merriam-webster.com)"@en, "Descripción estandardizada de las características de un conjunto de datos. (Fuente: https://dpej.rae.es/lema/metadato)"@es, "Donnée servant à caractériser une autre donnée, physique ou numérique. (Source : larousse.fr)"@fr ;
  skos:prefLabel "metadata"@en, "metadatos"@es, "métadonnées"@fr ;
  skos:inScheme <http://data.loterre.fr/ark:/67375/TSO> ;
  skos:broader <http://data.loterre.fr/ark:/67375/TSO-MJRKBMDW-Q> ;
  skos:related <http://data.loterre.fr/ark:/67375/TSO-TKRVHS3M-S> .

<http://data.loterre.fr/ark:/67375/TSO-RB0TPH2H-Q>
  a skos:Concept ;
  dc:created "2021-06-24"^^xsd:date ;
  dc:modified "2021-06-24"^^xsd:date ;
  skos:definition "Activité qui combine une intention « sérieuse » avec des ressorts ludiques. Des jeux ont été conçus pour faire participer la communauté de joueurs à la recherche scientifique en leur faisant résoudre à travers une interface ludique des problèmes difficiles à traiter de façon algorithmique. (Source : https://fr.wikipedia.org/wiki/Jeu_s%C3%A9rieux#Recherche_scientifique)"@fr ;
  skos:prefLabel "jeu sérieux"@fr, "juego serio"@es, "serious game"@en ;
  skos:inScheme <http://data.loterre.fr/ark:/67375/TSO> ;
  skos:broader <http://data.loterre.fr/ark:/67375/TSO-X3TNSQ40-M> ;
  skos:related <http://data.loterre.fr/ark:/67375/TSO-KBRVB4PD-K> ;
  skos:narrower <http://data.loterre.fr/ark:/67375/TSO-B8V78028-B> .

<http://data.loterre.fr/ark:/67375/TSO-WSB3R3KG-1>
  a skos:Concept ;
  dc:modified "2021-06-11"^^xsd:date ;
  skos:definition "A model based on a small number of unifying concepts, which may be used as a basis for education and for explaining standards to nonspecialists. Characteristics include: a representation of best practices; universal applicability; and reusability."@en ;
  skos:prefLabel "modelo de referencia"@es, "modèle de référence"@fr, "reference model"@en ;
  skos:inScheme <http://data.loterre.fr/ark:/67375/TSO> ;
  skos:broader <http://data.loterre.fr/ark:/67375/TSO-X3TNSQ40-M> ;
  skos:related <http://data.loterre.fr/ark:/67375/TSO-MV5H4HGJ-2> .

<http://data.loterre.fr/ark:/67375/TSO-HCPMHK1V-X>
  a skos:Concept ;
  dc:modified "2021-06-10"^^xsd:date ;
  skos:altLabel "URI"@fr, "Uniform Resource Identifier"@en, "identifiant universel de ressource"@fr, "identificador de recursos uniforme"@es ;
  skos:definition "Chaîne de caractères ASCII identifiant une ressource de manière permanente sur un réseau (par exemple une ressource Web), même si la ressource est déplacée ou supprimée."@fr ;
  skos:prefLabel "IUR"@fr, "URI"@en, "URI"@es ;
  skos:inScheme <http://data.loterre.fr/ark:/67375/TSO> ;
  skos:broader <http://data.loterre.fr/ark:/67375/TSO-H5ZG6DX6-4> .

<http://data.loterre.fr/ark:/67375/TSO-J3R15XFV-K>
  a skos:Concept ;
  dc:modified "2021-06-10"^^xsd:date ;
  skos:altLabel "web des données"@fr ;
  skos:definition "Initiative du W3C (Consortium World Wide Web) visant à favoriser la publication de données structurées sur le Web, non pas sous la forme de silos de données isolés les uns des autres, mais en les reliant entre elles pour constituer un réseau global d'informations. (Source : Wikipédia)"@fr, "The Web in which data, in addition to having meaning for humans, also have meaning for machines in such a way that they can be searched, found, interpreted, shared and reused among applications, organizations and communities. (Source: https://dlis.hypotheses.org/788)"@en ;
  skos:prefLabel "web de datos"@es, "web de données"@fr, "web of data"@en ;
  skos:inScheme <http://data.loterre.fr/ark:/67375/TSO> ;
  skos:broader <http://data.loterre.fr/ark:/67375/TSO-XWVJBKN6-S> ;
  skos:related <http://data.loterre.fr/ark:/67375/TSO-T161C80T-Q> .

<http://data.loterre.fr/ark:/67375/TSO-J64S3QDL-1>
  a skos:Concept ;
  skos:prefLabel "open science organisation"@en, "organisme œuvrant pour la science ouverte"@fr, "organismo ayudando ir hacia la ciencia abierta"@es ;
  skos:inScheme <http://data.loterre.fr/ark:/67375/TSO> ;
  skos:related <http://data.loterre.fr/ark:/67375/TSO-JFJGKFN2-H> ;
  skos:narrower <http://data.loterre.fr/ark:/67375/TSO-MZ8BL730-S>, <http://data.loterre.fr/ark:/67375/TSO-VQD3856X-4>, <http://data.loterre.fr/ark:/67375/TSO-QXK0M64M-N>, <http://data.loterre.fr/ark:/67375/TSO-BTFX00Q2-P>, <http://data.loterre.fr/ark:/67375/TSO-VPJV1Q5X-J>, <http://data.loterre.fr/ark:/67375/TSO-G4MG47JW-H>, <http://data.loterre.fr/ark:/67375/TSO-TJTXZ4LV-W>, <http://data.loterre.fr/ark:/67375/TSO-GXCQ58W9-H>, <http://data.loterre.fr/ark:/67375/TSO-RPJVDHMM-Q>, <http://data.loterre.fr/ark:/67375/TSO-Q3D3R4D9-C>, <http://data.loterre.fr/ark:/67375/TSO-RRVKQP85-7>, <http://data.loterre.fr/ark:/67375/TSO-C670N10N-B>, <http://data.loterre.fr/ark:/67375/TSO-FXLNHJK5-R>, <http://data.loterre.fr/ark:/67375/TSO-G587Q9G3-2>, <http://data.loterre.fr/ark:/67375/TSO-S9XQFTCQ-Q>, <http://data.loterre.fr/ark:/67375/TSO-GCQ559K4-Q>, <http://data.loterre.fr/ark:/67375/TSO-CW11LHBH-Q>, <http://data.loterre.fr/ark:/67375/TSO-FXS77K89-G>, <http://data.loterre.fr/ark:/67375/TSO-S9J32NCP-W>, <http://data.loterre.fr/ark:/67375/TSO-ZT32Z3F2-6>, <http://data.loterre.fr/ark:/67375/TSO-DKBRJ0N6-J>, <http://data.loterre.fr/ark:/67375/TSO-NG65T0DF-9>, <http://data.loterre.fr/ark:/67375/TSO-HK7N0SDD-S>, <http://data.loterre.fr/ark:/67375/TSO-FTDKPJ1X-Z>, <http://data.loterre.fr/ark:/67375/TSO-VPTBZS30-F>, <http://data.loterre.fr/ark:/67375/TSO-R3K91KN9-H>, <http://data.loterre.fr/ark:/67375/TSO-HXX9G512-G>, <http://data.loterre.fr/ark:/67375/TSO-F43HWMXG-K>, <http://data.loterre.fr/ark:/67375/TSO-T52K1CB6-X>, <http://data.loterre.fr/ark:/67375/TSO-VM3N240R-C>, <http://data.loterre.fr/ark:/67375/TSO-TNN44SLS-R>, <http://data.loterre.fr/ark:/67375/TSO-BD33KNNX-S>, <http://data.loterre.fr/ark:/67375/TSO-ZDBWP9RP-M>, <http://data.loterre.fr/ark:/67375/TSO-GCTBW7HJ-P>, <http://data.loterre.fr/ark:/67375/TSO-MFB71KWG-1>, <http://data.loterre.fr/ark:/67375/TSO-KCLNJ3JK-9>, <http://data.loterre.fr/ark:/67375/TSO-CQT7DBZS-F>, <http://data.loterre.fr/ark:/67375/TSO-HF09ZX0Z-Q> ;
  skos:topConceptOf <http://data.loterre.fr/ark:/67375/TSO> .

<http://data.loterre.fr/ark:/67375/TSO-DWM5ZS1M-P>
  a skos:Concept ;
  dc:modified "2021-06-30"^^xsd:date ;
  skos:altLabel "data codebook"@en, "repositorio de metadatos"@es ;
  skos:definition "A separate file where each variable of a dataset is defined, including units and ranges, and often includes other useful information for interpreting the dataset. (Source : Open Research Europe)"@en, "Collection de métadonnées ou de données de référence nécessaire à la conception d'une base de données relationnelle. (Source : collection de métadonnées ou de données de référence nécessaire à la conception d'une base de données relationnelle."@fr ;
  skos:prefLabel "data dictionary"@en, "diccionario de datos"@es, "dictionnaire des données"@fr ;
  skos:inScheme <http://data.loterre.fr/ark:/67375/TSO> ;
  skos:broader <http://data.loterre.fr/ark:/67375/TSO-T4KV78Z3-L> ;
  skos:related <http://data.loterre.fr/ark:/67375/TSO-ZQ5PMX6N-7> .

<http://data.loterre.fr/ark:/67375/TSO-R7K8WNB6-F>
  a skos:Concept ;
  dc:modified "2021-07-05"^^xsd:date ;
  skos:definition "Aplicación web de código abierto para conservar, compartir, citar, buscar y analizar datos de investigación."@es, "Application web à code source ouvert permettant de préserver, partager, citer, rechercher et analyser des données de recherche. (Source : https://fr.wikipedia.org/wiki/Dataverse)"@fr, "Open source web application to share, preserve, cite, explore, and analyze research data. It facilitates making data available to others, and allows you to replicate others' work more easily. Researchers, journals, data authors, publishers, data distributors, and affiliated institutions all receive academic credit and web visibility. (Source: https://dataverse.org/about)"@en ;
  skos:prefLabel "Dataverse"@en, "Dataverse"@es, "Dataverse"@fr ;
  skos:inScheme <http://data.loterre.fr/ark:/67375/TSO> ;
  skos:broader <http://data.loterre.fr/ark:/67375/TSO-LS0Q2K68-D> .

<http://data.loterre.fr/ark:/67375/TSO-QZKZVCDR-P>
  a skos:Concept ;
  dc:modified "2021-06-24"^^xsd:date ;
  skos:definition "Extension développée par un organisme non lucratif, qui vous permettra de repérer immédiatement si la page que vous visitez (y compris les sites des éditeurs) contient un ou plusieurs documents dont une version en ligne est accessible sur une archive ouverte, quelque part dans le monde. (Source : https://www.sciencespo.fr/bibliotheque/fr/enseignants-chercheurs/trucs-astuces/unpaywall.html)"@fr ;
  skos:prefLabel "Unpaywall"@en, "Unpaywall"@es, "Unpaywall"@fr ;
  skos:inScheme <http://data.loterre.fr/ark:/67375/TSO> ;
  skos:broader <http://data.loterre.fr/ark:/67375/TSO-WQMF6CT2-K> .

<http://data.loterre.fr/ark:/67375/TSO-MGZJDL80-2>
  a skos:Concept ;
  skos:altLabel "law"@en, "ley"@es, "loi"@fr ;
  skos:definition "Is a system of rules which are enforced through social institutions to govern behaviour. (Source : Foster)"@en ;
  skos:exactMatch <https://vocabularyserver.com/openscience/index.php?tema=53> ;
  skos:prefLabel "legal text"@en, "texte de loi"@fr, "texto jurídico"@es ;
  skos:inScheme <http://data.loterre.fr/ark:/67375/TSO> ;
  skos:broader <http://data.loterre.fr/ark:/67375/TSO-ZQ0Q8HMP-Q> ;
  skos:narrower <http://data.loterre.fr/ark:/67375/TSO-H96QTTW7-Z>, <http://data.loterre.fr/ark:/67375/TSO-FWFH6NFF-1>, <http://data.loterre.fr/ark:/67375/TSO-HZ81233X-G> .

<http://data.loterre.fr/ark:/67375/TSO-LV2TTMKZ-J>
  a skos:Concept ;
  dc:modified "2021-06-09"^^xsd:date ;
  skos:definition "Plan d'action issu de la conférence d'Amsterdam sur l'innovation en matière de science ouverte, qui s'est tenue les 4 et 5 avril 2016. Il définit deux objectifs principaux : permettre l’accès libre et total, d’ici 2020, à toutes les publications scientifiques et rendre systématique la possibilité de partage et de réutilisation des données pour toutes les recherches financées par des fonds publics. (Source : Ouvrir la science)"@fr, "This Call for Action is the main result of the Amsterdam conference on ‘Open Science– From Vision to Action’ hosted by the Netherlands’ EU presidency on 4 and 5 April 2016. Based on the input of all participating experts and stakeholders as well as outcomes of preceding international meetings and reports, a multi-actor approach was formulated to reach two important pan-European goals for 2020: full open access for all scientific publications and a fundamentally new approach towards optimal reuse of research data. (Source : Ouvrir la science)"@en ;
  skos:prefLabel "Amsterdam Call for Action on Open Science"@en, "llamada de acción de Amsterdam sobre ciencia abierta"@es, "plan d'action d'Amsterdam sur l'innovation en matière de science ouverte"@fr ;
  skos:inScheme <http://data.loterre.fr/ark:/67375/TSO> ;
  skos:broader <http://data.loterre.fr/ark:/67375/TSO-V6F4ZS65-G> .

<http://data.loterre.fr/ark:/67375/TSO-J8RJLSD1-C>
  a skos:Concept ;
  dc:modified "2021-06-29"^^xsd:date ;
  skos:altLabel "DORA"@en ;
  skos:definition "Declaration that recognizes the need to improve the ways in which researchers and the outputs of scholarly research are evaluated. (Source: https://sfdora.org/)"@en, "Déclaration qui affirme la nécessité de transformer les méthodes d'évaluation des résultats de la recherche scientifique. Il s'agit d'une initiative mondiale couvrant toutes les disciplines universitaires et tous les intervenants clés — agences de financement, établissements, éditeurs et chercheurs. (Source : https://www.ouvrirlascience.fr/declaration-de-san-francisco-sur-levaluation-de-la-recherche/)"@fr ;
  skos:prefLabel "San Francisco Declaration on Research Assessment"@en, "declaración de San Francisco sobre la evaluación de la investigación"@es, "déclaration de San-Francisco sur l'évaluation de la recherche"@fr ;
  skos:inScheme <http://data.loterre.fr/ark:/67375/TSO> ;
  skos:broader <http://data.loterre.fr/ark:/67375/TSO-V6F4ZS65-G> .

<http://data.loterre.fr/ark:/67375/TSO-CXNG80P6-X>
  a skos:Concept ;
  dc:modified "2021-06-29"^^xsd:date ;
  skos:definition "Déclaration de 2003 qui élargit la notion du libre accès à toutes les œuvres et données issues d’un travail de recherche, à tous les champs disciplinaires et au patrimoine culturel. Elle reprend les deux conditions définissant le libre accès de la Déclaration de Bethesda : un droit gratuit, irrévocable et mondial d’y accéder ; un dépôt dans au moins une archive en ligne."@fr, "International statement on open access and access to knowledge. It emerged from a conference on open access hosted in the Harnack House in Berlin by the Max Planck Society in 2003. (Source: https://en.wikipedia.org/wiki/Berlin_Declaration_on_Open_Access_to_Knowledge_in_the_Sciences_and_Humanities)"@en ;
  skos:prefLabel "Berlin declaration on Open Access to Knowledge in the Sciences and Humanities"@en, "Declaración de Berlín sobre Acceso Abierto al Conocimiento en Ciencias y Humanidades"@es, "déclaration de Berlin sur le libre accès à la connaissance en sciences exactes, sciences de la vie, sciences humaines et sociales"@fr ;
  skos:inScheme <http://data.loterre.fr/ark:/67375/TSO> ;
  skos:broader <http://data.loterre.fr/ark:/67375/TSO-K4MZGJ48-6> .

<http://data.loterre.fr/ark:/67375/TSO-BQ44K7KT-L>
  a skos:Concept ;
  dc:modified "2021-06-11"^^xsd:date ;
  skos:definition "Courses of actions relating to the online, free of cost, accessible data that can be used, reused and distributed provided that the data source is attributed and shared alike. (Source : Foster)"@en, "Lignes de conduite en lien avec l’ouverture des données pour qu’elles soient accessibles gratuitement en ligne et qu’on puisse les utiliser, réutiliser et distribuer à condition que leur source soit identifiée et que leur partage se fasse en vertu de la même licence ou d’une licence similaire. (Source : Foster)"@fr ;
  skos:exactMatch <https://vocabularyserver.com/openscience/index.php?tema=42> ;
  skos:prefLabel "open data policy"@en, "politique de données ouvertes"@fr, "política de datos abiertos"@es ;
  skos:inScheme <http://data.loterre.fr/ark:/67375/TSO> ;
  skos:broader <http://data.loterre.fr/ark:/67375/TSO-H0BSK47H-Z> .

<http://data.loterre.fr/ark:/67375/TSO-BKF02X3C-B>
  a skos:Concept ;
  dc:modified "2021-06-03"^^xsd:date ;
  skos:definition "Courses of actions relating to the online, free of cost access to peer reviewed scientific content with limited copyright and licensing restrictions. (Source : Foster)"@en, "Lignes de conduite liées à l’accès en ligne gratuit à du contenu scientifique évalué par les pairs, et ce, avec un nombre restreint de restrictions découlant du droit d’auteur et des licences. (Source : Foster)"@fr ;
  skos:exactMatch <https://vocabularyserver.com/openscience/index.php?tema=41> ;
  skos:prefLabel "open access policy"@en, "politique de libre accès"@fr, "política de acceso abierto"@es ;
  skos:inScheme <http://data.loterre.fr/ark:/67375/TSO> ;
  skos:broader <http://data.loterre.fr/ark:/67375/TSO-H0BSK47H-Z> .

<http://data.loterre.fr/ark:/67375/TSO-W04D2X5B-N>
  a skos:Concept ;
  dc:modified "2021-06-28"^^xsd:date ;
  skos:altLabel "gauche d'auteur"@fr ;
  skos:definition "concept opposé du copyright et proche du concept Creative Commons – qui s’en est inspiré. L’auteur, par ce système, autorise l’utilisation (copie, commercialisation…) et la modification de son œuvre mais l’œuvre copiée ou « dérivée » doit être produite et diffusée sous les mêmes conditions que l’œuvre originale. (source : https://openaccess.inist.fr/glossaire/ )"@fr ;
  skos:prefLabel "copyleft"@en, "copyleft"@es, "copyleft"@fr ;
  skos:inScheme <http://data.loterre.fr/ark:/67375/TSO> ;
  skos:broader <http://data.loterre.fr/ark:/67375/TSO-LJWH8NFT-D> ;
  skos:related <http://data.loterre.fr/ark:/67375/TSO-DSVQC015-X>, <http://data.loterre.fr/ark:/67375/TSO-ZQ3QKFX9-1> .

<http://data.loterre.fr/ark:/67375/TSO-VSV9ZJKQ-4>
  a skos:Concept ;
  dc:modified "2021-06-11"^^xsd:date ;
  skos:definition "Courses of actions adopted from organisations that supply money to researchers and research projects. (Source : Foster)"@en, "Lignes de conduite adoptées par des organismes qui financent la communauté de recherche et ses projets de recherche. (Source : Foster)"@fr ;
  skos:exactMatch <https://vocabularyserver.com/openscience/index.php?tema=38> ;
  skos:prefLabel "funders policy"@en, "politique des bailleurs de fonds"@fr, "política de donantes"@es ;
  skos:inScheme <http://data.loterre.fr/ark:/67375/TSO> ;
  skos:broader <http://data.loterre.fr/ark:/67375/TSO-QL0JTPZ5-J> .

<http://data.loterre.fr/ark:/67375/TSO-CV5H9HZH-V>
  a skos:Concept ;
  skos:definition "Best practice guidelines for applying Open Science and achieving its fundamental goals. (Source : Foster)"@en, "Lignes directrices sur les pratiques exemplaires dans l’application des principes de la science ouverte et dans l’atteinte de ses objectifs fondamentaux. (Source : Foster)"@fr ;
  skos:exactMatch <https://vocabularyserver.com/openscience/index.php?tema=6> ;
  skos:prefLabel "directrices sobre la ciencia abierta"@es, "lignes directrices sur la science ouverte"@fr, "open science guidelines"@en ;
  skos:inScheme <http://data.loterre.fr/ark:/67375/TSO> ;
  skos:broader <http://data.loterre.fr/ark:/67375/TSO-V0KSG0NC-P> ;
  skos:narrower <http://data.loterre.fr/ark:/67375/TSO-D91MV7TW-D>, <http://data.loterre.fr/ark:/67375/TSO-BV57RDXC-6>, <http://data.loterre.fr/ark:/67375/TSO-D9HJPTL6-X>, <http://data.loterre.fr/ark:/67375/TSO-DJ828LKC-C>, <http://data.loterre.fr/ark:/67375/TSO-TZVXPB5S-5>, <http://data.loterre.fr/ark:/67375/TSO-M6JMPCMG-1>, <http://data.loterre.fr/ark:/67375/TSO-DCJZX2TD-P>, <http://data.loterre.fr/ark:/67375/TSO-V25B9BQX-X>, <http://data.loterre.fr/ark:/67375/TSO-GKLZDCG9-4> .

<http://data.loterre.fr/ark:/67375/TSO-RJP3KXDF-1>
  a skos:Concept ;
  dc:modified "2021-06-02"^^xsd:date ;
  skos:definition "Refer to the standards relevant in the Research Data Management process. (Source : Foster)"@en ;
  skos:exactMatch <https://vocabularyserver.com/openscience/index.php?tema=51> ;
  skos:prefLabel "norma de gestión de datos de investigación"@es, "norme de gestion des données de recherche"@fr, "research data management standard"@en ;
  skos:inScheme <http://data.loterre.fr/ark:/67375/TSO> ;
  skos:broader <http://data.loterre.fr/ark:/67375/TSO-PPDJJQ22-H>, <http://data.loterre.fr/ark:/67375/TSO-T4KV78Z3-L> .

<http://data.loterre.fr/ark:/67375/TSO-RKX32RM6-2>
  a skos:Concept ;
  dc:modified "2021-06-22"^^xsd:date ;
  skos:definition "Echange de fonds entre individus en dehors des circuits financiers institutionnels. L'appel de fonds se fait à partir de la description d'un projet précis (artistique, humanitaire, entrepreneurial...), au moyen d'une plate-forme en ligne permettant de recueillir de nombreux apports de petits montants. Le financement peut prendre la forme d'un don, d'un prêt avec ou sans intérêts, ou encore d'un investissement en capital. (Source : https://www.economie.gouv.fr/cedef/financement-participatif#:~:text=Qu%27est-ce%20que%20le%20financement%20participatif%20%3F%20Le%20financement,financer%20un%20projet%20via%20une%20plateforme%20en%20ligne.)"@fr ;
  skos:prefLabel "crowdfunding"@en, "financement participatif"@fr, "financiación colectiva"@es ;
  skos:inScheme <http://data.loterre.fr/ark:/67375/TSO> ;
  skos:broader <http://data.loterre.fr/ark:/67375/TSO-MWXTBMQ8-9> .

<http://data.loterre.fr/ark:/67375/TSO-P2PM5GCP-8>
  a skos:Concept ;
  dc:modified "2021-07-05"^^xsd:date ;
  skos:altLabel "gold OA"@en, "gold open access"@en, "gold road"@en, "libre accès doré"@fr ;
  skos:definition "La voie dorée vers le libre accès est atteinte en publiant un article dans une revue. La revue doit être en libre accès (libre accès pur) ou se financer à l’aide d’abonnements mais offrir une option en libre accès (libre accès hybride). (Source : Foster)"@fr, "Los autores o las instituciones tienen que pagar los cargos de procesamiento de artículos para tener acceso a los materiales publicados. Es decir, pagan por adelantado para obtener a posteriori los documentos publicados de forma gratuita. (Fuente: https://universoabierto.org/2017/06/09/que-es-la-ruta-diamante-de-acceso-abierto/)"@es, "The gold route to open access is delivered via publishing an article in a journal. The journal may be an open access journal (pure open access), or a subscription based journal (hybrid open access) that offers an open access option. (Source : Foster)"@en ;
  skos:exactMatch <https://vocabularyserver.com/openscience/index.php?tema=16> ;
  skos:prefLabel "gold route"@en, "ruta dorada"@es, "voie dorée"@fr ;
  skos:inScheme <http://data.loterre.fr/ark:/67375/TSO> ;
  skos:broader <http://data.loterre.fr/ark:/67375/TSO-KHL25V0F-4> ;
  skos:related <http://data.loterre.fr/ark:/67375/TSO-RVCX7V2W-C> ;
  skos:narrower <http://data.loterre.fr/ark:/67375/TSO-DLBP9S2L-Z>, <http://data.loterre.fr/ark:/67375/TSO-G425PLR1-B>, <http://data.loterre.fr/ark:/67375/TSO-DCPLM2CT-F>, <http://data.loterre.fr/ark:/67375/TSO-PPGGLF1B-V>, <http://data.loterre.fr/ark:/67375/TSO-C4HBSRDM-X> .

<http://data.loterre.fr/ark:/67375/TSO-DVLD10C0-8>
  a skos:Concept ;
  dc:modified "2021-06-11"^^xsd:date ;
  skos:definition "Refer to a set of principles, typically mandated by various bodies, that should be followed when managing research data. (Source : Foster)"@en ;
  skos:exactMatch <https://vocabularyserver.com/openscience/index.php?tema=49> ;
  skos:prefLabel "politique de gestion des données de recherche"@fr, "política de gestión de datos de investigación"@es, "research data management policy"@en ;
  skos:inScheme <http://data.loterre.fr/ark:/67375/TSO> ;
  skos:broader <http://data.loterre.fr/ark:/67375/TSO-H0BSK47H-Z> .

<http://data.loterre.fr/ark:/67375/TSO-QF6TF23V-Q>
  a skos:Concept ;
  dc:modified "2021-06-29"^^xsd:date ;
  skos:definition "Peer validation process conducted openly on the Internet. (Source : Foster)"@en, "Processus de validation par les pairs mené de manière ouverte en ligne. (Source : Foster)"@fr ;
  skos:exactMatch <https://vocabularyserver.com/openscience/index.php?tema=31> ;
  skos:prefLabel "open peer review"@en, "revisión por pares abierta"@es, "évaluation ouverte par les pairs"@fr ;
  skos:inScheme <http://data.loterre.fr/ark:/67375/TSO> ;
  skos:broader <http://data.loterre.fr/ark:/67375/TSO-HK29ZRSC-0> .

<http://data.loterre.fr/ark:/67375/TSO-RZQ2K0K6-K>
  a skos:Concept ;
  dc:modified "2021-06-29"^^xsd:date ;
  skos:altLabel "open peer commentary"@en ;
  skos:definition "A variation of post-publication peer review, in which commentaries from specialists are solicited on published articles and the authors are invited to respond. (Source : https://en.wikipedia.org/wiki/Scholarly_peer_review#Open_peer_commentary)"@en, "Processus d'évaluation portant sur les articles publiés, les auteurs étant invités à répondre."@fr ;
  skos:prefLabel "comentario abierto"@es, "commentaire ouvert"@fr, "open commentary"@en ;
  skos:inScheme <http://data.loterre.fr/ark:/67375/TSO> ;
  skos:broader <http://data.loterre.fr/ark:/67375/TSO-KHGQZ6NK-4> .

<http://data.loterre.fr/ark:/67375/TSO-MSM5HV40-F>
  a skos:Concept ;
  skos:altLabel "altmetría"@es ;
  skos:definition "A project that produces article level metrics of scholarly articles from information collected from the Internet, such as social media sites, newspapers, and other sources. (Source : Foster)"@en, "Un projet qui produit des indicateurs sur les articles scientifiques à partir de l’information recueillie sur Internet, notamment sur les médias sociaux et dans les journaux. (Source : Foster)"@fr ;
  skos:exactMatch <https://vocabularyserver.com/openscience/index.php?tema=34> ;
  skos:prefLabel "altmetrics"@en, "mesure d’impact alternative"@fr, "métricas alternativas"@es ;
  skos:inScheme <http://data.loterre.fr/ark:/67375/TSO> ;
  skos:broader <http://data.loterre.fr/ark:/67375/TSO-T9Q25G6Q-S> .

<http://data.loterre.fr/ark:/67375/TSO-H93WKMMJ-B>
  a skos:Concept ;
  skos:definition "Projects relating to Open Science. (Source : Foster)"@en, "Projets liés à la science ouverte. (Source : Foster)"@fr ;
  skos:exactMatch <https://vocabularyserver.com/openscience/index.php?tema=10> ;
  skos:prefLabel "open science project"@en, "projet pour la science ouverte"@fr, "proyecto para la ciencia abierta"@es ;
  skos:inScheme <http://data.loterre.fr/ark:/67375/TSO> ;
  skos:related <http://data.loterre.fr/ark:/67375/TSO-JFJGKFN2-H> ;
  skos:narrower <http://data.loterre.fr/ark:/67375/TSO-F124WT34-H>, <http://data.loterre.fr/ark:/67375/TSO-MRHXBFZS-T>, <http://data.loterre.fr/ark:/67375/TSO-ZP6CXMWN-J>, <http://data.loterre.fr/ark:/67375/TSO-RJFTQR0V-N>, <http://data.loterre.fr/ark:/67375/TSO-LBHNZXQ6-L>, <http://data.loterre.fr/ark:/67375/TSO-FLVT4163-M>, <http://data.loterre.fr/ark:/67375/TSO-QL71JGQM-F>, <http://data.loterre.fr/ark:/67375/TSO-BKX9QBKJ-C>, <http://data.loterre.fr/ark:/67375/TSO-ZSC3265D-Z>, <http://data.loterre.fr/ark:/67375/TSO-JQQM0K0V-2>, <http://data.loterre.fr/ark:/67375/TSO-VRK75VT8-1> ;
  skos:topConceptOf <http://data.loterre.fr/ark:/67375/TSO> .

<http://data.loterre.fr/ark:/67375/TSO-QL0JTPZ5-J>
  a skos:Concept ;
  dc:modified "2021-06-11"^^xsd:date ;
  skos:definition "Appuis publics de la part d’organisations sur des enjeux spécifiques. (Source : Foster)"@fr, "Mentions émises de la part d’organisations sur des enjeux spécifiques."@fr, "Written endorsements by organisations on specific matters. (Source : Foster)"@en ;
  skos:exactMatch <https://vocabularyserver.com/openscience/index.php?tema=36> ;
  skos:prefLabel "organisational policy"@en, "politique organisationnelle"@fr, "política organizacional"@es ;
  skos:inScheme <http://data.loterre.fr/ark:/67375/TSO> ;
  skos:broader <http://data.loterre.fr/ark:/67375/TSO-H0BSK47H-Z> ;
  skos:narrower <http://data.loterre.fr/ark:/67375/TSO-FTK2F4DH-T>, <http://data.loterre.fr/ark:/67375/TSO-T6RG1XJN-7>, <http://data.loterre.fr/ark:/67375/TSO-VSV9ZJKQ-4> .

<http://data.loterre.fr/ark:/67375/TSO-ZMJ8VVB2-9>
  a skos:Concept ;
  dc:modified "2021-06-17"^^xsd:date ;
  skos:altLabel "negative data publication"@en, "null results publications"@en, "publication de données négatives"@fr, "publication de résultats non-probants"@fr ;
  skos:definition "Publication de résultats qui montrent l'invalidité d'une hypothèse ou d'une méthode de recherche."@fr, "The act of publishing results that do not support the hypothesis and nullify the aim of the research."@en ;
  skos:prefLabel "negative results publication"@en, "publicación de resultados negativos"@es, "publication de résultats négatifs"@fr ;
  skos:inScheme <http://data.loterre.fr/ark:/67375/TSO> ;
  skos:broader <http://data.loterre.fr/ark:/67375/TSO-QWKTFN2F-N> ;
  skos:related <http://data.loterre.fr/ark:/67375/TSO-XRBPKF38-J> .

<http://data.loterre.fr/ark:/67375/TSO-MRSCXRR9-2>
  a skos:Concept ;
  dc:modified "2021-06-04"^^xsd:date ;
  skos:definition "Les mégadonnées ouvertes sont d’immenses jeux de données qui sont parfois lourds à traiter. (Source : Foster)"@fr, "Open Big Data are massive data sets that sometimes is laborious to process. (Source : Foster)"@en ;
  skos:exactMatch <https://vocabularyserver.com/openscience/index.php?tema=18> ;
  skos:prefLabel "macrodatos abiertos"@es, "mégadonnées ouvertes"@fr, "open big data"@en ;
  skos:inScheme <http://data.loterre.fr/ark:/67375/TSO> ;
  skos:broader <http://data.loterre.fr/ark:/67375/TSO-V08MCZVP-H> .

<http://data.loterre.fr/ark:/67375/TSO-WZ0J1023-D>
  a skos:Concept ;
  dc:modified "2021-06-25"^^xsd:date ;
  skos:definition "License agreement which contains provisions that allow other individuals to reuse another creator's work, giving them four major freedoms. Without a special license, these uses are normally prohibited by copyright law or commercial license. Most free licenses are worldwide, royalty-free, non-exclusive, and perpetual, (Source : Wikipedia)"@en, "licence s'appliquant à une œuvre de l'esprit par laquelle l'auteur concède tous les droits ou une partie des droits que lui confère le droit d'auteur, en laissant au minimum quatre droits considérés fondamentaux aux utilisateurs : usage de l'œuvre ; étude de l'œuvre pour en comprendre le fonctionnement ou l'adapter à ses besoins ; modification (amélioration, extension et transformation) ou incorporation de l'œuvre en une œuvre dérivée ; redistribution de l'œuvre, c'est-à-dire sa diffusion à d'autres usagers, y compris commercialement. (Source Wikipedia)"@fr ;
  skos:exactMatch <https://vocabularyserver.com/openscience/index.php?tema=55> ;
  skos:prefLabel "licence libre"@fr, "licencia libre"@es, "open license"@en ;
  skos:inScheme <http://data.loterre.fr/ark:/67375/TSO> ;
  skos:broader <http://data.loterre.fr/ark:/67375/TSO-LJWH8NFT-D> ;
  skos:narrower <http://data.loterre.fr/ark:/67375/TSO-NCZNV1ZN-L>, <http://data.loterre.fr/ark:/67375/TSO-ZKK6WW4X-W>, <http://data.loterre.fr/ark:/67375/TSO-ZQ3QKFX9-1>, <http://data.loterre.fr/ark:/67375/TSO-T67S254S-S>, <http://data.loterre.fr/ark:/67375/TSO-QLJ4LTKK-K>, <http://data.loterre.fr/ark:/67375/TSO-PH7T4MNT-J> .

<http://data.loterre.fr/ark:/67375/TSO-G9J1WQ69-H>
  a skos:Concept ;
  dc:modified "2021-06-25"^^xsd:date ;
  skos:altLabel "OScH"@en, "matériel libre"@fr, "matériel ouvert"@fr, "open hardware"@en ;
  skos:definition "Open science hardware is the intersection of open source hardware and open science, where researchers and makers share instrument designs similar to code in free and open source software. (Source : https://medium.com/read-write-participate/supporting-open-science-hardware-1b1909e1f63b)"@en, "Tout matériel dont la conception peut être reproduite, les informations nécessaires à sa construction étant en libre accès."@fr ;
  skos:prefLabel "material científico abierto"@es, "matériel scientifique ouvert"@fr, "open science hardware"@en ;
  skos:inScheme <http://data.loterre.fr/ark:/67375/TSO> ;
  skos:broader <http://data.loterre.fr/ark:/67375/TSO-JFJGKFN2-H> ;
  skos:related <http://data.loterre.fr/ark:/67375/TSO-FXS77K89-G> .

<http://data.loterre.fr/ark:/67375/TSO-QXK0M64M-N>
  a skos:Concept ;
  dc:modified "2021-06-24"^^xsd:date ;
  skos:altLabel "IOI"@en ;
  skos:definition "Initiative ayant comme objectif d’obtenir un financement stable et constant, partout dans le monde, pour maintenir une infrastructure scientifique ouverte. (Source : https://www.ouvrirlascience.fr/jnso-2019/)"@fr ;
  skos:prefLabel "Invest in Open Infrastructure"@en, "Invest in Open Infrastructure"@es, "Invest in Open Infrastructure"@fr ;
  skos:inScheme <http://data.loterre.fr/ark:/67375/TSO> ;
  skos:broader <http://data.loterre.fr/ark:/67375/TSO-J64S3QDL-1> .

<http://data.loterre.fr/ark:/67375/TSO-X1K9R85M-K>
  a skos:Concept ;
  dc:modified "2021-06-24"^^xsd:date ;
  skos:altLabel "LOD"@en ;
  skos:definition "Mode de publication de données structurées qui permet de connecter et d'enrichir les métadonnées, de sorte que différentes représentations du même contenu peuvent être trouvées et que des liens peuvent être établis entre des ressources connexes."@fr ;
  skos:prefLabel "datos abiertos enlazados"@es, "données ouvertes liées"@fr, "linked open data"@en ;
  skos:inScheme <http://data.loterre.fr/ark:/67375/TSO> ;
  skos:broader <http://data.loterre.fr/ark:/67375/TSO-V08MCZVP-H> ;
  skos:related <http://data.loterre.fr/ark:/67375/TSO-BRLNRV51-S> .

<http://data.loterre.fr/ark:/67375/TSO-BRNV0DF5-3>
  a skos:Concept ;
  dc:modified "2021-07-05"^^xsd:date ;
  skos:definition "A podcast about Open Science, Open Access, Open Education, Open Data, Open Software, …"@en, "Un podcast sobre ciencia abierta, acceso abierto, educación abierta, datos abiertos, software de código abierto..."@es, "Un podcast sur la science ouverte, l'accès ouvert, l'éducation ouverte, les données ouvertes, les logiciels libres..."@fr ;
  skos:prefLabel "Open Science Talk"@en, "Open Science Talk"@es, "Open Science Talk"@fr ;
  skos:inScheme <http://data.loterre.fr/ark:/67375/TSO> ;
  skos:broader <http://data.loterre.fr/ark:/67375/TSO-DXZZDQSM-3> ;
  skos:related <http://data.loterre.fr/ark:/67375/TSO-MV5H4HGJ-2> .

<http://data.loterre.fr/ark:/67375/TSO-ZNX5Z1VV-S>
  a skos:Concept ;
  dc:created "2021-06-10"^^xsd:date ;
  dc:modified "2021-06-25"^^xsd:date ;
  skos:definition "Réservoir numérique contenant des documents issus de la recherche scientifique, généralement déposés par leurs auteurs, et permettant au grand public d'y accéder gratuitement et sans contraintes. (Source : https://fr.wikipedia.org/wiki/Archive_ouverte)"@fr ;
  skos:prefLabel "archive ouverte"@fr, "archivo abierto"@es, "open archive"@en ;
  skos:inScheme <http://data.loterre.fr/ark:/67375/TSO> ;
  skos:broader <http://data.loterre.fr/ark:/67375/TSO-W9KRS5Q3-6> ;
  skos:related <http://data.loterre.fr/ark:/67375/TSO-HZ175K8D-R> .

<http://data.loterre.fr/ark:/67375/TSO-VD8QW3Q6-7>
  a skos:Concept ;
  dc:modified "2021-06-29"^^xsd:date ;
  skos:altLabel "ROR identifier"@en, "Research Organization Registry identifier"@en ;
  skos:definition "Identifiant pérenne attribué à une organisme de recherche."@fr ;
  skos:prefLabel "ROR ID"@en, "identifiant ROR"@fr, "identificador ROR"@es ;
  skos:inScheme <http://data.loterre.fr/ark:/67375/TSO> ;
  skos:broader <http://data.loterre.fr/ark:/67375/TSO-H5ZG6DX6-4> .

<http://data.loterre.fr/ark:/67375/TSO-MJZBK64J-5>
  a skos:Concept ;
  dc:modified "2021-06-29"^^xsd:date ;
  skos:altLabel "DMP"@en, "PGD"@es, "PGD"@fr, "plan de gestion des données de recherche"@fr, "plan de gestión de datos de investigación"@es, "research data management plan"@en ;
  skos:definition "Formal document that outlines how to handle research data both during your research and after the research project is completed. (Source : Foster)"@en, "Outil de gestion des données qui se présente sous forme d’un document structuré en rubriques. Il a pour objectif de synthétiser la description et l’évolution des jeux de données d'un projet de recherche. Il prépare le partage, la réutilisation et la pérennisation des données. (Source : https://doranum.fr/plan-gestion-donnees-dmp/)"@fr ;
  skos:exactMatch <https://vocabularyserver.com/openscience/index.php?tema=47> ;
  skos:prefLabel "data management plan"@en, "plan de gestion des données"@fr, "plan de gestión de datos"@es ;
  skos:inScheme <http://data.loterre.fr/ark:/67375/TSO> ;
  skos:broader <http://data.loterre.fr/ark:/67375/TSO-T4KV78Z3-L> ;
  skos:related <http://data.loterre.fr/ark:/67375/TSO-GDCXNW8F-5> ;
  skos:narrower <http://data.loterre.fr/ark:/67375/TSO-QP6T79V4-5> .

<http://data.loterre.fr/ark:/67375/TSO-RGKFQW9J-K>
  a skos:Concept ;
  dc:modified "2021-06-24"^^xsd:date ;
  skos:definition "Droits conférés à l'individu par une création intellectuelle. Ils donnent généralement au créateur un droit exclusif sur l'utilisation de sa création pendant une certaine période. (Source : https://www.wto.org/french/tratop_f/trips_f/intel1_f.htm)"@fr, "Legally recognized exclusive rights to creations of the mind. (Source : Foster)"@en ;
  skos:exactMatch <https://vocabularyserver.com/openscience/index.php?tema=54> ;
  skos:prefLabel "Intellectual Property Rights"@en, "droits de propriété intellectuelle"@fr, "propiedad intelectual"@es ;
  skos:inScheme <http://data.loterre.fr/ark:/67375/TSO> ;
  skos:broader <http://data.loterre.fr/ark:/67375/TSO-ZQ0Q8HMP-Q> ;
  skos:related <http://data.loterre.fr/ark:/67375/TSO-HZ81233X-G> .

<http://data.loterre.fr/ark:/67375/TSO-T4KV78Z3-L>
  a skos:Concept ;
  dc:modified "2021-06-02"^^xsd:date ;
  skos:definition "Refer to the tools that assist in the Research Data Management process. (Source : Foster)"@en ;
  skos:exactMatch <https://vocabularyserver.com/openscience/index.php?tema=50> ;
  skos:prefLabel "herramienta de gestión de datos de investigación"@es, "outil de gestion des données de recherche"@fr, "research data management tool"@en ;
  skos:inScheme <http://data.loterre.fr/ark:/67375/TSO> ;
  skos:broader <http://data.loterre.fr/ark:/67375/TSO-V0KSG0NC-P> ;
  skos:related <http://data.loterre.fr/ark:/67375/TSO-GDCXNW8F-5> ;
  skos:narrower <http://data.loterre.fr/ark:/67375/TSO-DWM5ZS1M-P>, <http://data.loterre.fr/ark:/67375/TSO-RJP3KXDF-1>, <http://data.loterre.fr/ark:/67375/TSO-MJZBK64J-5>, <http://data.loterre.fr/ark:/67375/TSO-TKRVHS3M-S>, <http://data.loterre.fr/ark:/67375/TSO-XSC65JWB-F> .

<http://data.loterre.fr/ark:/67375/TSO-LS0Q2K68-D>
  a skos:Concept ;
  dc:modified "2021-06-10"^^xsd:date ;
  skos:definition "Refer to (online) services that assist in the Research Data Management process. (Source : Foster)"@en ;
  skos:exactMatch <https://vocabularyserver.com/openscience/index.php?tema=48> ;
  skos:prefLabel "data management service"@en, "service de gestion de données de recherche"@fr, "servicio de gestión de datos"@es ;
  skos:inScheme <http://data.loterre.fr/ark:/67375/TSO> ;
  skos:broader <http://data.loterre.fr/ark:/67375/TSO-V0HZ66HD-4> ;
  skos:narrower <http://data.loterre.fr/ark:/67375/TSO-G0NHM0CJ-G>, <http://data.loterre.fr/ark:/67375/TSO-GGMFZZJF-V>, <http://data.loterre.fr/ark:/67375/TSO-SXD143PV-3>, <http://data.loterre.fr/ark:/67375/TSO-W2TL7C50-G>, <http://data.loterre.fr/ark:/67375/TSO-TZDDF74F-J>, <http://data.loterre.fr/ark:/67375/TSO-B4WKXG50-6>, <http://data.loterre.fr/ark:/67375/TSO-R7K8WNB6-F>, <http://data.loterre.fr/ark:/67375/TSO-LGJTJ71S-5>, <http://data.loterre.fr/ark:/67375/TSO-S30N1B85-1>, <http://data.loterre.fr/ark:/67375/TSO-CX6BNH0X-Z>, <http://data.loterre.fr/ark:/67375/TSO-VDCNM6ZN-W> .

<http://data.loterre.fr/ark:/67375/TSO-ZQ5PMX6N-7>
  a skos:Concept ;
  dc:modified "2021-07-05"^^xsd:date ;
  skos:definition "Agrégation de données brutes ou dérivées présentant une certaine \"unité\", rassemblées pour former un ensemble cohérent. (Source : https://coop-ist.cirad.fr/)"@fr, "Colección de datos habitualmente tabulada.[...] contiene los valores para cada una de las variables, como por ejemplo la altura y el peso de un objeto, que corresponden a cada miembro del conjunto de datos. Cada uno de estos valores se conoce con el nombre de dato. El conjunto de datos puede incluir datos para uno o más miembros en función de su número de filas. (Fuente: https://es.wikipedia.org/wiki/Conjunto_de_datos)"@es ;
  skos:prefLabel "conjunto de datos"@es, "data set"@en, "jeu de données"@fr ;
  skos:inScheme <http://data.loterre.fr/ark:/67375/TSO> ;
  skos:broader <http://data.loterre.fr/ark:/67375/TSO-MJRKBMDW-Q> ;
  skos:related <http://data.loterre.fr/ark:/67375/TSO-DWM5ZS1M-P> .

<http://data.loterre.fr/ark:/67375/TSO-DJ828LKC-C>
  a skos:Concept ;
  dc:modified "2021-06-29"^^xsd:date ;
  skos:altLabel "COAR/SPARC principles"@en, "Good Practice Principles for Scholarly Communication Services"@en, "principios de buenas prácticas para servicios de comunicación académicos"@es ;
  skos:definition "Ensemble de sept bonnes pratiques élaboré par COAR et SPARC pour les services de communication savante, l'objectif étant de s'assurer que les services sont transparents, ouverts et soutiennent les objectifs visés."@fr, "Joint statement published in September 2017 by COAR and SPARC, related to the need to collaborate with others on actions that will ensure research communication services are better aligned with the aims of research. Accordingly, COAR and SPARC have developed seven good practice principles for scholarly communication services. The aim is to ensure that services are transparent, open, and support the aims of scholarship. (Source: https://www.infodocket.com/2019/01/29/coar-and-sparc-release-good-practice-principles-for-scholarly-communication-services/)"@en ;
  skos:prefLabel "Good Practice Principles"@en, "Good Practice Principles"@es, "Good Practice Principles"@fr ;
  skos:inScheme <http://data.loterre.fr/ark:/67375/TSO> ;
  skos:broader <http://data.loterre.fr/ark:/67375/TSO-CV5H9HZH-V> ;
  skos:related <http://data.loterre.fr/ark:/67375/TSO-B8PFXG89-F>, <http://data.loterre.fr/ark:/67375/TSO-G587Q9G3-2>, <http://data.loterre.fr/ark:/67375/TSO-HF09ZX0Z-Q> .

<http://data.loterre.fr/ark:/67375/TSO-V6F4ZS65-G>
  a skos:Concept ;
  skos:altLabel "open science initiative"@en ;
  skos:prefLabel "open science reference text"@en, "texte de référence sur la science ouverte"@fr, "texto de referencia a propósito de la ciencia abierta"@es ;
  skos:inScheme <http://data.loterre.fr/ark:/67375/TSO> ;
  skos:related <http://data.loterre.fr/ark:/67375/TSO-JFJGKFN2-H> ;
  skos:narrower <http://data.loterre.fr/ark:/67375/TSO-K4MZGJ48-6>, <http://data.loterre.fr/ark:/67375/TSO-FBNDZZDV-2>, <http://data.loterre.fr/ark:/67375/TSO-LV2TTMKZ-J>, <http://data.loterre.fr/ark:/67375/TSO-J8RJLSD1-C>, <http://data.loterre.fr/ark:/67375/TSO-TVL7X12H-M>, <http://data.loterre.fr/ark:/67375/TSO-T5VDL564-T>, <http://data.loterre.fr/ark:/67375/TSO-B7FV4N90-B>, <http://data.loterre.fr/ark:/67375/TSO-LBM5XNCF-J>, <http://data.loterre.fr/ark:/67375/TSO-FK1RPNQP-Z>, <http://data.loterre.fr/ark:/67375/TSO-WVJZTQCD-F> ;
  skos:topConceptOf <http://data.loterre.fr/ark:/67375/TSO> .

<http://data.loterre.fr/ark:/67375/TSO-BTFX00Q2-P>
  a skos:Concept ;
  dc:modified "2021-06-29"^^xsd:date ;
  skos:definition "A non-profit technology organization based in Charlottesville, Virginia with a mission to \"increase the openness, integrity, and reproducibility of scientific research. (Source : Wikipedia)"@en, "Organisme à but non lucratif situé à Charlottesville, en Virginie. Il a pour but de « favoriser l'ouverture, l'intégrité et la reproductibilité de la recherche scientifique » (Source : Wikipedia)"@fr, "Organización tecnológica sin fines de lucro con sede en Charlottesville, Virginia, con la misión de \"aumentar la apertura, integridad y reproducibilidad de la investigación científica\". (Fuente: Wikipedia)"@es ;
  skos:prefLabel "Center for Open Science"@en, "Center for Open Science"@es, "Center for Open Science"@fr ;
  skos:inScheme <http://data.loterre.fr/ark:/67375/TSO> ;
  skos:broader <http://data.loterre.fr/ark:/67375/TSO-J64S3QDL-1> ;
  skos:related <http://data.loterre.fr/ark:/67375/TSO-D91MV7TW-D>, <http://data.loterre.fr/ark:/67375/TSO-G3F0KPMJ-P>, <http://data.loterre.fr/ark:/67375/TSO-LSLV4BQG-0> .

<http://data.loterre.fr/ark:/67375/TSO-VPJV1Q5X-J>
  a skos:Concept ;
  dc:modified "2021-06-29"^^xsd:date ;
  skos:altLabel "CoSO"@fr ;
  skos:definition "Comité institué en 2018 par le Ministère français de l’enseignement supérieur, de la recherche et de l’innovation et présidé par le Directeur général de la recherche et de l’innovation. Il assure la mise en œuvre d’une politique de soutien à l’ouverture des publications et des données de la recherche et se décline en quatre collèges : publication, données de la recherche, compétences et formation, Europe et international. (Source : https://www.ouvrirlascience.fr/presentation-du-comite/)"@fr ;
  skos:prefLabel "Comité pour la science ouverte"@es, "Comité pour la science ouverte"@fr, "Open Science Committee"@en ;
  skos:inScheme <http://data.loterre.fr/ark:/67375/TSO> ;
  skos:broader <http://data.loterre.fr/ark:/67375/TSO-J64S3QDL-1> ;
  skos:related <http://data.loterre.fr/ark:/67375/TSO-JQQM0K0V-2>, <http://data.loterre.fr/ark:/67375/TSO-TNN44SLS-R>, <http://data.loterre.fr/ark:/67375/TSO-VPTBZS30-F> .

<http://data.loterre.fr/ark:/67375/TSO-G4MG47JW-H>
  a skos:Concept ;
  dc:modified "2021-07-05"^^xsd:date ;
  skos:altLabel "EOSC"@en, "EOSC"@es, "EOSC"@fr ;
  skos:definition "European Commission initiative, officially launched in November 2018, aiming at developing an infrastructure providing its users with services promoting open science practices. (Source : Wikipedia)"@en, "Iniciativa lanzada oficialmente en noviembre de 2018 por la Comisión Europea, cuyo objetivo es desarrollar una instalación que proporcione a sus usuarios servicios de computación en la nube para las prácticas de ciencia abierta."@es, "Initiative lancée officiellement en novembre 2018 par la Commission européenne, qui vise à développer un dispositif fournissant à ses utilisateurs des services d'informatique en nuage pour les pratiques de science ouverte. (Source : Wikipedia)"@fr ;
  skos:prefLabel "European Open Science Cloud"@en, "European Open Science Cloud"@es, "European Open Science Cloud"@fr ;
  skos:inScheme <http://data.loterre.fr/ark:/67375/TSO> ;
  skos:broader <http://data.loterre.fr/ark:/67375/TSO-J64S3QDL-1>, <http://data.loterre.fr/ark:/67375/TSO-V0HZ66HD-4> .

<http://data.loterre.fr/ark:/67375/TSO-NK8GHW7D-6>
  a skos:Concept ;
  dc:modified "2021-06-29"^^xsd:date ;
  skos:altLabel "BOAI"@en ;
  skos:definition "Déclaration de principe et de stratégie sur le libre accès aux recherches scientifiques, lancée en février 2002 : elle préconise l'auto-archivage institutionnel des publications par le chercheur ainsi que la création de nouvelles revues en accès libre. Elle propose aussi une aide pour les revues (anciennes ou nouvelles) qui accepteraient de travailler dans une optique de libre accès en ligne. Toutes les archives et publications doivent être compatibles OAI pour permettre une consultation en réseau. (Source : https://archivesic.ccsd.cnrs.fr/sic_00493625)"@fr ;
  skos:editorialNote "Link to the reference text: https://www.budapestopenaccessinitiative.org/read"@en, "https://www.budapestopenaccessinitiative.org/translations/spanish-translation"@es ;
  skos:prefLabel "Budapest Open Access Initiative"@en, "Budapest Open Access Initiative"@es, "initiative de Budapest pour l’accès ouvert"@fr ;
  skos:inScheme <http://data.loterre.fr/ark:/67375/TSO> ;
  skos:broader <http://data.loterre.fr/ark:/67375/TSO-K4MZGJ48-6> .

<http://data.loterre.fr/ark:/67375/TSO-D7TJZP51-Z>
  a skos:Concept ;
  dc:modified "2021-06-28"^^xsd:date ;
  skos:definition "Déclarations de principe rédigée au cours de la réunion du 11 avril 2003 au siège du Howard Hughes Medical Institute à Chevy Chase dans l’Etat de Maryland (USA). Elle définit deux conditions que doivent remplir les publications pour être en libre accès : un droit gratuit, irrévocable d’y accéder, de les copier, utiliser, distribuer et de réaliser des œuvres dérivées ; un dépôt dans une archive ouverte assurant le libre accès, l’interopérabilité et l’archivage à long terme. (Source : https://www.ouvrirlascience.fr/declaration-de-bethesda-pour-ledition-en-libre-acces/)"@fr ;
  skos:prefLabel "Bethesda Statement on Open Access Publishing"@en, "Declaración de Bethesda sobre la publicación del Acceso Ablerto"@es, "déclaration de Bethesda pour l’édition en libre accès"@fr ;
  skos:inScheme <http://data.loterre.fr/ark:/67375/TSO> ;
  skos:broader <http://data.loterre.fr/ark:/67375/TSO-K4MZGJ48-6> .

<http://data.loterre.fr/ark:/67375/TSO-PCHZG84P-8>
  a skos:Concept ;
  dc:modified "2021-06-25"^^xsd:date ;
  skos:definition "Données qui sous-tendent les résultats de la recherche scientifique et dont l'accès n'est soumis à aucune restriction, permettant à quiconque d'y accéder."@fr, "The data underpinning scientific research results that has no restrictions on its access, enabling anyone to access it. (Source: https://ec.europa.eu/info/research-and-innovation/strategy/strategy-2020-2024/our-digital-future/open-science/open-science-monitor/facts-and-figures-open-research-data_en)"@en ;
  skos:prefLabel "datos de investigación abiertos"@es, "données de recherche ouvertes"@fr, "open research data"@en ;
  skos:inScheme <http://data.loterre.fr/ark:/67375/TSO> ;
  skos:broader <http://data.loterre.fr/ark:/67375/TSO-DP8MN2RF-P>, <http://data.loterre.fr/ark:/67375/TSO-V08MCZVP-H> .

<http://data.loterre.fr/ark:/67375/TSO-DP8MN2RF-P>
  a skos:Concept ;
  dc:modified "2021-06-25"^^xsd:date ;
  skos:altLabel "données de la recherche"@fr ;
  skos:definition "Enregistrements factuels (chiffres, textes, images et sons), qui sont utilisés comme sources principales pour la recherche scientifique et sont généralement reconnus par la communauté scientifique comme nécessaires pour valider des résultats de recherche. (Source : https://scienceouverte.couperin.org/donnees-recherche-definitions/)"@fr ;
  skos:prefLabel "datos de investigación"@es, "données de recherche"@fr, "research data"@en ;
  skos:inScheme <http://data.loterre.fr/ark:/67375/TSO> ;
  skos:broader <http://data.loterre.fr/ark:/67375/TSO-MJRKBMDW-Q> ;
  skos:related <http://data.loterre.fr/ark:/67375/TSO-D9HJPTL6-X>, <http://data.loterre.fr/ark:/67375/TSO-GDCXNW8F-5>, <http://data.loterre.fr/ark:/67375/TSO-J0H32WL6-Z>, <http://data.loterre.fr/ark:/67375/TSO-J9P20ZD1-C>, <http://data.loterre.fr/ark:/67375/TSO-LBHNZXQ6-L>, <http://data.loterre.fr/ark:/67375/TSO-ZSC3265D-Z> ;
  skos:narrower <http://data.loterre.fr/ark:/67375/TSO-PCHZG84P-8> .

<http://data.loterre.fr/ark:/67375/TSO-TJTXZ4LV-W>
  a skos:Concept ;
  dc:modified "2021-06-29"^^xsd:date ;
  skos:altLabel "mathematics in open access"@en ;
  skos:definition "Fondation qui œuvre pour la transition des revues de mathématiques vers des modèles de publication respectant les principes du « libre accès juste ». (Source : https://www.ouvrirlascience.fr/comment-les-scientifiques-sorganisent-pour-saffranchir-des-aspects-commerciaux-des-revues/)"@fr, "Organization that facilitates conversion to fair open access of journals in mathematics (source: https://www.fairopenaccess.org/)"@en ;
  skos:prefLabel "mathOA"@en, "mathOA"@es, "mathOA"@fr ;
  skos:inScheme <http://data.loterre.fr/ark:/67375/TSO> ;
  skos:broader <http://data.loterre.fr/ark:/67375/TSO-J64S3QDL-1> ;
  skos:related <http://data.loterre.fr/ark:/67375/TSO-GCTBW7HJ-P> .

<http://data.loterre.fr/ark:/67375/TSO-PPGGLF1B-V>
  a skos:Concept ;
  dc:modified "2021-06-15"^^xsd:date ;
  skos:altLabel "modèle sponsor"@fr, "sponsor model"@en ;
  skos:definition "Modèle économique dans lequel le financement de la revue est pris en charge par une société savante, un organisme de recherche, une fondation… (source : https://openaccess.inist.fr/glossaire/ )"@fr ;
  skos:prefLabel "modèle sponsor-payeur"@fr, "sponsorship"@en, "sponsorship"@es ;
  skos:inScheme <http://data.loterre.fr/ark:/67375/TSO> ;
  skos:broader <http://data.loterre.fr/ark:/67375/TSO-P2PM5GCP-8> .

<http://data.loterre.fr/ark:/67375/TSO-NX4NVXX2-L>
  a skos:Concept ;
  dc:modified "2021-06-24"^^xsd:date ;
  skos:altLabel "ejournal superpuesta"@es, "epijournal"@en ;
  skos:definition "An open access, electronic journal that does not produce its own content, but selects and curates groups of articles that are already freely available online. (Source : Wikipedia)"@en, "Revue électronique en libre accès, alimentée par les articles déposés dans les archives ouvertes et non publiés par ailleurs. (Source : CCSD)"@fr ;
  skos:prefLabel "overlay journal"@en, "revista superpuesta"@es, "épirevue"@fr ;
  skos:inScheme <http://data.loterre.fr/ark:/67375/TSO> ;
  skos:broader <http://data.loterre.fr/ark:/67375/TSO-TM0MS2GV-7> ;
  skos:related <http://data.loterre.fr/ark:/67375/TSO-HS79BV00-V>, <http://data.loterre.fr/ark:/67375/TSO-NT6B4GTK-3> .

<http://data.loterre.fr/ark:/67375/TSO-TVL7X12H-M>
  a skos:Concept ;
  dc:modified "2021-07-05"^^xsd:date ;
  skos:definition "An initiative for Open Access publishing that was launched in September 2018. The plan is supported by cOAlition S, an international consortium of research funding and performing organisations. Plan S requires that, from 2021, scientific publications that result from research funded by public grants must be published in compliant Open Access journals or platforms. (Source: https://www.coalition-s.org/)"@en, "Initiative de la Commission européenne et de la cOAlition S lancée le 4 septembre 2018. Elle promeut l'édition scientifique en libre accès selon l'objectif : « Après le 1er janvier 2021, les publications scientifiques sur les résultats de la recherche financée sur fonds publics accordés par des agences de recherche ou des organismes de financement nationaux ou européens, doivent être publiées dans des revues ou sur des plateformes en accès libre. »"@fr ;
  skos:prefLabel "plan S"@en, "plan S"@es, "plan S"@fr ;
  skos:inScheme <http://data.loterre.fr/ark:/67375/TSO> ;
  skos:broader <http://data.loterre.fr/ark:/67375/TSO-V6F4ZS65-G> ;
  skos:related <http://data.loterre.fr/ark:/67375/TSO-GCQ559K4-Q> .

<http://data.loterre.fr/ark:/67375/TSO-H0BSK47H-Z>
  a skos:Concept ;
  skos:prefLabel "open science policy"@en, "politique de science ouverte"@fr, "política de ciencia abierta"@es ;
  skos:inScheme <http://data.loterre.fr/ark:/67375/TSO> ;
  skos:related <http://data.loterre.fr/ark:/67375/TSO-GQVTBXJ4-X>, <http://data.loterre.fr/ark:/67375/TSO-QXH951LF-0> ;
  skos:narrower <http://data.loterre.fr/ark:/67375/TSO-G4CFRKD0-L>, <http://data.loterre.fr/ark:/67375/TSO-BQ44K7KT-L>, <http://data.loterre.fr/ark:/67375/TSO-BKF02X3C-B>, <http://data.loterre.fr/ark:/67375/TSO-DVLD10C0-8>, <http://data.loterre.fr/ark:/67375/TSO-QL0JTPZ5-J> ;
  skos:topConceptOf <http://data.loterre.fr/ark:/67375/TSO> .

<http://data.loterre.fr/ark:/67375/TSO-C4HBSRDM-X>
  a skos:Concept ;
  dc:modified "2021-06-15"^^xsd:date ;
  skos:altLabel "reader-pays"@en, "reader-side fee model"@en ;
  skos:definition "correspond au modèle traditionnel de l’édition, l’abonnement. Le lecteur ne peut avoir accès qu’aux revues et aux ouvrages pour lesquels il a pris, mais le plus souvent il s’agit de son institution, un abonnement auprès d’un ou plusieurs éditeurs. (source : https://openaccess.inist.fr/glossaire/ )"@fr ;
  skos:prefLabel "modèle lecteur-payeur"@fr, "reader-payer model"@en, "reader-payer model"@es ;
  skos:inScheme <http://data.loterre.fr/ark:/67375/TSO> ;
  skos:broader <http://data.loterre.fr/ark:/67375/TSO-P2PM5GCP-8> .

<http://data.loterre.fr/ark:/67375/TSO-FWFH6NFF-1>
  a skos:Concept ;
  skos:altLabel "Regulation on the protection of natural persons with regard to the processing of personal data and on the free movement of such data, and repealing Directive 95/46/EC (Data Protection Directive)"@en, "Règlement (UE) 2016/679 du Parlement européen et du Conseil du 27 avril 2016, relatif à la protection des personnes physiques à l'égard du traitement des données à caractère personnel et à la libre circulation de ces données, et abrogeant la directive 95/46/CE"@fr, "general data protection regulation"@en, "reglamento general de protección de datos"@es, "règlement général sur la protection des données"@fr ;
  skos:definition "A regulation in EU law on data protection and privacy in the European Union (EU) and the European Economic Area (EEA). It also addresses the transfer of personal data outside the EU and EEA areas. (Source : wikipedia)"@en, "Règlement de l'Union européenne qui constitue le texte de référence en matière de protection des données à caractère personnel. Il renforce et unifie la protection des données pour les individus au sein de l'Union européenne. (Source : Wikipédia)"@fr, "seeks to create a harmonised data protection law framework across the EU. It aims to restitute the control of personal data to citizens, whilst imposing strict rules on those hosting and 'processing' these data, anywhere in the world. The Regulation also introduces rules relating to the free movement of personal data within and outside the EU. (source: https://open-science-training-handbook.gitbook.io/book/glossary)"@en ;
  skos:prefLabel "GDPR"@en, "RGPD"@es, "RGPD"@fr ;
  skos:inScheme <http://data.loterre.fr/ark:/67375/TSO> ;
  skos:broader <http://data.loterre.fr/ark:/67375/TSO-MGZJDL80-2> ;
  skos:related <http://data.loterre.fr/ark:/67375/TSO-RH261KDT-S> .

<http://data.loterre.fr/ark:/67375/TSO-RN1XP625-F>
  a skos:Concept ;
  dc:modified "2021-06-24"^^xsd:date ;
  skos:altLabel "journal hybride"@fr ;
  skos:definition "Revue accessible uniquement sous abonnement, mais dans laquelle un auteur est libre de publier ses travaux en libre accès, moyennant le versement de frais de publication supplémentaires. (source: https://openaccess.univ-rennes1.fr/les-revues-hybrides)"@fr, "a subscription journal in which some of the articles are open access at point of publication. (source: https://casrai.org/open-access-glossary/)"@en ;
  skos:prefLabel "hybrid journal"@en, "revista híbrida"@es, "revue hybride"@fr ;
  skos:inScheme <http://data.loterre.fr/ark:/67375/TSO> ;
  skos:broader <http://data.loterre.fr/ark:/67375/TSO-TM0MS2GV-7> ;
  skos:related <http://data.loterre.fr/ark:/67375/TSO-DCPLM2CT-F>, <http://data.loterre.fr/ark:/67375/TSO-QL8P69BW-V> .

<http://data.loterre.fr/ark:/67375/TSO-RVCX7V2W-C>
  a skos:Concept ;
  dc:modified "2021-07-05"^^xsd:date ;
  skos:definition "Revue qui met ses articles en ligne immédiatement à la disposition du lecteur sans obstacles financiers, juridiques ou techniques autres que ceux indissociables de l'accès à l'internet lui-même."@fr, "Una revista que pone sus artículos inmediatamente a disposición del lector en Internet sin más barreras financieras, legales o técnicas que las inseparables del propio acceso a Internet."@es, "scholarly journal that makes its articles immediately available online to the reader without financial, legal, or technical barriers other than those inseparable from gaining access to the internet itself. (source: https://casrai.org/open-access-glossary/)"@en ;
  skos:prefLabel "pure gold journal"@en, "revue nativement en libre accès"@es, "revue nativement en libre accès"@fr ;
  skos:inScheme <http://data.loterre.fr/ark:/67375/TSO> ;
  skos:broader <http://data.loterre.fr/ark:/67375/TSO-TM0MS2GV-7> ;
  skos:related <http://data.loterre.fr/ark:/67375/TSO-P2PM5GCP-8> .

<http://data.loterre.fr/ark:/67375/TSO-ZMQ5Z0BN-L>
  a skos:Concept ;
  dc:modified "2021-06-09"^^xsd:date ;
  skos:definition "Mode d'accès dans lequel les articles d'une revues sont dès leur mise en ligne accessibles à tous, sans abonnement. (source: https://salons.erudit.org/2017/10/18/libre-acces-immediat-et-libre-acces-differe)"@fr ;
  skos:prefLabel "immediate open access"@en, "libre acceso inmediato"@es, "libre accès immédiat"@fr ;
  skos:inScheme <http://data.loterre.fr/ark:/67375/TSO> ;
  skos:broader <http://data.loterre.fr/ark:/67375/TSO-STWL5MWS-W> .

<http://data.loterre.fr/ark:/67375/TSO-W81HHLG2-F>
  a skos:Concept ;
  dc:modified "2021-06-17"^^xsd:date ;
  skos:definition "opérations de validation successives que subit un document dans une archive ouverte. (source: https://openaccess.inist.fr/glossaire/)"@fr ;
  skos:prefLabel "estampación"@es, "estampillage"@fr, "stamping"@en ;
  skos:inScheme <http://data.loterre.fr/ark:/67375/TSO> ;
  skos:broader <http://data.loterre.fr/ark:/67375/TSO-KHGQZ6NK-4> .

<http://data.loterre.fr/ark:/67375/TSO-HK29ZRSC-0>
  a skos:Concept ;
  dc:modified "2021-06-29"^^xsd:date ;
  skos:altLabel "peer reviewing"@en, "validation par les pairs"@fr ;
  skos:definition "Activité collective des chercheurs qui jugent de façon critique les travaux d'autres chercheurs (leurs « pairs »). (Source : Wikipédia)"@fr ;
  skos:prefLabel "peer review"@en, "revisión por pares"@es, "évaluation par les pairs"@fr ;
  skos:inScheme <http://data.loterre.fr/ark:/67375/TSO> ;
  skos:broader <http://data.loterre.fr/ark:/67375/TSO-KHGQZ6NK-4> ;
  skos:related <http://data.loterre.fr/ark:/67375/TSO-MDD3CCP5-9> ;
  skos:narrower <http://data.loterre.fr/ark:/67375/TSO-QF6TF23V-Q> .

<http://data.loterre.fr/ark:/67375/TSO-DSVQC015-X>
  a skos:Concept ;
  dc:modified "2021-06-28"^^xsd:date ;
  skos:altLabel "derecho de autor"@es, "droit d'auteur"@fr ;
  skos:definition "Concept qui couvre les droits exclusifs accordés aux auteurs d’œuvres originales fixées sur un support matériel : droits de reproduction, d’adaptation, de distribution… (source : https://openaccess.inist.fr/glossaire/ )"@fr, "the aspect of Intellectual property that grants creators the right to permit (or not permit) the reproduction of their creations. It is distinct from trademark rights or moral rights. (source: https://open-science-training-handbook.gitbook.io/book/glossary)"@en ;
  skos:prefLabel "copyright"@en, "copyright"@es, "copyright"@fr ;
  skos:inScheme <http://data.loterre.fr/ark:/67375/TSO> ;
  skos:broader <http://data.loterre.fr/ark:/67375/TSO-LJWH8NFT-D> ;
  skos:related <http://data.loterre.fr/ark:/67375/TSO-W04D2X5B-N> .

<http://data.loterre.fr/ark:/67375/TSO-WH5JC3TT-G>
  a skos:Concept ;
  skos:definition "A suite of licences that set out the rights of authors and users, providing alternatives to the standard copyright. (Source : https://creativecommons.org/licenses/)"@en, "Contrat-type dans lequel les auteurs déterminent les droits attachés à l’œuvre qu’ils réalisent. Six contrats sont possibles en combinant quatre éléments de base qui sont : la paternité, la modification, l’utilisation commerciale et la réutilisation dans les mêmes conditions du contrat d’origine. Elles peuvent s’appliquer à tout type d’œuvres ou un ensemble d’œuvres. (source : https://openaccess.inist.fr/glossaire/ )"@fr ;
  skos:prefLabel "creative commons license"@en, "licence creative commons"@fr, "licencia creative commons"@es ;
  skos:inScheme <http://data.loterre.fr/ark:/67375/TSO> ;
  skos:broader <http://data.loterre.fr/ark:/67375/TSO-LJWH8NFT-D> ;
  skos:narrower <http://data.loterre.fr/ark:/67375/TSO-NCZNV1ZN-L>, <http://data.loterre.fr/ark:/67375/TSO-ZQ3QKFX9-1>, <http://data.loterre.fr/ark:/67375/TSO-ZK0KHM67-X>, <http://data.loterre.fr/ark:/67375/TSO-F844JJK0-Q>, <http://data.loterre.fr/ark:/67375/TSO-XNNFBR4D-D>, <http://data.loterre.fr/ark:/67375/TSO-LXH6ZFD2-J>, <http://data.loterre.fr/ark:/67375/TSO-QLJ4LTKK-K> .

<http://data.loterre.fr/ark:/67375/TSO-PBQJJSDV-W>
  a skos:Concept ;
  skos:altLabel "GNU GPL"@en, "GNU general public licence"@en, "GNU/GPL"@en, "GP"@en, "licence GNU/GPL"@fr, "licencia GNU GPL"@es ;
  skos:definition "A series of widely-used free software licenses that guarantee end users the freedom to run, study, share, and modify the software. (Source : Wikipedia)"@en, "free, copyleft license for software and other kinds of works. (source: https://www.gnu.org/licenses/gpl-3.0.fr.html)"@en, "licence qui fixe les conditions légales de distribution des logiciels libres du projet GNU. (source: https://www.techno-science.net/definition/620.html)"@fr ;
  skos:prefLabel "GNU general public license"@en, "licence publique générale GNU"@fr, "licencia pública general de GNU"@es ;
  skos:inScheme <http://data.loterre.fr/ark:/67375/TSO> ;
  skos:broader <http://data.loterre.fr/ark:/67375/TSO-T67S254S-S> .

<http://data.loterre.fr/ark:/67375/TSO-XBFF1KGS-V>
  a skos:Concept ;
  dc:modified "2021-06-11"^^xsd:date ;
  skos:definition "base de données qui supporte le protocole OAI-PMH et est constituée par un fournisseur de données. Elle contient des métadonnées qui sont disponibles dans différents formats afin de répondre à différents types de demandes. (Source : https://openaccess.inist.fr/glossaire/)"@fr ;
  skos:prefLabel "OAI repository"@en, "dépôt d'archives OAI"@fr, "repositorio de archivos OAI"@es ;
  skos:inScheme <http://data.loterre.fr/ark:/67375/TSO> ;
  skos:broader <http://data.loterre.fr/ark:/67375/TSO-W9KRS5Q3-6> ;
  skos:related <http://data.loterre.fr/ark:/67375/TSO-XHQSGQST-B> .

<http://data.loterre.fr/ark:/67375/TSO-TZVXPB5S-5>
  a skos:Concept ;
  dc:modified "2021-06-02"^^xsd:date ;
  skos:altLabel "CARE Principles for Indigenous Data Governance"@en, "principes CARE pour la gouvernance des données autochtones"@fr ;
  skos:definition "Principles developed by the Global Indigenous Data Alliance (GIDA) in 2019 to complement the FAIR principles and other movements towards Open Data, people and purpose-oriented, reflecting the crucial role of data in advancing Indigenous innovation and self-determination. These principles complement the existing FAIR principles encouraging open and other data movements to consider both people and purpose in their advocacy and pursuits. (source: https://www.gida-global.org/care)"@en, "complément aux principes FAIR et à d’autres mouvements en faveur des données ouvertes. […] Alors que les principes FAIR sont axés sur les données, les principes CARE s’orientent vers les personnes et les objectifs. (source: https://mackenziedatastream.ca/fr/article/fair-and-care-data-principles)"@fr ;
  skos:prefLabel "CARE principles"@en, "principes CARE"@fr, "principios CARE"@es ;
  skos:inScheme <http://data.loterre.fr/ark:/67375/TSO> ;
  skos:broader <http://data.loterre.fr/ark:/67375/TSO-CV5H9HZH-V> .

<http://data.loterre.fr/ark:/67375/TSO-M6JMPCMG-1>
  a skos:Concept ;
  dc:modified "2021-06-02"^^xsd:date ;
  skos:altLabel "charter of ECHO"@en ;
  skos:definition "aims at defining the criteria for adequate exploitation of the new media's potential for archival preservation, scholarly and educational exploration, as well as public distribution of the shared cultural heritage of mankind. (source: https://echo.mpiwg-berlin.mpg.de/policy/oa_basics/charter)"@en, "définit les critères d’une exploitation adéquate du patrimoine scientifique et culturel commun de l’humanité, tant pour la préservation des archives, que pour l’exploration scientifique ou pédagogique ou encore pour la diffusion auprès du public. (source: https://www.ouvrirlascience.fr/charte-echo/)"@fr ;
  skos:prefLabel "ECHO charter"@en, "carta ECHO"@es, "charte ECHO"@fr ;
  skos:inScheme <http://data.loterre.fr/ark:/67375/TSO> ;
  skos:broader <http://data.loterre.fr/ark:/67375/TSO-CV5H9HZH-V> .

<http://data.loterre.fr/ark:/67375/TSO-T5VDL564-T>
  a skos:Concept ;
  dc:modified "2021-06-03"^^xsd:date ;
  skos:definition "Principes qui posent des bases sur lesquelles les données scientifiques considérées comme ouvertes devraient reposer. Parce que ces données sont fondamentalement différentes des documents, les Principes Panton tentent de démontrer que la technologie, les licences et les stratégies de préservation des documents ne fonctionnent pas pour les données et que cela demande une approche différente. Par conséquent, les Principes sont conçus pour aider les scientifiques à partager facilement les données sans avoir à penser aux détails juridiques, le cadre essentiel étant déjà fourni. (source: https://wiki.teluq.ca/sci1014/index.php/Les_Principes_de_Panton)"@fr, "Principles written in July 2009 by Peter Murray-Rust, Cameron Neylon, Rufus Pollock and John Wilbanks at the Panton Arms on Panton Street in Cambridge, UK. They set out the basis on which scientific data must be based in order to qualify as open. These principles were then refined with the help of the members of the Open Knowledge Foundation Working Group on Open Data in Science and were officially launched in February 2010. (Source : https://www.pantonprinciples.org/)"@en ;
  skos:prefLabel "Panton principles"@en, "principes de Panton"@fr, "principios de Panton"@es ;
  skos:inScheme <http://data.loterre.fr/ark:/67375/TSO> ;
  skos:broader <http://data.loterre.fr/ark:/67375/TSO-V6F4ZS65-G> .

<http://data.loterre.fr/ark:/67375/TSO-H5ZG6DX6-4>
  a skos:Concept ;
  dc:modified "2021-06-25"^^xsd:date ;
  skos:altLabel "PI"@en, "PID"@es, "identifiant persistant"@fr, "persistent identifier"@en ;
  skos:definition "A unique and stable denomination (reference) of a digital resource (e.g. research data) through allocation of a code that can be persistently and explicitly referenced on the internet. (source: https://open-science-training-handbook.gitbook.io/book/glossary)"@en, "Chaîne de caractères alphanumériques qui désigne une ressource indépendamment de son emplacement et garantit un lien stable à la ressource en ligne, en faisant correspondre en permanence l’identité de la ressource à sa localisation sur le web."@fr ;
  skos:prefLabel "PID"@en, "identifiant pérenne"@fr, "identificador persistente"@es ;
  skos:inScheme <http://data.loterre.fr/ark:/67375/TSO> ;
  skos:broader <http://data.loterre.fr/ark:/67375/TSO-V0KSG0NC-P> ;
  skos:related <http://data.loterre.fr/ark:/67375/TSO-F43HWMXG-K>, <http://data.loterre.fr/ark:/67375/TSO-FLVT4163-M>, <http://data.loterre.fr/ark:/67375/TSO-JXVPRHLQ-P>, <http://data.loterre.fr/ark:/67375/TSO-QL71JGQM-F> ;
  skos:narrower <http://data.loterre.fr/ark:/67375/TSO-SVH6TCP0-3>, <http://data.loterre.fr/ark:/67375/TSO-NZB6R6Z5-J>, <http://data.loterre.fr/ark:/67375/TSO-M6RFTL22-T>, <http://data.loterre.fr/ark:/67375/TSO-FC8JNWR9-L>, <http://data.loterre.fr/ark:/67375/TSO-T487PDFX-7>, <http://data.loterre.fr/ark:/67375/TSO-GVVZFV2S-W>, <http://data.loterre.fr/ark:/67375/TSO-XHQRK84J-T>, <http://data.loterre.fr/ark:/67375/TSO-JK3TZ82D-D>, <http://data.loterre.fr/ark:/67375/TSO-HCPMHK1V-X>, <http://data.loterre.fr/ark:/67375/TSO-VD8QW3Q6-7>, <http://data.loterre.fr/ark:/67375/TSO-DKCFHCNB-D>, <http://data.loterre.fr/ark:/67375/TSO-NQNLFZ3L-0>, <http://data.loterre.fr/ark:/67375/TSO-SJ45BLDH-0>, <http://data.loterre.fr/ark:/67375/TSO-SDDGPBZK-G> .

<http://data.loterre.fr/ark:/67375/TSO-GXCQ58W9-H>
  a skos:Concept ;
  dc:modified "2021-06-22"^^xsd:date ;
  skos:definition "Not-for-profit membership organization that exists to make scholarly communications better. (source: https://www.crossref.org/about/)"@en, "Organisation à but non lucratif de droit américain1 jouant le rôle d'agence d'enregistrement et de registre des Digital Object Identifier (identifiant d'objet numérique). Lancée au début des années 2000 dans un effort de coopération entre les éditeurs, afin de permettre l'identification des objets numériques, notamment les articles et les revues académiques en ligne. (Source : https://fr.wikipedia.org/wiki/Crossref)"@fr ;
  skos:prefLabel "Crossref"@en, "Crossref"@es, "Crossref"@fr ;
  skos:inScheme <http://data.loterre.fr/ark:/67375/TSO> ;
  skos:broader <http://data.loterre.fr/ark:/67375/TSO-J64S3QDL-1> ;
  skos:related <http://data.loterre.fr/ark:/67375/TSO-T487PDFX-7> .

<http://data.loterre.fr/ark:/67375/TSO-RPJVDHMM-Q>
  a skos:Concept ;
  skos:definition "Consortium international de bibliothèques et services spécialisés dans les sciences de l'information, qui vise à faciliter l'archivage numérique ainsi que l'accès aux ressources numériques sur Internet, notamment par l'attribution d'un DOI à chacune d'entre elles. (source: https://fr.wikipedia.org/wiki/DataCite)"@fr, "Leading global non-profit organisation that provides persistent identifiers (DOIs) for research data and other research outputs (source: https://datacite.org/value.html)"@en ;
  skos:prefLabel "DataCite"@en, "DataCite"@es, "DataCite"@fr ;
  skos:inScheme <http://data.loterre.fr/ark:/67375/TSO> ;
  skos:broader <http://data.loterre.fr/ark:/67375/TSO-J64S3QDL-1> ;
  skos:related <http://data.loterre.fr/ark:/67375/TSO-QL71JGQM-F>, <http://data.loterre.fr/ark:/67375/TSO-T487PDFX-7>, <http://data.loterre.fr/ark:/67375/TSO-XQQ71S90-L> .

<http://data.loterre.fr/ark:/67375/TSO-Q3D3R4D9-C>
  a skos:Concept ;
  dc:modified "2021-06-29"^^xsd:date ;
  skos:altLabel "DCC"@en, "DCC"@es, "DCC"@fr ;
  skos:definition "Centre d'expertise du Royaume-Uni spécialisé dans le domaine de la conservation de l'information numérique, et en particulier de la gestion des données de recherche."@fr, "World-leading centre of expertise in digital information curation with a focus on building capacity, capability and skills for research data management. (source: https://www.dcc.ac.uk/about)"@en ;
  skos:prefLabel "Digital Curation Centre"@en, "Digital Curation Centre"@es, "Digital Curation Centre"@fr ;
  skos:inScheme <http://data.loterre.fr/ark:/67375/TSO> ;
  skos:broader <http://data.loterre.fr/ark:/67375/TSO-J64S3QDL-1> ;
  skos:related <http://data.loterre.fr/ark:/67375/TSO-GDCXNW8F-5> .

<http://data.loterre.fr/ark:/67375/TSO-RRVKQP85-7>
  a skos:Concept ;
  dc:modified "2021-06-25"^^xsd:date ;
  skos:altLabel "RDA"@en, "RDA"@fr ;
  skos:definition "A neutral social platform where international research data experts meet to exchange views and to agree on topics including social hurdles on data sharing, education and training challenges, data management plans and certification of data repositories, disciplinary and interdisciplinary interoperability, as well as technological aspects. (source: https://rd-alliance.org/about-rda)"@en, "Organisation créée en 2013 par la Commission européenne, la Fondation américaine de la science et américaine, le National Institute of Standards and Technology et le Australian Department of Innovation. Sa mission est de créer des passerelles sociales et techniques permettant un partage ouvert des données. (Source : https://fr.wikipedia.org/wiki/Research_Data_Alliance)"@fr ;
  skos:prefLabel "Research Data Alliance"@en, "Research Data Alliance"@es, "Research Data Alliance"@fr ;
  skos:inScheme <http://data.loterre.fr/ark:/67375/TSO> ;
  skos:broader <http://data.loterre.fr/ark:/67375/TSO-J64S3QDL-1> .

<http://data.loterre.fr/ark:/67375/TSO-C670N10N-B>
  a skos:Concept ;
  dc:modified "2021-06-24"^^xsd:date ;
  skos:altLabel "I4OA"@en ;
  skos:definition "Collaboration between scholarly publishers, infrastructure organizations, librarians, researchers and other interested parties to advocate and promote the unrestricted availability of the abstracts of the world's scholarly publications, particularly journal articles and book chapters, in trusted repositories where they are open and machine-accessible. (Source : https://i4oa.org/)"@en, "Initiative lancée en 2020, qui invite les éditeurs de publications scientifiques à rendre les résumés disponibles dans une infrastructure ouverte et accessible aux machines. (Source : https://openscience.pasteur.fr/2020/10/15/lancement-de-linitiative-pour-les-abstracts-ouverts-i4oa/)"@fr ;
  skos:prefLabel "Initiative for Open Abstracts"@en, "Initiative for Open Abstracts"@es, "Initiative for Open Abstracts"@fr ;
  skos:inScheme <http://data.loterre.fr/ark:/67375/TSO> ;
  skos:broader <http://data.loterre.fr/ark:/67375/TSO-J64S3QDL-1> .

<http://data.loterre.fr/ark:/67375/TSO-GHZRN0P9-2>
  a skos:Concept ;
  dc:modified "2021-06-25"^^xsd:date ;
  skos:altLabel "PKP"@en ;
  skos:definition "Multi-university initiative developing (free) open source software and conducting research to improve the quality and reach of scholarly publishing, (Source : https://pkp.sfu.ca/)"@en, "Organisation à but non lucratif fondée par des universités américaines et européennes, qui promeut l'importance de l'ouverture des résultats de la recherche financée par des fonds publics et sur le développement de stratégies pour la rendre possible, y compris au travers de solutions logicielles."@fr ;
  skos:prefLabel "Public Knowledge Project"@en, "Public Knowledge Project"@es, "Public Knowledge Project"@fr ;
  skos:inScheme <http://data.loterre.fr/ark:/67375/TSO> ;
  skos:broader <http://data.loterre.fr/ark:/67375/TSO-V0HZ66HD-4> .

<http://data.loterre.fr/ark:/67375/TSO-FXLNHJK5-R>
  a skos:Concept ;
  dc:modified "2021-06-24"^^xsd:date ;
  skos:altLabel "Global Sustainability Coalition for Open Science Services"@en, "Global Sustainability Coalition for Open Science Services"@es, "Global Sustainability Coalition for Open Science Services"@fr ;
  skos:definition "Network of influential organisations committed to helping secure OA and OS infrastructure well into the future. (Source : https://scoss.org/)"@en, "Réseau d’institutions de différents pays engagées dans la sécurisation de services et de ressources de soutien à la mise en œuvre de la science ouverte. Il fournit un cadre visant à mutualiser les financements, à stabiliser collectivement une infrastructure vitale de services scientifiques ouverts librement accessibles et assurer ainsi leur maintien sur le long terme. Plus de 200 institutions financent SCOSS. (Source : https://www.ouvrirlascience.fr/jnso-2019/)"@fr ;
  skos:prefLabel "SCOSS"@en, "SCOSS"@es, "SCOSS"@fr ;
  skos:inScheme <http://data.loterre.fr/ark:/67375/TSO> ;
  skos:broader <http://data.loterre.fr/ark:/67375/TSO-J64S3QDL-1> .

<http://data.loterre.fr/ark:/67375/TSO-G587Q9G3-2>
  a skos:Concept ;
  dc:modified "2021-06-24"^^xsd:date ;
  skos:definition "Coalition mondiale engagée à faire Ouvert la valeur par défaut pour la recherche et l'éducation. SPARC permet aux gens de résoudre de gros problèmes et de faire de nouvelles découvertes grâce à l'adoption de politiques et de pratiques qui font progresser l'accès ouvert, les données ouvertes et l'éducation ouverte. (Source : https://access2perspectives.org/fr/services/open-science/#:~:text=Rassemblement%20pour%20le%20mat%C3%A9riel%20Open,partage%20de%20technologies%20scientifiques%20ouvertes.)"@fr, "Dutch foundation committed to delivering on the promise of open access, open science, open scholarship and open education. (Source : https://sparceurope.org/)"@en ;
  skos:prefLabel "SPARC Europe"@en, "SPARC Europe"@es, "SPARC Europe"@fr ;
  skos:inScheme <http://data.loterre.fr/ark:/67375/TSO> ;
  skos:broader <http://data.loterre.fr/ark:/67375/TSO-J64S3QDL-1> ;
  skos:related <http://data.loterre.fr/ark:/67375/TSO-DJ828LKC-C>, <http://data.loterre.fr/ark:/67375/TSO-W1F4MWNS-F> .

<http://data.loterre.fr/ark:/67375/TSO-B66RVJ4T-J>
  a skos:Concept ;
  dc:created "2021-06-10"^^xsd:date ;
  dc:modified "2021-06-30"^^xsd:date ;
  skos:definition "Répertoire qui rassemble les coordonnées d'entités offrant des services liés à l'un des aspects de la science ouverte."@fr ;
  skos:prefLabel "open science registry"@en, "repertorio de ciencia abierta"@es, "répertoire de science ouverte"@fr ;
  skos:inScheme <http://data.loterre.fr/ark:/67375/TSO> ;
  skos:broader <http://data.loterre.fr/ark:/67375/TSO-V0HZ66HD-4> ;
  skos:narrower <http://data.loterre.fr/ark:/67375/TSO-WQ9RZCBH-P>, <http://data.loterre.fr/ark:/67375/TSO-QV209F26-T>, <http://data.loterre.fr/ark:/67375/TSO-JN2ZSNST-6>, <http://data.loterre.fr/ark:/67375/TSO-QXH951LF-0>, <http://data.loterre.fr/ark:/67375/TSO-J9P20ZD1-C>, <http://data.loterre.fr/ark:/67375/TSO-NHVK3QVC-F> .

<http://data.loterre.fr/ark:/67375/TSO-D2CGSDHD-L>
  a skos:Concept ;
  skos:altLabel "barrière mobile"@fr, "moving wall"@en ;
  skos:definition "Période pendant laquelle un article de revue, déposé dans une archive ouverte ou un réservoir, ne peut être accessible librement. (source: https://openaccess.inist.fr/glossaire/)"@fr ;
  skos:prefLabel "embargo"@en, "embargo"@es, "embargo"@fr ;
  skos:inScheme <http://data.loterre.fr/ark:/67375/TSO> ;
  skos:broader <http://data.loterre.fr/ark:/67375/TSO-PSFFQLXV-2> ;
  skos:related <http://data.loterre.fr/ark:/67375/TSO-BTR6P741-6> .

<http://data.loterre.fr/ark:/67375/TSO-DCJZX2TD-P>
  a skos:Concept ;
  dc:modified "2021-06-29"^^xsd:date ;
  skos:altLabel "POSI"@en ;
  skos:definition "Ces principes exposent les trois leviers sur lesquels une infrastructure ouverte doit agir afin de gagner la confiance de la communauté scientifique au sens large : la responsabilité (gouvernance), le financement (durabilité) et la protection des intérêts de la communauté."@fr, "Principles that propose three areas that an Open Infrastructure organization can address in order to garner the trust of the broader scholarly community: accountability (governance), funding (sustainability) and protection of community interests (insurance). (Source: https://doi.org/10.24343/C34W2H)"@en ;
  skos:prefLabel "Principles of Open Scholarly Infrastructure"@en, "Principles of Open Scholarly Infrastructure"@es, "Principles of Open Scholarly Infrastructure"@fr ;
  skos:inScheme <http://data.loterre.fr/ark:/67375/TSO> ;
  skos:broader <http://data.loterre.fr/ark:/67375/TSO-CV5H9HZH-V> .

<http://data.loterre.fr/ark:/67375/TSO-L9LLDHZ0-5>
  a skos:Concept ;
  dc:modified "2021-06-04"^^xsd:date ;
  skos:definition "Processus suivi par un chercheur pour mener à bien un projet ou une étude, de sa conception à la publication de ses données et résultats, et dans lequel toutes les étapes sont conformes aux pratiques de la science ouverte."@fr, "The process by which a researcher carries out a project or study, from its conception to the publication of its data and results, and in which all steps are consistent with open science practices."@en ;
  skos:prefLabel "ciclo abierto de la investigación"@es, "cycle ouvert de la recherche"@fr, "open research lifecycle"@en ;
  skos:inScheme <http://data.loterre.fr/ark:/67375/TSO> ;
  skos:broader <http://data.loterre.fr/ark:/67375/TSO-JFJGKFN2-H> .

<http://data.loterre.fr/ark:/67375/TSO-JB3N2FLX-R>
  a skos:Concept ;
  dc:modified "2021-06-29"^^xsd:date ;
  skos:definition "Mouvement visant à promouvoir la science ouverte à différents niveaux, en mettant en évidence et en soulignant les avantages sociétaux, professionnels et personnels qu'elle comporte."@fr, "Movement to promote open science at various levels of stakeholders, highlighting and stressing the societal, professional and personal advantages that it entails. (Source : The Open Science Training Handbook)"@en ;
  skos:prefLabel "open advocacy"@en, "promoción de la ciencia abierta"@es, "promotion de la science ouverte"@fr ;
  skos:inScheme <http://data.loterre.fr/ark:/67375/TSO> ;
  skos:broader <http://data.loterre.fr/ark:/67375/TSO-MV5H4HGJ-2> .

<http://data.loterre.fr/ark:/67375/TSO-MRHXBFZS-T>
  a skos:Concept ;
  dc:modified "2021-06-29"^^xsd:date ;
  skos:altLabel "Facilitate Open Science Training for European Research"@en, "Facilitate Open Science Training for European Research"@fr ;
  skos:definition "A 2-year EU-funded project, started 01/02/2014, to contribute to a real and lasting shift in the behaviour of European researchers to ensure that Open Science (OS) becomes the norm. This coordination initiative supported different stakeholders, especially young researchers, in adopting open access in the context of the European Research Area (ERA) and in complying with the open access policies and rules of participation set out for Horizon 2020 (H2020). FOSTER promoted the integration of open access principles and practice in the current research workflow by targeting the young researcher training environment. In addition, FOSTER strengthened the institutional training capacity to maintain compliance with the open access policies in the ERA and H2020, and facilitated the adoption, reinforcement and implementation of open access policies from other European funders, in line with the European Commission’s recommendation. (Source: https://www.fosteropenscience.eu/about#theproject)"@en, "Projet d'une durée de 2 ans, démarré le 01/02/2014, et financé par l'UE , dans le but de contribuer à un changement réel et durable du comportement des chercheurs européens afin que la science ouverte devienne la norme."@fr ;
  skos:prefLabel "FOSTER"@en, "FOSTER"@es, "FOSTER"@fr ;
  skos:inScheme <http://data.loterre.fr/ark:/67375/TSO> ;
  skos:broader <http://data.loterre.fr/ark:/67375/TSO-H93WKMMJ-B> .

<http://data.loterre.fr/ark:/67375/TSO-ZP6CXMWN-J>
  a skos:Concept ;
  dc:modified "2021-06-18"^^xsd:date ;
  skos:definition "Projet de recherche collaboratif qui apporte son soutien aux établissements et projets culturels et scientifiques en Europe qui détiennent ou enrichissent un patrimoine culturel grâce aux nouvelles technologies et aux nouveaux médias. (Source : ouvrirlascience.fr)"@fr ;
  skos:prefLabel "ECHO"@en, "ECHO"@es, "ECHO"@fr ;
  skos:inScheme <http://data.loterre.fr/ark:/67375/TSO> ;
  skos:broader <http://data.loterre.fr/ark:/67375/TSO-H93WKMMJ-B> .

<http://data.loterre.fr/ark:/67375/TSO-S9XQFTCQ-Q>
  a skos:Concept ;
  dc:modified "2021-06-29"^^xsd:date ;
  skos:altLabel "PLOS"@en, "PLoS"@en ;
  skos:definition "Organisme à but non lucratif qui publie des revues scientifiques anglophones en accès ouvert, sur la base de licences libres."@fr, "nonprofit open-access science, technology, and medicine publisher with a library of open-access journals and other scientific literature under an open-content license. (source: Wikipedia)"@en ;
  skos:prefLabel "Public Library of Science"@en, "Public Library of Science"@es, "Public Library of Science"@fr ;
  skos:inScheme <http://data.loterre.fr/ark:/67375/TSO> ;
  skos:broader <http://data.loterre.fr/ark:/67375/TSO-J64S3QDL-1> .

<http://data.loterre.fr/ark:/67375/TSO-XJJ971XL-H>
  a skos:Concept ;
  dc:modified "2021-07-05"^^xsd:date ;
  skos:altLabel "Scientific Electronic Library Online"@en, "Scientific Electronic Library Online"@es, "Scientific Electronic Library Online"@fr ;
  skos:definition "A bibliographic database, digital library, and cooperative electronic publishing model of open access journals. SciELO was created to meet the scientific communication needs of developing countries and provides an efficient way to increase visibility and access to scientific literature. Originally established in Brazil in 1997, today there are 16 countries in the SciELO network and its journal collections: Argentina, Bolivia, Brazil, Chile, Colombia, Costa Rica, Cuba, Ecuador, Mexico, Paraguay, Peru, Portugal, South Africa, Spain, Uruguay, and Venezuela. (Source: https://en.wikipedia.org/wiki/SciELO)"@en, "Portail coopératif de littérature scientifique principalement d'Amérique latine qui offre l'accès à des périodiques en texte intégral couvrant tous les domaines scientifiques. Les articles proposés sont principalement en espagnol. L'interface d'interrogation est en portugais et en anglais. (Source : Cirad)"@fr, "Repositorio multidisciplinario para depositar, preservar y difundir datos de investigación de artículos enviados, aprobados para publicación o ya publicados en revistas de la Red SciELO o depositados en SciELO Preprints. (Fuente: https://www.scielo.org/es/sobre-el-scielo/scielo-data-es/sobre-scielo-data-es/)"@es ;
  skos:prefLabel "SciELO"@en, "SciELO"@es, "SciELO"@fr ;
  skos:inScheme <http://data.loterre.fr/ark:/67375/TSO> ;
  skos:broader <http://data.loterre.fr/ark:/67375/TSO-CVMGJVKW-W> .

<http://data.loterre.fr/ark:/67375/TSO-RJFTQR0V-N>
  a skos:Concept ;
  dc:modified "2021-06-29"^^xsd:date ;
  skos:definition "A 30 month project (2015-2017) funded by the European Commission under the Horizon 2020 programme. It aimed to establish seamless integration between articles, data, and researchers across the research lifecycle. The project created a wealth of open resources and fostered a sustainable international e-infrastructure. The result was reduced duplication, economies of scale, richer research services, and opportunities for innovation. (Source : https://project-thor.eu/)"@en, "Projet de 30 mois (2015-2017) financé par la Commission européenne dans le cadre du programme Horizon 2020. Il visait à établir une intégration transparente entre les articles, les données et les chercheurs tout au long du cycle de vie de la recherche."@fr ;
  skos:prefLabel "THOR"@en, "THOR"@es, "THOR"@fr ;
  skos:inScheme <http://data.loterre.fr/ark:/67375/TSO> ;
  skos:broader <http://data.loterre.fr/ark:/67375/TSO-H93WKMMJ-B> .

<http://data.loterre.fr/ark:/67375/TSO-TKRVHS3M-S>
  a skos:Concept ;
  dc:modified "2021-06-22"^^xsd:date ;
  skos:altLabel "fichier lisez-moi"@fr ;
  skos:definition "Premier fichier qu’un développeur doit consulter avant d’entamer un projet. [...] Il contient habituellement des informations importantes à propos du système, du projet ou du logiciel en question. (Source : https://www.ionos.fr/digitalguide/sites-internet/developpement-web/fichier-readme/)"@fr ;
  skos:prefLabel "README file"@en, "archivo README"@es, "fichier README"@fr ;
  skos:inScheme <http://data.loterre.fr/ark:/67375/TSO> ;
  skos:broader <http://data.loterre.fr/ark:/67375/TSO-T4KV78Z3-L> ;
  skos:related <http://data.loterre.fr/ark:/67375/TSO-VF5K6BGT-F> .

<http://data.loterre.fr/ark:/67375/TSO-R1CSCWWG-D>
  a skos:Concept ;
  dc:modified "2021-06-15"^^xsd:date ;
  skos:definition "A bibliographic citation whose data needed to define it are freely available, downloadable and reusable. (Source : https://doi.org/10.6084/m9.figshare.6683855.v1)"@en, "Référence bibliographique en accès ouvert utilisée dans les publications scientifiques. (Source : hypotheses.org)"@fr ;
  skos:prefLabel "citación abierta"@es, "citation ouverte"@fr, "open citation"@en ;
  skos:inScheme <http://data.loterre.fr/ark:/67375/TSO> ;
  skos:broader <http://data.loterre.fr/ark:/67375/TSO-V08MCZVP-H> ;
  skos:related <http://data.loterre.fr/ark:/67375/TSO-MZ8BL730-S> .

<http://data.loterre.fr/ark:/67375/TSO-JBQFB4MB-P>
  a skos:Concept ;
  dc:modified "2021-06-10"^^xsd:date ;
  skos:definition "Catalogue collectif contenant des millions de notices pour des ressources en libre accès. Ce catalogue a été créé en collectant les collections en libre accès à travers le monde avec l'Open Archives Initiative Protocol for Metadata Harvesting (OAI-PMH). (Source : https://www.oclc.org/fr/oaister.html)"@fr, "Union catalog of millions of records that represent open access resources. This catalog was built through harvesting from open access collections worldwide using the Open Archives Initiative Protocol for Metadata Harvesting (OAI-PMH). (Source : https://www.oclc.org/en/oaister.html)"@en ;
  skos:prefLabel "OAIster"@en, "OAIster"@es, "OAIster"@fr ;
  skos:inScheme <http://data.loterre.fr/ark:/67375/TSO> ;
  skos:broader <http://data.loterre.fr/ark:/67375/TSO-JN2ZSNST-6> ;
  skos:related <http://data.loterre.fr/ark:/67375/TSO-P0WRKFZJ-X> .

<http://data.loterre.fr/ark:/67375/TSO-XTZMJ2W8-J>
  a skos:Concept ;
  dc:modified "2021-06-24"^^xsd:date ;
  skos:definition "Modèle selon lequel une revue impose des frais supplémentaires pour couvrir le coût de la publication, facturés en plus des frais de traitement des articles (APC)."@fr, "One of a number of supplementary charges imposed by some journals to cover the cost of publishing, and charged in addition to article processing charges (APCs). (source: https://casrai.org/open-access-glossary/)"@en ;
  skos:prefLabel "page charge"@en, "page charge"@es, "page charge"@fr ;
  skos:inScheme <http://data.loterre.fr/ark:/67375/TSO> ;
  skos:broader <http://data.loterre.fr/ark:/67375/TSO-MWXTBMQ8-9> .

<http://data.loterre.fr/ark:/67375/TSO-ZKK6WW4X-W>
  a skos:Concept ;
  dc:modified "2021-06-24"^^xsd:date ;
  skos:altLabel "Etalab V2.0 licence"@en, "Licence Etalab V2.0"@fr ;
  skos:definition "Licence libre française créée afin d'encadrer l'ouverture des données de l’État français. Elle est compatible avec les licences Open Government Licence (OGL) du Royaume-Uni, Open Data Commons Attribution (ODC-BY) de l'Open Knowledge Foundation et Creative Commons Attribution 2.0 (CC-BY 2.0) de Creative Commons et n'impose pas d'utiliser une licence identique sur les travaux dérivés des données couvertes. (Source : https://fr.wikipedia.org/wiki/Licence_ouverte_(%C3%89tat_fran%C3%A7ais))"@fr ;
  skos:prefLabel "Etalab V2.0 license"@en, "Licence Ouverte V2.0"@fr, "Licencia Etalab V2.0"@es ;
  skos:inScheme <http://data.loterre.fr/ark:/67375/TSO> ;
  skos:broader <http://data.loterre.fr/ark:/67375/TSO-WZ0J1023-D> ;
  skos:related <http://data.loterre.fr/ark:/67375/TSO-VM3N240R-C> .

<http://data.loterre.fr/ark:/67375/TSO-D2DS95K6-0>
  a skos:Concept ;
  dc:modified "2021-06-17"^^xsd:date ;
  skos:definition "Diversité culturelle appliquée au monde du livre. En écho à la biodiversité, elle fait référence à une nécessaire diversité des productions éditoriales mises à la disposition des lecteurs. (Source : Wikipédia https://fr.wikipedia.org/wiki/Bibliodiversit%C3%A9)"@fr, "The cultural diversity applied to the writing and publishing world. Echoing the concept of biodiversity, it refers to the need for a variety of publications to be available to readers within a given environment.('Source Wikipédia : https://en.wikipedia.org/wiki/Bibliodiversity)"@en ;
  skos:prefLabel "bibliodiversidad"@es, "bibliodiversity"@en, "bibliodiversité"@fr ;
  skos:inScheme <http://data.loterre.fr/ark:/67375/TSO> ;
  skos:broader <http://data.loterre.fr/ark:/67375/TSO-XWVJBKN6-S> .

<http://data.loterre.fr/ark:/67375/TSO-G33B1S7H-W>
  a skos:Concept ;
  dc:modified "2021-06-17"^^xsd:date ;
  skos:altLabel "RIM"@en, "RIS"@en, "current research information system"@en, "current research information system"@es, "current research information system"@fr, "research information management system"@en ;
  skos:definition "Bases de données et systèmes de gestion qui recensent, gèrent et échangent des métadonnées contextuelles relatives aux travaux scientifiques et savants menés dans un organisme de recherche ou parfois financés par une organisation."@fr, "Sometimes known as research information or research information management systems (RIS/RIMs). Databases and management systems that store, manage and exchange contextual metadata relating to research activities conducted at a research performing organisation or sometimes funded by an organisation. (Source: https://www.ouvrirlascience.fr/wp-content/uploads/2021/04/Openness-Profile-Modelling-research-evaluation-for-open-scholarship-March-2021.pdf)"@en ;
  skos:prefLabel "CRIS"@en, "CRIS"@es, "CRIS"@fr ;
  skos:inScheme <http://data.loterre.fr/ark:/67375/TSO> ;
  skos:broader <http://data.loterre.fr/ark:/67375/TSO-V0KSG0NC-P> .

<http://data.loterre.fr/ark:/67375/TSO-GCQ559K4-Q>
  a skos:Concept ;
  dc:modified "2021-07-05"^^xsd:date ;
  skos:definition "An international consortium of research funders that was launched on September 2018 to implement Plan S. The cOAlition S is supported by Science Europe, hosted and administered by the European Science Foundation. (Source: https://www.esf.org/our-services/choose-your-service/scientific-platforms-administration/coalition-s/)"@en, "Initiative visant à accélérer la transition vers un accès complet et immédiat aux publications scientifiques financés par des fonds publics, et annoncée le 4 septembre 2018 par Science Europe. (Source : https://www.inserm.fr/actualites-et-evenements/actualites/coalition-faire-open-access-realite-ici-2020)"@fr ;
  skos:prefLabel "cOAlition S"@en, "cOAlition S"@es, "cOAlition S"@fr ;
  skos:inScheme <http://data.loterre.fr/ark:/67375/TSO> ;
  skos:broader <http://data.loterre.fr/ark:/67375/TSO-J64S3QDL-1> ;
  skos:related <http://data.loterre.fr/ark:/67375/TSO-NKGK3HW9-N>, <http://data.loterre.fr/ark:/67375/TSO-TVL7X12H-M> .

<http://data.loterre.fr/ark:/67375/TSO-QT5MLV48-P>
  a skos:Concept ;
  dc:modified "2021-06-25"^^xsd:date ;
  skos:definition "Revue diffusée selon le modèle diamant de l'accès ouvert, c’est-à-dire gratuite pour les lecteurs et les auteurs."@fr ;
  skos:prefLabel "diamond journal"@en, "revista diamante"@es, "revue diamant"@fr ;
  skos:inScheme <http://data.loterre.fr/ark:/67375/TSO> ;
  skos:broader <http://data.loterre.fr/ark:/67375/TSO-TM0MS2GV-7> ;
  skos:related <http://data.loterre.fr/ark:/67375/TSO-HS79BV00-V> .

<http://data.loterre.fr/ark:/67375/TSO-ZQ3QKFX9-1>
  a skos:Concept ;
  dc:modified "2021-06-24"^^xsd:date ;
  skos:definition "A licence clause requiring that the original author is appropriately attributed and that derivative works have the same licence as the original. Compatible with free cultural works. (Source : http://www.righttoresearch.org/resources/OpenResearchGlossary)"@en, "Licence qui permet de remixer, d'adapter et de s'appuyer sur un travail, même à des fins commerciales, à condition que l'auteur soit crédité et que ces nouvelles créations soient proposées sous une licence identique. (Source : https://creativecommons.org/licenses/?lang=fr-FR)"@fr ;
  skos:prefLabel "CC-BY-SA license"@en, "licence CC-BY-SA"@fr, "licencia CC-BY-SA"@es ;
  skos:inScheme <http://data.loterre.fr/ark:/67375/TSO> ;
  skos:broader <http://data.loterre.fr/ark:/67375/TSO-WH5JC3TT-G>, <http://data.loterre.fr/ark:/67375/TSO-WZ0J1023-D> ;
  skos:related <http://data.loterre.fr/ark:/67375/TSO-W04D2X5B-N> .

<http://data.loterre.fr/ark:/67375/TSO-KSZ3VF36-P>
  a skos:Concept ;
  dc:modified "2021-06-02"^^xsd:date ;
  skos:altLabel "PO"@fr, "openness"@en ;
  skos:definition "A digital resource in which a research contributor's outputs and activities that support openness would be accessible in a single place. (Source : Knowledge Exchange)"@en, "Mécanisme qui prend en compte la diversité des activités de recherche et permet ainsi d'améliorer la reconnaissance et la rétribution de la pratique de la science ouverte. Il a vocation à être une ressource numérique dans laquelle les résultats et les activités d’un contributeur à la recherche qui concourent à son ouverture seraient accessibles en un seul endroit. (Source : Ouvrir la Science)"@fr ;
  skos:prefLabel "openness profile"@en, "perfil de apertura"@es, "profil d'ouverture"@fr ;
  skos:inScheme <http://data.loterre.fr/ark:/67375/TSO> ;
  skos:broader <http://data.loterre.fr/ark:/67375/TSO-V0KSG0NC-P> ;
  skos:related <http://data.loterre.fr/ark:/67375/TSO-DKBRJ0N6-J>, <http://data.loterre.fr/ark:/67375/TSO-T9Q25G6Q-S> .

<http://data.loterre.fr/ark:/67375/TSO-T67S254S-S>
  a skos:Concept ;
  dc:modified "2021-06-30"^^xsd:date ;
  skos:altLabel "licence à code ouvert"@fr ;
  skos:definition "Licence qui permet à un logiciel d'être librement utilisé, modifié et partagé."@fr, "License that allow software to be freely used, modified, and shared. (Source : https://opensource.org/licenses)"@en ;
  skos:prefLabel "licence open source"@fr, "licencia open source"@es, "open source licence"@en ;
  skos:inScheme <http://data.loterre.fr/ark:/67375/TSO> ;
  skos:broader <http://data.loterre.fr/ark:/67375/TSO-WZ0J1023-D> ;
  skos:narrower <http://data.loterre.fr/ark:/67375/TSO-PBQJJSDV-W>, <http://data.loterre.fr/ark:/67375/TSO-X11G8MG1-M>, <http://data.loterre.fr/ark:/67375/TSO-SMF21F74-3>, <http://data.loterre.fr/ark:/67375/TSO-X2MBVK0V-Z>, <http://data.loterre.fr/ark:/67375/TSO-LRT6FWVV-0>, <http://data.loterre.fr/ark:/67375/TSO-Z9Q5Q16G-F>, <http://data.loterre.fr/ark:/67375/TSO-FF03NR9V-N> .

<http://data.loterre.fr/ark:/67375/TSO-CW11LHBH-Q>
  a skos:Concept ;
  skos:altLabel "Open Archives Initiative"@en, "Open Archives Initiative"@es, "Open Archives Initiative"@fr, "aniciativa de archivos abiertos"@es ;
  skos:definition "An organisation that develops and promotes interoperability standards that aim to facilitate the efficient dissemination of content. The Open Archives Initiative has its roots in an effort to enhance access to e-print archives as a means of increasing the availability of scholarly communication. (Source : http://www.openarchives.org/organization/)"@en, "Organisation ayant pour mission de soulever et de résoudre les problèmes que pose l'interopérabilité des archives d'e-prints. (Source : Ifremer)"@fr, "Tiene su inicio en el año de 1999 con el objetivo de crear una plataforma simple para permitir la interoperabilidad de publicaciones cientificas en diversas disciplinas. (Fuente: http://accesoabierto.uanl.mx/glosario-de-terminos/)"@es ;
  skos:prefLabel "OAI"@en, "OAI"@es, "OAI"@fr ;
  skos:inScheme <http://data.loterre.fr/ark:/67375/TSO> ;
  skos:broader <http://data.loterre.fr/ark:/67375/TSO-J64S3QDL-1> ;
  skos:related <http://data.loterre.fr/ark:/67375/TSO-P0WRKFZJ-X> .

<http://data.loterre.fr/ark:/67375/TSO-B7FV4N90-B>
  a skos:Concept ;
  dc:modified "2021-06-29"^^xsd:date ;
  skos:definition "Déclaration conjointe signée par African Open Science Platform, AmeliCA, cOAlition S, OA2020 et SciELO le 1er mai 2019 lors de la réunion annuelle du Conseil mondial de la recherche à São Paulo, au Brésil. Les signataires sont unis dans leur mission commune de rendre les connaissances disponibles et accessibles."@fr, "Joint Declaration signed by the African Open Science Platform, AmeliCA, cOAlition S, OA2020, and SciELO on 1 May 2019 during the annual meeting of the Global Research Council in São Paulo, Brazil. They are united in their common mission of making knowledge available and accessible wherever it can have the greatest impact and help solve humanity’s challenges regardless of where it was produced. (Source: https://anr.fr/fileadmin/documents/2019/Sao-Paulo-Statement-OA-01052019.pdf)"@en ;
  skos:prefLabel "Declaración de São Paulo sobre acceso abierto"@es, "Déclaration de São Paulo pour le libre accès"@fr, "São Paulo Statement on Open Access"@en ;
  skos:inScheme <http://data.loterre.fr/ark:/67375/TSO> ;
  skos:broader <http://data.loterre.fr/ark:/67375/TSO-V6F4ZS65-G> ;
  skos:related <http://data.loterre.fr/ark:/67375/TSO-STWL5MWS-W> .

<http://data.loterre.fr/ark:/67375/TSO-J0H32WL6-Z>
  a skos:Concept ;
  dc:modified "2021-07-05"^^xsd:date ;
  skos:altLabel "Données de la recherche apprentissage numérique"@en, "Données de la recherche apprentissage numérique"@fr ;
  skos:definition "Plataforma que ofrece recursos para ayudar a la comunidad científica a gestionar y compartir sus datos."@es, "Plateforme proposant des ressources pour accompagner la communauté scientifique dans la gestion et le partage de ses données. (Source : Doranum)"@fr, "Platform offering resources to support the scientific community in managing and sharing its data."@en ;
  skos:prefLabel "DoRANum"@en, "DoRANum"@es, "DoRANum"@fr ;
  skos:inScheme <http://data.loterre.fr/ark:/67375/TSO> ;
  skos:broader <http://data.loterre.fr/ark:/67375/TSO-DXZZDQSM-3> ;
  skos:related <http://data.loterre.fr/ark:/67375/TSO-B8V78028-B>, <http://data.loterre.fr/ark:/67375/TSO-DP8MN2RF-P> .

<http://data.loterre.fr/ark:/67375/TSO-J9P20ZD1-C>
  a skos:Concept ;
  dc:modified "2021-06-10"^^xsd:date ;
  skos:altLabel "Optimiser le Partage et l’Interopérabilité des Données de la Recherche"@en, "Optimiser le Partage et l’Interopérabilité des Données de la Recherche"@es, "Optimiser le Partage et l’Interopérabilité des Données de la Recherche"@fr ;
  skos:definition "Portail mettant à disposition de la communauté de l’Enseignement Supérieur et de la Recherche un ensemble d’outils et de services facilitant la mise en application des principes FAIR."@fr ;
  skos:prefLabel "OPIDoR"@en, "OPIDoR"@es, "OPIDoR"@fr ;
  skos:inScheme <http://data.loterre.fr/ark:/67375/TSO> ;
  skos:broader <http://data.loterre.fr/ark:/67375/TSO-B66RVJ4T-J> ;
  skos:related <http://data.loterre.fr/ark:/67375/TSO-DP8MN2RF-P>, <http://data.loterre.fr/ark:/67375/TSO-M9JG3Z18-C> ;
  skos:narrower <http://data.loterre.fr/ark:/67375/TSO-SJ4WNCS6-L>, <http://data.loterre.fr/ark:/67375/TSO-VDCNM6ZN-W>, <http://data.loterre.fr/ark:/67375/TSO-XQQ71S90-L> .

<http://data.loterre.fr/ark:/67375/TSO-LBHNZXQ6-L>
  a skos:Concept ;
  dc:modified "2021-06-03"^^xsd:date ;
  skos:altLabel "Dispositif d’ACCompagnement sur les DATA"@fr ;
  skos:definition "Projet porté depuis 2019 par les bibliothèques universitaires de Lyon 1 et de Grenoble Alpes Université. En tant que pôles documentaires de référence en chimie et en physique, elles ont décidé de former un tandem au service de l’amélioration de la gestion des données de recherche dans ces deux domaines. (Source : https://www.datacc.org/a-propos/le-projet/)"@fr ;
  skos:prefLabel "Datacc'"@en, "Datacc'"@es, "Datacc'"@fr ;
  skos:inScheme <http://data.loterre.fr/ark:/67375/TSO> ;
  skos:broader <http://data.loterre.fr/ark:/67375/TSO-H93WKMMJ-B> ;
  skos:related <http://data.loterre.fr/ark:/67375/TSO-DP8MN2RF-P> .

<http://data.loterre.fr/ark:/67375/TSO-FXS77K89-G>
  a skos:Concept ;
  dc:modified "2021-06-24"^^xsd:date ;
  skos:altLabel "Gathering for Open Science Hardware"@en, "Gathering for Open Science Hardware"@es, "Gathering for Open Science Hardware"@fr ;
  skos:definition "Communauté mondiale diversifiée qui travaille à améliorer le partage de technologies scientifiques ouvertes. (Source : https://access2perspectives.org/fr/services/open-science/#:~:text=Rassemblement%20pour%20le%20mat%C3%A9riel%20Open,partage%20de%20technologies%20scientifiques%20ouvertes.)"@fr ;
  skos:prefLabel "GOSH"@en, "GOSH"@es, "GOSH"@fr ;
  skos:inScheme <http://data.loterre.fr/ark:/67375/TSO> ;
  skos:broader <http://data.loterre.fr/ark:/67375/TSO-J64S3QDL-1> ;
  skos:related <http://data.loterre.fr/ark:/67375/TSO-G9J1WQ69-H> .

<http://data.loterre.fr/ark:/67375/TSO-FLVT4163-M>
  a skos:Concept ;
  dc:modified "2021-06-29"^^xsd:date ;
  skos:definition "A 3-year project (December 2017 to December 2020) that aimed to extend the infrastructure for persistent identifiers (PIDs) as a core component of open research, in the EU and globally (source: https://www.project-freya.eu/en/about/mission)"@en, "Projet européen mené de 2017 à 2020 dans le cadre du Programme H2020 de la Commission européenne, avec pour objectif de réaliser une infrastructure pour les identifiant pérennes, composante européenne et mondiale essentielle à la science ouverte. (Source : https://bibliotheque.sciencespo-grenoble.fr/cms/articleview/id/516)"@fr ;
  skos:prefLabel "FREYA"@en, "FREYA"@es, "FREYA"@fr ;
  skos:inScheme <http://data.loterre.fr/ark:/67375/TSO> ;
  skos:broader <http://data.loterre.fr/ark:/67375/TSO-H93WKMMJ-B> ;
  skos:related <http://data.loterre.fr/ark:/67375/TSO-H5ZG6DX6-4> .

<http://data.loterre.fr/ark:/67375/TSO-QL71JGQM-F>
  a skos:Concept ;
  dc:modified "2021-06-29"^^xsd:date ;
  skos:altLabel "ORCID and DataCite Interoperability Network"@en, "ORCID and DataCite Interoperability Network"@es, "ORCID and DataCite Interoperability Network"@fr ;
  skos:definition "A 2-year project funded by the European Commission’s ‘Coordination and Support Action’ under the FP7 programme which started in September 2012. ODIN built on the ORCID and DataCite initiatives to uniquely identify scientists and data sets and connect this information across multiple services and infrastructures for scholarly communication. It addressed some of the critical open questions in the area related to referencing a data object, tracking of use and re-use and links between a data object, subsets, articles, rights statements and every person involved in its life-cycle. (Source: https://www.project-freya.eu/en/about/project-odin)"@en, "Projet de deux ans qui a débuté en septembre 2012, financé par l'\"Action de coordination et de soutien\" de la Commission européenne dans le cadre du programme FP7. ODIN s'est appuyé sur les initiatives ORCID et DataCite pour identifier de manière unique les scientifiques et les jeux de données et connecter ces informations à travers de multiples services et infrastructures."@fr ;
  skos:prefLabel "ODIN"@en, "ODIN"@es, "ODIN"@fr ;
  skos:inScheme <http://data.loterre.fr/ark:/67375/TSO> ;
  skos:broader <http://data.loterre.fr/ark:/67375/TSO-H93WKMMJ-B> ;
  skos:related <http://data.loterre.fr/ark:/67375/TSO-H5ZG6DX6-4>, <http://data.loterre.fr/ark:/67375/TSO-RPJVDHMM-Q>, <http://data.loterre.fr/ark:/67375/TSO-XHQRK84J-T> .

<http://data.loterre.fr/ark:/67375/TSO-NTQ23ZP5-B>
  a skos:Concept ;
  skos:altLabel "FI"@fr, "índice de impacto"@es ;
  skos:definition "Indicateur qui estime indirectement la visibilité d'une revue scientifique. Pour une année donnée, le FI d'une revue est égal à la moyenne des nombres de citations des articles de cette revue publiés durant les deux années précédentes. Dans un contexte de science ouverte, l'utilisation du FI est souvent considérée comme un biais dans le processus d'évaluation de la recherche, qui contribue en outre à consolider la position dominante des grands éditeurs scientifique."@fr, "Scientometric index that reflects the yearly average number of citations of articles published in the last two years in a given journal. (Source : Wikipedia)"@en ;
  skos:prefLabel "facteur d'impact"@fr, "factor de impacto"@es, "impact factor"@en ;
  skos:inScheme <http://data.loterre.fr/ark:/67375/TSO> ;
  skos:broader <http://data.loterre.fr/ark:/67375/TSO-T9Q25G6Q-S> ;
  skos:related <http://data.loterre.fr/ark:/67375/TSO-PSFFQLXV-2> .

<http://data.loterre.fr/ark:/67375/TSO-X11G8MG1-M>
  a skos:Concept ;
  dc:modified "2021-06-29"^^xsd:date ;
  skos:altLabel "Apache Licence 2.0"@en ;
  skos:definition "A free software license by the Apache Software Foundation. (Source : http://www.apache.org/licenses/)"@en, "Licence permissive, produite par l'Apache Software Foundation, imposant la mention du droit d’auteur, la licence ainsi que les modifications effectuées sur l’œuvre originale. (Source : http://vvlibri.org/fr/licence/apache-license-version-2/analysis)"@fr ;
  skos:prefLabel "Apache License 2.0"@en, "licence Apache 2.0"@fr, "licencia Apache 2.0"@es ;
  skos:inScheme <http://data.loterre.fr/ark:/67375/TSO> ;
  skos:broader <http://data.loterre.fr/ark:/67375/TSO-T67S254S-S> .

<http://data.loterre.fr/ark:/67375/TSO-SMF21F74-3>
  a skos:Concept ;
  dc:modified "2021-06-29"^^xsd:date ;
  skos:altLabel "free BSD licence"@en, "licencia FreeBSD (de 2 cláusulas)"@es, "simplified BSD licence"@en ;
  skos:definition "Licence libre utilisée pour la distribution de logiciels. Elle prévoit que la redistribution et l'utilisation, avec ou sans modification, sont autorisées à condition que les conditions suivantes soient respectées : 1. Les redistributions de code source doivent conserver l'avis de droit d'auteur ci-dessus, la présente liste de conditions et la clause de non-responsabilité suivante ; 2. Les redistributions sous forme binaire doivent reproduire l'avis de droit d'auteur ci-dessus, la présente liste de conditions et la clause de non-responsabilité suivante dans la documentation et/ou les autres documents fournis avec la distribution."@fr, "Redistribution and use in source and binary forms, with or without modification, are permitted provided that the following conditions are met: 1. Redistributions of source code must retain the above copyright notice, this list of conditions and the following disclaimer; 2. Redistributions in binary form must reproduce the above copyright notice, this list of conditions and the following disclaimer in the documentation and/or other materials provided with the distribution. (Source: https://opensource.org/licenses/BSD-2-Clause)"@en ;
  skos:prefLabel "BSD 2-Clause license"@en, "licence BSD-2 clause"@fr, "licencia BSD simplificada"@es ;
  skos:inScheme <http://data.loterre.fr/ark:/67375/TSO> ;
  skos:broader <http://data.loterre.fr/ark:/67375/TSO-T67S254S-S> .

<http://data.loterre.fr/ark:/67375/TSO-X2MBVK0V-Z>
  a skos:Concept ;
  dc:modified "2021-06-29"^^xsd:date ;
  skos:altLabel "BSD de 3 cláusulas"@es, "BSD modificada"@es, "BSD revisada"@es, "BSD-3"@es, "modified BSD licence"@en, "new BSD licence"@en, "revised BSD licence"@en ;
  skos:definition "Licence permissive imposant simplement la mention du droit d’auteur et de la licence. Le texte de la licence doit être distribué avec la clause d’exclusion de garantie. La licence BSD prohibe l’usage des noms de l’auteur et des contributeurs pour promouvoir le produit créé à partir du contenu sous cette licence. L’œuvre sous cette licence, l’œuvre modifiée ou intégrée à un projet plus grand, peuvent être distribuées sous une autre licence et sans le code source. La licence BSD ne couvre pas les brevets. (Source : http://vvlibri.org/fr/licence/bsd-3-clause/analysis)"@fr, "Redistribution and use in source and binary forms, with or without modification, are permitted provided that the following conditions are met: 1. Redistributions of source code must retain the above copyright notice, this list of conditions and the following disclaimer; 2. Redistributions in binary form must reproduce the above copyright notice, this list of conditions and the following disclaimer in the documentation and/or other materials provided with the distribution; 3. Neither the name of the copyright holder nor the names of its contributors may be used to endorse or promote products derived from this software without specific prior written permission. (Source: https://opensource.org/licenses/BSD-3-Clause)"@en ;
  skos:prefLabel "BSD 3-Clause license"@en, "licence BSD-3 clause"@fr, "nueva licencia BSD"@es ;
  skos:inScheme <http://data.loterre.fr/ark:/67375/TSO> ;
  skos:broader <http://data.loterre.fr/ark:/67375/TSO-T67S254S-S> .

<http://data.loterre.fr/ark:/67375/TSO-ZK0KHM67-X>
  a skos:Concept ;
  dc:modified "2021-06-24"^^xsd:date ;
  skos:definition "A licence clause allowing the reuse, sharing, and remixing of materials providing that it is for non-commercial purposes, providing the original author is appropriately attributed. Not compatible with free cultural works. (Source : http://www.righttoresearch.org/resources/OpenResearchGlossary)"@en, "Licence qui permet à d'autres personnes de remixer, d'adapter et de s'appuyer sur un travail, à des fins non commerciales. Bien que ces nouvelles œuvres doivent citer l'auteur du travail d'origine et être non commerciales, leurs auteurs ne sont pas tenus d'accorder une licence identique à ces œuvres dérivées. (Source : https://creativecommons.org/licenses/?lang=fr-FR)"@fr ;
  skos:prefLabel "CC-BY-NC license"@en, "licence CC-BY-NC"@fr, "licencia CC-BY- NC"@es ;
  skos:inScheme <http://data.loterre.fr/ark:/67375/TSO> ;
  skos:broader <http://data.loterre.fr/ark:/67375/TSO-KB9PPZQF-T>, <http://data.loterre.fr/ark:/67375/TSO-WH5JC3TT-G> .

<http://data.loterre.fr/ark:/67375/TSO-F844JJK0-Q>
  a skos:Concept ;
  dc:modified "2021-06-24"^^xsd:date ;
  skos:definition "Licence n’autorisant les autres qu’à télécharger des œuvres et à les partager tant que le créateur est crédité. On ne peut les modifier de quelque façon que ce soit ni les utiliser à des fins commerciales. (Source : https://creativecommons.org/licenses/?lang=fr-FR)"@fr ;
  skos:prefLabel "CC-BY-NC-ND license"@en, "licence CC-BY-NC-ND"@fr, "licencia CC-BY-NC-ND"@es ;
  skos:inScheme <http://data.loterre.fr/ark:/67375/TSO> ;
  skos:broader <http://data.loterre.fr/ark:/67375/TSO-KB9PPZQF-T>, <http://data.loterre.fr/ark:/67375/TSO-WH5JC3TT-G> .

<http://data.loterre.fr/ark:/67375/TSO-XNNFBR4D-D>
  a skos:Concept ;
  dc:modified "2021-06-24"^^xsd:date ;
  skos:definition "Licence qui permet à d'autres personnes de remixer, d'adapter et de s'inspirer du travail d'un tiers à des fins non commerciales, à condition de créditer le créateur du travail et d'accorder une licence à leurs nouvelles créations dans les mêmes conditions. (Source : https://creativecommons.org/licenses/?lang=fr-FR)"@fr ;
  skos:prefLabel "CC-BY-NC-SA license"@en, "licence CC-BY-NC-SA"@fr, "licencia CC-BY-NC-SA"@es ;
  skos:inScheme <http://data.loterre.fr/ark:/67375/TSO> ;
  skos:broader <http://data.loterre.fr/ark:/67375/TSO-KB9PPZQF-T>, <http://data.loterre.fr/ark:/67375/TSO-WH5JC3TT-G> .

<http://data.loterre.fr/ark:/67375/TSO-LXH6ZFD2-J>
  a skos:Concept ;
  dc:modified "2021-06-24"^^xsd:date ;
  skos:definition "A licence clause requiring that the original author is appropriately attributed and that derivatives are not made of the original works. Not compatible with free cultural works. (Source : http://www.righttoresearch.org/resources/OpenResearchGlossary)"@en, "Licence qui permet à d'autres personnes de réutiliser une œuvre à n'importe quelles fins, y compris commerciales ; toutefois, elle ne peut pas être adaptée et doit être attribuée à son auteur. (Source : https://creativecommons.org/licenses/?lang=fr-FR)"@fr ;
  skos:prefLabel "CC-BY-ND license"@en, "licence CC-BY-ND"@fr, "licencia CC-BY-ND"@es ;
  skos:inScheme <http://data.loterre.fr/ark:/67375/TSO> ;
  skos:broader <http://data.loterre.fr/ark:/67375/TSO-KB9PPZQF-T>, <http://data.loterre.fr/ark:/67375/TSO-WH5JC3TT-G> .

<http://data.loterre.fr/ark:/67375/TSO-LRT6FWVV-0>
  a skos:Concept ;
  dc:modified "2021-06-29"^^xsd:date ;
  skos:altLabel "CEA CNRS INRIA Logiciel Libre"@fr ;
  skos:definition "Licence de logiciel libre dont les auteurs sont le Commissariat à l'énergie atomique et aux énergies alternatives (CEA), le Centre National de la Recherche Scientifique (CNRS )et l'Institut National de Recherche en Informatique et en Automatique (Inria). Son objectif est de conférer aux utilisateurs la liberté de modification et de redistribution du logiciel régi par cette licence dans le cadre d'un modèle de diffusion en logiciel libre. (Source : http://vvlibri.org/fr/licence/cecill-21/legalcode/official)"@fr ;
  skos:prefLabel "CeCILL free software licence agreement"@en, "licence CeCILL"@fr, "licencia CeCILL"@es ;
  skos:inScheme <http://data.loterre.fr/ark:/67375/TSO> ;
  skos:broader <http://data.loterre.fr/ark:/67375/TSO-T67S254S-S> .

<http://data.loterre.fr/ark:/67375/TSO-N3CP621W-L>
  a skos:Concept ;
  dc:modified "2021-06-29"^^xsd:date ;
  skos:altLabel "Kopernio"@en ;
  skos:definition "Application développée par Clarivate Analytics permettant de repérer et de collecter rapidement et simplement les fichiers PDF d’articles de périodiques en accord avec les licences d’accès de son institution d’enseignement. (Source : https://carrefour.uquebec.ca/endnote/faq/quest-ce-que-endnote-click)"@fr ;
  skos:prefLabel "EndNote Click"@en, "EndNote Click"@es, "EndNote Click"@fr ;
  skos:inScheme <http://data.loterre.fr/ark:/67375/TSO> ;
  skos:broader <http://data.loterre.fr/ark:/67375/TSO-WQMF6CT2-K> .

<http://data.loterre.fr/ark:/67375/TSO-KD39PQLZ-P>
  a skos:Concept ;
  dc:modified "2021-06-24"^^xsd:date ;
  skos:definition "permet d’accéder facilement à Google Scholar pour faire une recherche à partir d’un texte trouvé sur une page Web ou d’un document pdf. [Cette extension] permet d’effectuer des recherches parmi de nombreuses sources universitaires (thèses universitaires, ouvrages scientifiques et articles académiques à comité de lecture). Le moteur trie les résultats en favorisant les articles les plus cités. (Source : http://www.sciencespo-grenoble.fr/les-ressources/beneficier-dune-formation/extensions/#:~:text=Lazy%20Scholar%20est%20une%20extension,la%20recommandation%20d%27autres%20articles)"@fr ;
  skos:prefLabel "Google Scholar button"@en, "botón de Google Académico"@es, "bouton Google Scholar"@fr ;
  skos:inScheme <http://data.loterre.fr/ark:/67375/TSO> ;
  skos:broader <http://data.loterre.fr/ark:/67375/TSO-WQMF6CT2-K> .

<http://data.loterre.fr/ark:/67375/TSO-PB3X8G4D-N>
  a skos:Concept ;
  dc:modified "2021-06-24"^^xsd:date ;
  skos:definition "Extension de navigateur permettant la recherche automatique du texte intégral en open access de l’article consulté, la consultation des métriques de citations, la mise à disposition de 900 styles de citations pour citer la référence consultée, la suggestion et la recommandation d’autres articles sur le thème recherché et l’enregistrement de l’historique de recherche. (Source : http://www.sciencespo-grenoble.fr/les-ressources/beneficier-dune-formation/extensions/#:~:text=Lazy%20Scholar%20est%20une%20extension,la%20recommandation%20d%27autres%20articles)"@fr ;
  skos:prefLabel "Lazy Scholar"@en, "Lazy Scholar"@es, "Lazy Scholar"@fr ;
  skos:inScheme <http://data.loterre.fr/ark:/67375/TSO> ;
  skos:broader <http://data.loterre.fr/ark:/67375/TSO-WQMF6CT2-K> .

<http://data.loterre.fr/ark:/67375/TSO-WKKLL52L-D>
  a skos:Concept ;
  dc:modified "2021-06-24"^^xsd:date ;
  skos:definition "Extension de navigateur qui facilite l’accès aux ressources numériques. [Elle] se manifeste sous forme de pop-up et vous signale les ressources accessibles via la bibliothèque. Si la bibliothèque n’est pas abonnée à une ressource, l’extension cherche une version en accès libre (open access) à proposer. (Source : http://www.sciencespo-grenoble.fr/les-ressources/beneficier-dune-formation/extensions/#:~:text=Lazy%20Scholar%20est%20une%20extension,la%20recommandation%20d%27autres%20articles)"@fr ;
  skos:prefLabel "Lean Library"@en, "Lean Library"@es, "Lean Library"@fr ;
  skos:inScheme <http://data.loterre.fr/ark:/67375/TSO> ;
  skos:broader <http://data.loterre.fr/ark:/67375/TSO-WQMF6CT2-K> .

<http://data.loterre.fr/ark:/67375/TSO-Z9Q5Q16G-F>
  a skos:Concept ;
  dc:modified "2021-06-28"^^xsd:date ;
  skos:altLabel "MIT licence"@en ;
  skos:definition "Licence très permissive qui implique peu de contraintes quant à la réutilisation du code, et sans copyleft. Elle est compatible avec de très nombreuses licences, notamment la GNU GPL. (Source : https://www.appvizer.fr/magazine/services-informatiques/gestion-licences/licence-open-source#la-licence-mit)"@fr ;
  skos:prefLabel "MIT license"@en, "licence MIT"@fr, "licencia MIT"@es ;
  skos:inScheme <http://data.loterre.fr/ark:/67375/TSO> ;
  skos:broader <http://data.loterre.fr/ark:/67375/TSO-T67S254S-S> .

<http://data.loterre.fr/ark:/67375/TSO-NDK3CG5V-9>
  a skos:Concept ;
  dc:modified "2021-06-24"^^xsd:date ;
  skos:definition "Permet la recherche d’articles de revues en accès libre. Pour savoir s’il existe une version gratuite de l’article consulté, il faut cliquer sur le logo orange présent dans la barre d’outils. Si une version gratuite est détectée, le PFD s’ouvre directement. Dans le cas contraire, il est possible de demander à l’auteur de rendre l’article disponible en libre accès. (Source : http://www.sciencespo-grenoble.fr/les-ressources/beneficier-dune-formation/extensions/#:~:text=Lazy%20Scholar%20est%20une%20extension,la%20recommandation%20d%27autres%20articles)"@fr ;
  skos:prefLabel "Open Access button"@en, "botón de Acceso Abierto"@es, "bouton Open Access"@fr ;
  skos:inScheme <http://data.loterre.fr/ark:/67375/TSO> ;
  skos:broader <http://data.loterre.fr/ark:/67375/TSO-WQMF6CT2-K> .

<http://data.loterre.fr/ark:/67375/TSO-PSFFQLXV-2>
  a skos:Concept ;
  skos:altLabel "practice detrimental to open science"@en ;
  skos:prefLabel "practice unfavorable to open science"@en, "pratique préjudiciable à la science ouverte"@fr, "práctica perjudicial para la ciencia abierta"@es ;
  skos:inScheme <http://data.loterre.fr/ark:/67375/TSO> ;
  skos:related <http://data.loterre.fr/ark:/67375/TSO-DCPLM2CT-F>, <http://data.loterre.fr/ark:/67375/TSO-J6QSX265-4>, <http://data.loterre.fr/ark:/67375/TSO-NTQ23ZP5-B> ;
  skos:narrower <http://data.loterre.fr/ark:/67375/TSO-D2CGSDHD-L>, <http://data.loterre.fr/ark:/67375/TSO-ZRVHF3XW-L>, <http://data.loterre.fr/ark:/67375/TSO-QMSRJLT3-C>, <http://data.loterre.fr/ark:/67375/TSO-WT63ZDZ1-T>, <http://data.loterre.fr/ark:/67375/TSO-NBSJSHH5-P>, <http://data.loterre.fr/ark:/67375/TSO-DDX6CQLL-1>, <http://data.loterre.fr/ark:/67375/TSO-XRBPKF38-J> ;
  skos:topConceptOf <http://data.loterre.fr/ark:/67375/TSO> .

<http://data.loterre.fr/ark:/67375/TSO-ZRVHF3XW-L>
  a skos:Concept ;
  dc:modified "2021-06-28"^^xsd:date ;
  skos:altLabel "deceptive publishing"@en, "publicación de solo escritura"@es, "publicación engañosa"@es, "write-only publishing"@en ;
  skos:definition "An exploitative academic publishing business model that involves charging publication fees to authors without checking articles for quality and legitimacy, and without providing editorial and publishing services that legitimate academic journals provide, whether open access or not. (Source: Wikipedia)"@en, "Édition qui détourne les possibilités de l'édition scientifique en libre accès à des fins mercantiles, où la recherche de profits prévaut sur les principes de rigueur scientifique et éditoriale habituellement respectés par les éditeurs de revues savantes. (Source : http://gdt.oqlf.gouv.qc.ca/ficheOqlf.aspx?Id_Fiche=26544672)"@fr ;
  skos:prefLabel "predatory publishing"@en, "publicación depredadora"@es, "édition prédatrice"@fr ;
  skos:inScheme <http://data.loterre.fr/ark:/67375/TSO> ;
  skos:broader <http://data.loterre.fr/ark:/67375/TSO-PSFFQLXV-2> ;
  skos:related <http://data.loterre.fr/ark:/67375/TSO-JL9MGMVK-W>, <http://data.loterre.fr/ark:/67375/TSO-WWM82SKD-Z> .

<http://data.loterre.fr/ark:/67375/TSO-DKCFHCNB-D>
  a skos:Concept ;
  dc:modified "2021-06-29"^^xsd:date ;
  skos:altLabel "GRID identifier"@en, "Global Research Identifier Database identifier"@en ;
  skos:definition "Identifiant unique .attribué à une institution référencée dans la base de données GRID, répertoire mondial d’institutions de tous types actives en matière de recherche académique."@fr, "Institutional identifier from the GRID.ac global research identifier database"@en ;
  skos:prefLabel "GRID ID"@en, "identifiant GRID"@fr, "identificador GRID"@es ;
  skos:inScheme <http://data.loterre.fr/ark:/67375/TSO> ;
  skos:broader <http://data.loterre.fr/ark:/67375/TSO-H5ZG6DX6-4> .

<http://data.loterre.fr/ark:/67375/TSO-NQNLFZ3L-0>
  a skos:Concept ;
  dc:modified "2021-06-29"^^xsd:date ;
  skos:altLabel "Research Activity Identifier"@en ;
  skos:definition "Identifiant pérenne attribué à un projet de recherche."@fr, "Persistent IDentifier for research projects"@en ;
  skos:prefLabel "RAiD"@en, "RAiD"@es, "RAiD"@fr ;
  skos:inScheme <http://data.loterre.fr/ark:/67375/TSO> ;
  skos:broader <http://data.loterre.fr/ark:/67375/TSO-H5ZG6DX6-4> .

<http://data.loterre.fr/ark:/67375/TSO-BKX9QBKJ-C>
  a skos:Concept ;
  dc:modified "2021-06-18"^^xsd:date ;
  skos:definition "A three year project (2017-2019) funded by the SA National Research Foundation (NRF), directed by CODATA, and managed by the Academy of Science of South Africa (ASSAf). The four focus areas to be explored during this project include the following: Open Science policy, Infrastructure in support of Open Science, Skills required and building capacity in support of Open Science, and Incentives for sharing science and data. (Source : ASSAf)"@en, "Projet étalé sur trois ans (de 2017 à 2019) créé par la Fondation nationale pour la recherche d'Afrique du Sud (NRF), dirigé par CODATA et géré par l'Académie des Sciences d'Afrique du Sud (ASSAf). Les quatre points de discussion de ce projet sont : la politique de la science ouverte, les infrastructures qui soutiennent la science ouverte, les compétences nécessaires et les capacités de construction pour soutenir la science ouverte, et enfin la promotion du partage de la science et des données. (Source: traduction du site Internet de l'ASSAf)"@fr ;
  skos:prefLabel "African Open Science Platform"@en, "African Open Science Platform"@es, "African Open Science Platform"@fr ;
  skos:inScheme <http://data.loterre.fr/ark:/67375/TSO> ;
  skos:broader <http://data.loterre.fr/ark:/67375/TSO-H93WKMMJ-B> .

<http://data.loterre.fr/ark:/67375/TSO-S9J32NCP-W>
  a skos:Concept ;
  skos:altLabel "Open Knowledge for Latin America and the Global South"@en ;
  skos:definition "A communication infrastructure for scholarly publishing and open science. Sustained cooperatively, this initiative focuses on a non-profit publishing model to preserve the scholarly and open nature of scientific communication. Sustained by the non-profit civil association “AmeliCA A.C.,” this initiative is led by the United Nations Educational, Scientific and Cultural Organization (UNESCO), the Latin American Council of Social Sciences (CLACSO) and the Network of Scientific Journals from Latin America, the Caribbean, Spain and Portugal (Redalyc). (Source : http://amelica.org/index.php/en/about/)"@en, "Infraestructura de comunicación para la publicación académica y la ciencia abierta. Es una iniciativa sostenida de forma cooperativa y centrada en el modelo de publicación sin fines de lucro para conservar la naturaleza académica y abierta de la comunicación científica. AmeliCA es sostenida por la asociación civil sin fines de lucro “AmeliCA A.C.”. La iniciativa es liderada por la Organización de las Naciones Unidas para la Educación, la Ciencia y la Cultura (UNESCO), el Consejo Latinoamericano de Ciencias Sociales (CLACSO) y la Red de Revistas Científicas de América Latina, el Caribe, España y Portugal (Redalyc) e impulsada desde su lanzamiento por la Universidad Autónoma del Estado de México (UAEM, México), la Universidad de Antioquia (UdeA, Colombia) y la Universidad Nacional de La Plata (UNLP, Argentina). (Fuente: http://amelica.org/index.php/que-es-ameli/)"@es, "Initiative communautaire, multi-institutionnelle, dont l'objectif est de mettre en place une solution collaborative, durable et non commerciale, pour soutenir l'accès ouvert aux connaissances produites en Amérique latine et dans les pays du Sud. Elle a été lancée en 2018 par l’Organisation des Nations Unies pour l’éducation, la science et la culture (UNESCO), le Conseil latino-américain des sciences sociales (CLACSO), le réseau des revues scientifiques d’Amérique latine et des Caraïbes, d’Espagne et du Portugal (REDALYC), l’Université autonome de l’État du Mexique (UAEM), l’Université d’Antioche (UDEA) et l’Université nationale de La Plata (UNLP).(Source : Ouvrir la Science)"@fr ;
  skos:prefLabel "AmeliCA"@en, "AmeliCA"@es, "AmeliCA"@fr ;
  skos:inScheme <http://data.loterre.fr/ark:/67375/TSO> ;
  skos:broader <http://data.loterre.fr/ark:/67375/TSO-J64S3QDL-1> .

<http://data.loterre.fr/ark:/67375/TSO-ZT32Z3F2-6>
  a skos:Concept ;
  dc:modified "2021-06-24"^^xsd:date ;
  skos:definition "TGIR (Très Grande Infrastructure de Recherche) qui structure l’accompagnement des communautés scientifiques SHS en matière d’infrastructure numérique pour les données de la recherche. (Source : https://www.huma-num.fr/)"@fr ;
  skos:prefLabel "Huma-Num"@en, "Huma-Num"@es, "Huma-Num"@fr ;
  skos:inScheme <http://data.loterre.fr/ark:/67375/TSO> ;
  skos:broader <http://data.loterre.fr/ark:/67375/TSO-J64S3QDL-1> .

<http://data.loterre.fr/ark:/67375/TSO-DKBRJ0N6-J>
  a skos:Concept ;
  dc:modified "2021-06-28"^^xsd:date ;
  skos:altLabel "KE"@en ;
  skos:definition "A collaboration between six national organisations, each responsible for supporting the development of ICT infrastructure for higher education and research. (Source: https://www.knowledge-exchange.info/)"@en, "Entité qui réunit six organisations représentatives de l’activité de recherche dans leur pays : CNRS (France), CSC (Finlande), DEIC (Danemark), DFG (Allemagne), JISC (Royaume-Uni), SURF (Pays-Bas). Leur objectif commun est d’examiner les problèmes de soutien à la recherche et de développement d’infrastructures et de services permettant l’utilisation des technologies numériques, de partager des solutions, de rechercher des approches sur les questions émergentes qui auront une influence concrète sur leurs activités, et de favoriser les échanges entre les membres de leurs différentes communautés nationales de recherche et d’enseignement supérieur. (Source : https://www.ouvrirlascience.fr/activites-de-knowledge-exchange-partenaires-pour-ameliorer-le-service-a-lesr/)"@fr ;
  skos:prefLabel "Knowledge Exchange"@en, "Knowledge Exchange"@es, "Knowledge Exchange"@fr ;
  skos:inScheme <http://data.loterre.fr/ark:/67375/TSO> ;
  skos:broader <http://data.loterre.fr/ark:/67375/TSO-J64S3QDL-1> ;
  skos:related <http://data.loterre.fr/ark:/67375/TSO-KSZ3VF36-P> .

<http://data.loterre.fr/ark:/67375/TSO-NG65T0DF-9>
  a skos:Concept ;
  skos:definition "Initiative lancée par la Société Max Planck en décembre 2015, à l’occasion de Berlin 12, qui prône la conversion du modèle de l’abonnement vers celui de l’accès ouvert. Les organismes de recherche sont invités à signer la déclaration d’intérêt pour manifester leur soutien à ce mouvement. (Source : Ouvrir la Science)"@fr ;
  skos:prefLabel "OA2020"@en, "OA2020"@es, "OA2020"@fr ;
  skos:inScheme <http://data.loterre.fr/ark:/67375/TSO> ;
  skos:broader <http://data.loterre.fr/ark:/67375/TSO-J64S3QDL-1> .

<http://data.loterre.fr/ark:/67375/TSO-HK7N0SDD-S>
  a skos:Concept ;
  dc:modified "2021-06-25"^^xsd:date ;
  skos:altLabel "Open Access Scholarly Publishing Association"@en, "Open Access Scholarly Publishing Association"@es, "Open Access Scholarly Publishing Association"@fr ;
  skos:definition "Association professionnelle qui représente les intérêts des éditeurs en libre accès (OA) à l'échelle mondiale dans toutes les disciplines scientifiques, techniques et universitaires. (Source : https://access2perspectives.org/fr/services/open-science/#)"@fr, "OASPA is a diverse community of organisations engaged in open scholarship. Our membership includes scholar-led and professional publishers of books and journals, across varied geographies and disciplines, as well as infrastructure and other services."@en ;
  skos:prefLabel "OASPA"@en, "OASPA"@es, "OASPA"@fr ;
  skos:inScheme <http://data.loterre.fr/ark:/67375/TSO> ;
  skos:broader <http://data.loterre.fr/ark:/67375/TSO-J64S3QDL-1> .

<http://data.loterre.fr/ark:/67375/TSO-FTDKPJ1X-Z>
  a skos:Concept ;
  dc:modified "2021-06-25"^^xsd:date ;
  skos:definition "Initiative ayant pour objectif principal de soutenir le travail de recherche des scientifiques européens en créant et en exploitant une infrastructure d’accès ouvert, robuste, durable et participative, responsable de la gestion, de l’analyse, de la manipulation, de la fourniture et (surtout) de la mise en réseau d’un très large éventail de publications scientifiques et de données de la recherche. (Source : https://scienceouverte.couperin.org/quest-ce-quopenaire/)"@fr, "OpenAIRE’s mission is closely linked to the mission of the European Commission: to provide unlimited, barrier free, open access to research outputs financed by public funding in Europe. (Source : OpenAIRE)"@en ;
  skos:prefLabel "OpenAIRE"@en, "OpenAIRE"@es, "OpenAIRE"@fr ;
  skos:inScheme <http://data.loterre.fr/ark:/67375/TSO> ;
  skos:broader <http://data.loterre.fr/ark:/67375/TSO-J64S3QDL-1> .

<http://data.loterre.fr/ark:/67375/TSO-VPTBZS30-F>
  a skos:Concept ;
  dc:modified "2021-06-29"^^xsd:date ;
  skos:altLabel "Permanent Secretariat (SPSO)"@en, "Secrétariat Permanent pour la Science Ouverte"@fr ;
  skos:definition "Organe du comité pour la science ouverte chargé de préparer les travaux du comité de pilotage de la science ouverte, et de veiller à la mise en œuvre de ses orientations et conclusions. Il coordonne l’action des collèges et groupes de travail, saisissant les groupes et synthétisant leurs contributions. (Source : https://www.ouvrirlascience.fr/presentation-du-comite/)"@fr ;
  skos:prefLabel "SPSO"@en, "SPSO"@es, "SPSO"@fr ;
  skos:inScheme <http://data.loterre.fr/ark:/67375/TSO> ;
  skos:broader <http://data.loterre.fr/ark:/67375/TSO-J64S3QDL-1> ;
  skos:related <http://data.loterre.fr/ark:/67375/TSO-VPJV1Q5X-J> .

<http://data.loterre.fr/ark:/67375/TSO-HZ81233X-G>
  a skos:Concept ;
  dc:modified "2021-06-24"^^xsd:date ;
  skos:altLabel "Directiva (UE) 2019/790 del Parlamento Europeo y del Consejo, de 17 de abril de 2019, sobre los derechos de autor y derechos afines en el mercado único digital"@es, "Directive (EU) 2019/790 of the European Parliament and of the Council of 17 April 2019 on copyright and related rights in the Digital Single Market"@en, "Directive (UE) 2019/790 du Parlement européen et du Conseil du 17 avril 2019 sur le droit d'auteur et les droits voisins dans le marché unique numérique"@fr, "Directive on Copyright in the Digital Single Market"@en ;
  skos:definition "Directive Européenne qui vise à instaurer un cadre global, dans lequel les créations intellectuelles, les auteurs, les éditeurs de contenus, les prestataires de services et les utilisateurs pourront tous bénéficier de règles plus claires, modernisées et adaptées à l’ère numérique."@fr ;
  skos:prefLabel "Directiva (UE) 2019/790"@es, "Directive (EU) 2019/790"@en, "Directive (UE) 2019/790"@fr ;
  skos:inScheme <http://data.loterre.fr/ark:/67375/TSO> ;
  skos:broader <http://data.loterre.fr/ark:/67375/TSO-MGZJDL80-2> ;
  skos:related <http://data.loterre.fr/ark:/67375/TSO-RGKFQW9J-K> .

<http://data.loterre.fr/ark:/67375/TSO-NJS8254Q-B>
  a skos:Concept ;
  dc:modified "2021-06-11"^^xsd:date ;
  skos:altLabel "accord de transformation"@fr, "négociation couplée abonnement / APC"@fr, "offsetting model"@en, "transformative arrangement"@en ;
  skos:definition "Négociation qui permet d’effectuer une transition vers l’accès ouvert et qui s’effectue en plusieurs étapes : coupler les dépenses APC & abonnements pour mieux les contrôler et convertir ensuite les dépenses d’abonnements vers des dépenses dédiées à l’accès ouvert. (Source : Irini Paltani-Sargologos. hal-02538844)"@fr ;
  skos:prefLabel "accord transformant"@fr, "acuerdo transformante"@es, "transformative agreement"@en ;
  skos:inScheme <http://data.loterre.fr/ark:/67375/TSO> ;
  skos:broader <http://data.loterre.fr/ark:/67375/TSO-MWXTBMQ8-9> .

<http://data.loterre.fr/ark:/67375/TSO-N8C284KM-Q>
  a skos:Concept ;
  dc:modified "2021-06-04"^^xsd:date ;
  skos:altLabel "AAM"@en, "accepted author manuscript"@en, "author's accepted manuscript"@en, "final peer-reviewed manuscript"@en, "manuscrit final examiné par les pairs"@fr, "post-print"@en, "post-print"@es, "post-print"@fr, "post-publication"@fr, "version finale du manuscrit examinée par les pairs"@fr ;
  skos:definition "Version définitive d’un manuscrit produit par un (des) auteur(s) après révision par les pairs, comportant les modifications apportées par les pairs mais sans la mise en forme de l’éditeur. (source: https://openaccess.inist.fr/glossaire/)"@fr ;
  skos:prefLabel "postimpresión"@es, "postprint"@en, "postpublication"@fr ;
  skos:inScheme <http://data.loterre.fr/ark:/67375/TSO> ;
  skos:broader <http://data.loterre.fr/ark:/67375/TSO-FP5VCTTB-4> .

<http://data.loterre.fr/ark:/67375/TSO-GLZ7M59Q-M>
  a skos:Concept ;
  dc:modified "2021-06-04"^^xsd:date ;
  skos:altLabel "AOM"@en, "author's original manuscript"@en, "manuscrito previo a la revisión por pares"@es, "preimpresión"@es, "preprint"@es, "préprint"@fr ;
  skos:definition "Preliminary report of work that has not been certified by peer review."@en, "Un manuscrito que aún no ha sido sometido a una revisión formal por pares, distribuido para recibir comentarios previos a la publicación por parte de otros investigadores. (Fuente: Foster)"@es, "Version d’un article qu'un auteur soumet au comité de rédaction d’une revue scientifique ou dépose dans une archive ouverte, et qui n'a pas encore été évalué par ses pairs."@fr ;
  skos:prefLabel "preprint"@en, "prepublicación"@es, "prépublication"@fr ;
  skos:inScheme <http://data.loterre.fr/ark:/67375/TSO> ;
  skos:broader <http://data.loterre.fr/ark:/67375/TSO-FP5VCTTB-4> ;
  skos:related <http://data.loterre.fr/ark:/67375/TSO-C4027K67-Q>, <http://data.loterre.fr/ark:/67375/TSO-KBZ7QKR9-W>, <http://data.loterre.fr/ark:/67375/TSO-L1X7N7S8-V>, <http://data.loterre.fr/ark:/67375/TSO-LQV42R36-F>, <http://data.loterre.fr/ark:/67375/TSO-MDD3CCP5-9>, <http://data.loterre.fr/ark:/67375/TSO-PZNHPP7J-7>, <http://data.loterre.fr/ark:/67375/TSO-R19NG9JL-2>, <http://data.loterre.fr/ark:/67375/TSO-RPCFB5QW-0>, <http://data.loterre.fr/ark:/67375/TSO-S784H10S-P>, <http://data.loterre.fr/ark:/67375/TSO-W9KRS5Q3-6>, <http://data.loterre.fr/ark:/67375/TSO-WD1R50MM-6>, <http://data.loterre.fr/ark:/67375/TSO-XHFB8590-0> .

<http://data.loterre.fr/ark:/67375/TSO-WLFCMS28-F>
  a skos:Concept ;
  dc:modified "2021-06-09"^^xsd:date ;
  skos:definition "Combinaison de l’accès ouvert (les textes sont accessibles sans identification et sans paiement) et d’une licence libre, permettant la réutilisation dans certaines conditions. (Source : https://bn.hypotheses.org/11434)"@fr ;
  skos:prefLabel "acceso libre"@es, "accès libre"@fr, "libre open access"@en ;
  skos:inScheme <http://data.loterre.fr/ark:/67375/TSO> ;
  skos:broader <http://data.loterre.fr/ark:/67375/TSO-STWL5MWS-W> .

<http://data.loterre.fr/ark:/67375/TSO-KGHBM8Z5-6>
  a skos:Concept ;
  dc:modified "2021-06-10"^^xsd:date ;
  skos:altLabel "BSO"@fr, "baromètre de la science ouverte"@fr ;
  skos:definition "Outil de mesure de l'évolution de l'accès ouvert aux publications en France à partir de données fiables, ouvertes et maîtrisées. Le baromètre concerne pour le moment l'accès ouvert aux publications. L'extension du périmètre à d'autres types d'objets (données de la recherche et logiciels notamment) est à l'étude. (Source : https://ministeresuprecherche.github.io/bso/)"@fr, "Tool which measure the trends of open access to publications in France using trustworthy, open and controlled data.The monitor focuses for now on the open access to publications. Extending the scope to other objects (in particular research data and software) is being explored. (Source : https://ministeresuprecherche.github.io/bso/)"@en ;
  skos:prefLabel "French open science monitor"@en, "baromètre français de la science ouverte"@es, "baromètre français de la science ouverte"@fr ;
  skos:inScheme <http://data.loterre.fr/ark:/67375/TSO> ;
  skos:broader <http://data.loterre.fr/ark:/67375/TSO-V0KSG0NC-P> ;
  skos:related <http://data.loterre.fr/ark:/67375/TSO-T9Q25G6Q-S>, <http://data.loterre.fr/ark:/67375/TSO-ZLCW75XN-W> .

<http://data.loterre.fr/ark:/67375/TSO-ZLCW75XN-W>
  a skos:Concept ;
  dc:modified "2021-06-09"^^xsd:date ;
  skos:altLabel "PNSO"@fr ;
  skos:definition "Plan d'action lancé en juillet 2018 par le Ministère de l’enseignement supérieur, de la recherche et de l’innovation français. Il définit 3 axes stratégiques pour inscrire la recherche française au cœur du mouvement mondial d’ouverture des données et de transparence de l’action publique : généraliser l’accès ouvert aux publications, structurer et ouvrir les données de la recherche, s’inscrire dans une dynamique durable, européenne et internationale. (Source : https://scienceouverte.couperin.org)"@fr ;
  skos:prefLabel "National plan for open science"@en, "Plan national pour la science ouverte"@fr, "plan nacional de ciencia abierta de Francia"@es ;
  skos:inScheme <http://data.loterre.fr/ark:/67375/TSO> ;
  skos:broader <http://data.loterre.fr/ark:/67375/TSO-T6RG1XJN-7> ;
  skos:related <http://data.loterre.fr/ark:/67375/TSO-KGHBM8Z5-6>, <http://data.loterre.fr/ark:/67375/TSO-RB9SXH7C-R> .

<http://data.loterre.fr/ark:/67375/TSO-KXB7P34Z-4>
  a skos:Concept ;
  dc:modified "2021-06-10"^^xsd:date ;
  skos:definition "Outil qui rassemble les métadonnées provenant de plusieurs fournisseurs de données et les rend accessibles dans un entrepôt OAI. (Source : https://openaccess.inist.fr/glossaire/)"@fr ;
  skos:prefLabel "aggregator"@en, "agregador"@es, "agrégateur"@fr ;
  skos:inScheme <http://data.loterre.fr/ark:/67375/TSO> ;
  skos:broader <http://data.loterre.fr/ark:/67375/TSO-XS8KGCJ0-V> .

<http://data.loterre.fr/ark:/67375/TSO-N9ZH1LS9-X>
  a skos:Concept ;
  dc:modified "2021-06-11"^^xsd:date ;
  skos:altLabel "FAIRitude"@fr ;
  skos:definition "Degree of compliance of a repository or service with the FAIR principles"@en, "Degré de conformation d'un entrepôt ou d'un service aux principes FAIR"@fr ;
  skos:prefLabel "FAIRness"@en, "madurez FAIR"@es, "maturité FAIR"@fr ;
  skos:inScheme <http://data.loterre.fr/ark:/67375/TSO> ;
  skos:broader <http://data.loterre.fr/ark:/67375/TSO-T9Q25G6Q-S> ;
  skos:related <http://data.loterre.fr/ark:/67375/TSO-VTC90GGC-T> .

<http://data.loterre.fr/ark:/67375/TSO-WFN6D4TN-J>
  a skos:Concept ;
  dc:modified "2021-06-10"^^xsd:date ;
  skos:altLabel "Mutualisation d'Informations sur les Revues et leurs Accès dans les Bases En Ligne"@fr ;
  skos:definition "Portail de signalement des accès aux revues scientifiques électroniques en sciences humaines et sociales. (Source : Wikipédia)"@fr ;
  skos:prefLabel "Mir@bel"@en, "Mir@bel"@es, "Mir@bel"@fr ;
  skos:inScheme <http://data.loterre.fr/ark:/67375/TSO> ;
  skos:broader <http://data.loterre.fr/ark:/67375/TSO-JN2ZSNST-6> .

<http://data.loterre.fr/ark:/67375/TSO-LSLV4BQG-0>
  a skos:Concept ;
  dc:modified "2021-06-25"^^xsd:date ;
  skos:altLabel "OSF"@en ;
  skos:definition "A free and open source project management tool that supports researchers throughout their entire project lifecycle. (Source: https://www.cos.io/products/osf)"@en, "Outil de gestion de projet gratuit et libre proposé par le Center for Open Science."@fr ;
  skos:prefLabel "Open Science Framework"@en, "Open Science Framework"@es, "Open Science Framework"@fr ;
  skos:inScheme <http://data.loterre.fr/ark:/67375/TSO> ;
  skos:broader <http://data.loterre.fr/ark:/67375/TSO-V0HZ66HD-4> ;
  skos:related <http://data.loterre.fr/ark:/67375/TSO-BTFX00Q2-P> .

<http://data.loterre.fr/ark:/67375/TSO-SZC96ZN0-H>
  a skos:Concept ;
  dc:modified "2021-07-05"^^xsd:date ;
  skos:definition "Biblioteca digital científica que permite la consulta y el uso gratuitos de colecciones completas de publicaciones científicas de diferentes disciplinas: humanidades y ciencias sociales, pero también ciencias ambientales y de la tierra."@es, "Bibliothèque numérique scientifique qui permet la consultation et l'exploitation libres et gratuites de collections complètes de publications scientifiques relevant de différentes disciplines : sciences humaines et sociales mais aussi en sciences de l’environnement et en sciences de la terre. (Source : http://info.persee.fr/)"@fr ;
  skos:prefLabel "Persée"@en, "Persée"@es, "Persée"@fr ;
  skos:inScheme <http://data.loterre.fr/ark:/67375/TSO> ;
  skos:broader <http://data.loterre.fr/ark:/67375/TSO-CVMGJVKW-W> .

<http://data.loterre.fr/ark:/67375/TSO-WQMF6CT2-K>
  a skos:Concept ;
  dc:modified "2021-07-05"^^xsd:date ;
  skos:altLabel "OA browser extension"@en, "OA browser plugin"@en ;
  skos:definition "Application qui s’installe directement sur un navigateur web et qui permet de retrouver la version d'un article scientifique légalement disponible en libre accès."@fr, "Browser plugin that searches repositories or preprint servers for articles having an open access version."@en ;
  skos:prefLabel "extension de recherche d'article en libre accès"@fr, "open access browser plugin"@en, "plugin de navegador en acceso libre"@es ;
  skos:inScheme <http://data.loterre.fr/ark:/67375/TSO> ;
  skos:broader <http://data.loterre.fr/ark:/67375/TSO-XS8KGCJ0-V> ;
  skos:narrower <http://data.loterre.fr/ark:/67375/TSO-QZKZVCDR-P>, <http://data.loterre.fr/ark:/67375/TSO-N3CP621W-L>, <http://data.loterre.fr/ark:/67375/TSO-KD39PQLZ-P>, <http://data.loterre.fr/ark:/67375/TSO-PB3X8G4D-N>, <http://data.loterre.fr/ark:/67375/TSO-WKKLL52L-D>, <http://data.loterre.fr/ark:/67375/TSO-NDK3CG5V-9>, <http://data.loterre.fr/ark:/67375/TSO-XPMQPVQD-6> .

<http://data.loterre.fr/ark:/67375/TSO-KB9PPZQF-T>
  a skos:Concept ;
  dc:modified "2021-06-07"^^xsd:date ;
  skos:altLabel "LLD"@fr, "licence de libre diffusion"@fr, "public copyright license"@en ;
  skos:definition "A license by which a copyright holder as licensor can grant additional copyright permissions to any and all persons in the general public as licensees"@en, "Licence s'appliquant à une œuvre de l'esprit par laquelle l'auteur concède certains des droits que lui offre le droit d'auteur quant à l'utilisation, à la modification, à la rediffusion et à la réutilisation de l'œuvre dans des œuvres dérivées. (Source Wikipedia)"@fr ;
  skos:prefLabel "licence ouverte"@fr, "licencia abierta"@es, "public license"@en ;
  skos:inScheme <http://data.loterre.fr/ark:/67375/TSO> ;
  skos:broader <http://data.loterre.fr/ark:/67375/TSO-LJWH8NFT-D> ;
  skos:narrower <http://data.loterre.fr/ark:/67375/TSO-ZK0KHM67-X>, <http://data.loterre.fr/ark:/67375/TSO-F844JJK0-Q>, <http://data.loterre.fr/ark:/67375/TSO-XNNFBR4D-D>, <http://data.loterre.fr/ark:/67375/TSO-LXH6ZFD2-J> .

<http://data.loterre.fr/ark:/67375/TSO-LBM5XNCF-J>
  a skos:Concept ;
  dc:modified "2021-06-28"^^xsd:date ;
  skos:definition "Appel lancé en 2015 par la Ligue des Bibliothèques Européennes de Recherche (LIBER), pour lever les contraintes de propriété intellectuelle et ouvrir les pratiques d’extraction des connaissances et de fouille de texte."@fr ;
  skos:prefLabel "Declaración de La Haya sobre la extracción de conocimiento útil en la era digital"@es, "Déclaration de La Haye sur l'extraction des connaissances à l'ère du numérique"@fr, "The Hague Declaration on Knowledge Discovery in the Digital Age"@en ;
  skos:inScheme <http://data.loterre.fr/ark:/67375/TSO> ;
  skos:broader <http://data.loterre.fr/ark:/67375/TSO-V6F4ZS65-G> .

<http://data.loterre.fr/ark:/67375/TSO-QLJ4LTKK-K>
  a skos:Concept ;
  dc:modified "2021-06-24"^^xsd:date ;
  skos:definition "A licence clause that allows the reuse, sharing, and remixing of materials providing the original author is appropriately attributed. Aside from attribution the CC-BY licence has no other restrictions on copying. Compatible with free cultural works. (Source : http://www.righttoresearch.org/resources/OpenResearchGlossary)"@en, "Licence qui permet à d'autres de distribuer, de remixer, d'adapter et d'utiliser un travail, même à des fins commerciales, à condition d'attribuer la création originale à son auteur. (Source : https://creativecommons.org/licenses/?lang=fr-FR)"@fr ;
  skos:prefLabel "CC-BY license"@en, "licence CC-BY"@fr, "licencia CC-BY"@es ;
  skos:inScheme <http://data.loterre.fr/ark:/67375/TSO> ;
  skos:broader <http://data.loterre.fr/ark:/67375/TSO-WH5JC3TT-G>, <http://data.loterre.fr/ark:/67375/TSO-WZ0J1023-D> .

<http://data.loterre.fr/ark:/67375/TSO-PH7T4MNT-J>
  a skos:Concept ;
  dc:modified "2021-06-22"^^xsd:date ;
  skos:altLabel "ODbL 1.0"@en, "Open Data Commons Open Database Licence 1.0"@en ;
  skos:definition "Contrat de licence ayant pour objet d’autoriser les utilisateurs à partager, modifier et utiliser librement la présente Base de données initiale tout en maintenant ces mêmes libertés pour les autres. (Source : http://vvlibri.org/fr/licence/odbl-10/legalcode/unofficial)"@fr ;
  skos:prefLabel "Licencia Abierta de Bases de Datos"@es, "Open Database License 1.0"@en, "licence ODbL"@fr ;
  skos:inScheme <http://data.loterre.fr/ark:/67375/TSO> ;
  skos:broader <http://data.loterre.fr/ark:/67375/TSO-WZ0J1023-D> .

<http://data.loterre.fr/ark:/67375/TSO-LJWH8NFT-D>
  a skos:Concept ;
  dc:modified "2021-06-24"^^xsd:date ;
  skos:altLabel "licence"@en ;
  skos:definition "Autorisation accordée à un tiers d'exploiter une production, sous certaines conditions."@fr ;
  skos:prefLabel "licence"@fr, "licencia"@es, "license"@en ;
  skos:inScheme <http://data.loterre.fr/ark:/67375/TSO> ;
  skos:broader <http://data.loterre.fr/ark:/67375/TSO-ZQ0Q8HMP-Q> ;
  skos:narrower <http://data.loterre.fr/ark:/67375/TSO-W04D2X5B-N>, <http://data.loterre.fr/ark:/67375/TSO-WZ0J1023-D>, <http://data.loterre.fr/ark:/67375/TSO-DSVQC015-X>, <http://data.loterre.fr/ark:/67375/TSO-WH5JC3TT-G>, <http://data.loterre.fr/ark:/67375/TSO-KB9PPZQF-T> .

<http://data.loterre.fr/ark:/67375/TSO-SJ45BLDH-0>
  a skos:Concept ;
  dc:modified "2021-06-29"^^xsd:date ;
  skos:altLabel "persistent URL"@en ;
  skos:definition "Identifiant pérenne développé par OCLC en 1995 URL persistant qui pointe vers un résolveur. Suite à une requête, le résolveur envoie une page contenant l’en-tête de redirection 302 et l’URL cible. (Source : https://archivengines.wordpress.com/2012/08/24/systeme-purl/)"@fr, "Persistant identifier developed by OCLC, that is directly actionable and binds only one single URL with the identifier."@en ;
  skos:prefLabel "PURL"@en, "PURL"@es, "PURL"@fr ;
  skos:inScheme <http://data.loterre.fr/ark:/67375/TSO> ;
  skos:broader <http://data.loterre.fr/ark:/67375/TSO-H5ZG6DX6-4> .

<http://data.loterre.fr/ark:/67375/TSO-QP6T79V4-5>
  a skos:Concept ;
  dc:modified "2021-06-25"^^xsd:date ;
  skos:altLabel "active DMP"@en, "maDMP"@en, "maDMP"@fr, "machine-readable DMP"@en, "plan de gestion de données actionnables par machine"@fr ;
  skos:definition "A concept that aims to make the DMP interoperable, automated and increasingly standardised. (Source: https://doi.org/10.1007/978-3-030-45442-5_15)"@en, "Plan de gestion de données lisible et exploitable par les machines, pour permettre l’exploitation optimale de son contenu."@fr ;
  skos:prefLabel "machine-actionable data management plan"@en, "plan de gestion des données automatisé"@fr, "plan de gestión de datos automatizado"@es ;
  skos:inScheme <http://data.loterre.fr/ark:/67375/TSO> ;
  skos:broader <http://data.loterre.fr/ark:/67375/TSO-MJZBK64J-5> .

<http://data.loterre.fr/ark:/67375/TSO-QC8N3MRN-X>
  a skos:Concept ;
  dc:modified "2021-06-30"^^xsd:date ;
  skos:definition "A bottom-up, stakeholder-driven and self-governed initiative that aims to implement the FAIR data principles, making data Findable, Accessible, Interoperable and Reusable (FAIR). It offers an open and inclusive ecosystem for individuals, institutions and organisations working together through Implementation Networks (INs). (Source: https://www.go-fair.org/go-fair-initiative/)"@en, "Initiative des Pays-Bas, de l’Allemagne et de la France qui propose le développement d'un environnement international de recherche enrichi par les données et soutient l'ouverture progressive des données de la recherche existant au sein des institutions scientifiques et académiques dans tous les domaines de la recherche et au-delà des frontières nationales. (Source : https://www.enseignementsup-recherche.gouv.fr/cid124728/science-ouverte-la-france-rejoint-go-fair-en-tant-que-co-fondatrice.html)"@fr ;
  skos:prefLabel "GO FAIR"@en, "GO FAIR"@es, "GO FAIR"@fr ;
  skos:inScheme <http://data.loterre.fr/ark:/67375/TSO> ;
  skos:broader <http://data.loterre.fr/ark:/67375/TSO-V0HZ66HD-4> .

<http://data.loterre.fr/ark:/67375/TSO-MJRKBMDW-Q>
  a skos:Concept ;
  dc:modified "2021-06-25"^^xsd:date ;
  skos:prefLabel "data type"@en, "tipo de dato"@es, "type de donnée"@fr ;
  skos:inScheme <http://data.loterre.fr/ark:/67375/TSO> ;
  skos:narrower <http://data.loterre.fr/ark:/67375/TSO-BRLNRV51-S>, <http://data.loterre.fr/ark:/67375/TSO-V08MCZVP-H>, <http://data.loterre.fr/ark:/67375/TSO-VF5K6BGT-F>, <http://data.loterre.fr/ark:/67375/TSO-ZQ5PMX6N-7>, <http://data.loterre.fr/ark:/67375/TSO-DP8MN2RF-P>, <http://data.loterre.fr/ark:/67375/TSO-D80R1KX4-5>, <http://data.loterre.fr/ark:/67375/TSO-MGRQT12J-W> ;
  skos:topConceptOf <http://data.loterre.fr/ark:/67375/TSO> .

<http://data.loterre.fr/ark:/67375/TSO-F2VJ1STQ-Z>
  a skos:Concept ;
  skos:definition "(Source: http://dx.doi.org/10.2139/ssrn.2272036)"@en, "Schématisation des motivations plaidant en faveur de l'ouverture de la science, regroupées en cinq familles, proposée par Sönke Bartling et Sascha Friesike en 2013. (Source: http://dx.doi.org/10.2139/ssrn.2272036)"@fr ;
  skos:prefLabel "escuela del pensamiento de la ciencia abierta"@es, "open science school of thought"@en, "école de pensée de la science ouverte"@fr ;
  skos:inScheme <http://data.loterre.fr/ark:/67375/TSO> ;
  skos:narrower <http://data.loterre.fr/ark:/67375/TSO-JFR1FLWQ-R>, <http://data.loterre.fr/ark:/67375/TSO-KFCWMBBV-K>, <http://data.loterre.fr/ark:/67375/TSO-D8FHMPQB-D>, <http://data.loterre.fr/ark:/67375/TSO-H9882CCM-4>, <http://data.loterre.fr/ark:/67375/TSO-Z0XXXG08-3> ;
  skos:topConceptOf <http://data.loterre.fr/ark:/67375/TSO> .

<http://data.loterre.fr/ark:/67375/TSO-KHFX8870-5>
  a skos:Concept ;
  dc:modified "2021-06-24"^^xsd:date ;
  skos:altLabel "accesibilidad"@es, "accessibility"@en, "accessibilité"@fr ;
  skos:definition "Principe [FAIR qui] encourage à stocker durablement les données et les métadonnées et à faciliter leur accès et/ou leur téléchargement, en spécifiant les conditions d’accès (accès ouvert ou restreint) et d’utilisation (licence). Une manière concrète de répondre à ce principe consiste à déposer les données dans un entrepôt qui assure leur stockage sur le long terme et les rend accessibles via un protocole ouvert (HTTP par exemple), aussi bien aux humains qu’aux machines. (Source : Esther Dzalé Yeumo, Les principes FAIR)"@fr ;
  skos:prefLabel "accesible"@es, "accessible"@en, "accessible"@fr ;
  skos:inScheme <http://data.loterre.fr/ark:/67375/TSO> ;
  skos:broader <http://data.loterre.fr/ark:/67375/TSO-D9HJPTL6-X> ;
  skos:related <http://data.loterre.fr/ark:/67375/TSO-GZ4Q18P7-8> .

<http://data.loterre.fr/ark:/67375/TSO-KG87BTKZ-L>
  a skos:Concept ;
  dc:modified "2021-06-25"^^xsd:date ;
  skos:altLabel "bronze open access"@en, "libre accès bronze"@fr ;
  skos:definition "A model in which articles are made freely available on a journal’s website. However, the journal could remove the free access to these articles at any moment. Additionally, there is no indication of how users are able to reuse the articles. (Source : https://www.lib.sfu.ca)"@en, "Version dégradée du libre accès doré, dans laquelle un article est disponible sans qu’il ne soit associé clairement à une licence de diffusion."@fr ;
  skos:prefLabel "bronze route"@en, "ruta bronce"@es, "voie de bronze"@fr ;
  skos:inScheme <http://data.loterre.fr/ark:/67375/TSO> ;
  skos:broader <http://data.loterre.fr/ark:/67375/TSO-KHL25V0F-4> .

<http://data.loterre.fr/ark:/67375/TSO-XPMQPVQD-6>
  a skos:Concept ;
  dc:modified "2021-06-02"^^xsd:date ;
  skos:altLabel "C&R"@fr ;
  skos:definition "Extension réalisée par le CNRS qui analyse l’ensemble des pages Internet visitées à la recherche d’identifiants documentaires (DOI, PMID…) et ajoute un lien si la ressource est disponible via Unpaywall, BibCnrs, Istex ou Panist."@fr ;
  skos:prefLabel "click & read"@en, "click & read"@es, "click & read"@fr ;
  skos:inScheme <http://data.loterre.fr/ark:/67375/TSO> ;
  skos:broader <http://data.loterre.fr/ark:/67375/TSO-WQMF6CT2-K> .

<http://data.loterre.fr/ark:/67375/TSO-K8VWLS9S-L>
  a skos:Concept ;
  dc:modified "2021-06-29"^^xsd:date ;
  skos:altLabel "partage de code source"@fr, "source code sharing"@en ;
  skos:definition "Open sharing of computational code"@en, "Partage ouvert de code informatique"@fr ;
  skos:prefLabel "code sharing"@en, "intercambio de código"@es, "partage de code"@fr ;
  skos:inScheme <http://data.loterre.fr/ark:/67375/TSO> ;
  skos:broader <http://data.loterre.fr/ark:/67375/TSO-QWKTFN2F-N> .

<http://data.loterre.fr/ark:/67375/TSO-QK42D772-3>
  a skos:Concept ;
  dc:created "2021-06-10"^^xsd:date ;
  dc:modified "2021-06-30"^^xsd:date ;
  skos:prefLabel "evaluation infrastructure"@en, "infraestructura para la evaluación"@es, "infrastructure d'évaluation"@fr ;
  skos:inScheme <http://data.loterre.fr/ark:/67375/TSO> ;
  skos:broader <http://data.loterre.fr/ark:/67375/TSO-V0HZ66HD-4> ;
  skos:narrower <http://data.loterre.fr/ark:/67375/TSO-X239JT56-0>, <http://data.loterre.fr/ark:/67375/TSO-MDD3CCP5-9>, <http://data.loterre.fr/ark:/67375/TSO-W1F4MWNS-F>, <http://data.loterre.fr/ark:/67375/TSO-WC4S5Z1Q-Z>, <http://data.loterre.fr/ark:/67375/TSO-L6TF72DL-D>, <http://data.loterre.fr/ark:/67375/TSO-WWM82SKD-Z>, <http://data.loterre.fr/ark:/67375/TSO-NKGK3HW9-N> .

<http://data.loterre.fr/ark:/67375/TSO-C4J2BDKS-X>
  a skos:Concept ;
  dc:modified "2021-07-05"^^xsd:date ;
  skos:altLabel "Library Genesis"@en ;
  skos:definition "A file-sharing based website for scholarly journal articles, academic and general-interest books, images, comics, and magazines. The site enables free access to content that is otherwise paywalled or not digitized elsewhere. Some publishers took LibGen to court, accusing the site of providing pirate access to articles and books. (Source : Wikipedia)"@en, "Moteur de recherche d'articles et de livres scientifiques qui facilite l'accès aux contenus soumis à un péage. Certains éditeurs ont entamé des poursuites judiciaires contre LibGen, l'accusant de pirater les accès aux articles et aux ouvrages."@fr, "Un motor de búsqueda de artículos y libros académicos que facilita el acceso a contenidos de pago. Algunas editoriales han emprendido acciones legales contra LibGen, acusándola de piratear el acceso a artículos y libros."@es ;
  skos:prefLabel "LibGen"@en, "LibGen"@es, "LibGen"@fr ;
  skos:inScheme <http://data.loterre.fr/ark:/67375/TSO> ;
  skos:broader <http://data.loterre.fr/ark:/67375/TSO-CVMGJVKW-W> ;
  skos:related <http://data.loterre.fr/ark:/67375/TSO-WT63ZDZ1-T> .

<http://data.loterre.fr/ark:/67375/TSO-WC4S5Z1Q-Z>
  a skos:Concept ;
  dc:modified "2021-07-05"^^xsd:date ;
  skos:definition "A website that allows users to discuss and review scientific research after publication, i.e. post-publication peer review. The site has served as a whistleblowing platform, in that it highlighted shortcomings in several high-profile papers, in some cases leading to retractions and to accusations of scientific fraud. Contrary to most platforms, it allows anonymous post-publication commenting, a controversial feature which is the main factor for its success. Consequently, accusations of libel have been levelled at some of PubPeer's users; correspondingly the website now requires commentators to use only facts that can be publicly verified. (Source : Wikipedia)"@en, "Site internet qui permet aux utilisateurs (principalement anonymes) d'émettre des commentaires sur des articles scientifiques en post-publication, mais aussi de signaler des soupçons de manquements à l'éthique scientifique. Certains chercheurs ont dénoncé en PubPeer un système de délation, des accusations de diffamation ont été adressées à certains des contributeurs de PubPeer. Le président-directeur général du CNRS a affirmé son opposition à l'utilisation de cette plateforme lorsqu'il dévoile le 13 novembre 2018 le « plan d’action [du CNRS] sur l’intégrité et la déontologie scientifiques », enjoignant aux chercheurs de ne pas correspondre sur ce site. (Source : Wikipédia)"@fr, "Sitio web que permite a los usuarios (principalmente anónimos) comentar artículos científicos en la fase posterior a su publicación, pero también denunciar presuntas infracciones de la ética científica. Algunos investigadores han denunciado que PubPeer es un sistema de denuncia, y se han formulado acusaciones de difamación contra algunos de los colaboradores de PubPeer. El presidente y director general del CNRS afirmó su oposición al uso de esta plataforma cuando dio a conocer el \"plan de acción [del CNRS] sobre la integridad y la ética científica\" el 13 de noviembre de 2018, instruyendo a los investigadores a no mantener correspondencia en este sitio."@es ;
  skos:prefLabel "PubPeer"@en, "PubPeer"@es, "PubPeer"@fr ;
  skos:inScheme <http://data.loterre.fr/ark:/67375/TSO> ;
  skos:broader <http://data.loterre.fr/ark:/67375/TSO-QK42D772-3> .

<http://data.loterre.fr/ark:/67375/TSO-KD25R88J-S>
  a skos:Concept ;
  dc:modified "2021-07-05"^^xsd:date ;
  skos:definition "Service fournissant un accès libre à des articles scientifiques obtenus par extraction automatique de contenu en contournant les péages classiques des éditeurs académiques. Il a été attaqué en justice par des maisons d'édition scientifique, pour atteinte au droit d'auteur. En novembre 2015, l'adresse originale, sci-hub.org, est fermée. Des domaines alternatifs sont alors mis en place. Le tribunal de grande instance de Paris ordonne le 7 mars 2019 à trois fournisseurs d'accès à internet de bloquer l'accès à Sci-Hub. (Source : Wikipédia)"@fr, "Servicio que proporciona acceso gratuito a artículos científicos obtenidos mediante la extracción automática de contenidos, evitando los peajes tradicionales de las editoriales académicas. Ha sido demandado por editoriales científicas por infracción de derechos de autor. En noviembre de 2015, la dirección original, sci-hub.org, se cerró. A continuación, se establecieron dominios alternativos. El 7 de marzo de 2019, el tribunal superior de París ordenó a tres proveedores de servicios de Internet que bloquearan el acceso a Sci-Hub."@es, "Web platform that provides free access to millions of research papers and books, without regard to copyright, by bypassing publishers' paywalls in various ways. Some publishers took Sci-Hub to court, accusing the site of providing pirate access to articles and books."@en ;
  skos:prefLabel "Sci-Hub"@en, "Sci-Hub"@es, "Sci-Hub"@fr ;
  skos:inScheme <http://data.loterre.fr/ark:/67375/TSO> ;
  skos:broader <http://data.loterre.fr/ark:/67375/TSO-CVMGJVKW-W> ;
  skos:related <http://data.loterre.fr/ark:/67375/TSO-WT63ZDZ1-T> .

<http://data.loterre.fr/ark:/67375/TSO-GZ4Q18P7-8>
  a skos:Concept ;
  dc:modified "2021-06-03"^^xsd:date ;
  skos:prefLabel "acceso a los datos"@es, "accès aux données"@fr, "data access"@en ;
  skos:inScheme <http://data.loterre.fr/ark:/67375/TSO> ;
  skos:broader <http://data.loterre.fr/ark:/67375/TSO-SMGMJFLJ-Q> ;
  skos:related <http://data.loterre.fr/ark:/67375/TSO-KHFX8870-5> .

<http://data.loterre.fr/ark:/67375/TSO-VNNFL8WB-H>
  a skos:Concept ;
  dc:modified "2021-06-17"^^xsd:date ;
  skos:altLabel "data anonymization"@en, "désidentification des données"@fr ;
  skos:definition "Traitement des données qui permet de publier des informations exemptes de données personnelles."@fr ;
  skos:prefLabel "anonimización de datos"@es, "anonymisation des données"@fr, "data anonymisation"@en ;
  skos:inScheme <http://data.loterre.fr/ark:/67375/TSO> ;
  skos:broader <http://data.loterre.fr/ark:/67375/TSO-MJLHMDNM-S> ;
  skos:related <http://data.loterre.fr/ark:/67375/TSO-RH261KDT-S> .

<http://data.loterre.fr/ark:/67375/TSO-GQVTBXJ4-X>
  a skos:Concept ;
  dc:modified "2021-06-17"^^xsd:date ;
  skos:definition "The process of managing the availability, usability, integrity and security of the data in a system, based on internal data standards and policies that also control data usage. (Source : https://searchdatamanagement.techtarget.com)"@en ;
  skos:prefLabel "data governance"@en, "gobernanza de datos"@es, "gouvernance des données"@fr ;
  skos:inScheme <http://data.loterre.fr/ark:/67375/TSO> ;
  skos:broader <http://data.loterre.fr/ark:/67375/TSO-NJ1CVNL6-F> ;
  skos:related <http://data.loterre.fr/ark:/67375/TSO-H0BSK47H-Z> .

<http://data.loterre.fr/ark:/67375/TSO-FJ7V5LJC-R>
  a skos:Concept ;
  dc:modified "2021-06-29"^^xsd:date ;
  skos:definition "Action qui consiste à spécifier un plan de recherche avant une étude et à le déposer dans un registre. Le pré-enregistrement sépare la recherche génératrice d'hypothèses (exploratoire) de la recherche de vérification d'hypothèses (confirmatoire)."@fr, "The act of specifying a research plan in advance of a study and submitting it to a registry. Preregistration separates hypothesis-generating (exploratory) from hypothesis-testing (confirmatory) research. (Source : https://www.cos.io/initiatives/prereg)"@en ;
  skos:prefLabel "preregistration"@en, "prerregistro"@es, "préenregistrement"@fr ;
  skos:inScheme <http://data.loterre.fr/ark:/67375/TSO> ;
  skos:broader <http://data.loterre.fr/ark:/67375/TSO-NJ1CVNL6-F> .

<http://data.loterre.fr/ark:/67375/TSO-XK0JJTS6-2>
  a skos:Concept ;
  dc:modified "2021-06-03"^^xsd:date ;
  skos:prefLabel "data reuse"@en, "reutilización de los datos"@es, "réutilisation des données"@fr ;
  skos:inScheme <http://data.loterre.fr/ark:/67375/TSO> ;
  skos:broader <http://data.loterre.fr/ark:/67375/TSO-SMGMJFLJ-Q> ;
  skos:related <http://data.loterre.fr/ark:/67375/TSO-D80R1KX4-5>, <http://data.loterre.fr/ark:/67375/TSO-X4ZW5XQD-G> ;
  skos:narrower <http://data.loterre.fr/ark:/67375/TSO-BSS8DN99-W>, <http://data.loterre.fr/ark:/67375/TSO-WBDZJK00-P>, <http://data.loterre.fr/ark:/67375/TSO-JWXHV1CM-9> .

<http://data.loterre.fr/ark:/67375/TSO-QWKTFN2F-N>
  a skos:Concept ;
  dc:modified "2021-06-03"^^xsd:date ;
  skos:prefLabel "data sharing"@en, "intercambio de datos"@es, "partage des données"@fr ;
  skos:inScheme <http://data.loterre.fr/ark:/67375/TSO> ;
  skos:broader <http://data.loterre.fr/ark:/67375/TSO-SMGMJFLJ-Q> ;
  skos:related <http://data.loterre.fr/ark:/67375/TSO-D9HJPTL6-X> ;
  skos:narrower <http://data.loterre.fr/ark:/67375/TSO-ZMJ8VVB2-9>, <http://data.loterre.fr/ark:/67375/TSO-K8VWLS9S-L> .

<http://data.loterre.fr/ark:/67375/TSO-QL8P69BW-V>
  a skos:Concept ;
  dc:modified "2021-06-24"^^xsd:date ;
  skos:definition "In the context of Open Access, double-dipping occurs when a journal has an article processing charge (APC) for publishing an author’s work, as well as requiring payment (usually through a subscription fee) by the potential user of the work. This model makes the institution or author pay twice to access the work. (Source : http://openaccess.ox.ac.uk/glossary/)"@en, "Modèle selon lequel une revue perçoit des frais de traitement des articles (APC) pour publier le travail d'un auteur et exige également un paiement (généralement sous forme d'abonnement) de la part de l'utilisateur potentiel du travail. Ce modèle fait que l'institution ou l'auteur paie deux fois pour accéder à l'œuvre."@fr ;
  skos:prefLabel "doble pago"@es, "double paiement"@fr, "double-dipping"@en ;
  skos:inScheme <http://data.loterre.fr/ark:/67375/TSO> ;
  skos:broader <http://data.loterre.fr/ark:/67375/TSO-MWXTBMQ8-9> ;
  skos:related <http://data.loterre.fr/ark:/67375/TSO-RN1XP625-F> .

<http://data.loterre.fr/ark:/67375/TSO-JDVCT02T-P>
  a skos:Concept ;
  dc:modified "2021-06-24"^^xsd:date ;
  skos:altLabel "findability"@en, "repérabilité"@fr, "trouvabilité"@fr ;
  skos:definition "Principe [qui] a pour objectif de faciliter la découverte des données par les humains et les systèmes informatiques et requiert une description et une indexation des données et des métadonnées. (Source : Esther Dzalé Yeumo, Les principes FAIR)"@fr ;
  skos:prefLabel "encontrable"@es, "facile à trouver"@fr, "findable"@en ;
  skos:inScheme <http://data.loterre.fr/ark:/67375/TSO> ;
  skos:broader <http://data.loterre.fr/ark:/67375/TSO-D9HJPTL6-X> ;
  skos:related <http://data.loterre.fr/ark:/67375/TSO-VDVFXBCR-C> .

<http://data.loterre.fr/ark:/67375/TSO-T0GXV6XC-Z>
  a skos:Concept ;
  dc:modified "2021-07-05"^^xsd:date ;
  skos:altLabel "grey open access"@en, "libre accès gris"@fr ;
  skos:definition "A model in which authors upload their work on academic social networks (ie. ResearchGate, Academia.edu) or personal/departmental webpages. This can be problematic because the author might be infringing on their publishers’ license agreement. (Source : https://www.lib.sfu.ca)"@en, "Un modelo en el que los autores suben sus trabajos a las redes sociales académicas (por ejemplo, ResearchGate, Academia.edu) o a las páginas web personales o del laboratorio."@es, "Un modèle dans lequel les auteurs téléchargent leurs travaux sur des réseaux sociaux universitaires (par exemple ResearchGate, Academia.edu) ou sur des pages web personnelles ou de leur laboratoire."@fr ;
  skos:prefLabel "grey route"@en, "ruta gris"@es, "voie grise"@fr ;
  skos:inScheme <http://data.loterre.fr/ark:/67375/TSO> ;
  skos:broader <http://data.loterre.fr/ark:/67375/TSO-KHL25V0F-4> .

<http://data.loterre.fr/ark:/67375/TSO-PM46WP7W-P>
  a skos:Concept ;
  dc:modified "2021-06-24"^^xsd:date ;
  skos:definition "A bibliographic database dedicated to Economics and available freely on the Internet, it uses the RePEc database. (Source : https://ideas.repec.org/)"@en, "Base de données bibliographiques dédiée au domaine de l'économie et librement accessible en ligne."@fr ;
  skos:prefLabel "IDEAS"@en, "IDEAS"@es, "IDEAS"@fr ;
  skos:inScheme <http://data.loterre.fr/ark:/67375/TSO> ;
  skos:broader <http://data.loterre.fr/ark:/67375/TSO-V0HZ66HD-4> ;
  skos:related <http://data.loterre.fr/ark:/67375/TSO-HXX9G512-G> .

<http://data.loterre.fr/ark:/67375/TSO-C676TDJV-H>
  a skos:Concept ;
  dc:modified "2021-06-24"^^xsd:date ;
  skos:altLabel "interoperabilidad"@es, "interoperabilidad semántica"@es, "interoperability"@en, "interopérabilité"@fr, "interopérabilité sémantique"@fr, "semantic interoperability"@en ;
  skos:definition "[Principe FAIR qui] peut se décomposer en : téléchargeable, utilisable, intelligible, et combinable avec d'autres données, par des humains et des machines. Une implémentation courante de ce principe consiste à utiliser les technologies du Web sémantique (RDF, OWL, SKOS) pour représenter et lier les données et les métadonnées. (Source : Esther Dzalé Yeumo, Les principes FAIR)"@fr ;
  skos:prefLabel "interoperable"@en, "interoperable"@es, "intéropérable"@fr ;
  skos:inScheme <http://data.loterre.fr/ark:/67375/TSO> ;
  skos:broader <http://data.loterre.fr/ark:/67375/TSO-D9HJPTL6-X> ;
  skos:related <http://data.loterre.fr/ark:/67375/TSO-BRLNRV51-S>, <http://data.loterre.fr/ark:/67375/TSO-WBDZJK00-P> .

<http://data.loterre.fr/ark:/67375/TSO-QMSRJLT3-C>
  a skos:Concept ;
  skos:altLabel "efecto red"@es, "externalidad de red"@es ;
  skos:definition "Phenomenon in which the value of participating in an activity increases with the number of participants. The consequence is that members of a group are disadvantaged when deviating from existing norms. For example, a researcher choosing to publish in an open access journal rather than a more ‘prestigious’ subscription journal, could result in reviewers of the author’s future funding applications taking a less favourable view of their work. (source: Knowledge Exchange)"@en, "Phénomène dans lequel le prestige lié à la participation à une activité augmente avec le nombre de participants. La conséquence est que les membres d'un groupe sont désavantagés lorsqu'ils s'écartent des normes existantes. Par exemple, un chercheur choisissant de publier dans une revue en libre accès plutôt que dans une revue plus \"prestigieuse\" sur abonnement, pourrait amener les évaluateurs des futures demandes de financement de l'auteur à porter un jugement moins favorable sur son travail. (source: Knowledge Exchange)"@fr ;
  skos:prefLabel "efecto de red"@es, "effet de réseau"@fr, "network effect"@en ;
  skos:inScheme <http://data.loterre.fr/ark:/67375/TSO> ;
  skos:broader <http://data.loterre.fr/ark:/67375/TSO-PSFFQLXV-2> .

<http://data.loterre.fr/ark:/67375/TSO-ZSC3265D-Z>
  a skos:Concept ;
  dc:modified "2021-06-10"^^xsd:date ;
  skos:altLabel "Open badge ecosystem for the recognition of skills in research data management and sharing"@en ;
  skos:definition "Projet Erasmus+ de 3 ans (09/2019-08/2022) ayant pour vocation de concevoir un écosystème pour reconnaître des compétences liées à la gestion et au partage des données de la recherche. La reconnaissance des compétences se fera au travers d’open badges. (Source : https://urfist.univ-cotedazur.fr)"@fr ;
  skos:prefLabel "Oberred"@en, "Oberred"@es, "Oberred"@fr ;
  skos:inScheme <http://data.loterre.fr/ark:/67375/TSO> ;
  skos:broader <http://data.loterre.fr/ark:/67375/TSO-H93WKMMJ-B> ;
  skos:related <http://data.loterre.fr/ark:/67375/TSO-DP8MN2RF-P> .

<http://data.loterre.fr/ark:/67375/TSO-FC2GVFL9-R>
  a skos:Concept ;
  skos:definition "Evénement annuel qui se tient la dernière semaine d'octobre partout en France et vise à promouvoir le libre accès au cours de diverses manifestations (journées d'étude, conférences, dépôt-parties, etc.) (source: https://science-ouverte.parisnanterre.fr/)"@fr ;
  skos:prefLabel "Open Access Week"@en, "Open Access Week"@es, "Open Access Week"@fr ;
  skos:inScheme <http://data.loterre.fr/ark:/67375/TSO> ;
  skos:broader <http://data.loterre.fr/ark:/67375/TSO-KG7FR9LH-R> .

<http://data.loterre.fr/ark:/67375/TSO-QF2RDTPG-H>
  a skos:Concept ;
  dc:modified "2021-06-29"^^xsd:date ;
  skos:altLabel "credencial digital de código abierto"@es, "open badge"@fr ;
  skos:definition "Dispositif numérique qui se présente sous forme d’icône et qui est utilisé pour confirmer l'acquisition d’aptitudes, de connaissances ou de compétences. (Source : https://fr.wikipedia.org/wiki/Badge_num%C3%A9rique)"@fr ;
  skos:prefLabel "badge ouvert"@fr, "insignia abierta"@es, "open badge"@en ;
  skos:inScheme <http://data.loterre.fr/ark:/67375/TSO> ;
  skos:broader <http://data.loterre.fr/ark:/67375/TSO-X3TNSQ40-M> ;
  skos:related <http://data.loterre.fr/ark:/67375/TSO-MV5H4HGJ-2> ;
  skos:narrower <http://data.loterre.fr/ark:/67375/TSO-G3F0KPMJ-P> .

<http://data.loterre.fr/ark:/67375/TSO-WT63ZDZ1-T>
  a skos:Concept ;
  dc:modified "2021-06-25"^^xsd:date ;
  skos:definition "Bibliothèque numérique donnant librement accès à un contenu normalement masqué ou difficilement accessible, protégé par des frais d'abonnement ou des droits d'auteur. La plupart des bibliothèques de l'ombre sont illégales car elles violent les droits d'auteur."@fr, "Online databases of readily available content that is normally obscured or otherwise not readily accessible. Such databases may be inaccessible for a number of reasons, including the use of paywalls, copyright controls, or other barriers to accessibility placed upon the content by its original owners. Most shadow libraries are illegal as ubiquitously examples of large-scale copyright infringement. (Source : Wikipedia)"@en ;
  skos:prefLabel "biblioteca en la sombra"@es, "bibliothèque de l'ombre"@fr, "shadow library"@en ;
  skos:inScheme <http://data.loterre.fr/ark:/67375/TSO> ;
  skos:broader <http://data.loterre.fr/ark:/67375/TSO-PSFFQLXV-2> ;
  skos:related <http://data.loterre.fr/ark:/67375/TSO-C4J2BDKS-X>, <http://data.loterre.fr/ark:/67375/TSO-KD25R88J-S> .

<http://data.loterre.fr/ark:/67375/TSO-Z0X2RFQK-4>
  a skos:Concept ;
  dc:modified "2021-06-25"^^xsd:date ;
  skos:altLabel "Directory of Open Access Repositories"@en, "Directory of Open Access Repositories"@es, "Directory of Open Access Repositories"@fr ;
  skos:definition "A quality-assured, global Directory of Open Access Repositories launched in 2005 as the product of a collaborative project between the University of Nottingham and Lund University, funded by OSI, Jisc, SPARC Europe and CURL. (Source : https://v2.sherpa.ac.uk/opendoar/about.html)"@en, "Répertoire mondial de dépôts en libre accès lancé en 2005 en collaboration entre l'Université de Nottingham et l'Université de Lund, et financé par l'OSI, Jisc, SPARC Europe et CURL."@fr ;
  skos:prefLabel "OpenDOAR"@en, "OpenDOAR"@es, "OpenDOAR"@fr ;
  skos:inScheme <http://data.loterre.fr/ark:/67375/TSO> ;
  skos:broader <http://data.loterre.fr/ark:/67375/TSO-WQ9RZCBH-P> ;
  skos:related <http://data.loterre.fr/ark:/67375/TSO-W9KRS5Q3-6> .

<http://data.loterre.fr/ark:/67375/TSO-L6TF72DL-D>
  a skos:Concept ;
  dc:modified "2021-07-05"^^xsd:date ;
  skos:altLabel "Quality Open Access Market"@en, "Quality Open Access Market"@es, "Quality Open Access Market"@fr ;
  skos:definition "A market place for scientific and scholarly journals which publish articles in open access. In QOAM, academic authors score the experience they have had with the journal’s peer review and editorial board from 1 to 5 via a concise journal score card. The QoS indicator of a journal is then defined as the product of the average score of the journal and the ‘robustness’ of this score. (Source: https://www.qoam.eu/about)"@en, "Plataforma para la evaluación cualitativa de las revistas científicas, directamente por la comunidad científica: se calcula una tarjeta de puntuación de la revista según las opiniones expresadas."@es, "Plateforme permettant l'évaluation qualitative des revues scientifiques, faite directement par la communauté scientifique : un Journal Score Card est calculé en fonction des avis émis. (Source : https://scienceouverte.couperin.org/)"@fr ;
  skos:prefLabel "QOAM"@en, "QOAM"@es, "QOAM"@fr ;
  skos:inScheme <http://data.loterre.fr/ark:/67375/TSO> ;
  skos:broader <http://data.loterre.fr/ark:/67375/TSO-QK42D772-3> .

<http://data.loterre.fr/ark:/67375/TSO-R3K91KN9-H>
  a skos:Concept ;
  skos:altLabel "OKF"@en ;
  skos:definition "A global, non-profit network that promotes and shares information at no charge, including both content and data. (Source : Wikipedia)"@en, "Association à but non lucratif de droit britannique promouvant la culture libre, en particulier les contenus libres et l'open data. (Source : Wikipédia)"@fr ;
  skos:prefLabel "Open Knowledge Foundation"@en, "Open Knowledge Foundation"@es, "Open Knowledge Foundation"@fr ;
  skos:inScheme <http://data.loterre.fr/ark:/67375/TSO> ;
  skos:broader <http://data.loterre.fr/ark:/67375/TSO-J64S3QDL-1> .

<http://data.loterre.fr/ark:/67375/TSO-G3F0KPMJ-P>
  a skos:Concept ;
  dc:modified "2021-06-03"^^xsd:date ;
  skos:definition "Incentive developed by the Center for Open Science for authors who share data or materials and who preregister studies and/or analysis plans. (Source : https://www.cos.io/)"@en ;
  skos:prefLabel "Open Science Badge"@en, "badge de science ouverte"@fr, "insignia de ciencia abierta"@es ;
  skos:inScheme <http://data.loterre.fr/ark:/67375/TSO> ;
  skos:broader <http://data.loterre.fr/ark:/67375/TSO-QF2RDTPG-H> ;
  skos:related <http://data.loterre.fr/ark:/67375/TSO-BTFX00Q2-P> .

<http://data.loterre.fr/ark:/67375/TSO-B8RHV59S-0>
  a skos:Concept ;
  dc:modified "2021-06-30"^^xsd:date ;
  skos:definition "Entrepôt qui rassemble les données qui se trouvent dans des entrepôts subsidiaires. (Source : https://tel.archives-ouvertes.fr/tel-00922600/)"@fr ;
  skos:prefLabel "aggregating repository"@en, "almacén de agregación"@es, "entrepôt agrégateur"@fr ;
  skos:inScheme <http://data.loterre.fr/ark:/67375/TSO> ;
  skos:broader <http://data.loterre.fr/ark:/67375/TSO-W9KRS5Q3-6> .

<http://data.loterre.fr/ark:/67375/TSO-MV5H4HGJ-2>
  a skos:Concept ;
  skos:prefLabel "diffusion de la science ouverte"@fr, "distribución de la ciencia abierta"@es, "open science dissemination"@en ;
  skos:inScheme <http://data.loterre.fr/ark:/67375/TSO> ;
  skos:broader <http://data.loterre.fr/ark:/67375/TSO-SMGMJFLJ-Q> ;
  skos:related <http://data.loterre.fr/ark:/67375/TSO-B8V78028-B>, <http://data.loterre.fr/ark:/67375/TSO-BRNV0DF5-3>, <http://data.loterre.fr/ark:/67375/TSO-GW6WNBGQ-X>, <http://data.loterre.fr/ark:/67375/TSO-QF2RDTPG-H>, <http://data.loterre.fr/ark:/67375/TSO-WSB3R3KG-1> ;
  skos:narrower <http://data.loterre.fr/ark:/67375/TSO-JB3N2FLX-R>, <http://data.loterre.fr/ark:/67375/TSO-KG7FR9LH-R>, <http://data.loterre.fr/ark:/67375/TSO-KM81Q24P-C> .

<http://data.loterre.fr/ark:/67375/TSO-KG7FR9LH-R>
  a skos:Concept ;
  dc:modified "2021-06-30"^^xsd:date ;
  skos:definition "Evènements visant à promouvoir la science ouverte et/ou former des personnes dans ce domaine."@fr ;
  skos:prefLabel "evento de ciencia abierta"@es, "manifestation sur la science ouverte"@fr, "open science meeting"@en ;
  skos:inScheme <http://data.loterre.fr/ark:/67375/TSO> ;
  skos:broader <http://data.loterre.fr/ark:/67375/TSO-MV5H4HGJ-2> ;
  skos:narrower <http://data.loterre.fr/ark:/67375/TSO-FC2GVFL9-R>, <http://data.loterre.fr/ark:/67375/TSO-M9JG3Z18-C> .

<http://data.loterre.fr/ark:/67375/TSO-KM81Q24P-C>
  a skos:Concept ;
  dc:modified "2021-06-30"^^xsd:date ;
  skos:definition "Guides ou séances d'apprentissage pour aider les chercheurs à rendre leurs travaux ouverts."@fr ;
  skos:prefLabel "capacitación para la ciencia abierta"@es, "formation à la science ouverte"@fr, "open science training"@en ;
  skos:inScheme <http://data.loterre.fr/ark:/67375/TSO> ;
  skos:broader <http://data.loterre.fr/ark:/67375/TSO-MV5H4HGJ-2> .

<http://data.loterre.fr/ark:/67375/TSO-NBSJSHH5-P>
  a skos:Concept ;
  skos:altLabel "blanchiment par les données"@fr, "open washing"@en, "orangewashing"@en ;
  skos:definition "Having an appearance of open-source and open-licensing for marketing purposes, while continuing proprietary practices. (Source : http://www.righttoresearch.org/resources/OpenResearchGlossary)"@en, "Procédé de marketing ou de relations publiques laissant croire qu'une initiative s'inscrit dans le mouvement de la culture libre. (Source : Wikipédia)"@fr, "Se aproxima a un movimiento internacional enfocado en denunciar aseveraciones posiblemente falsas acerca de la apertura de una compañía de tecnologías o contenidos, usualmente con fines publicitarios. (Fuente: https://www.lmspulse.com/2017/que-es-openwashing-investigando-el-caso-de-canvas-lms/)"@es ;
  skos:prefLabel "openwashing"@en, "openwashing"@es, "ouvertisation"@fr ;
  skos:inScheme <http://data.loterre.fr/ark:/67375/TSO> ;
  skos:broader <http://data.loterre.fr/ark:/67375/TSO-PSFFQLXV-2> .

<http://data.loterre.fr/ark:/67375/TSO-DDX6CQLL-1>
  a skos:Concept ;
  dc:modified "2021-06-22"^^xsd:date ;
  skos:altLabel "mur de péage"@fr, "péage de lecture numérique"@fr, "verrou d'accès payant"@fr ;
  skos:definition "Méthode de restriction d'accès à un contenu numérique dans le but d'amener le lecteur à souscrire un abonnement payant. (Source : https://fr.wikipedia.org/wiki/Paywall)"@fr, "restriction via a financial barrier to research, often implemented by legacy publishers. Can be removed by personal or institutional subscription. (source: http://www.righttoresearch.org/resources/OpenResearchGlossary/index.shtml)"@en ;
  skos:prefLabel "muro de pago"@es, "paywall"@en, "péage"@fr ;
  skos:inScheme <http://data.loterre.fr/ark:/67375/TSO> ;
  skos:broader <http://data.loterre.fr/ark:/67375/TSO-PSFFQLXV-2> .

<http://data.loterre.fr/ark:/67375/TSO-RH261KDT-S>
  a skos:Concept ;
  dc:modified "2021-06-25"^^xsd:date ;
  skos:altLabel "DCP"@fr, "donnée personnelle"@fr ;
  skos:definition "Toute information se rapportant à une personne physique identifiée ou identifiable. (Source : https://www.cnil.fr/fr/definition/donnee-personnelle)"@fr ;
  skos:prefLabel "dato personal"@es, "donnée à caractère personnel"@fr, "personal data"@en ;
  skos:inScheme <http://data.loterre.fr/ark:/67375/TSO> ;
  skos:broader <http://data.loterre.fr/ark:/67375/TSO-MGRQT12J-W> ;
  skos:related <http://data.loterre.fr/ark:/67375/TSO-F2SDG44T-9>, <http://data.loterre.fr/ark:/67375/TSO-FWFH6NFF-1>, <http://data.loterre.fr/ark:/67375/TSO-VNNFL8WB-H> .

<http://data.loterre.fr/ark:/67375/TSO-XRBPKF38-J>
  a skos:Concept ;
  dc:modified "2021-06-22"^^xsd:date ;
  skos:altLabel "reporting bias"@en ;
  skos:definition "Désigne en science le fait que les chercheurs et les revues scientifiques ont bien plus tendance à publier des expériences ayant obtenu un résultat positif (statistiquement significatif) que des expériences ayant obtenu un résultat négatif (soutenant l'hypothèse nulle). Il donne aux lecteurs une perception biaisée (vers le positif) de l'état de la recherche. (Source : http://dictionnaire.sensagent.leparisien.fr/Biais%20de%20publication/fr-fr/)"@fr, "occurs when certain aspects of a study are systematically not reported transparently, creating wastage and redundancy through selective reporting or non-publishing. (source: https://open-science-training-handbook.gitbook.io/book/glossary)"@en ;
  skos:prefLabel "biais de publication"@fr, "publication bias"@en, "sesgos en la publicación"@es ;
  skos:inScheme <http://data.loterre.fr/ark:/67375/TSO> ;
  skos:broader <http://data.loterre.fr/ark:/67375/TSO-PSFFQLXV-2> ;
  skos:related <http://data.loterre.fr/ark:/67375/TSO-ZMJ8VVB2-9> .

<http://data.loterre.fr/ark:/67375/TSO-GRJ351P7-S>
  a skos:Concept ;
  dc:modified "2021-06-30"^^xsd:date ;
  skos:definition "A publishing format used by over 250 journals that emphasizes the importance of the research question and the quality of methodology by conducting peer review prior to data collection. High quality protocols are then provisionally accepted for publication if the authors follow through with the registered methodology. This format is designed to reward best practices in adhering to the hypothetico-deductive model of the scientific method. It eliminates a variety of questionable research practices, including low statistical power, selective reporting of results, and publication bias, while allowing complete flexibility to report serendipitous findings. (Source : https://www.cos.io/initiatives/registered-reports)"@en, "Type d'article empirique conçu pour éliminer les biais de publication et mettre en œuvre les meilleures pratiques scientifiques. [Des revues qui proposent] des rapports enregistrés acceptent de façon provisoire un article basé sur un protocole d'étude précédemment soumis considéré comme méthodologiquement adapté et répondent à une importante question scientifique. Après l'acceptation provisoire de leur travail, les auteurs peuvent effectuer leur recherche en sachant que les résultats ne détermineront pas la publication de l'article. Conjointement, les lecteurs de l'article final estimeront plus facilement la reproductibilité de l'article car les révisions des prévisions initiales de l'étude et des plans d'analyse ont été menées de façon indépendante. (Source : https://www.elsevier.com/fr-fr/open-science/science-and-society/research-integrity)"@fr ;
  skos:prefLabel "informe registrado"@es, "rapport enregistré"@fr, "registered report"@en ;
  skos:inScheme <http://data.loterre.fr/ark:/67375/TSO> ;
  skos:broader <http://data.loterre.fr/ark:/67375/TSO-V0KSG0NC-P> .

<http://data.loterre.fr/ark:/67375/TSO-HXX9G512-G>
  a skos:Concept ;
  skos:altLabel "Research Papers in Economics"@en, "Research Papers in Economics"@es, "Research Papers in Economics"@fr ;
  skos:definition "A collaborative effort of hundreds of volunteers in many countries to enhance the dissemination of research in economics. (Source : Wikipedia)"@en, "Projet collaboratif de plusieurs centaines de volontaires de 79 pays destiné à permettre la plus large diffusion de la recherche en économie. (Source : Wikipédia)"@fr ;
  skos:prefLabel "RePEC"@en, "RePEC"@es, "RePEC"@fr ;
  skos:inScheme <http://data.loterre.fr/ark:/67375/TSO> ;
  skos:broader <http://data.loterre.fr/ark:/67375/TSO-J64S3QDL-1> ;
  skos:related <http://data.loterre.fr/ark:/67375/TSO-PM46WP7W-P> .

<http://data.loterre.fr/ark:/67375/TSO-SDDGPBZK-G>
  a skos:Concept ;
  dc:modified "2021-06-25"^^xsd:date ;
  skos:altLabel "ResearcherID"@en, "ResearcherID"@fr ;
  skos:definition "Identifiant pérenne attribué aux résultats des chercheurs et aux enregistrements de publications dans le Web of Science, anciennement nommé ResearcherID."@fr, "Persistent identifier assigned to researcher outputs and publication records in Web of Science."@en ;
  skos:prefLabel "Publons"@en, "Publons"@es, "Publons"@fr ;
  skos:inScheme <http://data.loterre.fr/ark:/67375/TSO> ;
  skos:broader <http://data.loterre.fr/ark:/67375/TSO-H5ZG6DX6-4> .

<http://data.loterre.fr/ark:/67375/TSO-TWKDXTXK-N>
  a skos:Concept ;
  skos:definition "A blog that reports on retractions of scientific papers and on related topics. Its parent organization is the Center for Scientific Integrity. (Source Wikipedia)"@en, "Blog que informa sobre las retracciones de artículos científicos y sobre temas relacionados. (fuente: Wikipedia)"@es, "Blog qui analyse les rétractations d'articles scientifiques et commente des sujets liés à l'intégrité scientifique."@fr ;
  skos:prefLabel "Retraction Watch"@en, "Retraction Watch"@es, "Retraction Watch"@fr ;
  skos:inScheme <http://data.loterre.fr/ark:/67375/TSO> ;
  skos:broader <http://data.loterre.fr/ark:/67375/TSO-V0HZ66HD-4> .

<http://data.loterre.fr/ark:/67375/TSO-X4ZW5XQD-G>
  a skos:Concept ;
  dc:modified "2021-06-24"^^xsd:date ;
  skos:altLabel "reusability"@en, "reutilizabilidad"@es, "réutilisabilité"@fr ;
  skos:definition "Principe [FAIR qui] met en avant les caractéristiques qui rendent les données utilisables pour de futures recherches ou d’autres finalités (enseignement, innovation, reproduction/transparence de la science). Pour que les données soient réutilisables par d’autres, leur partage doit avant tout être accompagné d’une licence qui précise les conditions de leur utilisation. Ensuite, il est utile de décrire leur provenance et de fournir toute information permettant de les contextualiser."@fr ;
  skos:prefLabel "reusable"@en, "reutilizable"@es, "réutilisable"@fr ;
  skos:inScheme <http://data.loterre.fr/ark:/67375/TSO> ;
  skos:broader <http://data.loterre.fr/ark:/67375/TSO-D9HJPTL6-X> ;
  skos:related <http://data.loterre.fr/ark:/67375/TSO-XK0JJTS6-2> .

<http://data.loterre.fr/ark:/67375/TSO-NCN8QNX0-N>
  a skos:Concept ;
  dc:modified "2021-06-29"^^xsd:date ;
  skos:altLabel "no-transfer of rights strategy"@en ;
  skos:definition "A strategy whereby the authors or their institutions retain copyright as well as the rights that are necessary to make a version of their work immediately available under an open license. (Source : cOAlition S)"@en, "Stratégie qui permet aux chercheurs qui souhaitent publier dans des revues sous abonnement de conserver l’intégralité de leurs droits sur les articles dont ils sont les auteurs et d’en déposer la version acceptée pour publication dans une archive ouverte dès la date de publication, grâce à l’utilisation de la licence Creative Commons CC-BY. (Source : Ouvrir la Science)"@fr ;
  skos:prefLabel "estrategia de no cesión de derechos"@es, "rights retention strategy"@en, "stratégie de non-cession des droits"@fr ;
  skos:inScheme <http://data.loterre.fr/ark:/67375/TSO> ;
  skos:broader <http://data.loterre.fr/ark:/67375/TSO-SMGMJFLJ-Q> .

<http://data.loterre.fr/ark:/67375/TSO-WG6NKQ9W-M>
  a skos:Concept ;
  dc:modified "2021-06-24"^^xsd:date ;
  skos:altLabel "Sponsoring Consortium for Open Access Publishing in Particle Physics"@en, "Sponsoring Consortium for Open Access Publishing in Particle Physics"@es, "Sponsoring Consortium for Open Access Publishing in Particle Physics"@fr ;
  skos:definition "A partnership of over three thousand libraries, key funding agencies and research centers in 44 countries and 3 intergovernmental organisations. Working with leading publishers, SCOAP3 has converted key journals in the field of High-Energy Physics to Open Access at no cost for authors. SCOAP3 centrally pays publishers for costs involved in providing Open Access, publishers, in turn, reduce subscription fees to all their customers, who can re-direct these funds to contribute to SCOAP3. (Source : a one-of-its-kind partnership of over three thousand libraries, key funding agencies and research centers in 44 countries and 3 intergovernmental organisations. Working with leading publishers, SCOAP3 has converted key journals in the field of High-Energy Physics to Open Access at no cost for authors. SCOAP3 centrally pays publishers for costs involved in providing Open Access, publishers, in turn, reduce subscription fees to all their customers, who can re-direct these funds to contribute to SCOAP3. (Source: https://scoap3.org/)"@en, "Consortium formé d’agences de financement, d’organismes de recherche, de bibliothèques et de consortia de bibliothèques, créé en novembre 2006 pour promouvoir le libre accès à l’échelle planétaire. (Source : https://publications-prairial.fr/arabesques/index.php?id=688)"@fr ;
  skos:prefLabel "SCOAP3"@en, "SCOAP3"@es, "SCOAP3"@fr ;
  skos:inScheme <http://data.loterre.fr/ark:/67375/TSO> ;
  skos:broader <http://data.loterre.fr/ark:/67375/TSO-T52K1CB6-X> .

<http://data.loterre.fr/ark:/67375/TSO-T161C80T-Q>
  a skos:Concept ;
  dc:modified "2021-06-10"^^xsd:date ;
  skos:altLabel "toile sémantique"@fr ;
  skos:definition "Extension du Web standardisée par le World Wide Web Consortium (W3C). Ces standards encouragent l'utilisation de formats de données et de protocoles d'échange normés sur le Web, en s'appuyant sur les modèles Resource Description Framework (RDF) et Web Ontology Language (OWL). (Source : wikipédia)"@fr, "Extension of the World Wide Web through standards set by the World Wide Web Consortium (W3C). The goal of the Semantic Web is to make Internet data machine-readable. To enable the encoding of semantics with the data, technologies such as Resource Description Framework (RDF) and Web Ontology Language (OWL) are used."@en ;
  skos:prefLabel "semantic web"@en, "web semántica"@es, "web sémantique"@fr ;
  skos:inScheme <http://data.loterre.fr/ark:/67375/TSO> ;
  skos:broader <http://data.loterre.fr/ark:/67375/TSO-XWVJBKN6-S> ;
  skos:related <http://data.loterre.fr/ark:/67375/TSO-J3R15XFV-K> .

<http://data.loterre.fr/ark:/67375/TSO-V25B9BQX-X>
  a skos:Concept ;
  dc:modified "2021-06-02"^^xsd:date ;
  skos:definition "Vise à établir un consensus mondial sur la science ouverte grâce à un processus inclusif, transparent et consultatif impliquant tous les pays et toutes les parties prenantes. Elle a pour objet de définir les valeurs et principes communs relatifs à la science ouverte, et de proposer des mesures concrètes sur l’accès libre et les données ouvertes, assorties de propositions visant à rapprocher les citoyens de la science, ainsi que d’engagements facilitant la production et la diffusion des connaissances scientifiques dans le monde. (source: https://en.unesco.org/sites/default/files/open_science_brochure_fr.pdf)"@fr ;
  skos:prefLabel "UNESCO Recommendation on Open Science"@en, "recomendación de la UNESCO sobre la ciencia abierta"@es, "recommandation de l'UNESCO sur la science ouverte"@fr ;
  skos:inScheme <http://data.loterre.fr/ark:/67375/TSO> ;
  skos:broader <http://data.loterre.fr/ark:/67375/TSO-CV5H9HZH-V> ;
  skos:related <http://data.loterre.fr/ark:/67375/TSO-FK1RPNQP-Z> .

<http://data.loterre.fr/ark:/67375/TSO-VJVHPV6M-P>
  a skos:Concept ;
  dc:modified "2021-06-29"^^xsd:date ;
  skos:altLabel "registry of research data repositories"@en, "registry of research data repositories"@es, "registry of research data repositories"@fr ;
  skos:definition "Registre mondial des entrepôts de données de recherche. Ils peuvent être parcourus par sujet, pays ou type de contenu, et recherchés par une combinaison de 41 attributs différents. (Source : https://www.ouvrirlascience.fr/registry-of-research-data-repositories-re3data-org/)"@fr ;
  skos:prefLabel "re3data"@en, "re3data"@es, "re3data"@fr ;
  skos:inScheme <http://data.loterre.fr/ark:/67375/TSO> ;
  skos:broader <http://data.loterre.fr/ark:/67375/TSO-WQ9RZCBH-P> .

<http://data.loterre.fr/ark:/67375/TSO-F43HWMXG-K>
  a skos:Concept ;
  dc:modified "2021-06-25"^^xsd:date ;
  skos:altLabel "Research Organization Registry"@en, "Research Organization Registry"@es, "Research Organization Registry"@fr ;
  skos:definition "A community-led project to develop an open, sustainable, usable, and unique identifier for every research organization in the world.(Source : https://ror.org/)"@en, "Initiative visant à agir de manière coordonnée pour réduire l’effort visant à rendre les identifiants universels."@fr ;
  skos:prefLabel "ROR"@en, "ROR"@es, "ROR"@fr ;
  skos:inScheme <http://data.loterre.fr/ark:/67375/TSO> ;
  skos:broader <http://data.loterre.fr/ark:/67375/TSO-J64S3QDL-1> ;
  skos:related <http://data.loterre.fr/ark:/67375/TSO-H5ZG6DX6-4> .

<http://data.loterre.fr/ark:/67375/TSO-JXVPRHLQ-P>
  a skos:Concept ;
  skos:altLabel "Identifiants et Référentiels pour l'enseignement supérieur et la recherche"@fr ;
  skos:definition "Application Web permettant à des utilisateurs et à des applications clientes d’interroger et consulter les autorités des catalogues Calames, Sudoc et theses.fr."@fr ;
  skos:prefLabel "IdRef"@en, "IdRef"@es, "IdRef"@fr ;
  skos:inScheme <http://data.loterre.fr/ark:/67375/TSO> ;
  skos:broader <http://data.loterre.fr/ark:/67375/TSO-V0HZ66HD-4> ;
  skos:related <http://data.loterre.fr/ark:/67375/TSO-H5ZG6DX6-4> .

<http://data.loterre.fr/ark:/67375/TSO-T52K1CB6-X>
  a skos:Concept ;
  dc:modified "2021-06-11"^^xsd:date ;
  skos:altLabel "funding organisation"@en, "grant-giving organisation"@en, "research funding organisation"@en ;
  skos:prefLabel "agence de financement"@fr, "agencia de financiación"@es, "funding agency"@en ;
  skos:inScheme <http://data.loterre.fr/ark:/67375/TSO> ;
  skos:broader <http://data.loterre.fr/ark:/67375/TSO-J64S3QDL-1> ;
  skos:related <http://data.loterre.fr/ark:/67375/TSO-NHVK3QVC-F> ;
  skos:narrower <http://data.loterre.fr/ark:/67375/TSO-WG6NKQ9W-M>, <http://data.loterre.fr/ark:/67375/TSO-RB9SXH7C-R>, <http://data.loterre.fr/ark:/67375/TSO-LR2FMP5P-6>, <http://data.loterre.fr/ark:/67375/TSO-N0VLP1P2-S>, <http://data.loterre.fr/ark:/67375/TSO-G3FV93X6-N> .

<http://data.loterre.fr/ark:/67375/TSO-RB9SXH7C-R>
  a skos:Concept ;
  dc:modified "2021-06-24"^^xsd:date ;
  skos:altLabel "Fondo Nacional para la Ciencia Abierta"@es, "Fonds National pour la Science Ouverte"@fr, "National Fund for Open Science"@en ;
  skos:definition "Organisation qui vise à soutenir des initiatives françaises en science ouverte à travers la mise en place d’appels à projets. Sa création est issue de l'axe « Généraliser l’accès ouvert aux publications » du Plan national pour la Science Ouverte annoncé en juillet 2018 par la ministre de l'Enseignement supérieur, de la Recherche et de l'Innovation, Frédérique Vidal. Il est financé par le ministère et reçoit des contributions complémentaires en provenance de la communauté de l'enseignement supérieur, de la recherche et de l'innovation, (Source : https://www.enseignementsup-recherche.gouv.fr/)"@fr ;
  skos:prefLabel "FNSO"@en, "FNSO"@es, "FNSO"@fr ;
  skos:inScheme <http://data.loterre.fr/ark:/67375/TSO> ;
  skos:broader <http://data.loterre.fr/ark:/67375/TSO-T52K1CB6-X> ;
  skos:related <http://data.loterre.fr/ark:/67375/TSO-ZLCW75XN-W> .

<http://data.loterre.fr/ark:/67375/TSO-VM3N240R-C>
  a skos:Concept ;
  skos:definition "Département de la direction interministérielle du numérique (DINUM), dont les missions et l’organisation sont fixées par le décret du 30 Octobre 2019. Il coordonne notamment la conception et la mise en œuvre de la stratégie de l’État Français dans le domaine de la donnée. (Source : https://www.data.gouv.fr/fr/organizations/etalab/)"@fr ;
  skos:prefLabel "Etalab"@en, "Etalab"@es, "Etalab"@fr ;
  skos:inScheme <http://data.loterre.fr/ark:/67375/TSO> ;
  skos:broader <http://data.loterre.fr/ark:/67375/TSO-J64S3QDL-1> ;
  skos:related <http://data.loterre.fr/ark:/67375/TSO-ZKK6WW4X-W> .

<http://data.loterre.fr/ark:/67375/TSO-WWM82SKD-Z>
  a skos:Concept ;
  dc:modified "2021-06-10"^^xsd:date ;
  skos:definition "A platform that helps researchers identify trusted journals and publishers for their research. Through a range of tools and practical resources, this international, cross-sector initiative aims to educate researchers, promote integrity, and build trust in credible research and publications. (Source : https://thinkchecksubmit.org/)"@en, "Plateforme qui aide les chercheurs à identifier des revues de qualité pour leurs recherches. C’est une simple liste de contrôle que les chercheurs peuvent utiliser pour évaluer les titres d’un journal ou d’un éditeur. (Source : http://thinkchecksubmit.org)"@fr ;
  skos:prefLabel "Think Check Submit"@en, "Think Check Submit"@es, "Think Check Submit"@fr ;
  skos:inScheme <http://data.loterre.fr/ark:/67375/TSO> ;
  skos:broader <http://data.loterre.fr/ark:/67375/TSO-QK42D772-3> ;
  skos:related <http://data.loterre.fr/ark:/67375/TSO-ZRVHF3XW-L> .

<http://data.loterre.fr/ark:/67375/TSO-TNN44SLS-R>
  a skos:Concept ;
  skos:altLabel "Bibliothèque Scientifique Numérique"@fr ;
  skos:definition "Dispositif de pilotage en charge des questions d’Information scientifique et technique (IST) en France de 2007 à 2017. Elle évolue en 2018 vers la Science ouverte et devient le Comité pour la science ouverte (CoSO)."@fr ;
  skos:prefLabel "BSN"@en, "BSN"@es, "BSN"@fr ;
  skos:inScheme <http://data.loterre.fr/ark:/67375/TSO> ;
  skos:broader <http://data.loterre.fr/ark:/67375/TSO-J64S3QDL-1> ;
  skos:related <http://data.loterre.fr/ark:/67375/TSO-VPJV1Q5X-J> .

<http://data.loterre.fr/ark:/67375/TSO-B8V78028-B>
  a skos:Concept ;
  dc:modified "2021-06-24"^^xsd:date ;
  skos:definition "Jeu coopératif créé par l’équipe DoRANum pour animer de façon ludique les formations sur la gestion et le partage des données de la recherche."@fr ;
  skos:prefLabel "GopenDore"@en, "GopenDore"@es, "GopenDore"@fr ;
  skos:inScheme <http://data.loterre.fr/ark:/67375/TSO> ;
  skos:broader <http://data.loterre.fr/ark:/67375/TSO-RB0TPH2H-Q> ;
  skos:related <http://data.loterre.fr/ark:/67375/TSO-J0H32WL6-Z>, <http://data.loterre.fr/ark:/67375/TSO-MV5H4HGJ-2> .

<http://data.loterre.fr/ark:/67375/TSO-LR2FMP5P-6>
  a skos:Concept ;
  skos:definition "EU's key funding programme for research and innovation until 2027."@en, "Programa Marco de Investigación e Innovación para el período 2021-2027 (Fuente: https://acmservicios.com)"@es, "Programme-cadre de l'Union européenne pour la recherche et l'innovation pour la période allant de 2021 à 2027"@fr ;
  skos:prefLabel "Horizon Europe"@en, "Horizon Europe"@fr, "Horizonte Europa"@es ;
  skos:inScheme <http://data.loterre.fr/ark:/67375/TSO> ;
  skos:broader <http://data.loterre.fr/ark:/67375/TSO-T52K1CB6-X> .

<http://data.loterre.fr/ark:/67375/TSO-NHVK3QVC-F>
  a skos:Concept ;
  dc:modified "2021-06-25"^^xsd:date ;
  skos:definition "An open registry of grant-giving organization names and identifiers, which you use to find funder IDs and include them as part of your metadata deposits. (Source : https://www.crossref.org/services/funder-registry/)"@en, "Répertoire ouvert maintenu par CrossRef, permettant de trouver les noms et les identifiants d'organismes financeurs, afin de les inclure dans les dépôts de métadonnées."@fr ;
  skos:prefLabel "Funder Registry"@en, "Funder Registry"@es, "Funder Registry"@fr ;
  skos:inScheme <http://data.loterre.fr/ark:/67375/TSO> ;
  skos:broader <http://data.loterre.fr/ark:/67375/TSO-B66RVJ4T-J> ;
  skos:related <http://data.loterre.fr/ark:/67375/TSO-T52K1CB6-X> .

<http://data.loterre.fr/ark:/67375/TSO-GW6WNBGQ-X>
  a skos:Concept ;
  dc:modified "2021-07-05"^^xsd:date ;
  skos:altLabel "civic science"@en ;
  skos:definition "Production scientifique qui répond aux objectifs et aux attentes de la société à l’égard de la recherche."@fr, "Trabajo científico realizado voluntariamente por miembros del público en general, a menudo en colaboración con o bajo la dirección de científicos profesionales e instituciones científicas. (Fuente: https://www.biodiversidad.gob.mx/cienciaciudadana/que-es)"@es ;
  skos:prefLabel "ciencia ciudadana"@es, "citizen science"@en, "science citoyenne"@fr ;
  skos:inScheme <http://data.loterre.fr/ark:/67375/TSO> ;
  skos:broader <http://data.loterre.fr/ark:/67375/TSO-JFJGKFN2-H> ;
  skos:related <http://data.loterre.fr/ark:/67375/TSO-MV5H4HGJ-2> .

<http://data.loterre.fr/ark:/67375/TSO-KBRVB4PD-K>
  a skos:Concept ;
  dc:created "2021-06-24"^^xsd:date ;
  dc:modified "2021-07-05"^^xsd:date ;
  skos:altLabel "CS"@en, "crowd science"@en, "crowd-sourced science"@en, "participatory action research"@en, "participatory monitoring"@en, "public participation in scientific research"@en, "science collaborative"@fr, "volunteer monitoring"@en ;
  skos:definition "Forme de production de connaissances scientifiques à laquelle des acteurs non-scientifiques-professionnels — qu’il s’agisse d’individus ou de groupes — participent de façon active et délibérée (source : DOI 10.15454/1.4606201248693647E12)"@fr, "Involucramiento activo de los ciudadanos y las ciudadanas en los procesos de toma de decisiones públicas que tienen repercusión en sus vidas. (Fuente: https://www.minjusticia.gob.cl/participacion-ciudadana/)"@es, "Scientific research and monitoring driven and controlled by local communities, and characterized by place-based knowledge, social learning, collective action and empowerment. (Source: https://www.sciencedirect.com/science/article/pii/S1462901119300942)"@en ;
  skos:prefLabel "community science"@en, "participación ciudadana"@es, "science participative"@fr ;
  skos:inScheme <http://data.loterre.fr/ark:/67375/TSO> ;
  skos:broader <http://data.loterre.fr/ark:/67375/TSO-JFJGKFN2-H> ;
  skos:related <http://data.loterre.fr/ark:/67375/TSO-RB0TPH2H-Q> .

<http://data.loterre.fr/ark:/67375/TSO-JFR1FLWQ-R>
  a skos:Concept ;
  skos:definition "Ecole de pensée qui s'occupe de développer des méthodes alternatives pour déterminer l'impact scientifique . Cette école reconnaît que les mesures de l'impact scientifique sont cruciales pour la réputation d'un chercheur, les possibilités de financement et le développement de carrière. (Source: https://fr.other.wiki/wiki/Open_Science#Measurement_school)"@fr ;
  skos:prefLabel "escuela de la medición"@es, "measurement school"@en, "école de mesure"@fr ;
  skos:inScheme <http://data.loterre.fr/ark:/67375/TSO> ;
  skos:broader <http://data.loterre.fr/ark:/67375/TSO-F2VJ1STQ-Z> ;
  skos:related <http://data.loterre.fr/ark:/67375/TSO-W30LBC9X-X> .

<http://data.loterre.fr/ark:/67375/TSO-D80R1KX4-5>
  a skos:Concept ;
  dc:modified "2021-06-24"^^xsd:date ;
  skos:definition "Data derived from the interpretation of data originally produced by another researcher, available in journals, repositories, archives and other publications"@en, "Données issues de l'interprétation de données initialement produites par un autre chercheur, disponibles dans les revues, les entrepôts, les archives et autres publications."@fr ;
  skos:prefLabel "datos secundarios"@es, "donnée secondaire"@fr, "secondary data"@en ;
  skos:inScheme <http://data.loterre.fr/ark:/67375/TSO> ;
  skos:broader <http://data.loterre.fr/ark:/67375/TSO-MJRKBMDW-Q> ;
  skos:related <http://data.loterre.fr/ark:/67375/TSO-XK0JJTS6-2> .

<http://data.loterre.fr/ark:/67375/TSO-ZWDW27C7-Q>
  a skos:Concept ;
  dc:modified "2021-07-05"^^xsd:date ;
  skos:definition "A model that respects the FOAA open access publishing principles: 1-The journal has a transparent ownership structure, and is controlled by and responsive to the scholarly community; 2-Authors of articles in the journal retain copyright; 3-All articles are published open access and an explicit open access licence is used; 4-Submission and publication is not conditional in any way on the payment of a fee from the author or their employing institution, or on membership of an institution or society; 5-Any fees paid on behalf of the journal to publishers are low, transparent, and in proportion to the work carried out. (Source: https://www.fairopenaccess.org/the-fair-open-access-principles/)"@en, "Modèle qui respecte les principes de publication en accès libre énoncés par la FOAA : 1-La revue a une structure de propriété transparente, elle est contrôlée par la communauté scientifique et répond à ses besoins ; 2-Les auteurs des articles publiés dans la revue conservent leurs droits d'auteur ; 3-Tous les articles sont publiés en accès libre et une licence explicite d'accès libre est utilisée ; 4-La soumission et la publication ne sont en aucun cas conditionnées par le paiement d'une redevance par l'auteur ou l'institution qui l'emploie, ou par l'adhésion à une institution ou une société ; 5-Tous les frais payés aux éditeurs au nom de la revue sont faibles, transparents et proportionnels au travail effectué."@fr, "Un modelo que respeta los principios de publicación de acceso abierto de la FOAA: 1-La revista tiene una estructura de propiedad transparente, y está controlada por la comunidad académica y responde a ella; 2-Los autores de los artículos de la revista conservan los derechos de autor; 3-Todos los artículos se publican en acceso abierto y se utiliza una licencia explícita de acceso abierto; 4-La presentación y publicación no está condicionada en modo alguno al pago de una cuota por parte del autor o de su institución empleadora, ni a la pertenencia a una institución o sociedad; 5-Las cuotas que se pagan en nombre de la revista a los editores son bajas, transparentes y proporcionales al trabajo realizado. (Fuente: https://www.fairopenaccess.org/the-fair-open-access-principles/ )"@es ;
  skos:prefLabel "fair open access"@en, "fair open access"@es, "libre accès juste"@fr ;
  skos:inScheme <http://data.loterre.fr/ark:/67375/TSO> ;
  skos:broader <http://data.loterre.fr/ark:/67375/TSO-STWL5MWS-W> ;
  skos:related <http://data.loterre.fr/ark:/67375/TSO-GCTBW7HJ-P> .

<http://data.loterre.fr/ark:/67375/TSO-GKLZDCG9-4>
  a skos:Concept ;
  dc:modified "2021-06-29"^^xsd:date ;
  skos:altLabel "FOAA principles"@en ;
  skos:definition "Principes énoncés par la FOAA pour favoriser le libre accès FAIR aux revues et articles scientifiques."@fr ;
  skos:prefLabel "Fair Open Acces principles"@en, "principes du Fair Open Access"@fr, "principios del Fair Open Access"@es ;
  skos:inScheme <http://data.loterre.fr/ark:/67375/TSO> ;
  skos:broader <http://data.loterre.fr/ark:/67375/TSO-CV5H9HZH-V> ;
  skos:related <http://data.loterre.fr/ark:/67375/TSO-GCTBW7HJ-P>, <http://data.loterre.fr/ark:/67375/TSO-JKWW3PW1-7> .

<http://data.loterre.fr/ark:/67375/TSO-BD33KNNX-S>
  a skos:Concept ;
  dc:modified "2021-06-29"^^xsd:date ;
  skos:altLabel "linguistic in open access"@en ;
  skos:definition "Organisation qui œuvre pour la transition des revues de linguistique vers des modèles de publication respectant les principes du « libre accès juste »."@fr, "Organization that facilitates conversion to fair open access of journals in linguistics (source: https://www.fairopenaccess.org/)"@en ;
  skos:prefLabel "lingOA"@en, "lingOA"@es, "lingOA"@fr ;
  skos:inScheme <http://data.loterre.fr/ark:/67375/TSO> ;
  skos:broader <http://data.loterre.fr/ark:/67375/TSO-J64S3QDL-1> ;
  skos:related <http://data.loterre.fr/ark:/67375/TSO-GCTBW7HJ-P> .

<http://data.loterre.fr/ark:/67375/TSO-FK1RPNQP-Z>
  a skos:Concept ;
  dc:modified "2021-06-29"^^xsd:date ;
  skos:definition "International Science Council’s (ISC) response to the UNESCO global consultation on open science. It brings together strands of work that have developed within the ISC community to create a draft working paper that will be further developed through consultation with the Council’s members as a formal ISC position paper on open science. (Source : https://en.unesco.org/sites/default/files/isc_paper_for_unesco_open_science_consultation_2020.pdf)"@en, "Réponse de l'International Science Council (ISC) à la consultation mondiale de l'UNESCO sur la science ouverte."@fr ;
  skos:prefLabel "Open Science for the 21st Century"@en, "Open Science for the 21st Century"@es, "Open Science for the 21st Century"@fr ;
  skos:inScheme <http://data.loterre.fr/ark:/67375/TSO> ;
  skos:broader <http://data.loterre.fr/ark:/67375/TSO-V6F4ZS65-G> ;
  skos:related <http://data.loterre.fr/ark:/67375/TSO-KCLNJ3JK-9>, <http://data.loterre.fr/ark:/67375/TSO-V25B9BQX-X> .

<http://data.loterre.fr/ark:/67375/TSO-JQQM0K0V-2>
  a skos:Concept ;
  dc:modified "2021-06-03"^^xsd:date ;
  skos:definition "Groupe-projet créé dans le cadre de la fondation du Comité pour la science ouverte (CoSO) via l’AMI du Ministère de la Recherche, Ses objectifs étaient de définir des principes et des critères de soutien aux initiatives affichant une exemplarité en matière d’accès ouvert et de bibliodiversité. Il s'est réuni d’octobre 2018 à juin 2019. (Source: https://www.ouvrirlascience.fr/construire-la-bibliodiversite/)"@fr ;
  skos:prefLabel "Construire la bibliodiversité"@en, "Construire la bibliodiversité"@es, "Construire la bibliodiversité"@fr ;
  skos:inScheme <http://data.loterre.fr/ark:/67375/TSO> ;
  skos:broader <http://data.loterre.fr/ark:/67375/TSO-H93WKMMJ-B> ;
  skos:related <http://data.loterre.fr/ark:/67375/TSO-VPJV1Q5X-J> .

<http://data.loterre.fr/ark:/67375/TSO-XSC65JWB-F>
  a skos:Concept ;
  dc:modified "2021-06-11"^^xsd:date ;
  skos:definition "A document that makes clear the terms under which the data can be used. (Source : Open Research Europe)"@en, "Document qui précise les conditions dans lesquelles des données peuvent être utilisées."@fr ;
  skos:prefLabel "accord d'utilisation des données"@fr, "acuerdo de uso de datos"@es, "data use agreement"@en ;
  skos:inScheme <http://data.loterre.fr/ark:/67375/TSO> ;
  skos:broader <http://data.loterre.fr/ark:/67375/TSO-T4KV78Z3-L> ;
  skos:related <http://data.loterre.fr/ark:/67375/TSO-MGRQT12J-W> .

<http://data.loterre.fr/ark:/67375/TSO-MGRQT12J-W>
  a skos:Concept ;
  dc:modified "2021-06-25"^^xsd:date ;
  skos:definition "Data that must be protected against unwanted disclosure. Access to sensitive data should be safeguarded. Protection of sensitive data may be required for legal or ethical reasons, for issues pertaining to personal privacy, or for proprietary considerations. (Source : OpenAIRE)"@en, "Données qui doivent être protégées contre toute divulgation non désirée. La protection des données sensibles peut être requise pour des raisons juridiques ou éthiques, pour des questions relatives à la vie privée ou pour des considérations de propriété."@fr ;
  skos:prefLabel "datos sensibles"@es, "donnée sensible"@fr, "sensitive data"@en ;
  skos:inScheme <http://data.loterre.fr/ark:/67375/TSO> ;
  skos:broader <http://data.loterre.fr/ark:/67375/TSO-MJRKBMDW-Q> ;
  skos:related <http://data.loterre.fr/ark:/67375/TSO-XSC65JWB-F> ;
  skos:narrower <http://data.loterre.fr/ark:/67375/TSO-RH261KDT-S> .

<http://data.loterre.fr/ark:/67375/TSO-N0VLP1P2-S>
  a skos:Concept ;
  dc:modified "2021-06-07"^^xsd:date ;
  skos:altLabel "ANR"@en, "ANR"@es, "ANR"@fr ;
  skos:definition "Agency founded in 2005 to promote French project-based research and to stimulate innovation by promoting the emergence of collaborative multidisciplinary projects and encouraging collaboration between the public and private sectors. (Source : ANR)"@en, "Etablissement public à caractère administratif français, placé sous la tutelle du ministère de l'Enseignement supérieur, de la Recherche et de l'Innovation. L'Agence met en oeuvre le financement de la recherche sur projets, pour les opérateurs publics en coopération entre eux ou avec des entreprises. (Source : ANR)"@fr ;
  skos:prefLabel "Agence nationale de la recherche"@fr, "Agence nationale de la recherche (Francia)"@es, "French National Research Agency"@en ;
  skos:inScheme <http://data.loterre.fr/ark:/67375/TSO> ;
  skos:broader <http://data.loterre.fr/ark:/67375/TSO-T52K1CB6-X> .

<http://data.loterre.fr/ark:/67375/TSO-LJ49Q4WZ-R>
  a skos:Concept ;
  dc:modified "2021-06-24"^^xsd:date ;
  skos:altLabel "TDR"@en, "Trustworthy Digital Repository"@en, "trustworthy repository"@en ;
  skos:definition "Data repository evaluated by an independent authority that endorsed its trustworthiness and awarded it a label."@en, "Entrepôt de données évalué par un organisme indépendant qui en a reconnu la fiabilité, au travers d'un label."@fr ;
  skos:prefLabel "almacén certificado"@es, "certified repository"@en, "entrepôt certifié"@fr ;
  skos:inScheme <http://data.loterre.fr/ark:/67375/TSO> ;
  skos:broader <http://data.loterre.fr/ark:/67375/TSO-W9KRS5Q3-6> ;
  skos:related <http://data.loterre.fr/ark:/67375/TSO-TC1HRLFR-8> .

<http://data.loterre.fr/ark:/67375/TSO-K8V0VJW2-2>
  a skos:Concept ;
  dc:modified "2021-06-11"^^xsd:date ;
  skos:definition "Data repository advised by an organisation, based on quality criteria such as “mission”, “community/recognition”, “legal and contractual compliance”, “access/accessibility”, “technical structure/interface”, “retrievability” or “preservation”. (Source : https://datascience.codata.org/article/10.5334/dsj-2017-042/)"@en, "Entrepôt de données conseillé par une organisation, sur la base de critères de qualité tels que \"mission\", \"communauté/reconnaissance\", \"conformité légale et contractuelle\", \"accès/accessibilité\", \"structure technique/interface\", \"trouvabilité\" ou \"préservation\"."@fr ;
  skos:prefLabel "almacén recomendado"@es, "entrepôt recommandé"@fr, "recommended repository"@en ;
  skos:inScheme <http://data.loterre.fr/ark:/67375/TSO> ;
  skos:broader <http://data.loterre.fr/ark:/67375/TSO-W9KRS5Q3-6> .

<http://data.loterre.fr/ark:/67375/TSO-LS688VQ2-2>
  a skos:Concept ;
  dc:modified "2021-06-10"^^xsd:date ;
  skos:altLabel "Méthodes et outils pour l’édition structurée"@fr ;
  skos:definition "Infrastructure conçue à l’usage des éditeurs et au service de l’activité éditoriale de l’ensemble des établissements publics d’enseignement supérieur et de recherche français. Elle a pour pour missions principales, d’une part de fournir un ensemble d’outils et de méthodes propres à permettre la constitution de fonds éditoriaux structurés et, d’autre part d’assurer des fonctions de diffusion des produits éditoriaux, numériques ou imprimés, au plus près des missions, des besoins et des objectifs de diffusion des résultats et des données de la recherche et en pleine connaissance des impératifs de l’idéal d’Open Access et des enjeux économiques qui les sous-tendent. (Source : http://www.metopes.fr)"@fr, "Infrastructure that aims to propose a set of tools and methods to allow the distribution of digital content in standardized environments with high interoperability potential. Métopes contributes to global rationalization of the publishing process by promoting the implementation of new multimedia distribution strategies and ensuring the sustainability of content and metadata. (Source: https://doi.org/10.5281/zenodo.2545575)"@en ;
  skos:prefLabel "Métopes"@en, "Métopes"@es, "Métopes"@fr ;
  skos:inScheme <http://data.loterre.fr/ark:/67375/TSO> ;
  skos:broader <http://data.loterre.fr/ark:/67375/TSO-WZ6DJ64Q-P> .

<http://data.loterre.fr/ark:/67375/TSO-LGJTJ71S-5>
  a skos:Concept ;
  dc:modified "2021-07-05"^^xsd:date ;
  skos:altLabel "PROduction et GEstion de DOnnées"@fr ;
  skos:definition "French large infrastructure that ensures the implementation of a public policy for social sciences and humanities. It focuses especially on research on law, economics, geography, management, history, political sciences and sociology. (Source: http://www.progedo.fr/progedo/missions/)"@en, "Gran infraestructura de investigación francesa encargada de promover y estructurar una política de datos públicos para la investigación en ciencias sociales. Es de especial interés para la investigación en derecho, economía, geografía, gestión, historia, ciencias políticas y sociología."@es, "Très Grande Infrastructure de Recherche française chargée d’impulser et structurer une politique publique des données pour la recherche en sciences sociales. Elle intéresse particulièrement la recherche en droit, économie, géographie, gestion, histoire, sciences politiques et sociologie. (Source : http://www.progedo.fr/progedo/missions/)"@fr ;
  skos:prefLabel "Progedo"@en, "Progedo"@es, "Progedo"@fr ;
  skos:inScheme <http://data.loterre.fr/ark:/67375/TSO> ;
  skos:broader <http://data.loterre.fr/ark:/67375/TSO-LS0Q2K68-D> .

<http://data.loterre.fr/ark:/67375/TSO-S30N1B85-1>
  a skos:Concept ;
  dc:modified "2021-06-24"^^xsd:date ;
  skos:altLabel "CDS"@fr ;
  skos:definition "Centre de données voué à la collecte et à la distribution dans le monde entier de données astronomiques."@fr, "Centro de datos que colecciona y distribuye la información astronómica."@es, "Data center dedicated to the collection and worldwide distribution of astronomical data and related information. (Source: http://cdsweb.u-strasbg.fr/about)"@en ;
  skos:prefLabel "Centre de données astronomiques de Strasbourg"@es, "Centre de données astronomiques de Strasbourg"@fr, "Strasbourg astronomical Data Center"@en ;
  skos:inScheme <http://data.loterre.fr/ark:/67375/TSO> ;
  skos:broader <http://data.loterre.fr/ark:/67375/TSO-LS0Q2K68-D> ;
  skos:related <http://data.loterre.fr/ark:/67375/TSO-XZ5703Z4-Q> .

<http://data.loterre.fr/ark:/67375/TSO-CX6BNH0X-Z>
  a skos:Concept ;
  dc:modified "2021-07-05"^^xsd:date ;
  skos:definition "A research infrastructure dedicated to Earth System observation data. (Source: https://www.data-terra.org/en/)"@en, "Infraestructura de investigación que permite disponer de datos atmosféricos, climáticos, oceanográficos, sísmicos y espaciales para entender y predecir la historia, el funcionamiento y la evolución del sistema terrestre de forma integrada."@es, "Infrastructure de recherche dont le but est de mettre à disposition des données atmosphériques, climatiques, océanographiques, sismiques et spatiales, pour comprendre et prévoir de manière intégrée l'histoire, le fonctionnement et l'évolution du système Terre."@fr ;
  skos:prefLabel "Data Terra"@en, "Data Terra"@es, "Data Terra"@fr ;
  skos:inScheme <http://data.loterre.fr/ark:/67375/TSO> ;
  skos:broader <http://data.loterre.fr/ark:/67375/TSO-LS0Q2K68-D> ;
  skos:related <http://data.loterre.fr/ark:/67375/TSO-XZ5703Z4-Q> .

<http://data.loterre.fr/ark:/67375/TSO-VGLQ1M4D-M>
  a skos:Concept ;
  dc:modified "2021-06-24"^^xsd:date ;
  skos:altLabel "Global Open Access Portal"@en, "Global Open Access Portal"@es, "Global Open Access Portal"@fr, "portal mundial del acceso abierto"@es ;
  skos:definition "A knowledge portal funded by the Governments of Colombia, Denmark, Norway, and the United States Department of State, It presents a current snapshot of the status of Open Access (OA) to scientific information in 158 countries worldwide, (Source: http://www.unesco.org/new/en/communication-and-information/portals-and-platforms/goap/)"@en, "Financiado por los Gobiernos de Colombia, Dinamarca, Noruega y el Departamento de Estado de los Estados Unidos de América. Presenta una visión actual de la situación del acceso abierto (OA) a la información científica en todo el mundo.(fuente: https://accesoabierto.biblioteca.ulpgc.es/2011/11/04/portal-mundial-del-acceso-abierto-global-open-access-portal/)"@es, "Portail web qui présente un état des lieux du libre accès à l’information scientifique à travers le monde. Il se veut une vitrine mondiale du libre accès à l’information scientifique, et a été lancé lors d’un événement parallèle organisé dans le cadre de la 36e session de la Conférence générale de l’UNESCO, en novembre 2011, à Paris. (Source http://bibliofrance.org/index.php/ressources/droits-d-auteurs/22-open-data/72-global-open-access-portal-goap)"@fr ;
  skos:prefLabel "GOAP"@en, "GOAP"@es, "GOAP"@fr ;
  skos:inScheme <http://data.loterre.fr/ark:/67375/TSO> ;
  skos:broader <http://data.loterre.fr/ark:/67375/TSO-DXZZDQSM-3> .

<http://data.loterre.fr/ark:/67375/TSO-M32F3P1Q-K>
  a skos:Concept ;
  skos:altLabel "Directory of Open Access scholarly Resources"@en, "Directory of Open Access scholarly Resources"@es, "Directory of Open Access scholarly Resources"@fr ;
  skos:definition "A service offered by the ISSN International Centre with the support of the Communication and Information Sector of UNESCO. It provides a free access to those ISSN bibliographic records which describe scholarly resources in Open Access: journals, monographic series, conference proceedings, academic repositories and scholarly blogs. (Source: https://www.issn.org/services/online-services/road-the-directory-of-open-access-scholarly-resources/)"@en, "Service proposé par le Centre International de l’ISSN avec le soutien du Secteur Communication et information de l’UNESCO. Il donne accès gratuitement à un sous-ensemble de notices bibliographiques du Portail ISSN qui décrivent des ressources scientifiques en libre accès identifiées par un ISSN: revues, séries monographiques, actes de conférences, archives ouvertes institutionnelles et carnets de recherche."@fr ;
  skos:prefLabel "ROAD"@en, "ROAD"@es, "ROAD"@fr ;
  skos:inScheme <http://data.loterre.fr/ark:/67375/TSO> ;
  skos:broader <http://data.loterre.fr/ark:/67375/TSO-V0HZ66HD-4> .

<http://data.loterre.fr/ark:/67375/TSO-NKGK3HW9-N>
  a skos:Concept ;
  dc:modified "2021-06-24"^^xsd:date ;
  skos:definition "A web-based tool which provides clear advice to researchers on how they can comply with their funder’s Plan S-aligned Open Access policy when seeking to publish in their chosen journal. (Source : cOAlition S)"@en, "Outil en ligne opéré par la cOAlition S qui permet aux chercheurs d’identifier rapidement la politique science ouverte du journal de leur choix, de visualiser les voies de publication possibles et ainsi de vérifier la compatibilité de la revue dans laquelle ils souhaitent publier avec le Plan S et la politique science ouverte de l’ANR. (Source : Ouvrir la Science)"@fr ;
  skos:prefLabel "Journal Checker Tool"@en, "Journal Checker Tool"@es, "Journal Checker Tool"@fr ;
  skos:inScheme <http://data.loterre.fr/ark:/67375/TSO> ;
  skos:broader <http://data.loterre.fr/ark:/67375/TSO-QK42D772-3> ;
  skos:related <http://data.loterre.fr/ark:/67375/TSO-GCQ559K4-Q> .

<http://data.loterre.fr/ark:/67375/TSO-M9JG3Z18-C>
  a skos:Concept ;
  dc:modified "2021-06-29"^^xsd:date ;
  skos:definition "Cycle d'ateliers pratiques et ludiques sur les bonnes pratiques de gestion et de partage des données de recherche, organisé par OPIDoR"@fr ;
  skos:prefLabel "OPIDoR tour"@en, "OPIDoR tour"@es, "OPIDoR tour"@fr ;
  skos:inScheme <http://data.loterre.fr/ark:/67375/TSO> ;
  skos:broader <http://data.loterre.fr/ark:/67375/TSO-KG7FR9LH-R> ;
  skos:related <http://data.loterre.fr/ark:/67375/TSO-J9P20ZD1-C> .

<http://data.loterre.fr/ark:/67375/TSO-ZDBWP9RP-M>
  a skos:Concept ;
  dc:modified "2021-06-24"^^xsd:date ;
  skos:altLabel "Consortium unifié des établissements universitaires et de recherche pour l'accès aux publications numériques"@fr, "consortium Couperin.org"@fr ;
  skos:definition "Association à but non lucratif financée par les cotisations des établissements membres et subventionnée par le Ministère Français de l’Enseignement Supérieur, de la Recherche et de l’Innovation. Il a entre autres pour mission de développer un réseau national de compétences et d'échanges en matière de documentation électronique notamment concernant les politiques d'acquisitions, les modèles de facturation des éditeurs, les plans de développement de collections, l’accès ouvert aux productions scientifiques, la gestion des données de la recherche, le soutien à la science ouverte, l'ergonomie d'accès, les statistiques d'usage, les indicateurs. (Source : https://www.couperin.org/presentation/missions-2)"@fr ;
  skos:prefLabel "Couperin"@en, "Couperin"@es, "Couperin"@fr ;
  skos:inScheme <http://data.loterre.fr/ark:/67375/TSO> ;
  skos:broader <http://data.loterre.fr/ark:/67375/TSO-J64S3QDL-1> .

<http://data.loterre.fr/ark:/67375/TSO-G3FV93X6-N>
  a skos:Concept ;
  dc:modified "2021-06-29"^^xsd:date ;
  skos:definition "Structure rassemblant les principales organisations européennes de financement de la recherche, créée en octobre 2011 et basée à Bruxelles."@fr, "The European association representing the interests of major public research performing and research funding organisations. (Source : https://www.scienceeurope.org/ )"@en ;
  skos:prefLabel "Science Europe"@en, "Science Europe"@es, "Science Europe"@fr ;
  skos:inScheme <http://data.loterre.fr/ark:/67375/TSO> ;
  skos:broader <http://data.loterre.fr/ark:/67375/TSO-T52K1CB6-X> .

<http://data.loterre.fr/ark:/67375/TSO-GCTBW7HJ-P>
  a skos:Concept ;
  dc:modified "2021-06-29"^^xsd:date ;
  skos:altLabel "FOAA"@en, "FOAA"@es, "FOAA"@fr ;
  skos:definition "Organisation néerlandaise à but non lucratif, lancée en 2017, qui est à l'origine des \"Fair Open Access Principles\"."@fr ;
  skos:prefLabel "Fair Open Acces Alliance"@es, "Fair Open Access Alliance"@en, "Fair Open Access Alliance"@fr ;
  skos:inScheme <http://data.loterre.fr/ark:/67375/TSO> ;
  skos:broader <http://data.loterre.fr/ark:/67375/TSO-J64S3QDL-1> ;
  skos:related <http://data.loterre.fr/ark:/67375/TSO-BD33KNNX-S>, <http://data.loterre.fr/ark:/67375/TSO-GKLZDCG9-4>, <http://data.loterre.fr/ark:/67375/TSO-TJTXZ4LV-W>, <http://data.loterre.fr/ark:/67375/TSO-VQD3856X-4>, <http://data.loterre.fr/ark:/67375/TSO-ZWDW27C7-Q> .

<http://data.loterre.fr/ark:/67375/TSO-MFB71KWG-1>
  a skos:Concept ;
  dc:modified "2021-06-29"^^xsd:date ;
  skos:altLabel "OLH"@en ;
  skos:definition "A charitable organisation dedicated to publishing open access scholarship in the humanities, with no author-facing article processing charges (source: https://www.openlibhums.org/site/about/)"@en, "Organisation qui se consacre à la publication d'études en libre accès dans le domaine des sciences humaines, sans frais de traitement des articles pour les auteurs."@fr ;
  skos:prefLabel "Open Library of Humanities"@en, "Open Library of Humanities"@es, "Open Library of Humanities"@fr ;
  skos:inScheme <http://data.loterre.fr/ark:/67375/TSO> ;
  skos:broader <http://data.loterre.fr/ark:/67375/TSO-J64S3QDL-1> .

<http://data.loterre.fr/ark:/67375/TSO-KCLNJ3JK-9>
  a skos:Concept ;
  dc:modified "2021-06-24"^^xsd:date ;
  skos:altLabel "CIS"@fr, "Consejo internacional de la ciencia"@es, "ISC"@en, "ISC"@es ;
  skos:definition "A non-governmental organization with a unique global membership that advances science as a global public good."@en, "Organisation internationale non gouvernementale fondée en juillet 2018 par la fusion du Conseil international pour la science et du Conseil international des sciences sociales. (Source : https://fr.wikipedia.org/wiki/Conseil_international_des_sciences)"@fr ;
  skos:prefLabel "Conseil international des sciences"@fr, "Consejo científico internacional"@es, "International Science Council"@en ;
  skos:inScheme <http://data.loterre.fr/ark:/67375/TSO> ;
  skos:broader <http://data.loterre.fr/ark:/67375/TSO-J64S3QDL-1> ;
  skos:related <http://data.loterre.fr/ark:/67375/TSO-FK1RPNQP-Z> .

<http://data.loterre.fr/ark:/67375/TSO-VRK75VT8-1>
  a skos:Concept ;
  dc:modified "2021-06-18"^^xsd:date ;
  skos:definition "Projet européen d’infrastructure OpenMinTeD dont l’objectif est de mettre en place une plateforme informatique en ligne, encourageant et facilitant l’utilisation des technologies de fouille de textes (text and data mining : TDM) pour la recherche. (Source : https://www.inrae.fr/actualites/openminted)"@fr ;
  skos:prefLabel "OpenMinTeD"@en, "OpenMinTeD"@es, "OpenMinTeD"@fr ;
  skos:inScheme <http://data.loterre.fr/ark:/67375/TSO> ;
  skos:broader <http://data.loterre.fr/ark:/67375/TSO-H93WKMMJ-B> .

<http://data.loterre.fr/ark:/67375/TSO-KFCWMBBV-K>
  a skos:Concept ;
  skos:definition "Ecole de pensée fondée sur l'hypothèse que la recherche «efficace» dépend de la disponibilité des outils et des applications. Par conséquent, le «but» de l'école est de promouvoir la création de plates-formes, d'outils et de services à la disposition des scientifiques. (Source : https://fr.other.wiki/wiki/Open_Science#Infrastructure_School)"@fr ;
  skos:prefLabel "escuela de infraestructura"@es, "infrastructure school"@en, "école d'infrastructure"@fr ;
  skos:inScheme <http://data.loterre.fr/ark:/67375/TSO> ;
  skos:broader <http://data.loterre.fr/ark:/67375/TSO-F2VJ1STQ-Z> .

<http://data.loterre.fr/ark:/67375/TSO-D8FHMPQB-D>
  a skos:Concept ;
  skos:definition "Ecole de pensée qui vise à rendre la science accessible à un public plus large. Elle se caractérise donc par deux grands courants : l'un plaide pour l'accès du processus de recherche aux masses, tandis que l'autre plaide pour un accès accru au produit scientifique pour le public. (Source : https://fr.other.wiki/wiki/Open_Science#Infrastructure_School)"@fr ;
  skos:prefLabel "escuela pública"@es, "public school"@en, "école publique"@fr ;
  skos:inScheme <http://data.loterre.fr/ark:/67375/TSO> ;
  skos:broader <http://data.loterre.fr/ark:/67375/TSO-F2VJ1STQ-Z> .

<http://data.loterre.fr/ark:/67375/TSO-H9882CCM-4>
  a skos:Concept ;
  skos:definition "Ecole de pensée qui se préoccupe du concept d'accès au savoir. Au lieu de se concentrer sur l'accessibilité de la recherche et sa compréhensibilité, les partisans de cette école se concentrent sur l'accès des produits de la recherche au public. (Source : https://fr.other.wiki/wiki/Open_Science#Infrastructure_School)"@fr ;
  skos:prefLabel "democratic school"@en, "escuela democrática"@es, "école démocratique"@fr ;
  skos:inScheme <http://data.loterre.fr/ark:/67375/TSO> ;
  skos:broader <http://data.loterre.fr/ark:/67375/TSO-F2VJ1STQ-Z> .

<http://data.loterre.fr/ark:/67375/TSO-Z0XXXG08-3>
  a skos:Concept ;
  skos:definition "Ecole de pensée qui considère l'Open Science comme la possibilité de rendre la création et la diffusion des connaissances plus efficaces en augmentant la collaboration tout au long du processus de recherche. Les partisans soutiennent que la science pourrait être optimisée en modularisant le processus et en ouvrant la chaîne de valeur scientifique. (Source : https://fr.other.wiki/wiki/Open_Science#Infrastructure_School)"@fr ;
  skos:prefLabel "escuela pragmática"@es, "pragmatic school"@en, "école pragmatique"@fr ;
  skos:inScheme <http://data.loterre.fr/ark:/67375/TSO> ;
  skos:broader <http://data.loterre.fr/ark:/67375/TSO-F2VJ1STQ-Z> .

<http://data.loterre.fr/ark:/67375/TSO-JL9MGMVK-W>
  a skos:Concept ;
  dc:created "2021-06-04"^^xsd:date ;
  dc:modified "2021-06-10"^^xsd:date ;
  skos:definition "Journals that publish work without proper peer review and which charge scholars sometimes huge fees to submit should not be allowed to share space with legitimate journals and publishers, whether open access or not. (Source: https://predatoryjournals.com)"@en, "Revue au contenu pseudo-scientifique faisant très peu cas des questions de qualité et d’intégrité scientifique, au fonctionnement opaque et qui ne répond pas aux recommandations éditoriales. (Source : https://www.unilim.fr/scd/2021/02/19/les-revues-predatrices-comment-les-reconnaitre-et-sen-premunir/)"@fr ;
  skos:prefLabel "predatory journal"@en, "revista depredadora"@es, "revue prédatrice"@fr ;
  skos:inScheme <http://data.loterre.fr/ark:/67375/TSO> ;
  skos:broader <http://data.loterre.fr/ark:/67375/TSO-TM0MS2GV-7> ;
  skos:related <http://data.loterre.fr/ark:/67375/TSO-ZRVHF3XW-L> .

<http://data.loterre.fr/ark:/67375/TSO-X3TNSQ40-M>
  a skos:Concept ;
  dc:created "2021-06-10"^^xsd:date ;
  dc:modified "2021-06-10"^^xsd:date ;
  skos:prefLabel "dissemination tool"@en, "herramienta de difusión"@es, "outil de diffusion"@fr ;
  skos:inScheme <http://data.loterre.fr/ark:/67375/TSO> ;
  skos:broader <http://data.loterre.fr/ark:/67375/TSO-V0KSG0NC-P> ;
  skos:related <http://data.loterre.fr/ark:/67375/TSO-DXZZDQSM-3> ;
  skos:narrower <http://data.loterre.fr/ark:/67375/TSO-DDH5932P-J>, <http://data.loterre.fr/ark:/67375/TSO-RW8FM312-M>, <http://data.loterre.fr/ark:/67375/TSO-RB0TPH2H-Q>, <http://data.loterre.fr/ark:/67375/TSO-WSB3R3KG-1>, <http://data.loterre.fr/ark:/67375/TSO-QF2RDTPG-H> .

<http://data.loterre.fr/ark:/67375/TSO-HZ175K8D-R>
  a skos:Concept ;
  dc:created "2021-06-10"^^xsd:date ;
  dc:modified "2021-06-30"^^xsd:date ;
  skos:prefLabel "infraestructura de archivo abierto"@es, "infrastructure de type archive ouverte"@fr, "open archive infrastructure"@en ;
  skos:inScheme <http://data.loterre.fr/ark:/67375/TSO> ;
  skos:broader <http://data.loterre.fr/ark:/67375/TSO-V0HZ66HD-4> ;
  skos:related <http://data.loterre.fr/ark:/67375/TSO-ZNX5Z1VV-S> ;
  skos:narrower <http://data.loterre.fr/ark:/67375/TSO-RPCFB5QW-0>, <http://data.loterre.fr/ark:/67375/TSO-LQV42R36-F>, <http://data.loterre.fr/ark:/67375/TSO-WD1R50MM-6>, <http://data.loterre.fr/ark:/67375/TSO-PZNHPP7J-7>, <http://data.loterre.fr/ark:/67375/TSO-L1X7N7S8-V>, <http://data.loterre.fr/ark:/67375/TSO-XF2L7W5Z-V>, <http://data.loterre.fr/ark:/67375/TSO-PGSFQSNR-1>, <http://data.loterre.fr/ark:/67375/TSO-C4027K67-Q>, <http://data.loterre.fr/ark:/67375/TSO-KBZ7QKR9-W>, <http://data.loterre.fr/ark:/67375/TSO-H6LP405X-S>, <http://data.loterre.fr/ark:/67375/TSO-S784H10S-P>, <http://data.loterre.fr/ark:/67375/TSO-R19NG9JL-2>, <http://data.loterre.fr/ark:/67375/TSO-XHFB8590-0>, <http://data.loterre.fr/ark:/67375/TSO-DKQM5BJJ-3>, <http://data.loterre.fr/ark:/67375/TSO-KZW10WMN-H> .

<http://data.loterre.fr/ark:/67375/TSO-WZ6DJ64Q-P>
  a skos:Concept ;
  dc:created "2021-06-10"^^xsd:date ;
  dc:modified "2021-06-10"^^xsd:date ;
  skos:prefLabel "plataforma de publicación"@es, "plateforme d'édition"@fr, "publishing platform"@en ;
  skos:inScheme <http://data.loterre.fr/ark:/67375/TSO> ;
  skos:broader <http://data.loterre.fr/ark:/67375/TSO-V0HZ66HD-4> ;
  skos:narrower <http://data.loterre.fr/ark:/67375/TSO-Z3M8CHXM-K>, <http://data.loterre.fr/ark:/67375/TSO-CTWNT4VX-W>, <http://data.loterre.fr/ark:/67375/TSO-NT6B4GTK-3>, <http://data.loterre.fr/ark:/67375/TSO-MSSFPBQ3-S>, <http://data.loterre.fr/ark:/67375/TSO-RCJ760D7-P>, <http://data.loterre.fr/ark:/67375/TSO-LS688VQ2-2> .

<http://data.loterre.fr/ark:/67375/TSO-SJ4WNCS6-L>
  a skos:Concept ;
  dc:created "2021-06-10"^^xsd:date ;
  dc:modified "2021-06-29"^^xsd:date ;
  skos:definition "Catalogue qui a pour objectif de cartographier les services français dédiés aux données scientifiques, hébergé par l’Inist-CNRS qui en assure la modération. (Source : https://cat.opidor.fr/index.php/Cat_OPIDoR:%C3%80_propos)"@fr ;
  skos:prefLabel "Cat OPIDoR"@en, "Cat OPIDoR"@es, "Cat OPIDoR"@fr ;
  skos:inScheme <http://data.loterre.fr/ark:/67375/TSO> ;
  skos:broader <http://data.loterre.fr/ark:/67375/TSO-J9P20ZD1-C>, <http://data.loterre.fr/ark:/67375/TSO-WQ9RZCBH-P> .

<http://data.loterre.fr/ark:/67375/TSO-VDCNM6ZN-W>
  a skos:Concept ;
  dc:created "2021-06-10"^^xsd:date ;
  dc:modified "2021-07-05"^^xsd:date ;
  skos:definition "Herramienta que ayuda a crear planes de gestión de datos en línea a disposición de la enseñanza superior y la investigación. Está alojado y gestionado por Inist-CNRS."@es, "Outil d’aide à la création en ligne de plans de gestion de données mis à disposition de l’Enseignement Supérieur et de la Recherche. Il est hébergé et géré par l’Inist-CNRS."@fr, "Tool to help create online data management plans available to Higher Education and Research. It is hosted and managed by Inist-CNRS."@en ;
  skos:prefLabel "DMP OPIDoR"@en, "DMP OPIDoR"@es, "DMP OPIDoR"@fr ;
  skos:inScheme <http://data.loterre.fr/ark:/67375/TSO> ;
  skos:broader <http://data.loterre.fr/ark:/67375/TSO-J9P20ZD1-C>, <http://data.loterre.fr/ark:/67375/TSO-LS0Q2K68-D> .

<http://data.loterre.fr/ark:/67375/TSO-XQQ71S90-L>
  a skos:Concept ;
  dc:created "2021-06-10"^^xsd:date ;
  dc:modified "2021-06-25"^^xsd:date ;
  skos:definition "Application destinée aux organismes de recherche disposant d’un compte auprès d’un membre DataCite et souhaitant gérer et attribuer en masse des DOI de façon \"user friendly\". (Source : https://www.inist.fr/realisations/pid-opidor/)"@fr ;
  skos:prefLabel "PID OPIDoR"@en, "PID OPIDoR"@es, "PID OPIDoR"@fr ;
  skos:inScheme <http://data.loterre.fr/ark:/67375/TSO> ;
  skos:broader <http://data.loterre.fr/ark:/67375/TSO-J9P20ZD1-C> ;
  skos:related <http://data.loterre.fr/ark:/67375/TSO-RPJVDHMM-Q>, <http://data.loterre.fr/ark:/67375/TSO-T487PDFX-7> .

<http://data.loterre.fr/ark:/67375/TSO-XW567W8B-4>
  a skos:Concept ;
  dc:created "2021-06-24"^^xsd:date ;
  dc:modified "2021-07-05"^^xsd:date ;
  skos:definition "An online tool which helps researchers and data managers assess their level of awareness of the requirements for making datasets findable, accessible, interoperable, and reusable (FAIR) before uploading them into a data repository. (Source:https://www.fairsfair.eu/news/fairsfair-launches-fair-awareness-assessment-tool)"@en, "Plataforma que ayuda a los investigadores y gestores de datos a evaluar su nivel de conocimiento sobre los principios FAIR antes de depositar sus datos en un almacén."@es, "Plateforme qui aide les chercheurs et les gestionnaires de données à évaluer leur niveau de connaissance sur les principes FAIR avant de déposer leurs données dans un entrepôt."@fr ;
  skos:prefLabel "FAIR-Aware"@en, "FAIR-Aware"@es, "FAIR-Aware"@fr ;
  skos:inScheme <http://data.loterre.fr/ark:/67375/TSO> ;
  skos:broader <http://data.loterre.fr/ark:/67375/TSO-DXZZDQSM-3> ;
  skos:related <http://data.loterre.fr/ark:/67375/TSO-D9HJPTL6-X> .

<http://data.loterre.fr/ark:/67375/TSO-TC1HRLFR-8>
  a skos:Concept ;
  dc:created "2021-06-24"^^xsd:date ;
  dc:modified "2021-06-24"^^xsd:date ;
  skos:definition "Outil qui atteste qu’un entrepôt est « de confiance » pour les personnes qui utilisent les données qu’il met à disposition, mais aussi pour ceux dont il gère les données. (Source : https://www.ouvrirlascience.fr/)"@fr ;
  skos:prefLabel "certificación de infraestructuras de datos"@es, "certification des infrastructures de données"@fr, "data repository certification"@en ;
  skos:inScheme <http://data.loterre.fr/ark:/67375/TSO> ;
  skos:broader <http://data.loterre.fr/ark:/67375/TSO-SMGMJFLJ-Q> ;
  skos:related <http://data.loterre.fr/ark:/67375/TSO-CQT7DBZS-F>, <http://data.loterre.fr/ark:/67375/TSO-LJ49Q4WZ-R> .

<http://data.loterre.fr/ark:/67375/TSO-CQT7DBZS-F>
  a skos:Concept ;
  dc:created "2021-06-24"^^xsd:date ;
  dc:modified "2021-06-24"^^xsd:date ;
  skos:definition "International, community based, non-governmental, and non-profit organization promoting sustainable and trustworthy data infrastructures and offers to any interested data repository a core level certification based on the DSA–WDS Core Trustworthy Data Repositories Requirements catalogue and procedures. (Source: https://www.coretrustseal.org/about/)"@en, "Organisation internationale, communautaire, non gouvernementale et à but non lucratif qui promeut des infrastructures de données durables et fiables et offre à tout dépôt de données intéressé une certification fondée sur les exigences DSA-WDS."@fr ;
  skos:prefLabel "Core Trust Seal"@es, "Core Trust Seal"@fr, "CoreTrust Seal"@en ;
  skos:inScheme <http://data.loterre.fr/ark:/67375/TSO> ;
  skos:broader <http://data.loterre.fr/ark:/67375/TSO-J64S3QDL-1> ;
  skos:related <http://data.loterre.fr/ark:/67375/TSO-TC1HRLFR-8> .

<http://data.loterre.fr/ark:/67375/TSO-GP1DN83S-L>
  a skos:Concept ;
  dc:created "2021-06-25"^^xsd:date ;
  dc:modified "2021-06-25"^^xsd:date ;
  skos:definition "A multi-disciplinary aggregator of Open Access journals and papers, \"gold\" and \"hybrid\". (Source : https://paperity.org/about/)"@en, "Base de données agrégeant le signalement de revues et d'articles multidisciplinaires en libre accès."@fr ;
  skos:prefLabel "Paperity"@en, "Paperity"@es, "Paperity"@fr ;
  skos:inScheme <http://data.loterre.fr/ark:/67375/TSO> ;
  skos:broader <http://data.loterre.fr/ark:/67375/TSO-JN2ZSNST-6> .

<http://data.loterre.fr/ark:/67375/TSO-KBZ7QKR9-W>
  a skos:Concept ;
  dc:created "2021-06-25"^^xsd:date ;
  dc:modified "2021-06-25"^^xsd:date ;
  skos:altLabel "Accelerating Science and Publication in biology"@en ;
  skos:definition "A scientist-driven nonprofit working to drive open and innovative communication in the life sciences. The organisation promotes the productive use of preprints for research dissemination and transparent peer review and feedback on all research outputs. (Source: https://asapbio.org/about-us)"@en, "Organisme à but non lucratif qui promeut la transparence et l'innovation dans la communication des sciences de la vie. ASAPbio recueille des informations sur les serveurs de prépublications et propose une liste des produits et services. (Source : https://www.ouvrirlascience.fr/landscape-of-products-and-services-for-sharing-preprints/)"@fr ;
  skos:prefLabel "ASAPbio"@en, "ASAPbio"@es, "ASAPbio"@fr ;
  skos:inScheme <http://data.loterre.fr/ark:/67375/TSO> ;
  skos:broader <http://data.loterre.fr/ark:/67375/TSO-HZ175K8D-R> ;
  skos:related <http://data.loterre.fr/ark:/67375/TSO-GLZ7M59Q-M>, <http://data.loterre.fr/ark:/67375/TSO-XZ5703Z4-Q> .

<http://data.loterre.fr/ark:/67375/TSO-H6LP405X-S>
  a skos:Concept ;
  dc:created "2021-06-25"^^xsd:date ;
  dc:modified "2021-06-25"^^xsd:date ;
  skos:definition "A free submission, distribution, and archive service for unpublished preprints in chemistry and related areas. ChemRxiv gives researchers across a broad range of fields related to the chemical sciences the opportunity to share early results with colleagues and receive recommendations for improvement, ahead of formal peer review and publication. (Source: https://chemrxiv.org/engage/chemrxiv/about-information?show=about-site)"@en, "Serveur de prépublications dédié à la communauté de la chimie et des domaines connexes."@fr ;
  skos:prefLabel "ChemRxiv"@en, "ChemRxiv"@es, "ChemRxiv"@fr ;
  skos:semanticRelation <http://data.loterre.fr/ark:/67375/TSO-GLZ7M59Q-M>, <http://data.loterre.fr/ark:/67375/TSO-XZ5703Z4-Q> ;
  skos:inScheme <http://data.loterre.fr/ark:/67375/TSO> ;
  skos:broader <http://data.loterre.fr/ark:/67375/TSO-HZ175K8D-R> .

<http://data.loterre.fr/ark:/67375/TSO-S784H10S-P>
  a skos:Concept ;
  dc:created "2021-06-25"^^xsd:date ;
  dc:modified "2021-06-25"^^xsd:date ;
  skos:definition "A preprint archive for Paleontology. (Source: https://paleorxiv.org/)"@en, "Archive de prépublications en paléontologie. (Source : https://paleorxiv.org/)"@fr ;
  skos:prefLabel "PaleorXiv"@en, "PaleorXiv"@es, "PaleorXiv"@fr ;
  skos:inScheme <http://data.loterre.fr/ark:/67375/TSO> ;
  skos:broader <http://data.loterre.fr/ark:/67375/TSO-HZ175K8D-R> ;
  skos:related <http://data.loterre.fr/ark:/67375/TSO-GLZ7M59Q-M>, <http://data.loterre.fr/ark:/67375/TSO-XZ5703Z4-Q> .

<http://data.loterre.fr/ark:/67375/TSO-R19NG9JL-2>
  a skos:Concept ;
  dc:created "2021-06-25"^^xsd:date ;
  dc:modified "2021-06-25"^^xsd:date ;
  skos:definition "Archive de prépublications en ingénierie. (Source : https://engrxiv.org/)"@fr, "The open archive of engineering. (Source: https://engrxiv.org/)"@en ;
  skos:prefLabel "engrXiv"@en, "engrXiv"@es, "engrXiv"@fr ;
  skos:inScheme <http://data.loterre.fr/ark:/67375/TSO> ;
  skos:broader <http://data.loterre.fr/ark:/67375/TSO-HZ175K8D-R> ;
  skos:related <http://data.loterre.fr/ark:/67375/TSO-GLZ7M59Q-M>, <http://data.loterre.fr/ark:/67375/TSO-XZ5703Z4-Q> .

<http://data.loterre.fr/ark:/67375/TSO-XHFB8590-0>
  a skos:Concept ;
  dc:created "2021-06-25"^^xsd:date ;
  dc:modified "2021-06-25"^^xsd:date ;
  skos:definition "Archive de prépublications en sciences sociales. (Source : https://osf.io/preprints/socarxiv/)"@fr, "Open archive of the social sciences. (Source: https://osf.io/preprints/socarxiv/)"@en ;
  skos:prefLabel "SocArXiv"@en, "SocArXiv"@es, "SocArXiv"@fr ;
  skos:inScheme <http://data.loterre.fr/ark:/67375/TSO> ;
  skos:broader <http://data.loterre.fr/ark:/67375/TSO-HZ175K8D-R> ;
  skos:related <http://data.loterre.fr/ark:/67375/TSO-GLZ7M59Q-M>, <http://data.loterre.fr/ark:/67375/TSO-XZ5703Z4-Q> .

<http://data.loterre.fr/ark:/67375/TSO-FF03NR9V-N>
  a skos:Concept ;
  dc:created "2021-06-25"^^xsd:date ;
  dc:modified "2021-06-25"^^xsd:date ;
  skos:altLabel "CERN OHL"@en, "CERN OHL"@es ;
  skos:definition "Licence crée par le CERN et utilisée pour des projets de matériel libre."@fr ;
  skos:prefLabel "CERN Open Hardware License"@en, "licence CERN-OHL"@fr, "licencia de hardware abierto CERN"@es ;
  skos:inScheme <http://data.loterre.fr/ark:/67375/TSO> ;
  skos:broader <http://data.loterre.fr/ark:/67375/TSO-T67S254S-S> .

<http://data.loterre.fr/ark:/67375/TSO-WVJZTQCD-F>
  a skos:Concept ;
  dc:created "2021-06-29"^^xsd:date ;
  dc:modified "2021-06-29"^^xsd:date ;
  skos:definition "Initiative lancée à Helsinki en janvier 2019, pour appeler les acteurs de la recherche à soutenir la diffusion des résultats de la recherche dans l’intérêt de la société, à protéger les infrastructures nationales permettant la publication de recherches pertinentes au niveau local et à promouvoir la diversité linguistique dans les systèmes d’évaluation et de financement de la recherche. (Source : https://www.ouvrirlascience.fr/initiative-dhelsinki-sur-le-multilinguisme-dans-la-communication-savante/)"@fr, "This initiative lauched in 2019 encourages policy-makers, leaders, universities, research institutions, research funders, libraries, and researchers to support dissemination of research results for the full benefit of the society; protect national infrastructures for publishing locally relevant research; promote language diversity in research assessment, evaluation, and funding systems. (Source: https://www.helsinki-initiative.org/en)"@en ;
  skos:prefLabel "Helsinki Initiative on Multilingualism in Scholarly Communication"@en, "Iniciativa Helsinki sobre Multilingüismo en la Comunicación Científica"@es, "Initiative d’Helsinki sur le multilinguisme dans la communication savante"@fr ;
  skos:inScheme <http://data.loterre.fr/ark:/67375/TSO> ;
  skos:broader <http://data.loterre.fr/ark:/67375/TSO-V6F4ZS65-G> .

<http://data.loterre.fr/ark:/67375/TSO-DKQM5BJJ-3>
  a skos:Concept ;
  dc:created "2021-06-29"^^xsd:date ;
  dc:modified "2021-06-29"^^xsd:date ;
  skos:definition "A preprint server for Geosciences."@en, "Archive de dépôt et de diffusion de prépublications en sciences de la Terre."@fr ;
  skos:prefLabel "EarthArXiv"@en, "EarthArXiv"@es, "EarthArXiv"@fr ;
  skos:inScheme <http://data.loterre.fr/ark:/67375/TSO> ;
  skos:broader <http://data.loterre.fr/ark:/67375/TSO-HZ175K8D-R> .

<http://data.loterre.fr/ark:/67375/TSO-KZW10WMN-H>
  a skos:Concept ;
  dc:created "2021-06-29"^^xsd:date ;
  dc:modified "2021-06-29"^^xsd:date ;
  skos:definition "Infrastructure de recherche européenne distribuée ayant pour mission le développement de la communication savante ouverte en sciences humaines et sociales"@fr, "The Research Infrastructure supporting open scholarly communication in the social sciences and humanities (SSH) in the European Research Area. Its mission is to coordinate and federate resources in Europe to efficiently address the scholarly communication needs of European researchers in the field of SSH. (Source: https://www.operas-eu.org/about/)"@en ;
  skos:prefLabel "OPERAS"@en, "OPERAS"@es, "OPERAS"@fr ;
  skos:inScheme <http://data.loterre.fr/ark:/67375/TSO> ;
  skos:broader <http://data.loterre.fr/ark:/67375/TSO-HZ175K8D-R> .

<http://data.loterre.fr/ark:/67375/TSO-HF09ZX0Z-Q>
  a skos:Concept ;
  dc:created "2021-06-29"^^xsd:date ;
  dc:modified "2021-06-29"^^xsd:date ;
  skos:altLabel "Confederation of Open Access Repositories"@en ;
  skos:definition "An international association with 151 members and partners from around the world representing libraries, universities, research institutions, government funders and others. COAR brings together individual repositories and repository networks in order to build capacity, align policies and practices, and act as a global voice for the repository community. (Source: https://www.coar-repositories.org/about-coar/)"@en, "Association internationale dont l'objectif est de promouvoir les archives ouvertes à un niveau mondial, de soutenir la communauté et faire progresser l'adoption de nouvelles pratiques pour assurer l'ouverture et l'accès aux résultats de la recherche scientifique. (Source : https://www.ouvrirlascience.fr/confederation-of-open-access-repositories-coar/)"@fr ;
  skos:prefLabel "COAR"@en, "COAR"@es, "COAR"@fr ;
  skos:inScheme <http://data.loterre.fr/ark:/67375/TSO> ;
  skos:broader <http://data.loterre.fr/ark:/67375/TSO-J64S3QDL-1> ;
  skos:related <http://data.loterre.fr/ark:/67375/TSO-DJ828LKC-C> .

<http://data.loterre.fr/ark:/67375/TSO-JCX2HR5K-4>
  a skos:Concept ;
  dc:created "2021-07-05"^^xsd:date ;
  dc:modified "2021-07-05"^^xsd:date ;
  skos:altLabel "data article"@en, "data descriptor"@en, "publication de données"@fr ;
  skos:definition "A scholarly journal publication whose primary purpose is to describe a dataset or a group of datasets, rather than to report a research investigation. As such, it contains facts about data, not hypotheses and arguments in support of the data, as found in a conventional research article. (Source: https://pensoft.net/img/upl/file/DataPaperPoster.pdf)"@en, "Publication qui décrit un jeu de données scientifiques, notamment à l’aide d’informations structurées appelées métadonnées. Contrairement aux articles de recherches classiques, les data papers fournissent une voie formalisée au partage des données plutôt que tester des hypothèses ou présenter de nouvelles analyses. (Source : https://doranum.fr/data-paper-data-journal/fiche-synthetique/)"@fr ;
  skos:prefLabel "data paper"@en, "data paper"@es, "data paper"@fr ;
  skos:inScheme <http://data.loterre.fr/ark:/67375/TSO> ;
  skos:broader <http://data.loterre.fr/ark:/67375/TSO-XS8KGCJ0-V> ;
  skos:related <http://data.loterre.fr/ark:/67375/TSO-P0JM96T2-W> .

<http://data.loterre.fr/ark:/67375/TSO-P0JM96T2-W>
  a skos:Concept ;
  dc:created "2021-07-05"^^xsd:date ;
  dc:modified "2021-07-05"^^xsd:date ;
  skos:altLabel "journal de données"@fr, "revue de données"@fr ;
  skos:definition "A scholarly journal that publishes articles about datasets, or data papers."@en, "Revue dédiée à la publication d'articles qui décrivent un jeu de données, ou data papers."@fr ;
  skos:prefLabel "data journal"@en, "data journal"@es, "data journal"@fr ;
  skos:inScheme <http://data.loterre.fr/ark:/67375/TSO> ;
  skos:broader <http://data.loterre.fr/ark:/67375/TSO-XS8KGCJ0-V> ;
  skos:related <http://data.loterre.fr/ark:/67375/TSO-G591ZH6Q-X>, <http://data.loterre.fr/ark:/67375/TSO-JCX2HR5K-4> .
